@prefix cc: <https://w3id.org/costumeCore/ontology/> .
@prefix dcterms: <http://purl.org/dc/terms/> .
@prefix owl: <http://www.w3.org/2002/07/owl#> .
@prefix rdf: <http://www.w3.org/1999/02/22-rdf-syntax-ns#> .
@prefix rdfs: <http://www.w3.org/2000/01/rdf-schema#> .
@prefix vra: <http://purl.org/vra/> .

cc:CC00019 a owl:NamedIndividual ;
    rdfs:label "jewel"@en ;
    dcterms:identifier "CC00019" .

cc:CC00023 a owl:NamedIndividual ;
    rdfs:label "scoop neck"@en ;
    dcterms:identifier "CC00023" .

cc:CC00042 a owl:NamedIndividual ;
    rdfs:label "portrait collar"@en ;
    dcterms:identifier "CC00042" .

cc:CC00079 a owl:NamedIndividual ;
    rdfs:label "drawloom"@en ;
    dcterms:identifier "CC00079" .

cc:CC00111 a owl:NamedIndividual ;
    rdfs:label "hourglass (silhouette)"@en ;
    dcterms:identifier "CC00111" .

cc:CC00115 a owl:NamedIndividual ;
    rdfs:label "Polonaise"@en ;
    dcterms:description [ rdfs:label "various styles of women's garments, generally with a decoratively draped overskirt"@en ;
            dcterms:creator "The J. Paul Getty Trust" ;
            dcterms:license <https://opendatacommons.org/licenses/by/1-0/> ;
            dcterms:rights <https://rightsstatements.org/vocab/InC/1.0/> ;
            dcterms:source <http://www.getty.edu/research/tools/vocabularies/aat/> ],
        "various styles of women's garments, generally with a decoratively draped overskirt"@en ;
    dcterms:identifier "CC00115" .

cc:CC00117 a owl:NamedIndividual ;
    rdfs:label "robe a l'Anglaise"@en ;
    dcterms:identifier "CC00117" .

cc:CC00118 a owl:NamedIndividual ;
    rdfs:label "robe a la Francaise"@en ;
    dcterms:identifier "CC00118" .

cc:CC00120 a owl:NamedIndividual ;
    rdfs:label "S-curve"@en ;
    dcterms:identifier "CC00120" .

cc:CC00132 a owl:NamedIndividual ;
    rdfs:label "Juliet sleeve"@en ;
    dcterms:identifier "CC00132" .

cc:CC00134 a owl:NamedIndividual ;
    rdfs:label "lantern sleeve"@en ;
    dcterms:identifier "CC00134" .

cc:CC00140 a owl:NamedIndividual ;
    rdfs:label "sleeve panes"@en ;
    dcterms:identifier "CC00140" .

cc:CC00154 a owl:NamedIndividual ;
    rdfs:label "basque"@en ;
    dcterms:identifier "CC00154" .

cc:CC00165 a owl:NamedIndividual ;
    rdfs:label "box-pleated"@en ;
    dcterms:description [ rdfs:label "Wide double pleats, with the material folded under at each side. For wide double pleats having the flat fold turned in rather than out, use \"inverted pleats.\""@en ;
            dcterms:creator "The J. Paul Getty Trust" ;
            dcterms:license <https://opendatacommons.org/licenses/by/1-0/> ;
            dcterms:rights <https://rightsstatements.org/vocab/InC/1.0/> ;
            dcterms:source <http://www.getty.edu/vow/AATFullDisplay?find=pleat&logic=AND&note=&english=N&prev_page=1&subjectid=300228368> ],
        "Wide double pleats, with the material folded under at each side. For wide double pleats having the flat fold turned in rather than out, use \"inverted pleats.\""@en ;
    dcterms:identifier "CC00165" .

cc:CC00169 a owl:NamedIndividual ;
    rdfs:label "flounced skirt"@en ;
    dcterms:identifier "CC00169" .

cc:CC00174 a owl:NamedIndividual ;
    rdfs:label "peg-top"@en ;
    dcterms:identifier "CC00174" .

cc:CC00178 a owl:NamedIndividual ;
    rdfs:label "prairie skirt"@en ;
    dcterms:identifier "CC00178" .

cc:CC00181 a owl:NamedIndividual ;
    rdfs:label "swagged"@en ;
    dcterms:identifier "CC00181" .

cc:CC00210 a owl:NamedIndividual ;
    rdfs:label "double-weave"@en ;
    dcterms:identifier "CC00210" .

cc:CC00240 a owl:NamedIndividual ;
    rdfs:label "sheared pile"@en ;
    dcterms:identifier "CC00240" .

cc:CC00263 a owl:NamedIndividual ;
    rdfs:label "cowl sleeve"@en ;
    dcterms:identifier "CC00263" .

cc:CC00331 a owl:NamedIndividual ;
    rdfs:label "straight grain"@en ;
    dcterms:identifier "CC00331" .

cc:CC00332 a owl:NamedIndividual ;
    rdfs:label "lengthwise grain"@en ;
    dcterms:identifier "CC00332" .

cc:CC00333 a owl:NamedIndividual ;
    rdfs:label "crosswise grain"@en ;
    dcterms:identifier "CC00333" .

cc:CC00516 a owl:NamedIndividual ;
    rdfs:label "mermaid"@en ;
    dcterms:identifier "CC00516" .

cc:cataloguerWithDate a owl:ObjectProperty ;
    rdfs:label "Cataloguer With Date"@en ;
    dcterms:identifier "cataloguerWithDate" ;
    rdfs:comment """Full names of all catalogers, with the date in parentheses, in the format YYYY-MM-DD.

When additions are made to the catalog record, additional names and dates should be added and existing entries should not be deleted."""@en .

cc:cbLengthIn a owl:ObjectProperty ;
    rdfs:label "Center Back Length"@en ;
    dcterms:identifier "cbLengthIn" ;
    rdfs:comment "The center back measurement from top edge (neckline or waist) to hem, in inches, as decimals to the nearest quarter inch."@en .

cc:cfLengthIn a owl:ObjectProperty ;
    rdfs:label "Center Front Length"@en ;
    dcterms:identifier "cfLengthIn" ;
    rdfs:comment "The center front measurement from top edge (neckline or waist) to hem, in inches, as decimals to the nearest quarter inch."@en .

cc:chestIn a owl:ObjectProperty ;
    rdfs:label "Chest"@en ;
    dcterms:identifier "chestIn" ;
    rdfs:comment "The measurement straight around the fullest part of the chest, in inches, as decimals to the nearest quarter inch."@en .

cc:classification a owl:ObjectProperty ;
    rdfs:label "Classification"@en ;
    dcterms:identifier "classification" ;
    rdfs:comment "A classification term should be applied for all costume items, such as \"Costume,\" or \"Fashion.\" This may vary based on the larger overall collection in which these objects will be published."@en ;
    rdfs:range [ a owl:Class ;
            owl:oneOf ( cc:CC00482 ) ] .

cc:closure a owl:ObjectProperty ;
    rdfs:label "Closure"@en ;
    dcterms:identifier "closure" ;
    rdfs:comment "Each closure used on the garment."@en ;
    rdfs:range [ a owl:Class ;
            owl:oneOf ( cc:CC00001 cc:CC00002 cc:CC00003 cc:CC00004 cc:CC00005 cc:CC00006 cc:CC00008 cc:CC00009 cc:CC00010 cc:CC00011 cc:CC00012 cc:CC00013 cc:CC00515 ) ] .

cc:closurePlacement a owl:ObjectProperty ;
    rdfs:label "Closure Placement"@en ;
    dcterms:identifier "closurePlacement" ;
    rdfs:comment "Each placement of closures on the item."@en ;
    rdfs:range [ a owl:Class ;
            owl:oneOf ( cc:CC00348 cc:CC00349 cc:CC00350 cc:CC00351 cc:CC00352 cc:CC00353 cc:CC00354 ) ] .

cc:collar a owl:ObjectProperty ;
    rdfs:label "Collar"@en ;
    dcterms:identifier "collar" ;
    rdfs:comment "Each term that describes the collar of the garment."@en ;
    rdfs:range [ a owl:Class ;
            owl:oneOf ( cc:CC00029 cc:CC00037 cc:CC00039 cc:CC00040 cc:CC00043 cc:CC00045 cc:CC00047 cc:CC00048 cc:CC00258 cc:CC00629 ) ] .

cc:colorMain a owl:ObjectProperty ;
    rdfs:label "Color Main"@en ;
    dcterms:identifier "colorMain" ;
    rdfs:comment "The most dominant color in the garment."@en ;
    rdfs:range [ a owl:Class ;
            owl:oneOf ( cc:CC00049 cc:CC00050 cc:CC00051 cc:CC00052 cc:CC00053 cc:CC00054 cc:CC00055 cc:CC00056 cc:CC00057 cc:CC00058 cc:CC00059 cc:CC00060 cc:CC00061 cc:CC00062 cc:CC00063 cc:CC00064 cc:CC00065 cc:CC00066 cc:CC00067 cc:CC00068 cc:CC00069 cc:CC00070 cc:CC00071 cc:CC00072 cc:CC00073 cc:CC00290 ) ] .

cc:colorSecondary a owl:ObjectProperty ;
    rdfs:label "Color Secondary"@en ;
    dcterms:identifier "colorSecondary" ;
    rdfs:comment "Any additional colors in the garment."@en ;
    rdfs:range [ a owl:Class ;
            owl:oneOf ( cc:CC00049 cc:CC00050 cc:CC00051 cc:CC00052 cc:CC00053 cc:CC00054 cc:CC00055 cc:CC00056 cc:CC00057 cc:CC00058 cc:CC00059 cc:CC00060 cc:CC00061 cc:CC00062 cc:CC00063 cc:CC00064 cc:CC00065 cc:CC00066 cc:CC00067 cc:CC00068 cc:CC00069 cc:CC00070 cc:CC00071 cc:CC00072 cc:CC00073 cc:CC00290 ) ] .

cc:condition a owl:ObjectProperty ;
    rdfs:label "Condition Term"@en ;
    dcterms:identifier "condition" ;
    rdfs:comment "A single term to indicate a rating of the overall condition of the object."@en ;
    rdfs:range [ a owl:Class ;
            owl:oneOf ( cc:CC00415 cc:CC00416 cc:CC00417 cc:CC00418 cc:CC00419 ) ] .

cc:conditionDescription a owl:ObjectProperty ;
    rdfs:label "Condition Description"@en ;
    dcterms:identifier "conditionDescription" ;
    rdfs:comment """Narrative description of the overall physical condition, characteristics, and completeness of a work, describing where each issue is located on the garment. 

This may incorporate details checked off on a separate worksheet."""@en .

cc:costOriginal a owl:ObjectProperty ;
    rdfs:label "Cost Original"@en ;
    dcterms:identifier "costOriginal" ;
    rdfs:comment "The cost of the object when originally created, indicating the units (dollars, etc.)"@en .

cc:costumeComponents a owl:ObjectProperty ;
    rdfs:label "Costume Components"@en ;
    dcterms:identifier "costumeComponents" ;
    rdfs:comment "Each additional component of the garment not included elsewhere."@en ;
    rdfs:range [ a owl:Class ;
            owl:oneOf ( cc:CC00018 cc:CC00142 cc:CC00176 cc:CC00184 cc:CC00287 cc:CC00327 cc:CC00394 cc:CC00395 cc:CC00396 cc:CC00397 cc:CC00398 cc:CC00399 cc:CC00400 cc:CC00492 cc:CC00493 cc:CC00580 cc:CC00581 cc:CC00598 cc:CC00599 ) ] .

cc:dimensionsOther a owl:ObjectProperty ;
    rdfs:label "Measurements Other"@en ;
    dcterms:identifier "dimensionsOther" ;
    rdfs:comment "Any other measurements that are notable on this garment, in inches, as decimals to the nearest quarter inch. Describe what the measurement is of, in parentheses, after the measurement."@en .

cc:dressType a owl:ObjectProperty ;
    rdfs:label "Dress Type"@en ;
    dcterms:identifier "dressType" ;
    rdfs:comment "Each term that describes the type of dress."@en ;
    rdfs:range [ a owl:Class ;
            owl:oneOf ( cc:CC00007 cc:CC00108 cc:CC00109 cc:CC00110 cc:CC00112 cc:CC00114 cc:CC00121 cc:CC00122 cc:CC00123 cc:CC00124 cc:CC00125 cc:CC00126 cc:CC00323 cc:CC00379 cc:CC00494 cc:CC00496 cc:CC00501 cc:CC00502 cc:CC00520 cc:CC00522 ) ] .

cc:exhibitions a owl:ObjectProperty ;
    rdfs:label "Exhibitions"@en ;
    dcterms:identifier "exhibitions" ;
    rdfs:comment "A list of all exhibitions that included this object,  including the title or name of each exhibition, its location, and other pertinent information."@en .

cc:fiber a owl:ObjectProperty ;
    rdfs:label "Fiber"@en ;
    dcterms:identifier "fiber" ;
    rdfs:comment "Each term for the type of fiber used in the materials of the object, distinguished from the textile type, trimmings, or other materials."@en ;
    rdfs:range [ a owl:Class ;
            owl:oneOf ( cc:CC00160 cc:CC00195 cc:CC00196 cc:CC00197 cc:CC00201 cc:CC00202 cc:CC00205 cc:CC00213 cc:CC00216 cc:CC00225 cc:CC00226 cc:CC00230 cc:CC00233 cc:CC00234 cc:CC00235 cc:CC00242 cc:CC00243 cc:CC00244 cc:CC00250 cc:CC00273 cc:CC00274 cc:CC00282 cc:CC00288 cc:CC00299 cc:CC00303 cc:CC00630 ) ] .

cc:function a owl:ObjectProperty ;
    rdfs:label "Function"@en ;
    dcterms:identifier "function" ;
    rdfs:comment "Each function for which the object was worn. "@en ;
    rdfs:range [ a owl:Class ;
            owl:oneOf ( cc:CC00345 cc:CC00368 cc:CC00370 cc:CC00371 cc:CC00372 cc:CC00374 cc:CC00376 cc:CC00378 cc:CC00380 cc:CC00458 cc:CC00478 cc:CC00507 cc:CC00509 cc:CC00519 cc:CC00582 cc:CC00583 ) ] .

cc:gender a owl:ObjectProperty ;
    rdfs:label "Gender"@en ;
    dcterms:identifier "gender" ;
    rdfs:comment "The gender for which the object was originally intended."@en ;
    rdfs:range [ a owl:Class ;
            owl:oneOf ( cc:CC00364 cc:CC00365 cc:CC00366 cc:CC00479 cc:CC00480 ) ] .

cc:hasTechnique a owl:ObjectProperty ;
    rdfs:label "Technique"@en ;
    dcterms:identifier "hasTechnique" ;
    rdfs:comment """Each process involved in making the object. 

Do not include a description of where the technique is in evidence on the garment: that should be a part of the narrative description."""@en ;
    rdfs:range [ a owl:Class ;
            owl:oneOf ( cc:CC00074 cc:CC00075 cc:CC00076 cc:CC00077 cc:CC00078 cc:CC00080 cc:CC00082 cc:CC00083 cc:CC00084 cc:CC00085 cc:CC00086 cc:CC00087 cc:CC00088 cc:CC00089 cc:CC00090 cc:CC00092 cc:CC00093 cc:CC00094 cc:CC00095 cc:CC00096 cc:CC00097 cc:CC00098 cc:CC00100 cc:CC00101 cc:CC00103 cc:CC00116 cc:CC00127 cc:CC00170 cc:CC00173 cc:CC00254 cc:CC00257 cc:CC00325 cc:CC00393 cc:CC00514 cc:CC00597 ) ] ;
    rdfs:subPropertyOf vra:hasTechnique .

cc:hemCircumferenceIn a owl:ObjectProperty ;
    rdfs:label "Hem Circumference"@en ;
    dcterms:identifier "hemCircumferenceIn" ;
    rdfs:comment "The measurement all around the hem, in inches, as decimals to the nearest quarter inch."@en .

cc:hipsIn a owl:ObjectProperty ;
    rdfs:label "Hips"@en ;
    dcterms:identifier "hipsIn" ;
    rdfs:comment "The measurement straight around the fullest part of the hips, in inches, as decimals to the nearest quarter inch."@en .

cc:icomType a owl:ObjectProperty ;
    rdfs:label "ICOM Type"@en ;
    dcterms:identifier "icomType" ;
    rdfs:comment "The second and third level classes from the ICOM Vocabulary."@en ;
    rdfs:range [ a owl:Class ;
            owl:oneOf ( cc:CC00345 cc:CC00457 cc:CC00458 cc:CC00459 cc:CC00461 cc:CC00462 cc:CC00463 cc:CC00464 cc:CC00465 cc:CC00466 cc:CC00467 cc:CC00468 cc:CC00469 cc:CC00470 cc:CC00471 cc:CC00472 cc:CC00473 cc:CC00474 cc:CC00475 cc:CC00476 cc:CC00477 ) ] .

cc:length a owl:ObjectProperty ;
    rdfs:label "Length"@en ;
    dcterms:identifier "length" ;
    rdfs:comment "Each length of the object, where the hem lands on the body."@en ;
    rdfs:range [ a owl:Class ;
            owl:oneOf ( cc:CC00185 cc:CC00186 cc:CC00187 cc:CC00188 cc:CC00189 cc:CC00191 cc:CC00192 cc:CC00194 cc:CC00626 cc:CC00627 ) ] .

cc:lifeStages a owl:ObjectProperty ;
    rdfs:label "Life Stages"@en ;
    dcterms:identifier "lifeStages" ;
    rdfs:comment "Each age of the wearer for which the object was intended."@en ;
    rdfs:range [ a owl:Class ;
            owl:oneOf ( cc:CC00382 cc:CC00383 cc:CC00384 cc:CC00385 cc:CC00386 cc:CC00387 ) ] .

cc:liturgicalType a owl:ObjectProperty ;
    rdfs:label "Liturgical Type"@en ;
    dcterms:identifier "liturgicalType" ;
    rdfs:comment "Each type of liturgical garment or accessory."@en ;
    rdfs:range [ a owl:Class ;
            owl:oneOf ( cc:CC00441 cc:CC00442 cc:CC00443 cc:CC00444 cc:CC00445 cc:CC00446 cc:CC00447 cc:CC00448 cc:CC00449 cc:CC00450 cc:CC00451 cc:CC00452 ) ] .

cc:mannequin a owl:ObjectProperty ;
    rdfs:label "Mannequin"@en ;
    dcterms:identifier "mannequin" ;
    rdfs:comment "The size and year, or name, of any mannequins the garment fits on for display."@en .

cc:material a owl:ObjectProperty ;
    rdfs:label "Material"@en ;
    dcterms:identifier "material" ;
    rdfs:comment "Each material in the object."@en ;
    rdfs:range [ a owl:Class ;
            owl:oneOf ( cc:CC00160 cc:CC00195 cc:CC00196 cc:CC00197 cc:CC00199 cc:CC00200 cc:CC00201 cc:CC00202 cc:CC00203 cc:CC00204 cc:CC00205 cc:CC00206 cc:CC00208 cc:CC00211 cc:CC00212 cc:CC00213 cc:CC00214 cc:CC00215 cc:CC00216 cc:CC00217 cc:CC00218 cc:CC00219 cc:CC00220 cc:CC00221 cc:CC00222 cc:CC00224 cc:CC00225 cc:CC00226 cc:CC00227 cc:CC00229 cc:CC00230 cc:CC00232 cc:CC00233 cc:CC00234 cc:CC00235 cc:CC00236 cc:CC00238 cc:CC00239 cc:CC00241 cc:CC00242 cc:CC00243 cc:CC00244 cc:CC00245 cc:CC00247 cc:CC00248 cc:CC00249 cc:CC00250 cc:CC00259 cc:CC00260 cc:CC00261 cc:CC00262 cc:CC00264 cc:CC00266 cc:CC00267 cc:CC00268 cc:CC00269 cc:CC00270 cc:CC00272 cc:CC00273 cc:CC00274 cc:CC00275 cc:CC00276 cc:CC00278 cc:CC00279 cc:CC00280 cc:CC00281 cc:CC00282 cc:CC00283 cc:CC00284 cc:CC00285 cc:CC00286 cc:CC00288 cc:CC00289 cc:CC00292 cc:CC00293 cc:CC00294 cc:CC00295 cc:CC00296 cc:CC00297 cc:CC00298 cc:CC00299 cc:CC00302 cc:CC00303 cc:CC00304 cc:CC00305 cc:CC00306 cc:CC00307 cc:CC00308 cc:CC00311 cc:CC00312 cc:CC00313 cc:CC00314 cc:CC00315 cc:CC00316 cc:CC00317 cc:CC00318 cc:CC00319 cc:CC00321 cc:CC00322 cc:CC00594 cc:CC00628 cc:CC00630 ) ] ;
    rdfs:subPropertyOf vra:material .

cc:neckline a owl:ObjectProperty ;
    rdfs:label "Neckline"@en ;
    dcterms:identifier "neckline" ;
    rdfs:comment "Each type of neckline of the garment."@en ;
    rdfs:range [ a owl:Class ;
            owl:oneOf ( cc:CC00014 cc:CC00015 cc:CC00016 cc:CC00017 cc:CC00020 cc:CC00021 cc:CC00024 cc:CC00025 cc:CC00026 cc:CC00027 cc:CC00034 cc:CC00035 cc:CC00119 cc:CC00489 cc:CC00490 cc:CC00491 ) ] .

cc:otherMaterials a owl:ObjectProperty ;
    rdfs:label "Other Materials"@en ;
    dcterms:identifier "otherMaterials" ;
    rdfs:comment "Any other material terms that do not describe fibers, textiles, or trimmings."@en ;
    rdfs:range [ a owl:Class ;
            owl:oneOf ( cc:CC00199 cc:CC00211 cc:CC00215 cc:CC00220 cc:CC00224 cc:CC00232 cc:CC00241 cc:CC00248 cc:CC00249 cc:CC00259 cc:CC00261 cc:CC00267 cc:CC00279 cc:CC00284 cc:CC00292 cc:CC00295 cc:CC00296 cc:CC00297 cc:CC00302 cc:CC00305 cc:CC00306 cc:CC00308 cc:CC00311 cc:CC00313 cc:CC00318 cc:CC00322 ) ] .

cc:pantsType a owl:ObjectProperty ;
    rdfs:label "Pants Type"@en ;
    dcterms:identifier "pantsType" ;
    rdfs:comment "Each term that describes the length and shape of pants."@en ;
    rdfs:range [ a owl:Class ;
            owl:oneOf ( cc:CC00420 cc:CC00422 cc:CC00423 cc:CC00424 cc:CC00425 cc:CC00426 cc:CC00427 cc:CC00429 cc:CC00432 cc:CC00433 cc:CC00434 cc:CC00435 cc:CC00436 cc:CC00517 cc:CC00524 ) ] .

cc:pattern a owl:ObjectProperty ;
    rdfs:label "Pattern"@en ;
    dcterms:identifier "pattern" ;
    rdfs:comment "Each design motif appearing on the object."@en ;
    rdfs:range [ a owl:Class ;
            owl:oneOf ( cc:CC00277 cc:CC00300 cc:CC00453 cc:CC00454 cc:CC00455 cc:CC00456 cc:CC00584 cc:CC00585 cc:CC00586 cc:CC00587 cc:CC00588 cc:CC00589 cc:CC00590 cc:CC00591 cc:CC00592 cc:CC00593 cc:CC00595 cc:CC00596 ) ] .

cc:privateInformation a owl:ObjectProperty ;
    rdfs:label "Private Information"@en ;
    dcterms:identifier "privateInformation" ;
    rdfs:comment "Any information that doesn't fit elsewhere, and isn't suited for public view (for example private stories or communication with the donor)."@en .

cc:publicInformation a owl:ObjectProperty ;
    rdfs:label "Public Information"@en ;
    dcterms:identifier "publicInformation" ;
    rdfs:comment """A brief narrative about the object, with any interesting / important information (numbers in parentheses can provide links to external references, which then are also listed in reference field).

Include MLA style parenthetical citations to references listed in References field as needed."""@en .

cc:rights a owl:ObjectProperty ;
    rdfs:label "Rights"@en ;
    dcterms:identifier "rights" ;
    rdfs:comment "A standardized rights statement. In most cases, clothing artifacts are not protected by copyright, but may be represented in images that are under copyright."@en ;
    rdfs:range [ a owl:Class ;
            owl:oneOf ( cc:CC00613 cc:CC00614 cc:CC00615 cc:CC00616 cc:CC00617 cc:CC00618 cc:CC00619 cc:CC00620 cc:CC00621 cc:CC00622 cc:CC00623 cc:CC00624 cc:CC00625 ) ] ;
    rdfs:subPropertyOf dcterms:rights .

cc:size a owl:ObjectProperty ;
    rdfs:label "Size"@en ;
    dcterms:identifier "size" ;
    rdfs:comment "The size of the object, if shown on a label or otherwise identified."@en .

cc:skirtType a owl:ObjectProperty ;
    rdfs:label "Skirt Type"@en ;
    dcterms:identifier "skirtType" ;
    rdfs:comment "Each term that describes the skirt of the garment."@en ;
    rdfs:range [ a owl:Class ;
            owl:oneOf ( cc:CC00102 cc:CC00129 cc:CC00164 cc:CC00166 cc:CC00167 cc:CC00168 cc:CC00171 cc:CC00175 cc:CC00177 cc:CC00179 cc:CC00180 cc:CC00182 cc:CC00183 cc:CC00251 cc:CC00255 cc:CC00510 cc:CC00511 cc:CC00512 cc:CC00513 ) ] .

cc:sleeveLength a owl:ObjectProperty ;
    rdfs:label "Sleeve Length"@en ;
    dcterms:identifier "sleeveLength" ;
    rdfs:comment "Each term that describes the length of the sleeves of the garment."@en ;
    rdfs:range [ a owl:Class ;
            owl:oneOf ( cc:CC00144 cc:CC00145 cc:CC00146 cc:CC00147 cc:CC00148 cc:CC00149 ) ] .

cc:sleeveType a owl:ObjectProperty ;
    rdfs:label "Sleeve Type"@en ;
    dcterms:identifier "sleeveType" ;
    rdfs:comment "Each term that describes the shape of the sleeves of the garment."@en ;
    rdfs:range [ a owl:Class ;
            owl:oneOf ( cc:CC00128 cc:CC00130 cc:CC00131 cc:CC00135 cc:CC00136 cc:CC00137 cc:CC00138 cc:CC00139 cc:CC00141 cc:CC00150 cc:CC00256 cc:CC00326 cc:CC00355 cc:CC00356 cc:CC00357 cc:CC00362 cc:CC00367 cc:CC00401 ) ] .

cc:socioEconomicClass a owl:ObjectProperty ;
    rdfs:label "Socio Economic Class"@en ;
    dcterms:identifier "socioEconomicClass" ;
    rdfs:comment "Each term that indicates the socioeconomic class of the person(s) who wore the object. This can have multiple values to show that the object was passed up or down through different classes."@en ;
    rdfs:range [ a owl:Class ;
            owl:oneOf ( cc:CC00389 cc:CC00390 cc:CC00391 ) ] .

cc:storageLocation a owl:ObjectProperty ;
    rdfs:label "Storage Location"@en ;
    dcterms:identifier "storageLocation" ;
    rdfs:comment "Where the garment has been put away in storage, for example by shelf section, ex. \"C4\""@en .

cc:temporal a owl:ObjectProperty ;
    rdfs:label "Style Period"@en ;
    dcterms:identifier "temporal" ;
    rdfs:comment """Each decade (or longer fashion style periods) in which the object was made or used. 

Do not include an apostrophe in a decade name; just add an "s," like "1950s.\""""@en ;
    rdfs:range [ a owl:Class ;
            owl:oneOf ( cc:CC00527 cc:CC00528 cc:CC00529 cc:CC00530 cc:CC00531 cc:CC00532 cc:CC00533 cc:CC00534 cc:CC00535 cc:CC00536 cc:CC00537 cc:CC00538 cc:CC00539 cc:CC00540 cc:CC00541 cc:CC00542 cc:CC00543 cc:CC00544 cc:CC00545 cc:CC00546 cc:CC00547 cc:CC00548 cc:CC00549 cc:CC00550 cc:CC00551 cc:CC00552 cc:CC00553 cc:CC00554 cc:CC00555 cc:CC00556 cc:CC00557 cc:CC00558 cc:CC00559 cc:CC00560 cc:CC00561 cc:CC00562 cc:CC00563 cc:CC00564 cc:CC00565 cc:CC00566 cc:CC00567 cc:CC00568 cc:CC00569 cc:CC00570 cc:CC00571 cc:CC00572 cc:CC00573 cc:CC00574 cc:CC00575 cc:CC00576 cc:CC00577 cc:CC00578 cc:CC00579 ) ] ;
    rdfs:subPropertyOf dcterms:temporal .

cc:textileMaterials a owl:ObjectProperty ;
    rdfs:label "Textile Materials"@en ;
    dcterms:identifier "textileMaterials" ;
    rdfs:comment "Each term for materials produced from component fibers, distinguished from the fibers, trimmings, or other materials."@en ;
    rdfs:range [ a owl:Class ;
            owl:oneOf ( cc:CC00200 cc:CC00203 cc:CC00204 cc:CC00206 cc:CC00208 cc:CC00212 cc:CC00214 cc:CC00217 cc:CC00218 cc:CC00219 cc:CC00221 cc:CC00222 cc:CC00227 cc:CC00229 cc:CC00236 cc:CC00239 cc:CC00245 cc:CC00247 cc:CC00260 cc:CC00266 cc:CC00268 cc:CC00269 cc:CC00270 cc:CC00275 cc:CC00280 cc:CC00281 cc:CC00283 cc:CC00285 cc:CC00289 cc:CC00293 cc:CC00294 cc:CC00298 cc:CC00315 cc:CC00316 cc:CC00319 cc:CC00594 ) ] .

cc:treatment a owl:ObjectProperty ;
    rdfs:label "Treatment"@en ;
    dcterms:identifier "treatment" ;
    rdfs:comment "All procedures that have been completed to repair, conserve, stabilize, or display an object, in a narrative paragraph."@en .

cc:trimming a owl:ObjectProperty ;
    rdfs:label "Trimming"@en ;
    dcterms:identifier "trimming" ;
    rdfs:comment "Each term for decorative material added to an object, distinguished from the fibers, textile type,  or other materials."@en ;
    rdfs:range [ a owl:Class ;
            owl:oneOf ( cc:CC00238 cc:CC00262 cc:CC00264 cc:CC00272 cc:CC00276 cc:CC00278 cc:CC00286 cc:CC00304 cc:CC00307 cc:CC00312 cc:CC00317 cc:CC00321 cc:CC00628 ) ] .

cc:type a owl:ObjectProperty ;
    rdfs:label "Type"@en ;
    dcterms:identifier "type" ;
    rdfs:comment "All clothing objects will have DCMI type \"Physical Object.\" "@en ;
    rdfs:range [ a owl:Class ;
            owl:oneOf ( cc:CC00403 cc:CC00404 cc:CC00405 cc:CC00406 cc:CC00407 cc:CC00408 cc:CC00409 cc:CC00410 cc:CC00411 cc:CC00412 cc:CC00413 cc:CC00414 ) ] ;
    rdfs:subPropertyOf dcterms:type .

cc:underarmToWaistIn a owl:ObjectProperty ;
    rdfs:label "Underarm To Waist"@en ;
    dcterms:identifier "underarmToWaistIn" ;
    rdfs:comment "The measurement from armpit to waist at the side seam, in inches, as decimals to the nearest quarter inch."@en .

cc:waistIn a owl:ObjectProperty ;
    rdfs:label "Waist"@en ;
    dcterms:identifier "waistIn" ;
    rdfs:comment "The measurement straight around the narrowest part of the waist, in inches, as decimals to the nearest quarter inch."@en .

cc:waistline a owl:ObjectProperty ;
    rdfs:label "Waistline"@en ;
    dcterms:identifier "waistline" ;
    rdfs:comment "Each term that describes the level and shape of the waist of the garment."@en ;
    rdfs:range [ a owl:Class ;
            owl:oneOf ( cc:CC00151 cc:CC00152 cc:CC00153 cc:CC00156 cc:CC00157 cc:CC00158 cc:CC00159 cc:CC00161 cc:CC00162 cc:CC00228 ) ] .

cc:workType a owl:ObjectProperty ;
    rdfs:label "Work Type"@en ;
    dcterms:identifier "workType" ;
    rdfs:comment "Each top-level work type of the object. More specific terms are possible as sub-categories, in other fields, or can be included in the description."@en ;
    rdfs:range [ a owl:Class ;
            owl:oneOf ( cc:CC00046 cc:CC00106 cc:CC00335 cc:CC00339 cc:CC00341 cc:CC00342 cc:CC00343 cc:CC00344 cc:CC00345 cc:CC00346 cc:CC00428 cc:CC00525 cc:CC00600 cc:CC00601 cc:CC00602 cc:CC00603 cc:CC00604 cc:CC00605 cc:CC00606 cc:CC00607 cc:CC00608 cc:CC00610 cc:CC00611 ) ] .

cc:wornBy a owl:ObjectProperty ;
    rdfs:label "Worn by"@en ;
    dcterms:identifier "wornBy" ;
    rdfs:comment "Full name(s) of anyone known to have worn a costume artifact."@en ;
    rdfs:subPropertyOf <http://www.wikidata.org/entity/P7376> .

<http://vocab.getty.edu/aat/300009766> a owl:NamedIndividual ;
    owl:sameAs cc:CC00587 .

<http://vocab.getty.edu/aat/300009791> a owl:NamedIndividual ;
    owl:sameAs cc:CC00453 .

<http://vocab.getty.edu/aat/300009811> a owl:NamedIndividual ;
    owl:sameAs cc:CC00455 .

<http://vocab.getty.edu/aat/300010128> a owl:NamedIndividual ;
    owl:sameAs cc:CC00456 .

<http://vocab.getty.edu/aat/300010135> a owl:NamedIndividual ;
    owl:sameAs cc:CC00277 .

<http://vocab.getty.edu/aat/300010230> a owl:NamedIndividual ;
    owl:sameAs cc:CC00454 .

<http://vocab.getty.edu/aat/300010305> a owl:NamedIndividual ;
    owl:sameAs cc:CC00156 .

<http://vocab.getty.edu/aat/300010357> a owl:NamedIndividual ;
    owl:sameAs cc:CC00488 .

<http://vocab.getty.edu/aat/300010662> a owl:NamedIndividual ;
    owl:sameAs cc:CC00302 .

<http://vocab.getty.edu/aat/300010797> a owl:NamedIndividual ;
    owl:sameAs cc:CC00215 .

<http://vocab.getty.edu/aat/300010806> a owl:NamedIndividual ;
    owl:sameAs cc:CC00304 .

<http://vocab.getty.edu/aat/300010900> a owl:NamedIndividual ;
    owl:sameAs cc:CC00224 .

<http://vocab.getty.edu/aat/300010946> a owl:NamedIndividual ;
    owl:sameAs cc:CC00265 .

<http://vocab.getty.edu/aat/300011063> a owl:NamedIndividual ;
    owl:sameAs cc:CC00322 .

<http://vocab.getty.edu/aat/300011809> a owl:NamedIndividual ;
    owl:sameAs cc:CC00276 .

<http://vocab.getty.edu/aat/300011811> a owl:NamedIndividual ;
    owl:sameAs cc:CC00279 .

<http://vocab.getty.edu/aat/300011816> a owl:NamedIndividual ;
    owl:sameAs cc:CC00201 .

<http://vocab.getty.edu/aat/300011819> a owl:NamedIndividual ;
    owl:sameAs cc:CC00282 .

<http://vocab.getty.edu/aat/300011827> a owl:NamedIndividual ;
    owl:sameAs cc:CC00297 .

<http://vocab.getty.edu/aat/300011829> a owl:NamedIndividual ;
    owl:sameAs cc:CC00241 .

<http://vocab.getty.edu/aat/300011835> a owl:NamedIndividual ;
    owl:sameAs cc:CC00292 .

<http://vocab.getty.edu/aat/300011840> a owl:NamedIndividual ;
    owl:sameAs cc:CC00308 .

<http://vocab.getty.edu/aat/300011845> a owl:NamedIndividual ;
    owl:sameAs cc:CC00220 .

<http://vocab.getty.edu/aat/300011908> a owl:NamedIndividual ;
    owl:sameAs cc:CC00311 .

<http://vocab.getty.edu/aat/300011914> a owl:NamedIndividual ;
    owl:sameAs cc:CC00249 .

<http://vocab.getty.edu/aat/300012941> a owl:NamedIndividual ;
    owl:sameAs cc:CC00306 .

<http://vocab.getty.edu/aat/300012959> a owl:NamedIndividual ;
    owl:sameAs cc:CC00309 .

<http://vocab.getty.edu/aat/300014041> a owl:NamedIndividual ;
    owl:sameAs cc:CC00630 .

<http://vocab.getty.edu/aat/300014043> a owl:NamedIndividual ;
    owl:sameAs cc:CC00216 .

<http://vocab.getty.edu/aat/300014051> a owl:NamedIndividual ;
    owl:sameAs cc:CC00303 .

<http://vocab.getty.edu/aat/300014058> a owl:NamedIndividual ;
    owl:sameAs cc:CC00244 .

<http://vocab.getty.edu/aat/300014059> a owl:NamedIndividual ;
    owl:sameAs cc:CC00235 .

<http://vocab.getty.edu/aat/300014067> a owl:NamedIndividual ;
    owl:sameAs cc:CC00205 .

<http://vocab.getty.edu/aat/300014069> a owl:NamedIndividual ;
    owl:sameAs cc:CC00221 .

<http://vocab.getty.edu/aat/300014071> a owl:NamedIndividual ;
    owl:sameAs cc:CC00234 .

<http://vocab.getty.edu/aat/300014080> a owl:NamedIndividual ;
    owl:sameAs cc:CC00204 .

<http://vocab.getty.edu/aat/300014083> a owl:NamedIndividual ;
    owl:sameAs cc:CC00281 .

<http://vocab.getty.edu/aat/300014087> a owl:NamedIndividual ;
    owl:sameAs cc:CC00293 .

<http://vocab.getty.edu/aat/300014107> a owl:NamedIndividual ;
    owl:sameAs cc:CC00212 .

<http://vocab.getty.edu/aat/300014109> a owl:NamedIndividual ;
    owl:sameAs cc:CC00296 .

<http://vocab.getty.edu/aat/300014224> a owl:NamedIndividual ;
    owl:sameAs cc:CC00267 .

<http://vocab.getty.edu/aat/300014247> a owl:NamedIndividual ;
    owl:sameAs cc:CC00272 .

<http://vocab.getty.edu/aat/300014248> a owl:NamedIndividual ;
    owl:sameAs cc:CC00305 .

<http://vocab.getty.edu/aat/300014250> a owl:NamedIndividual ;
    owl:sameAs cc:CC00313 .

<http://vocab.getty.edu/aat/300014462> a owl:NamedIndividual ;
    owl:sameAs cc:CC00230 .

<http://vocab.getty.edu/aat/300014502> a owl:NamedIndividual ;
    owl:sameAs cc:CC00318 .

<http://vocab.getty.edu/aat/300014570> a owl:NamedIndividual ;
    owl:sameAs cc:CC00232 .

<http://vocab.getty.edu/aat/300014585> a owl:NamedIndividual ;
    owl:sameAs cc:CC00248 .

<http://vocab.getty.edu/aat/300014668> a owl:NamedIndividual ;
    owl:sameAs cc:CC00238 .

<http://vocab.getty.edu/aat/300014801> a owl:NamedIndividual ;
    owl:sameAs cc:CC00259 .

<http://vocab.getty.edu/aat/300015029> a owl:NamedIndividual ;
    owl:sameAs cc:CC00295 .

<http://vocab.getty.edu/aat/300022238> a owl:NamedIndividual ;
    owl:sameAs cc:CC00486 .

<http://vocab.getty.edu/aat/300024967> a owl:NamedIndividual ;
    owl:sameAs cc:CC00447 .

<http://vocab.getty.edu/aat/300026029> a owl:NamedIndividual ;
    owl:sameAs cc:CC00484 .

<http://vocab.getty.edu/aat/300037335> a owl:NamedIndividual ;
    owl:sameAs cc:CC00483 .

<http://vocab.getty.edu/aat/300045514> a owl:NamedIndividual ;
    owl:sameAs cc:CC00284 .

<http://vocab.getty.edu/aat/300045611> a owl:NamedIndividual ;
    owl:sameAs cc:CC00481 .

<http://vocab.getty.edu/aat/300046133> a owl:NamedIndividual ;
    owl:sameAs cc:CC00337 .

<http://vocab.getty.edu/aat/300046135> a owl:NamedIndividual ;
    owl:sameAs cc:CC00422 .

<http://vocab.getty.edu/aat/300046140> a owl:NamedIndividual ;
    owl:sameAs cc:CC00602 .

<http://vocab.getty.edu/aat/300046143> a owl:NamedIndividual ;
    owl:sameAs cc:CC00106 .

<http://vocab.getty.edu/aat/300046159> a owl:NamedIndividual ;
    owl:sameAs cc:CC00335 .

<http://vocab.getty.edu/aat/300046164> a owl:NamedIndividual ;
    owl:sameAs cc:CC00112 .

<http://vocab.getty.edu/aat/300046167> a owl:NamedIndividual ;
    owl:sameAs cc:CC00339 .

<http://vocab.getty.edu/aat/300046171> a owl:NamedIndividual ;
    owl:sameAs cc:CC00133 .

<http://vocab.getty.edu/aat/300046174> a owl:NamedIndividual ;
    owl:sameAs cc:CC00501 .

<http://vocab.getty.edu/aat/300046184> a owl:NamedIndividual ;
    owl:sameAs cc:CC00430 .

<http://vocab.getty.edu/aat/300046186> a owl:NamedIndividual ;
    owl:sameAs cc:CC00114 .

<http://vocab.getty.edu/aat/300051508> a owl:NamedIndividual ;
    owl:sameAs cc:CC00004 .

<http://vocab.getty.edu/aat/300053319> a owl:NamedIndividual ;
    owl:sameAs cc:CC00097 .

<http://vocab.getty.edu/aat/300053632> a owl:NamedIndividual ;
    owl:sameAs cc:CC00078 .

<http://vocab.getty.edu/aat/300053634> a owl:NamedIndividual ;
    owl:sameAs cc:CC00086 .

<http://vocab.getty.edu/aat/300053638> a owl:NamedIndividual ;
    owl:sameAs cc:CC00076 .

<http://vocab.getty.edu/aat/300053642> a owl:NamedIndividual ;
    owl:sameAs cc:CC00101 .

<http://vocab.getty.edu/aat/300053643> a owl:NamedIndividual ;
    owl:sameAs cc:CC00085 .

<http://vocab.getty.edu/aat/300053646> a owl:NamedIndividual ;
    owl:sameAs cc:CC00074 .

<http://vocab.getty.edu/aat/300053651> a owl:NamedIndividual ;
    owl:sameAs cc:CC00087 .

<http://vocab.getty.edu/aat/300053652> a owl:NamedIndividual ;
    owl:sameAs cc:CC00090 .

<http://vocab.getty.edu/aat/300053653> a owl:NamedIndividual ;
    owl:sameAs cc:CC00254 .

<http://vocab.getty.edu/aat/300053656> a owl:NamedIndividual ;
    owl:sameAs cc:CC00098 .

<http://vocab.getty.edu/aat/300053786> a owl:NamedIndividual ;
    owl:sameAs cc:CC00082 .

<http://vocab.getty.edu/aat/300053826> a owl:NamedIndividual ;
    owl:sameAs cc:CC00080 .

<http://vocab.getty.edu/aat/300053867> a owl:NamedIndividual ;
    owl:sameAs cc:CC00096 .

<http://vocab.getty.edu/aat/300053914> a owl:NamedIndividual ;
    owl:sameAs cc:CC00083 .

<http://vocab.getty.edu/aat/300054216> a owl:NamedIndividual ;
    owl:sameAs cc:CC00092 .

<http://vocab.getty.edu/aat/300055481> a owl:NamedIndividual ;
    owl:sameAs cc:CC00390 .

<http://vocab.getty.edu/aat/300055483> a owl:NamedIndividual ;
    owl:sameAs cc:CC00391 .

<http://vocab.getty.edu/aat/300055485> a owl:NamedIndividual ;
    owl:sameAs cc:CC00389 .

<http://vocab.getty.edu/aat/300061985> a owl:NamedIndividual ;
    owl:sameAs cc:CC00257 .

<http://vocab.getty.edu/aat/300078755> a owl:NamedIndividual ;
    owl:sameAs cc:CC00162 .

<http://vocab.getty.edu/aat/300080226> a owl:NamedIndividual ;
    owl:sameAs cc:CC00006 .

<http://vocab.getty.edu/aat/300123034> a owl:NamedIndividual ;
    owl:sameAs cc:CC00173 .

<http://vocab.getty.edu/aat/300124707> a owl:NamedIndividual ;
    owl:sameAs cc:CC00065 .

<http://vocab.getty.edu/aat/300126225> a owl:NamedIndividual ;
    owl:sameAs cc:CC00067 .

<http://vocab.getty.edu/aat/300126734> a owl:NamedIndividual ;
    owl:sameAs cc:CC00064 .

<http://vocab.getty.edu/aat/300127490> a owl:NamedIndividual ;
    owl:sameAs cc:CC00052 .

<http://vocab.getty.edu/aat/300127794> a owl:NamedIndividual ;
    owl:sameAs cc:CC00073 .

<http://vocab.getty.edu/aat/300128438> a owl:NamedIndividual ;
    owl:sameAs cc:CC00059 .

<http://vocab.getty.edu/aat/300129361> a owl:NamedIndividual ;
    owl:sameAs cc:CC00051 .

<http://vocab.getty.edu/aat/300129784> a owl:NamedIndividual ;
    owl:sameAs cc:CC00072 .

<http://vocab.getty.edu/aat/300130257> a owl:NamedIndividual ;
    owl:sameAs cc:CC00066 .

<http://vocab.getty.edu/aat/300130811> a owl:NamedIndividual ;
    owl:sameAs cc:CC00058 .

<http://vocab.getty.edu/aat/300130920> a owl:NamedIndividual ;
    owl:sameAs cc:CC00050 .

<http://vocab.getty.edu/aat/300132861> a owl:NamedIndividual ;
    owl:sameAs cc:CC00219 .

<http://vocab.getty.edu/aat/300132876> a owl:NamedIndividual ;
    owl:sameAs cc:CC00270 .

<http://vocab.getty.edu/aat/300132879> a owl:NamedIndividual ;
    owl:sameAs cc:CC00273 .

<http://vocab.getty.edu/aat/300132896> a owl:NamedIndividual ;
    owl:sameAs cc:CC00269 .

<http://vocab.getty.edu/aat/300132902> a owl:NamedIndividual ;
    owl:sameAs cc:CC00239 .

<http://vocab.getty.edu/aat/300133711> a owl:NamedIndividual ;
    owl:sameAs cc:CC00247 .

<http://vocab.getty.edu/aat/300133751> a owl:NamedIndividual ;
    owl:sameAs cc:CC00310 .

<http://vocab.getty.edu/aat/300136012> a owl:NamedIndividual ;
    owl:sameAs cc:CC00485 .

<http://vocab.getty.edu/aat/300148821> a owl:NamedIndividual ;
    owl:sameAs cc:CC00606 .

<http://vocab.getty.edu/aat/300162391> a owl:NamedIndividual ;
    owl:sameAs cc:CC00271 .

<http://vocab.getty.edu/aat/300163224> a owl:NamedIndividual ;
    owl:sameAs cc:CC00475 .

<http://vocab.getty.edu/aat/300163295> a owl:NamedIndividual ;
    owl:sameAs cc:CC00208 .

<http://vocab.getty.edu/aat/300179869> a owl:NamedIndividual ;
    owl:sameAs cc:CC00487 .

<http://vocab.getty.edu/aat/300183634> a owl:NamedIndividual ;
    owl:sameAs cc:CC00260 .

<http://vocab.getty.edu/aat/300183741> a owl:NamedIndividual ;
    owl:sameAs cc:CC00206 .

<http://vocab.getty.edu/aat/300183798> a owl:NamedIndividual ;
    owl:sameAs cc:CC00314 .

<http://vocab.getty.edu/aat/300183896> a owl:NamedIndividual ;
    owl:sameAs cc:CC00307 .

<http://vocab.getty.edu/aat/300189588> a owl:NamedIndividual ;
    owl:sameAs cc:CC00382 .

<http://vocab.getty.edu/aat/300189590> a owl:NamedIndividual ;
    owl:sameAs cc:CC00383 .

<http://vocab.getty.edu/aat/300189595> a owl:NamedIndividual ;
    owl:sameAs cc:CC00384 .

<http://vocab.getty.edu/aat/300189598> a owl:NamedIndividual ;
    owl:sameAs cc:CC00385 .

<http://vocab.getty.edu/aat/300189599> a owl:NamedIndividual ;
    owl:sameAs cc:CC00386 .

<http://vocab.getty.edu/aat/300189603> a owl:NamedIndividual ;
    owl:sameAs cc:CC00387 .

<http://vocab.getty.edu/aat/300192989> a owl:NamedIndividual ;
    owl:sameAs cc:CC00226 .

<http://vocab.getty.edu/aat/300197322> a owl:NamedIndividual ;
    owl:sameAs cc:CC00443 .

<http://vocab.getty.edu/aat/300198926> a owl:NamedIndividual ;
    owl:sameAs cc:CC00612 .

<http://vocab.getty.edu/aat/300204872> a owl:NamedIndividual ;
    owl:sameAs cc:CC00446 .

<http://vocab.getty.edu/aat/300204880> a owl:NamedIndividual ;
    owl:sameAs cc:CC00451 .

<http://vocab.getty.edu/aat/300204912> a owl:NamedIndividual ;
    owl:sameAs cc:CC00321 .

<http://vocab.getty.edu/aat/300209261> a owl:NamedIndividual ;
    owl:sameAs cc:CC00482 .

<http://vocab.getty.edu/aat/300209266> a owl:NamedIndividual ;
    owl:sameAs cc:CC00459 .

<http://vocab.getty.edu/aat/300209267> a owl:NamedIndividual ;
    owl:sameAs cc:CC00345 .

<http://vocab.getty.edu/aat/300209268> a owl:NamedIndividual ;
    owl:sameAs cc:CC00461 .

<http://vocab.getty.edu/aat/300209274> a owl:NamedIndividual ;
    owl:sameAs cc:CC00463 .

<http://vocab.getty.edu/aat/300209275> a owl:NamedIndividual ;
    owl:sameAs cc:CC00471 .

<http://vocab.getty.edu/aat/300209278> a owl:NamedIndividual ;
    owl:sameAs cc:CC00477 .

<http://vocab.getty.edu/aat/300209279> a owl:NamedIndividual ;
    owl:sameAs cc:CC00476 .

<http://vocab.getty.edu/aat/300209280> a owl:NamedIndividual ;
    owl:sameAs cc:CC00603 .

<http://vocab.getty.edu/aat/300209282> a owl:NamedIndividual ;
    owl:sameAs cc:CC00469 .

<http://vocab.getty.edu/aat/300209283> a owl:NamedIndividual ;
    owl:sameAs cc:CC00468 .

<http://vocab.getty.edu/aat/300209285> a owl:NamedIndividual ;
    owl:sameAs cc:CC00608 .

<http://vocab.getty.edu/aat/300209286> a owl:NamedIndividual ;
    owl:sameAs cc:CC00610 .

<http://vocab.getty.edu/aat/300209826> a owl:NamedIndividual ;
    owl:sameAs cc:CC00323 .

<http://vocab.getty.edu/aat/300209837> a owl:NamedIndividual ;
    owl:sameAs cc:CC00113 .

<http://vocab.getty.edu/aat/300209844> a owl:NamedIndividual ;
    owl:sameAs cc:CC00611 .

<http://vocab.getty.edu/aat/300209852> a owl:NamedIndividual ;
    owl:sameAs cc:CC00604 .

<http://vocab.getty.edu/aat/300209863> a owl:NamedIndividual ;
    owl:sameAs cc:CC00342 .

<http://vocab.getty.edu/aat/300209868> a owl:NamedIndividual ;
    owl:sameAs cc:CC00125 .

<http://vocab.getty.edu/aat/300209869> a owl:NamedIndividual ;
    owl:sameAs cc:CC00126 .

<http://vocab.getty.edu/aat/300209874> a owl:NamedIndividual ;
    owl:sameAs cc:CC00336 .

<http://vocab.getty.edu/aat/300209876> a owl:NamedIndividual ;
    owl:sameAs cc:CC00155 .

<http://vocab.getty.edu/aat/300209885> a owl:NamedIndividual ;
    owl:sameAs cc:CC00016 .

<http://vocab.getty.edu/aat/300209896> a owl:NamedIndividual ;
    owl:sameAs cc:CC00041 .

<http://vocab.getty.edu/aat/300209900> a owl:NamedIndividual ;
    owl:sameAs cc:CC00343 .

<http://vocab.getty.edu/aat/300209904> a owl:NamedIndividual ;
    owl:sameAs cc:CC00346 .

<http://vocab.getty.edu/aat/300209918> a owl:NamedIndividual ;
    owl:sameAs cc:CC00426 .

<http://vocab.getty.edu/aat/300209919> a owl:NamedIndividual ;
    owl:sameAs cc:CC00427 .

<http://vocab.getty.edu/aat/300209926> a owl:NamedIndividual ;
    owl:sameAs cc:CC00431 .

<http://vocab.getty.edu/aat/300209928> a owl:NamedIndividual ;
    owl:sameAs cc:CC00179 .

<http://vocab.getty.edu/aat/300209930> a owl:NamedIndividual ;
    owl:sameAs cc:CC00525 .

<http://vocab.getty.edu/aat/300209932> a owl:NamedIndividual ;
    owl:sameAs cc:CC00341 .

<http://vocab.getty.edu/aat/300209934> a owl:NamedIndividual ;
    owl:sameAs cc:CC00435 .

<http://vocab.getty.edu/aat/300209935> a owl:NamedIndividual ;
    owl:sameAs cc:CC00344 .

<http://vocab.getty.edu/aat/300209984> a owl:NamedIndividual ;
    owl:sameAs cc:CC00605 .

<http://vocab.getty.edu/aat/300209991> a owl:NamedIndividual ;
    owl:sameAs cc:CC00046 .

<http://vocab.getty.edu/aat/300210015> a owl:NamedIndividual ;
    owl:sameAs cc:CC00356 .

<http://vocab.getty.edu/aat/300210017> a owl:NamedIndividual ;
    owl:sameAs cc:CC00400 .

<http://vocab.getty.edu/aat/300210052> a owl:NamedIndividual ;
    owl:sameAs cc:CC00028 .

<http://vocab.getty.edu/aat/300210054> a owl:NamedIndividual ;
    owl:sameAs cc:CC00030 .

<http://vocab.getty.edu/aat/300210062> a owl:NamedIndividual ;
    owl:sameAs cc:CC00036 .

<http://vocab.getty.edu/aat/300210423> a owl:NamedIndividual ;
    owl:sameAs cc:CC00444 .

<http://vocab.getty.edu/aat/300210424> a owl:NamedIndividual ;
    owl:sameAs cc:CC00445 .

<http://vocab.getty.edu/aat/300210429> a owl:NamedIndividual ;
    owl:sameAs cc:CC00448 .

<http://vocab.getty.edu/aat/300210431> a owl:NamedIndividual ;
    owl:sameAs cc:CC00449 .

<http://vocab.getty.edu/aat/300210488> a owl:NamedIndividual ;
    owl:sameAs cc:CC00394 .

<http://vocab.getty.edu/aat/300210517> a owl:NamedIndividual ;
    owl:sameAs cc:CC00397 .

<http://vocab.getty.edu/aat/300210527> a owl:NamedIndividual ;
    owl:sameAs cc:CC00398 .

<http://vocab.getty.edu/aat/300210530> a owl:NamedIndividual ;
    owl:sameAs cc:CC00358 .

<http://vocab.getty.edu/aat/300210535> a owl:NamedIndividual ;
    owl:sameAs cc:CC00367 .

<http://vocab.getty.edu/aat/300210537> a owl:NamedIndividual ;
    owl:sameAs cc:CC00524 .

<http://vocab.getty.edu/aat/300210542> a owl:NamedIndividual ;
    owl:sameAs cc:CC00105 .

<http://vocab.getty.edu/aat/300210554> a owl:NamedIndividual ;
    owl:sameAs cc:CC00107 .

<http://vocab.getty.edu/aat/300210564> a owl:NamedIndividual ;
    owl:sameAs cc:CC00123 .

<http://vocab.getty.edu/aat/300210580> a owl:NamedIndividual ;
    owl:sameAs cc:CC00104 .

<http://vocab.getty.edu/aat/300211599> a owl:NamedIndividual ;
    owl:sameAs cc:CC00470 .

<http://vocab.getty.edu/aat/300211601> a owl:NamedIndividual ;
    owl:sameAs cc:CC00464 .

<http://vocab.getty.edu/aat/300211602> a owl:NamedIndividual ;
    owl:sameAs cc:CC00467 .

<http://vocab.getty.edu/aat/300211788> a owl:NamedIndividual ;
    owl:sameAs cc:CC00121 .

<http://vocab.getty.edu/aat/300212393> a owl:NamedIndividual ;
    owl:sameAs cc:CC00378 .

<http://vocab.getty.edu/aat/300212499> a owl:NamedIndividual ;
    owl:sameAs cc:CC00340 .

<http://vocab.getty.edu/aat/300214558> a owl:NamedIndividual ;
    owl:sameAs cc:CC00517 .

<http://vocab.getty.edu/aat/300215860> a owl:NamedIndividual ;
    owl:sameAs cc:CC00493 .

<http://vocab.getty.edu/aat/300216195> a owl:NamedIndividual ;
    owl:sameAs cc:CC00172 .

<http://vocab.getty.edu/aat/300216954> a owl:NamedIndividual ;
    owl:sameAs cc:CC00434 .

<http://vocab.getty.edu/aat/300217242> a owl:NamedIndividual ;
    owl:sameAs cc:CC00029 .

<http://vocab.getty.edu/aat/300220740> a owl:NamedIndividual ;
    owl:sameAs cc:CC00609 .

<http://vocab.getty.edu/aat/300220742> a owl:NamedIndividual ;
    owl:sameAs cc:CC00334 .

<http://vocab.getty.edu/aat/300221269> a owl:NamedIndividual ;
    owl:sameAs cc:CC00478 .

<http://vocab.getty.edu/aat/300221446> a owl:NamedIndividual ;
    owl:sameAs cc:CC00425 .

<http://vocab.getty.edu/aat/300221447> a owl:NamedIndividual ;
    owl:sameAs cc:CC00440 .

<http://vocab.getty.edu/aat/300221449> a owl:NamedIndividual ;
    owl:sameAs cc:CC00423 .

<http://vocab.getty.edu/aat/300221453> a owl:NamedIndividual ;
    owl:sameAs cc:CC00439 .

<http://vocab.getty.edu/aat/300221685> a owl:NamedIndividual ;
    owl:sameAs cc:CC00452 .

<http://vocab.getty.edu/aat/300221756> a owl:NamedIndividual ;
    owl:sameAs cc:CC00450 .

<http://vocab.getty.edu/aat/300224227> a owl:NamedIndividual ;
    owl:sameAs cc:CC00370 .

<http://vocab.getty.edu/aat/300224235> a owl:NamedIndividual ;
    owl:sameAs cc:CC00395 .

<http://vocab.getty.edu/aat/300224243> a owl:NamedIndividual ;
    owl:sameAs cc:CC00194 .

<http://vocab.getty.edu/aat/300224244> a owl:NamedIndividual ;
    owl:sameAs cc:CC00399 .

<http://vocab.getty.edu/aat/300224429> a owl:NamedIndividual ;
    owl:sameAs cc:CC00396 .

<http://vocab.getty.edu/aat/300225910> a owl:NamedIndividual ;
    owl:sameAs cc:CC00465 .

<http://vocab.getty.edu/aat/300226607> a owl:NamedIndividual ;
    owl:sameAs cc:CC00437 .

<http://vocab.getty.edu/aat/300227771> a owl:NamedIndividual ;
    owl:sameAs cc:CC00261 .

<http://vocab.getty.edu/aat/300227779> a owl:NamedIndividual ;
    owl:sameAs cc:CC00200 .

<http://vocab.getty.edu/aat/300227801> a owl:NamedIndividual ;
    owl:sameAs cc:CC00268 .

<http://vocab.getty.edu/aat/300227830> a owl:NamedIndividual ;
    owl:sameAs cc:CC00628 .

<http://vocab.getty.edu/aat/300227846> a owl:NamedIndividual ;
    owl:sameAs cc:CC00287 .

<http://vocab.getty.edu/aat/300227854> a owl:NamedIndividual ;
    owl:sameAs cc:CC00223 .

<http://vocab.getty.edu/aat/300227874> a owl:NamedIndividual ;
    owl:sameAs cc:CC00095 .

<http://vocab.getty.edu/aat/300227906> a owl:NamedIndividual ;
    owl:sameAs cc:CC00231 .

<http://vocab.getty.edu/aat/300228360> a owl:NamedIndividual ;
    owl:sameAs cc:CC00163 .

<http://vocab.getty.edu/aat/300231237> a owl:NamedIndividual ;
    owl:sameAs cc:CC00170 .

<http://vocab.getty.edu/aat/300231250> a owl:NamedIndividual ;
    owl:sameAs cc:CC00093 .

<http://vocab.getty.edu/aat/300232162> a owl:NamedIndividual ;
    owl:sameAs cc:CC00094 .

<http://vocab.getty.edu/aat/300232185> a owl:NamedIndividual ;
    owl:sameAs cc:CC00312 .

<http://vocab.getty.edu/aat/300232186> a owl:NamedIndividual ;
    owl:sameAs cc:CC00264 .

<http://vocab.getty.edu/aat/300234006> a owl:NamedIndividual ;
    owl:sameAs cc:CC00262 .

<http://vocab.getty.edu/aat/300235440> a owl:NamedIndividual ;
    owl:sameAs cc:CC00075 .

<http://vocab.getty.edu/aat/300236656> a owl:NamedIndividual ;
    owl:sameAs cc:CC00473 .

<http://vocab.getty.edu/aat/300236657> a owl:NamedIndividual ;
    owl:sameAs cc:CC00474 .

<http://vocab.getty.edu/aat/300239260> a owl:NamedIndividual ;
    owl:sameAs cc:CC00001 .

<http://vocab.getty.edu/aat/300239261> a owl:NamedIndividual ;
    owl:sameAs cc:CC00002 .

<http://vocab.getty.edu/aat/300239270> a owl:NamedIndividual ;
    owl:sameAs cc:CC00008 .

<http://vocab.getty.edu/aat/300239275> a owl:NamedIndividual ;
    owl:sameAs cc:CC00012 .

<http://vocab.getty.edu/aat/300239276> a owl:NamedIndividual ;
    owl:sameAs cc:CC00013 .

<http://vocab.getty.edu/aat/300239307> a owl:NamedIndividual ;
    owl:sameAs cc:CC00010 .

<http://vocab.getty.edu/aat/300239342> a owl:NamedIndividual ;
    owl:sameAs cc:CC00009 .

<http://vocab.getty.edu/aat/300239408> a owl:NamedIndividual ;
    owl:sameAs cc:CC00580 .

<http://vocab.getty.edu/aat/300239507> a owl:NamedIndividual ;
    owl:sameAs cc:CC00515 .

<http://vocab.getty.edu/aat/300243428> a owl:NamedIndividual ;
    owl:sameAs cc:CC00242 .

<http://vocab.getty.edu/aat/300243430> a owl:NamedIndividual ;
    owl:sameAs cc:CC00250 .

<http://vocab.getty.edu/aat/300245257> a owl:NamedIndividual ;
    owl:sameAs cc:CC00436 .

<http://vocab.getty.edu/aat/300247475> a owl:NamedIndividual ;
    owl:sameAs cc:CC00003 .

<http://vocab.getty.edu/aat/300248030> a owl:NamedIndividual ;
    owl:sameAs cc:CC00372 .

<http://vocab.getty.edu/aat/300248709> a owl:NamedIndividual ;
    owl:sameAs cc:CC00176 .

<http://vocab.getty.edu/aat/300248711> a owl:NamedIndividual ;
    owl:sameAs cc:CC00523 .

<http://vocab.getty.edu/aat/300249434> a owl:NamedIndividual ;
    owl:sameAs cc:CC00245 .

<http://vocab.getty.edu/aat/300249438> a owl:NamedIndividual ;
    owl:sameAs cc:CC00229 .

<http://vocab.getty.edu/aat/300249444> a owl:NamedIndividual ;
    owl:sameAs cc:CC00285 .

<http://vocab.getty.edu/aat/300249448> a owl:NamedIndividual ;
    owl:sameAs cc:CC00275 .

<http://vocab.getty.edu/aat/300249449> a owl:NamedIndividual ;
    owl:sameAs cc:CC00203 .

<http://vocab.getty.edu/aat/300251645> a owl:NamedIndividual ;
    owl:sameAs cc:CC00600 .

<http://vocab.getty.edu/aat/300253474> a owl:NamedIndividual ;
    owl:sameAs cc:CC00266 .

<http://vocab.getty.edu/aat/300253720> a owl:NamedIndividual ;
    owl:sameAs cc:CC00327 .

<http://vocab.getty.edu/aat/300253738> a owl:NamedIndividual ;
    owl:sameAs cc:CC00150 .

<http://vocab.getty.edu/aat/300253741> a owl:NamedIndividual ;
    owl:sameAs cc:CC00357 .

<http://vocab.getty.edu/aat/300253745> a owl:NamedIndividual ;
    owl:sameAs cc:CC00022 .

<http://vocab.getty.edu/aat/300253790> a owl:NamedIndividual ;
    owl:sameAs cc:CC00199 .

<http://vocab.getty.edu/aat/300254540> a owl:NamedIndividual ;
    owl:sameAs cc:CC00011 .

<http://vocab.getty.edu/aat/300254632> a owl:NamedIndividual ;
    owl:sameAs cc:CC00503 .

<http://vocab.getty.edu/aat/300254833> a owl:NamedIndividual ;
    owl:sameAs cc:CC00514 .

<http://vocab.getty.edu/aat/300255177> a owl:NamedIndividual ;
    owl:sameAs cc:CC00379 .

<http://vocab.getty.edu/aat/300255803> a owl:NamedIndividual ;
    owl:sameAs cc:CC00373 .

<http://vocab.getty.edu/aat/300256611> a owl:NamedIndividual ;
    owl:sameAs cc:CC00315 .

<http://vocab.getty.edu/aat/300256616> a owl:NamedIndividual ;
    owl:sameAs cc:CC00217 .

<http://vocab.getty.edu/aat/300256819> a owl:NamedIndividual ;
    owl:sameAs cc:CC00433 .

<http://vocab.getty.edu/aat/300257459> a owl:NamedIndividual ;
    owl:sameAs cc:CC00084 .

<http://vocab.getty.edu/aat/300257463> a owl:NamedIndividual ;
    owl:sameAs cc:CC00088 .

<http://vocab.getty.edu/aat/300257544> a owl:NamedIndividual ;
    owl:sameAs cc:CC00438 .

<http://vocab.getty.edu/aat/300259717> a owl:NamedIndividual ;
    owl:sameAs cc:CC00142 .

<http://vocab.getty.edu/aat/300260366> a owl:NamedIndividual ;
    owl:sameAs cc:CC00428 .

<http://vocab.getty.edu/aat/300262720> a owl:NamedIndividual ;
    owl:sameAs cc:CC00420 .

<http://vocab.getty.edu/aat/300263386> a owl:NamedIndividual ;
    owl:sameAs cc:CC00298 .

<http://vocab.getty.edu/aat/300264024> a owl:NamedIndividual ;
    owl:sameAs cc:CC00081 .

<http://vocab.getty.edu/aat/300264031> a owl:NamedIndividual ;
    owl:sameAs cc:CC00091 .

<http://vocab.getty.edu/aat/300264038> a owl:NamedIndividual ;
    owl:sameAs cc:CC00207 .

<http://vocab.getty.edu/aat/300264622> a owl:NamedIndividual ;
    owl:sameAs cc:CC00100 .

<http://vocab.getty.edu/aat/300265060> a owl:NamedIndividual ;
    owl:sameAs cc:CC00371 .

<http://vocab.getty.edu/aat/300265255> a owl:NamedIndividual ;
    owl:sameAs cc:CC00441 .

<http://vocab.getty.edu/aat/300266234> a owl:NamedIndividual ;
    owl:sameAs cc:CC00049 .

<http://vocab.getty.edu/aat/300266242> a owl:NamedIndividual ;
    owl:sameAs cc:CC00055 .

<http://vocab.getty.edu/aat/300266248> a owl:NamedIndividual ;
    owl:sameAs cc:CC00069 .

<http://vocab.getty.edu/aat/300266714> a owl:NamedIndividual ;
    owl:sameAs cc:CC00377 .

<http://vocab.getty.edu/aat/300310123> a owl:NamedIndividual ;
    owl:sameAs cc:CC00294 .

<http://vocab.getty.edu/aat/300310125> a owl:NamedIndividual ;
    owl:sameAs cc:CC00243 .

<http://vocab.getty.edu/aat/300311024> a owl:NamedIndividual ;
    owl:sameAs cc:CC00071 .

<http://vocab.getty.edu/aat/300311051> a owl:NamedIndividual ;
    owl:sameAs cc:CC00070 .

<http://vocab.getty.edu/aat/300311067> a owl:NamedIndividual ;
    owl:sameAs cc:CC00063 .

<http://vocab.getty.edu/aat/300311131> a owl:NamedIndividual ;
    owl:sameAs cc:CC00060 .

<http://vocab.getty.edu/aat/300311171> a owl:NamedIndividual ;
    owl:sameAs cc:CC00290 .

<http://vocab.getty.edu/aat/300311173> a owl:NamedIndividual ;
    owl:sameAs cc:CC00061 .

<http://vocab.getty.edu/aat/300311191> a owl:NamedIndividual ;
    owl:sameAs cc:CC00057 .

<http://vocab.getty.edu/aat/300311477> a owl:NamedIndividual ;
    owl:sameAs cc:CC00056 .

<http://vocab.getty.edu/aat/300375298> a owl:NamedIndividual ;
    owl:sameAs cc:CC00190 .

<http://vocab.getty.edu/aat/300375299> a owl:NamedIndividual ;
    owl:sameAs cc:CC00193 .

<http://vocab.getty.edu/aat/300375581> a owl:NamedIndividual ;
    owl:sameAs cc:CC00299 .

<http://vocab.getty.edu/aat/300375755> a owl:NamedIndividual ;
    owl:sameAs cc:CC00374 .

<http://vocab.getty.edu/aat/300379341> a owl:NamedIndividual ;
    owl:sameAs cc:CC00365 .

<http://vocab.getty.edu/aat/300379344> a owl:NamedIndividual ;
    owl:sameAs cc:CC00364 .

<http://vocab.getty.edu/aat/300379829> a owl:NamedIndividual ;
    owl:sameAs cc:CC00233 .

<http://vocab.getty.edu/aat/300379924> a owl:NamedIndividual ;
    owl:sameAs cc:CC00089 .

<http://vocab.getty.edu/aat/300380171> a owl:NamedIndividual ;
    owl:sameAs cc:CC00288 .

<http://vocab.getty.edu/aat/300386429> a owl:NamedIndividual ;
    owl:sameAs cc:CC00077 .

<http://vocab.getty.edu/aat/300386559> a owl:NamedIndividual ;
    owl:sameAs cc:CC00196 .

<http://vocab.getty.edu/aat/300386672> a owl:NamedIndividual ;
    owl:sameAs cc:CC00197 .

<http://vocab.getty.edu/aat/300391016> a owl:NamedIndividual ;
    owl:sameAs cc:CC00429 .

<http://vocab.getty.edu/aat/300400479> a owl:NamedIndividual ;
    owl:sameAs cc:CC00286 .

<http://vocab.getty.edu/aat/300400593> a owl:NamedIndividual ;
    owl:sameAs cc:CC00227 .

<http://vocab.getty.edu/aat/300400621> a owl:NamedIndividual ;
    owl:sameAs cc:CC00421 .

<http://vocab.getty.edu/aat/300400693> a owl:NamedIndividual ;
    owl:sameAs cc:CC00198 .

<http://vocab.getty.edu/aat/300403905> a owl:NamedIndividual ;
    owl:sameAs cc:CC00202 .

<http://vocab.getty.edu/aat/300403910> a owl:NamedIndividual ;
    owl:sameAs cc:CC00368 .

<http://vocab.getty.edu/aat/300403912> a owl:NamedIndividual ;
    owl:sameAs cc:CC00280 .

<http://vocab.getty.edu/aat/300404361> a owl:NamedIndividual ;
    owl:sameAs cc:CC00211 .

<http://vocab.getty.edu/aat/300410339> a owl:NamedIndividual ;
    owl:sameAs cc:CC00289 .

<http://vocab.getty.edu/aat/300411405> a owl:NamedIndividual ;
    owl:sameAs cc:CC00480 .

<http://vocab.getty.edu/aat/300411417> a owl:NamedIndividual ;
    owl:sameAs cc:CC00479 .

<http://vocab.getty.edu/aat/300411698> a owl:NamedIndividual ;
    owl:sameAs cc:CC00031 .

<http://vocab.getty.edu/aat/300411733> a owl:NamedIndividual ;
    owl:sameAs cc:CC00143 .

<http://vocab.getty.edu/aat/300411736> a owl:NamedIndividual ;
    owl:sameAs cc:CC00607 .

<http://vocab.getty.edu/aat/300411738> a owl:NamedIndividual ;
    owl:sameAs cc:CC00180 .

<http://vocab.getty.edu/aat/300411740> a owl:NamedIndividual ;
    owl:sameAs cc:CC00424 .

<http://vocab.getty.edu/aat/300411741> a owl:NamedIndividual ;
    owl:sameAs cc:CC00432 .

<http://vocab.getty.edu/aat/300411750> a owl:NamedIndividual ;
    owl:sameAs cc:CC00366 .

<http://vocab.getty.edu/aat/300411755> a owl:NamedIndividual ;
    owl:sameAs cc:CC00507 .

<http://vocab.getty.edu/aat/300411756> a owl:NamedIndividual ;
    owl:sameAs cc:CC00380 .

<http://vocab.getty.edu/aat/300411762> a owl:NamedIndividual ;
    owl:sameAs cc:CC00509 .

<http://vocab.getty.edu/aat/300411766> a owl:NamedIndividual ;
    owl:sameAs cc:CC00369 .

<http://vocab.getty.edu/aat/300411863> a owl:NamedIndividual ;
    owl:sameAs cc:CC00300 .

<http://vocab.getty.edu/aat/300417854> a owl:NamedIndividual ;
    owl:sameAs cc:CC00301 .

<http://vocab.getty.edu/aat/300417856> a owl:NamedIndividual ;
    owl:sameAs cc:CC00237 .

<http://vocab.getty.edu/aat/300417868> a owl:NamedIndividual ;
    owl:sameAs cc:CC00209 .

<http://vocab.getty.edu/aat/300417877> a owl:NamedIndividual ;
    owl:sameAs cc:CC00007 .

<http://vocab.getty.edu/aat/300417880> a owl:NamedIndividual ;
    owl:sameAs cc:CC00274 .

<http://vocab.getty.edu/aat/300417883> a owl:NamedIndividual ;
    owl:sameAs cc:CC00214 .

<http://vocab.getty.edu/aat/300417888> a owl:NamedIndividual ;
    owl:sameAs cc:CC00376 .

<http://vocab.getty.edu/aat/300426171> a owl:NamedIndividual ;
    owl:sameAs cc:CC00324 .

<http://www.wikidata.org/entity/#N/A> a owl:NamedIndividual ;
    owl:sameAs cc:CC00142 .

<http://www.wikidata.org/entity/Q1034198> a owl:NamedIndividual ;
    owl:sameAs cc:CC00602 .

<http://www.wikidata.org/entity/Q1043590> a owl:NamedIndividual ;
    owl:sameAs cc:CC00021 .

<http://www.wikidata.org/entity/Q1045372> a owl:NamedIndividual ;
    owl:sameAs cc:CC00037 .

<http://www.wikidata.org/entity/Q10461476> a owl:NamedIndividual ;
    owl:sameAs cc:CC00514 .

<http://www.wikidata.org/entity/Q10638846> a owl:NamedIndividual ;
    owl:sameAs cc:CC00502 .

<http://www.wikidata.org/entity/Q10707950> a owl:NamedIndividual ;
    owl:sameAs cc:CC00520 .

<http://www.wikidata.org/entity/Q11018285> a owl:NamedIndividual ;
    owl:sameAs cc:CC00499 .

<http://www.wikidata.org/entity/Q11284623> a owl:NamedIndividual ;
    owl:sameAs cc:CC00505 .

<http://www.wikidata.org/entity/Q116887> a owl:NamedIndividual ;
    owl:sameAs cc:CC00490 .

<http://www.wikidata.org/entity/Q1262096> a owl:NamedIndividual ;
    owl:sameAs cc:CC00291 .

<http://www.wikidata.org/entity/Q1323314> a owl:NamedIndividual ;
    owl:sameAs cc:CC00612 .

<http://www.wikidata.org/entity/Q1333132> a owl:NamedIndividual ;
    owl:sameAs cc:CC00138 .

<http://www.wikidata.org/entity/Q13383825> a owl:NamedIndividual ;
    owl:sameAs cc:CC00428 .

<http://www.wikidata.org/entity/Q1341710> a owl:NamedIndividual ;
    owl:sameAs cc:CC00327 .

<http://www.wikidata.org/entity/Q1348773> a owl:NamedIndividual ;
    owl:sameAs cc:CC00283 .

<http://www.wikidata.org/entity/Q1349227> a owl:NamedIndividual ;
    owl:sameAs cc:CC00371 .

<http://www.wikidata.org/entity/Q1353860> a owl:NamedIndividual ;
    owl:sameAs cc:CC00628 .

<http://www.wikidata.org/entity/Q140101> a owl:NamedIndividual ;
    owl:sameAs cc:CC00591 .

<http://www.wikidata.org/entity/Q1410477> a owl:NamedIndividual ;
    owl:sameAs cc:CC00583 .

<http://www.wikidata.org/entity/Q14290457> a owl:NamedIndividual ;
    owl:sameAs cc:CC00589 .

<http://www.wikidata.org/entity/Q1435365> a owl:NamedIndividual ;
    owl:sameAs cc:CC00607 .

<http://www.wikidata.org/entity/Q1485316> a owl:NamedIndividual ;
    owl:sameAs cc:CC00513 .

<http://www.wikidata.org/entity/Q14952> a owl:NamedIndividual ;
    owl:sameAs cc:CC00608 .

<http://www.wikidata.org/entity/Q151948> a owl:NamedIndividual ;
    owl:sameAs cc:CC00511 .

<http://www.wikidata.org/entity/Q15411420> a owl:NamedIndividual ;
    owl:sameAs cc:CC00012 .

<http://www.wikidata.org/entity/Q1544262> a owl:NamedIndividual ;
    owl:sameAs cc:CC00047 .

<http://www.wikidata.org/entity/Q161439> a owl:NamedIndividual ;
    owl:sameAs cc:CC00610 .

<http://www.wikidata.org/entity/Q1615371> a owl:NamedIndividual ;
    owl:sameAs cc:CC00493 .

<http://www.wikidata.org/entity/Q161928> a owl:NamedIndividual ;
    owl:sameAs cc:CC00603 .

<http://www.wikidata.org/entity/Q1637220> a owl:NamedIndividual ;
    owl:sameAs cc:CC00510 .

<http://www.wikidata.org/entity/Q169031> a owl:NamedIndividual ;
    owl:sameAs cc:CC00606 .

<http://www.wikidata.org/entity/Q16949531> a owl:NamedIndividual ;
    owl:sameAs cc:CC00323 .

<http://www.wikidata.org/entity/Q1700971> a owl:NamedIndividual ;
    owl:sameAs cc:CC00597 .

<http://www.wikidata.org/entity/Q1751458> a owl:NamedIndividual ;
    owl:sameAs cc:CC00020 .

<http://www.wikidata.org/entity/Q18121766> a owl:NamedIndividual ;
    owl:sameAs cc:CC00177 .

<http://www.wikidata.org/entity/Q19022> a owl:NamedIndividual ;
    owl:sameAs cc:CC00578 .

<http://www.wikidata.org/entity/Q192244> a owl:NamedIndividual ;
    owl:sameAs cc:CC00529 .

<http://www.wikidata.org/entity/Q192500> a owl:NamedIndividual ;
    owl:sameAs cc:CC00530 .

<http://www.wikidata.org/entity/Q193242> a owl:NamedIndividual ;
    owl:sameAs cc:CC00532 .

<http://www.wikidata.org/entity/Q193480> a owl:NamedIndividual ;
    owl:sameAs cc:CC00533 .

<http://www.wikidata.org/entity/Q193679> a owl:NamedIndividual ;
    owl:sameAs cc:CC00534 .

<http://www.wikidata.org/entity/Q195923> a owl:NamedIndividual ;
    owl:sameAs cc:CC00539 .

<http://www.wikidata.org/entity/Q196113> a owl:NamedIndividual ;
    owl:sameAs cc:CC00592 .

<http://www.wikidata.org/entity/Q196292> a owl:NamedIndividual ;
    owl:sameAs cc:CC00540 .

<http://www.wikidata.org/entity/Q196375> a owl:NamedIndividual ;
    owl:sameAs cc:CC00541 .

<http://www.wikidata.org/entity/Q196467> a owl:NamedIndividual ;
    owl:sameAs cc:CC00542 .

<http://www.wikidata.org/entity/Q196549> a owl:NamedIndividual ;
    owl:sameAs cc:CC00543 .

<http://www.wikidata.org/entity/Q196647> a owl:NamedIndividual ;
    owl:sameAs cc:CC00544 .

<http://www.wikidata.org/entity/Q197012> a owl:NamedIndividual ;
    owl:sameAs cc:CC00546 .

<http://www.wikidata.org/entity/Q198144> a owl:NamedIndividual ;
    owl:sameAs cc:CC00548 .

<http://www.wikidata.org/entity/Q198469> a owl:NamedIndividual ;
    owl:sameAs cc:CC00549 .

<http://www.wikidata.org/entity/Q199545> a owl:NamedIndividual ;
    owl:sameAs cc:CC00553 .

<http://www.wikidata.org/entity/Q199912> a owl:NamedIndividual ;
    owl:sameAs cc:CC00556 .

<http://www.wikidata.org/entity/Q2058306> a owl:NamedIndividual ;
    owl:sameAs cc:CC00492 .

<http://www.wikidata.org/entity/Q20732506> a owl:NamedIndividual ;
    owl:sameAs cc:CC00135 .

<http://www.wikidata.org/entity/Q2117537> a owl:NamedIndividual ;
    owl:sameAs cc:CC00137 .

<http://www.wikidata.org/entity/Q212527> a owl:NamedIndividual ;
    owl:sameAs cc:CC00195 .

<http://www.wikidata.org/entity/Q2143346> a owl:NamedIndividual ;
    owl:sameAs cc:CC00319 .

<http://www.wikidata.org/entity/Q21972880> a owl:NamedIndividual ;
    owl:sameAs cc:CC00357 .

<http://www.wikidata.org/entity/Q223269> a owl:NamedIndividual ;
    owl:sameAs cc:CC00525 .

<http://www.wikidata.org/entity/Q2238808> a owl:NamedIndividual ;
    owl:sameAs cc:CC00599 .

<http://www.wikidata.org/entity/Q22921095> a owl:NamedIndividual ;
    owl:sameAs cc:CC00512 .

<http://www.wikidata.org/entity/Q23301561> a owl:NamedIndividual ;
    owl:sameAs cc:CC00045 .

<http://www.wikidata.org/entity/Q24016353> a owl:NamedIndividual ;
    owl:sameAs cc:CC00256 .

<http://www.wikidata.org/entity/Q2411228> a owl:NamedIndividual ;
    owl:sameAs cc:CC00054 .

<http://www.wikidata.org/entity/Q2429962> a owl:NamedIndividual ;
    owl:sameAs cc:CC00590 .

<http://www.wikidata.org/entity/Q244554> a owl:NamedIndividual ;
    owl:sameAs cc:CC00580 .

<http://www.wikidata.org/entity/Q2466122> a owl:NamedIndividual ;
    owl:sameAs cc:CC00014 .

<http://www.wikidata.org/entity/Q2524539> a owl:NamedIndividual ;
    owl:sameAs cc:CC00605 .

<http://www.wikidata.org/entity/Q2553036> a owl:NamedIndividual ;
    owl:sameAs cc:CC00596 .

<http://www.wikidata.org/entity/Q2569037> a owl:NamedIndividual ;
    owl:sameAs cc:CC00116 .

<http://www.wikidata.org/entity/Q26468> a owl:NamedIndividual ;
    owl:sameAs cc:CC00584 .

<http://www.wikidata.org/entity/Q2862826> a owl:NamedIndividual ;
    owl:sameAs cc:CC00320 .

<http://www.wikidata.org/entity/Q29125416> a owl:NamedIndividual ;
    owl:sameAs cc:CC00128 .

<http://www.wikidata.org/entity/Q29125938> a owl:NamedIndividual ;
    owl:sameAs cc:CC00148 .

<http://www.wikidata.org/entity/Q29126275> a owl:NamedIndividual ;
    owl:sameAs cc:CC00145 .

<http://www.wikidata.org/entity/Q29126653> a owl:NamedIndividual ;
    owl:sameAs cc:CC00147 .

<http://www.wikidata.org/entity/Q29129961> a owl:NamedIndividual ;
    owl:sameAs cc:CC00356 .

<http://www.wikidata.org/entity/Q29130192> a owl:NamedIndividual ;
    owl:sameAs cc:CC00367 .

<http://www.wikidata.org/entity/Q29353484> a owl:NamedIndividual ;
    owl:sameAs cc:CC00611 .

<http://www.wikidata.org/entity/Q29405103> a owl:NamedIndividual ;
    owl:sameAs cc:CC00506 .

<http://www.wikidata.org/entity/Q29473093> a owl:NamedIndividual ;
    owl:sameAs cc:CC00258 .

<http://www.wikidata.org/entity/Q29473272> a owl:NamedIndividual ;
    owl:sameAs cc:CC00039 .

<http://www.wikidata.org/entity/Q29473382> a owl:NamedIndividual ;
    owl:sameAs cc:CC00629 .

<http://www.wikidata.org/entity/Q29514179> a owl:NamedIndividual ;
    owl:sameAs cc:CC00005 .

<http://www.wikidata.org/entity/Q29583212> a owl:NamedIndividual ;
    owl:sameAs cc:CC00027 .

<http://www.wikidata.org/entity/Q29583217> a owl:NamedIndividual ;
    owl:sameAs cc:CC00119 .

<http://www.wikidata.org/entity/Q29583222> a owl:NamedIndividual ;
    owl:sameAs cc:CC00024 .

<http://www.wikidata.org/entity/Q29583224> a owl:NamedIndividual ;
    owl:sameAs cc:CC00491 .

<http://www.wikidata.org/entity/Q29583225> a owl:NamedIndividual ;
    owl:sameAs cc:CC00044 .

<http://www.wikidata.org/entity/Q29655994> a owl:NamedIndividual ;
    owl:sameAs cc:CC00355 .

<http://www.wikidata.org/entity/Q29741669> a owl:NamedIndividual ;
    owl:sameAs cc:CC00326 .

<http://www.wikidata.org/entity/Q3037506> a owl:NamedIndividual ;
    owl:sameAs cc:CC00350 .

<http://www.wikidata.org/entity/Q30588951> a owl:NamedIndividual ;
    owl:sameAs cc:CC00495 .

<http://www.wikidata.org/entity/Q3247116> a owl:NamedIndividual ;
    owl:sameAs cc:CC00114 .

<http://www.wikidata.org/entity/Q3434328> a owl:NamedIndividual ;
    owl:sameAs cc:CC00500 .

<http://www.wikidata.org/entity/Q345127> a owl:NamedIndividual ;
    owl:sameAs cc:CC00604 .

<http://www.wikidata.org/entity/Q34644> a owl:NamedIndividual ;
    owl:sameAs cc:CC00575 .

<http://www.wikidata.org/entity/Q34653> a owl:NamedIndividual ;
    owl:sameAs cc:CC00576 .

<http://www.wikidata.org/entity/Q35014> a owl:NamedIndividual ;
    owl:sameAs cc:CC00574 .

<http://www.wikidata.org/entity/Q35024> a owl:NamedIndividual ;
    owl:sameAs cc:CC00577 .

<http://www.wikidata.org/entity/Q35702> a owl:NamedIndividual ;
    owl:sameAs cc:CC00570 .

<http://www.wikidata.org/entity/Q35724> a owl:NamedIndividual ;
    owl:sameAs cc:CC00573 .

<http://www.wikidata.org/entity/Q35736> a owl:NamedIndividual ;
    owl:sameAs cc:CC00569 .

<http://www.wikidata.org/entity/Q3603737> a owl:NamedIndividual ;
    owl:sameAs cc:CC00109 .

<http://www.wikidata.org/entity/Q362200> a owl:NamedIndividual ;
    owl:sameAs cc:CC00600 .

<http://www.wikidata.org/entity/Q36297> a owl:NamedIndividual ;
    owl:sameAs cc:CC00572 .

<http://www.wikidata.org/entity/Q363031> a owl:NamedIndividual ;
    owl:sameAs cc:CC00526 .

<http://www.wikidata.org/entity/Q36561> a owl:NamedIndividual ;
    owl:sameAs cc:CC00571 .

<http://www.wikidata.org/entity/Q36574> a owl:NamedIndividual ;
    owl:sameAs cc:CC00567 .

<http://www.wikidata.org/entity/Q36585> a owl:NamedIndividual ;
    owl:sameAs cc:CC00568 .

<http://www.wikidata.org/entity/Q38324> a owl:NamedIndividual ;
    owl:sameAs cc:CC00561 .

<http://www.wikidata.org/entity/Q38674> a owl:NamedIndividual ;
    owl:sameAs cc:CC00565 .

<http://www.wikidata.org/entity/Q38971> a owl:NamedIndividual ;
    owl:sameAs cc:CC00566 .

<http://www.wikidata.org/entity/Q39484> a owl:NamedIndividual ;
    owl:sameAs cc:CC00560 .

<http://www.wikidata.org/entity/Q39577> a owl:NamedIndividual ;
    owl:sameAs cc:CC00557 .

<http://www.wikidata.org/entity/Q39844> a owl:NamedIndividual ;
    owl:sameAs cc:CC00563 .

<http://www.wikidata.org/entity/Q39847> a owl:NamedIndividual ;
    owl:sameAs cc:CC00564 .

<http://www.wikidata.org/entity/Q39908> a owl:NamedIndividual ;
    owl:sameAs cc:CC00609 .

<http://www.wikidata.org/entity/Q40196> a owl:NamedIndividual ;
    owl:sameAs cc:CC00558 .

<http://www.wikidata.org/entity/Q40601> a owl:NamedIndividual ;
    owl:sameAs cc:CC00594 .

<http://www.wikidata.org/entity/Q40927> a owl:NamedIndividual ;
    owl:sameAs cc:CC00562 .

<http://www.wikidata.org/entity/Q42519> a owl:NamedIndividual ;
    owl:sameAs cc:CC00058 .

<http://www.wikidata.org/entity/Q42995> a owl:NamedIndividual ;
    owl:sameAs cc:CC00537 .

<http://www.wikidata.org/entity/Q43065851> a owl:NamedIndividual ;
    owl:sameAs cc:CC00087 .

<http://www.wikidata.org/entity/Q43299785> a owl:NamedIndividual ;
    owl:sameAs cc:CC00508 .

<http://www.wikidata.org/entity/Q43370> a owl:NamedIndividual ;
    owl:sameAs cc:CC00547 .

<http://www.wikidata.org/entity/Q43970> a owl:NamedIndividual ;
    owl:sameAs cc:CC00551 .

<http://www.wikidata.org/entity/Q44140> a owl:NamedIndividual ;
    owl:sameAs cc:CC00527 .

<http://www.wikidata.org/entity/Q44407651> a owl:NamedIndividual ;
    owl:sameAs cc:CC00278 .

<http://www.wikidata.org/entity/Q44659> a owl:NamedIndividual ;
    owl:sameAs cc:CC00559 .

<http://www.wikidata.org/entity/Q44859> a owl:NamedIndividual ;
    owl:sameAs cc:CC00554 .

<http://www.wikidata.org/entity/Q46011> a owl:NamedIndividual ;
    owl:sameAs cc:CC00545 .

<http://www.wikidata.org/entity/Q46050> a owl:NamedIndividual ;
    owl:sameAs cc:CC00538 .

<http://www.wikidata.org/entity/Q46245> a owl:NamedIndividual ;
    owl:sameAs cc:CC00528 .

<http://www.wikidata.org/entity/Q47089651> a owl:NamedIndividual ;
    owl:sameAs cc:CC00630 .

<http://www.wikidata.org/entity/Q4764964> a owl:NamedIndividual ;
    owl:sameAs cc:CC00593 .

<http://www.wikidata.org/entity/Q48058> a owl:NamedIndividual ;
    owl:sameAs cc:CC00555 .

<http://www.wikidata.org/entity/Q48121> a owl:NamedIndividual ;
    owl:sameAs cc:CC00550 .

<http://www.wikidata.org/entity/Q48158> a owl:NamedIndividual ;
    owl:sameAs cc:CC00531 .

<http://www.wikidata.org/entity/Q4851616> a owl:NamedIndividual ;
    owl:sameAs cc:CC00489 .

<http://www.wikidata.org/entity/Q48528> a owl:NamedIndividual ;
    owl:sameAs cc:CC00552 .

<http://www.wikidata.org/entity/Q4854234> a owl:NamedIndividual ;
    owl:sameAs cc:CC00029 .

<http://www.wikidata.org/entity/Q48563> a owl:NamedIndividual ;
    owl:sameAs cc:CC00535 .

<http://www.wikidata.org/entity/Q48595> a owl:NamedIndividual ;
    owl:sameAs cc:CC00536 .

<http://www.wikidata.org/entity/Q5064153> a owl:NamedIndividual ;
    owl:sameAs cc:CC00582 .

<http://www.wikidata.org/entity/Q5184798> a owl:NamedIndividual ;
    owl:sameAs cc:CC00015 .

<http://www.wikidata.org/entity/Q5225562> a owl:NamedIndividual ;
    owl:sameAs cc:CC00393 .

<http://www.wikidata.org/entity/Q5254472> a owl:NamedIndividual ;
    owl:sameAs cc:CC00497 .

<http://www.wikidata.org/entity/Q534495> a owl:NamedIndividual ;
    owl:sameAs cc:CC00579 .

<http://www.wikidata.org/entity/Q543923> a owl:NamedIndividual ;
    owl:sameAs cc:CC00068 .

<http://www.wikidata.org/entity/Q5647451> a owl:NamedIndividual ;
    owl:sameAs cc:CC00255 .

<http://www.wikidata.org/entity/Q5856> a owl:NamedIndividual ;
    owl:sameAs cc:CC00244 .

<http://www.wikidata.org/entity/Q63505185> a owl:NamedIndividual ;
    owl:sameAs cc:CC00598 .

<http://www.wikidata.org/entity/Q635784> a owl:NamedIndividual ;
    owl:sameAs cc:CC00494 .

<http://www.wikidata.org/entity/Q64780667> a owl:NamedIndividual ;
    owl:sameAs cc:CC00030 .

<http://www.wikidata.org/entity/Q67608772> a owl:NamedIndividual ;
    owl:sameAs cc:CC00338 .

<http://www.wikidata.org/entity/Q7140985> a owl:NamedIndividual ;
    owl:sameAs cc:CC00375 .

<http://www.wikidata.org/entity/Q7341111> a owl:NamedIndividual ;
    owl:sameAs cc:CC00504 .

<http://www.wikidata.org/entity/Q73419282> a owl:NamedIndividual ;
    owl:sameAs cc:CC00026 .

<http://www.wikidata.org/entity/Q73514132> a owl:NamedIndividual ;
    owl:sameAs cc:CC00130 .

<http://www.wikidata.org/entity/Q73540348> a owl:NamedIndividual ;
    owl:sameAs cc:CC00363 .

<http://www.wikidata.org/entity/Q73540794> a owl:NamedIndividual ;
    owl:sameAs cc:CC00328 .

<http://www.wikidata.org/entity/Q73545207> a owl:NamedIndividual ;
    owl:sameAs cc:CC00146 .

<http://www.wikidata.org/entity/Q766204> a owl:NamedIndividual ;
    owl:sameAs cc:CC00362 .

<http://www.wikidata.org/entity/Q77004674> a owl:NamedIndividual ;
    owl:sameAs cc:CC00017 .

<http://www.wikidata.org/entity/Q778180> a owl:NamedIndividual ;
    owl:sameAs cc:CC00077 .

<http://www.wikidata.org/entity/Q7933576> a owl:NamedIndividual ;
    owl:sameAs cc:CC00392 .

<http://www.wikidata.org/entity/Q797446> a owl:NamedIndividual ;
    owl:sameAs cc:CC00053 .

<http://www.wikidata.org/entity/Q8054544> a owl:NamedIndividual ;
    owl:sameAs cc:CC00184 .

<http://www.wikidata.org/entity/Q83328052> a owl:NamedIndividual ;
    owl:sameAs cc:CC00032 .

<http://www.wikidata.org/entity/Q83328209> a owl:NamedIndividual ;
    owl:sameAs cc:CC00033 .

<http://www.wikidata.org/entity/Q83328363> a owl:NamedIndividual ;
    owl:sameAs cc:CC00034 .

<http://www.wikidata.org/entity/Q83328663> a owl:NamedIndividual ;
    owl:sameAs cc:CC00035 .

<http://www.wikidata.org/entity/Q83328812> a owl:NamedIndividual ;
    owl:sameAs cc:CC00038 .

<http://www.wikidata.org/entity/Q83328891> a owl:NamedIndividual ;
    owl:sameAs cc:CC00048 .

<http://www.wikidata.org/entity/Q83329279> a owl:NamedIndividual ;
    owl:sameAs cc:CC00043 .

<http://www.wikidata.org/entity/Q83329964> a owl:NamedIndividual ;
    owl:sameAs cc:CC00025 .

<http://www.wikidata.org/entity/Q83332399> a owl:NamedIndividual ;
    owl:sameAs cc:CC00175 .

<http://www.wikidata.org/entity/Q83332911> a owl:NamedIndividual ;
    owl:sameAs cc:CC00183 .

<http://www.wikidata.org/entity/Q83333769> a owl:NamedIndividual ;
    owl:sameAs cc:CC00164 .

<http://www.wikidata.org/entity/Q83333837> a owl:NamedIndividual ;
    owl:sameAs cc:CC00129 .

<http://www.wikidata.org/entity/Q83333892> a owl:NamedIndividual ;
    owl:sameAs cc:CC00251 .

<http://www.wikidata.org/entity/Q83333946> a owl:NamedIndividual ;
    owl:sameAs cc:CC00166 .

<http://www.wikidata.org/entity/Q83333994> a owl:NamedIndividual ;
    owl:sameAs cc:CC00168 .

<http://www.wikidata.org/entity/Q83334145> a owl:NamedIndividual ;
    owl:sameAs cc:CC00171 .

<http://www.wikidata.org/entity/Q83334198> a owl:NamedIndividual ;
    owl:sameAs cc:CC00182 .

<http://www.wikidata.org/entity/Q836934> a owl:NamedIndividual ;
    owl:sameAs cc:CC00496 .

<http://www.wikidata.org/entity/Q858090> a owl:NamedIndividual ;
    owl:sameAs cc:CC00325 .

<http://www.wikidata.org/entity/Q881659> a owl:NamedIndividual ;
    owl:sameAs cc:CC00199 .

<http://www.wikidata.org/entity/Q890119> a owl:NamedIndividual ;
    owl:sameAs cc:CC00601 .

<http://www.wikidata.org/entity/Q911389> a owl:NamedIndividual ;
    owl:sameAs cc:CC00588 .

<http://www.wikidata.org/entity/Q937704> a owl:NamedIndividual ;
    owl:sameAs cc:CC00586 .

<http://www.wikidata.org/entity/Q997545> a owl:NamedIndividual ;
    owl:sameAs cc:CC00040 .

<http://www.wikidata.org/entity/http://www.wikidata.org/entity/Q29129637> a owl:NamedIndividual ;
    owl:sameAs cc:CC00150 .

cc:CC00018 a owl:NamedIndividual ;
    rdfs:label "inset"@en ;
    dcterms:identifier "CC00018" .

cc:CC00022 a owl:NamedIndividual ;
    rdfs:label "round gown"@en ;
    dcterms:description [ rdfs:label "Refers to 18th- and 19th-century full-length gowns cut without a center front opening in the skirt and usually without a train."@en ;
            dcterms:creator "The J. Paul Getty Trust" ;
            dcterms:license <https://opendatacommons.org/licenses/by/1-0/> ;
            dcterms:rights <https://rightsstatements.org/vocab/InC/1.0/> ;
            dcterms:source <http://www.getty.edu/research/tools/vocabularies/aat/> ],
        "Refers to 18th- and 19th-century full-length gowns cut without a center front opening in the skirt and usually without a train."@en ;
    dcterms:identifier "CC00022" ;
    owl:sameAs <http://vocab.getty.edu/aat/300253745> .

cc:CC00028 a owl:NamedIndividual ;
    rdfs:label "ascot"@en ;
    dcterms:description [ rdfs:label "Neckcloths with broad ends usually looped and tied under the chin and sometimes secured by a stickpin."@en ;
            dcterms:creator "The J. Paul Getty Trust" ;
            dcterms:license <https://opendatacommons.org/licenses/by/1-0/> ;
            dcterms:rights <https://rightsstatements.org/vocab/InC/1.0/> ;
            dcterms:source <http://www.getty.edu/vow/AATFullDisplay?find=ascot&logic=AND&note=&english=N&prev_page=1&subjectid=300210052> ],
        "Neckcloths with broad ends usually looped and tied under the chin and sometimes secured by a stickpin."@en ;
    dcterms:identifier "CC00028" ;
    owl:sameAs <http://vocab.getty.edu/aat/300210052> .

cc:CC00031 a owl:NamedIndividual ;
    rdfs:label "bow collar"@en ;
    dcterms:description [ rdfs:label "Applied clothing accessories that may be made of rope, ribbon or fabric. These consist of knots with two loops and two ends, fixed into decorative elements attached to clothing or other objects."@en ;
            dcterms:creator "The J. Paul Getty Trust" ;
            dcterms:license <https://opendatacommons.org/licenses/by/1-0/> ;
            dcterms:rights <https://rightsstatements.org/vocab/InC/1.0/> ;
            dcterms:source <http://www.getty.edu/research/tools/vocabularies/aat/> ],
        "Applied clothing accessories that may be made of rope, ribbon or fabric. These consist of knots with two loops and two ends, fixed into decorative elements attached to clothing or other objects."@en ;
    dcterms:identifier "CC00031" ;
    owl:sameAs <http://vocab.getty.edu/aat/300411698> .

cc:CC00032 a owl:NamedIndividual ;
    rdfs:label "Chelsea collar"@en ;
    dcterms:description [ rdfs:label "A woman's collar for a low V-neckline, with a stand and long points, popular in the 1960s and 1970s."@en ;
            dcterms:creator "Wikipedia" ;
            dcterms:license <https://creativecommons.org/publicdomain/mark/1.0/> ;
            dcterms:rights <https://creativecommons.org/publicdomain/mark/1.0/> ;
            dcterms:source <https://en.wikipedia.org/wiki/Collar_(clothing)> ],
        "A woman's collar for a low V-neckline, with a stand and long points, popular in the 1960s and 1970s."@en ;
    dcterms:identifier "CC00032" ;
    owl:sameAs <http://www.wikidata.org/entity/Q83328052> .

cc:CC00033 a owl:NamedIndividual ;
    rdfs:label "convertible collar"@en ;
    dcterms:description [ rdfs:label "A collar designed to be worn with the neck button either fastened or unfastened."@en ;
            dcterms:creator "Wikipedia" ;
            dcterms:license <https://creativecommons.org/publicdomain/mark/1.0/> ;
            dcterms:rights <https://creativecommons.org/publicdomain/mark/1.0/> ;
            dcterms:source <https://en.wikipedia.org/wiki/Collar_(clothing)> ],
        "A collar designed to be worn with the neck button either fastened or unfastened."@en ;
    dcterms:identifier "CC00033" ;
    owl:sameAs <http://www.wikidata.org/entity/Q83328209> .

cc:CC00036 a owl:NamedIndividual ;
    rdfs:label "jabot"@en ;
    dcterms:description [ rdfs:label "Detachable, made-up cascades of soft fabric, often lace, worn at the center front of the neckline over other garments. (AAT)"@en ;
            dcterms:creator "The J. Paul Getty Trust" ;
            dcterms:license <https://opendatacommons.org/licenses/by/1-0/> ;
            dcterms:rights <https://rightsstatements.org/vocab/InC/1.0/> ;
            dcterms:source <http://www.getty.edu/research/tools/vocabularies/aat/> ],
        "Detachable, made-up cascades of soft fabric, often lace, worn at the center front of the neckline over other garments. (AAT)"@en ;
    dcterms:identifier "CC00036" ;
    owl:sameAs <http://vocab.getty.edu/aat/300210062> .

cc:CC00038 a owl:NamedIndividual ;
    rdfs:label "Napoleon collar"@en ;
    dcterms:description [ rdfs:label "A turnover collar, associated with Emperor Napoleon I Bonaparte's military uniforms; fairly rigid in construction and open at the front, rising high and shaped to frame the wearer's neck and lower head"@en ;
            dcterms:creator "Wikipedia" ;
            dcterms:license <https://creativecommons.org/publicdomain/mark/1.0/> ;
            dcterms:rights <https://creativecommons.org/publicdomain/mark/1.0/> ;
            dcterms:source <https://en.wikipedia.org/wiki/Collar_(clothing)> ],
        "A turnover collar, associated with Emperor Napoleon I Bonaparte's military uniforms; fairly rigid in construction and open at the front, rising high and shaped to frame the wearer's neck and lower head"@en ;
    dcterms:identifier "CC00038" ;
    owl:sameAs <http://www.wikidata.org/entity/Q83328812> .

cc:CC00041 a owl:NamedIndividual ;
    rdfs:label "polo shirt collar"@en ;
    dcterms:identifier "CC00041" ;
    owl:sameAs <http://vocab.getty.edu/aat/300209896> .

cc:CC00044 a owl:NamedIndividual ;
    rdfs:label "ruffled collar"@en ;
    dcterms:identifier "CC00044" ;
    owl:sameAs <http://www.wikidata.org/entity/Q29583225> .

cc:CC00081 a owl:NamedIndividual ;
    rdfs:label "embroidery"@en ;
    dcterms:description [ rdfs:label "Refers to works characterized by a pattern or design executed in stitches using thread or fine wire. The designs are typically executed on textiles, but leather, paper, or another media may also be used; the designs may be intended to be framed, or to decorate apparel, bed linens, furniture coverings, pillows, altar cloths, ceremonial hangings, or other items."@en ;
            dcterms:creator "The J. Paul Getty Trust" ;
            dcterms:license <https://opendatacommons.org/licenses/by/1-0/> ;
            dcterms:rights <https://rightsstatements.org/vocab/InC/1.0/> ;
            dcterms:source <http://www.getty.edu/research/tools/vocabularies/aat/> ],
        "Refers to works characterized by a pattern or design executed in stitches using thread or fine wire. The designs are typically executed on textiles, but leather, paper, or another media may also be used; the designs may be intended to be framed, or to decorate apparel, bed linens, furniture coverings, pillows, altar cloths, ceremonial hangings, or other items."@en ;
    dcterms:identifier "CC00081" ;
    owl:sameAs <http://vocab.getty.edu/aat/300264024> .

cc:CC00091 a owl:NamedIndividual ;
    rdfs:label "needlepoint"@en ;
    dcterms:description [ rdfs:label "Refers to works created with a needle and thread on fabric or a mesh of canvas. The works are characterized by designs that are executed by using the grid of the fabric to count out the desired position of various stitches or colors in the design."@en ;
            dcterms:creator "The J. Paul Getty Trust" ;
            dcterms:license <https://opendatacommons.org/licenses/by/1-0/> ;
            dcterms:rights <https://rightsstatements.org/vocab/InC/1.0/> ;
            dcterms:source <http://www.getty.edu/research/tools/vocabularies/aat/> ],
        "Refers to works created with a needle and thread on fabric or a mesh of canvas. The works are characterized by designs that are executed by using the grid of the fabric to count out the desired position of various stitches or colors in the design."@en ;
    dcterms:identifier "CC00091" ;
    owl:sameAs <http://vocab.getty.edu/aat/300264031> .

cc:CC00103 a owl:NamedIndividual ;
    rdfs:label "bias-cut"@en ;
    dcterms:identifier "CC00103" .

cc:CC00104 a owl:NamedIndividual ;
    rdfs:label "bustle"@en ;
    dcterms:description [ rdfs:label "Frames of varied construction worn at or below the waist in the back to distend the garment backward at the hips."@en ;
            dcterms:creator "The J. Paul Getty Trust" ;
            dcterms:license <https://opendatacommons.org/licenses/by/1-0/> ;
            dcterms:rights <https://rightsstatements.org/vocab/InC/1.0/> ;
            dcterms:source <http://www.getty.edu/research/tools/vocabularies/aat/> ],
        "Frames of varied construction worn at or below the waist in the back to distend the garment backward at the hips."@en ;
    dcterms:identifier "CC00104" ;
    owl:sameAs <http://vocab.getty.edu/aat/300210580> .

cc:CC00105 a owl:NamedIndividual ;
    rdfs:label "chemise"@en ;
    dcterms:description [ rdfs:label "Loose-fitting, straight-hanging shirtlike underwear with or without sleeves, usually extending to the hip or knee."@en ;
            dcterms:creator "The J. Paul Getty Trust" ;
            dcterms:license <https://opendatacommons.org/licenses/by/1-0/> ;
            dcterms:rights <https://rightsstatements.org/vocab/InC/1.0/> ;
            dcterms:source <http://www.getty.edu/research/tools/vocabularies/aat/> ],
        "Loose-fitting, straight-hanging shirtlike underwear with or without sleeves, usually extending to the hip or knee."@en ;
    dcterms:identifier "CC00105" ;
    owl:sameAs <http://vocab.getty.edu/aat/300210542> .

cc:CC00107 a owl:NamedIndividual ;
    rdfs:label "crinoline"@en ;
    dcterms:description [ rdfs:label "Petticoats originally made with a stiff, woven fabric of horsehair, linen, cotton, or wool. Later often used in conjunction with hoops of whalebone or steel."@en ;
            dcterms:creator "The J. Paul Getty Trust" ;
            dcterms:license <https://opendatacommons.org/licenses/by/1-0/> ;
            dcterms:rights <https://rightsstatements.org/vocab/InC/1.0/> ;
            dcterms:source <http://www.getty.edu/research/tools/vocabularies/aat/> ],
        "Petticoats originally made with a stiff, woven fabric of horsehair, linen, cotton, or wool. Later often used in conjunction with hoops of whalebone or steel."@en ;
    dcterms:identifier "CC00107" ;
    owl:sameAs <http://vocab.getty.edu/aat/300210554> .

cc:CC00108 a owl:NamedIndividual ;
    rdfs:label "drop-waist"@en ;
    dcterms:identifier "CC00108" .

cc:CC00110 a owl:NamedIndividual ;
    rdfs:label "fit and flare"@en ;
    dcterms:identifier "CC00110" .

cc:CC00113 a owl:NamedIndividual ;
    rdfs:label "mantua"@en ;
    dcterms:description [ rdfs:label "Type of ladies' garment that first developed in the 1670s in Europe; they were relatively loose, gown- or coat-like garments worn belted at the waist with a long train draped at the hips to reveal the front of the matching petticoat below. This style replaced the earlier stiff, constricting boned bodice-and-skirt style previously worn by women. As the style evolved, the pleats at the front were reduced in number and the bodice was opened, with the torso now covered by a stiffened piece of fabric known as a stomacher. Originally an informal style, the mantua gradually developed as formal dress and the skirt grew to extraordinary proportions. The mantua was thought to display silk designs to their best advantage, as they were draped rather than cut; as such, it is believed the garment was named after Mantua, Italy, where expensive silks were produced. However, it has also been suggested that the name derives from manteau, the French term for a coat."@en ;
            dcterms:creator "The J. Paul Getty Trust" ;
            dcterms:license <https://opendatacommons.org/licenses/by/1-0/> ;
            dcterms:rights <https://rightsstatements.org/vocab/InC/1.0/> ;
            dcterms:source <http://www.getty.edu/research/tools/vocabularies/aat/> ],
        "Type of ladies' garment that first developed in the 1670s in Europe; they were relatively loose, gown- or coat-like garments worn belted at the waist with a long train draped at the hips to reveal the front of the matching petticoat below. This style replaced the earlier stiff, constricting boned bodice-and-skirt style previously worn by women. As the style evolved, the pleats at the front were reduced in number and the bodice was opened, with the torso now covered by a stiffened piece of fabric known as a stomacher. Originally an informal style, the mantua gradually developed as formal dress and the skirt grew to extraordinary proportions. The mantua was thought to display silk designs to their best advantage, as they were draped rather than cut; as such, it is believed the garment was named after Mantua, Italy, where expensive silks were produced. However, it has also been suggested that the name derives from manteau, the French term for a coat."@en ;
    dcterms:identifier "CC00113" ;
    owl:sameAs <http://vocab.getty.edu/aat/300209837> .

cc:CC00122 a owl:NamedIndividual ;
    rdfs:label "shirtwaist dress"@en ;
    dcterms:description [ rdfs:label "Dresses having a shirtwaist bodice, typically including a center front button or stud placket opening, cuffs, and a collar, imitating certain details of a man's shirt. The bodice is attached straight or full skirt, often having a belt at the waist."@en ;
            dcterms:creator "The J. Paul Getty Trust" ;
            dcterms:license <https://opendatacommons.org/licenses/by/1-0/> ;
            dcterms:rights <https://rightsstatements.org/vocab/InC/1.0/> ;
            dcterms:source <http://www.getty.edu/research/tools/vocabularies/aat/> ],
        "Dresses having a shirtwaist bodice, typically including a center front button or stud placket opening, cuffs, and a collar, imitating certain details of a man's shirt. The bodice is attached straight or full skirt, often having a belt at the waist."@en ;
    dcterms:identifier "CC00122" .

cc:CC00124 a owl:NamedIndividual ;
    rdfs:label "trapeze dress"@en ;
    dcterms:identifier "CC00124" .

cc:CC00127 a owl:NamedIndividual ;
    rdfs:label "wrapping"@en ;
    dcterms:description [ rdfs:label "Covering or enclosing entirely or to a great extent with a flexible material, especially by winding or folding."@en ;
            dcterms:creator "The J. Paul Getty Trust" ;
            dcterms:license <https://opendatacommons.org/licenses/by/1-0/> ;
            dcterms:rights <https://rightsstatements.org/vocab/InC/1.0/> ;
            dcterms:source <http://www.getty.edu/research/tools/vocabularies/aat/> ],
        "Covering or enclosing entirely or to a great extent with a flexible material, especially by winding or folding."@en ;
    dcterms:identifier "CC00127" .

cc:CC00131 a owl:NamedIndividual ;
    rdfs:label "dolman sleeve"@en ;
    dcterms:identifier "CC00131" .

cc:CC00133 a owl:NamedIndividual ;
    rdfs:label "kimono"@en ;
    dcterms:description [ rdfs:label "Loose, wide-sleeved garments fastened around the waist with an obi or broad sash, traditionally worn by Japanese men and women."@en ;
            dcterms:creator "The J. Paul Getty Trust" ;
            dcterms:license <https://opendatacommons.org/licenses/by/1-0/> ;
            dcterms:rights <https://rightsstatements.org/vocab/InC/1.0/> ;
            dcterms:source <http://www.getty.edu/research/tools/vocabularies/aat/> ],
        "Loose, wide-sleeved garments fastened around the waist with an obi or broad sash, traditionally worn by Japanese men and women."@en ;
    dcterms:identifier "CC00133" ;
    owl:sameAs <http://vocab.getty.edu/aat/300046171> .

cc:CC00136 a owl:NamedIndividual ;
    rdfs:label "petal sleeve"@en ;
    dcterms:identifier "CC00136" .

cc:CC00139 a owl:NamedIndividual ;
    rdfs:label "roll-up sleeves"@en ;
    dcterms:identifier "CC00139" .

cc:CC00141 a owl:NamedIndividual ;
    rdfs:label "straight"@en ;
    dcterms:identifier "CC00141" .

cc:CC00143 a owl:NamedIndividual ;
    rdfs:label "sleeveless pullovers"@en ;
    dcterms:identifier "CC00143" ;
    owl:sameAs <http://vocab.getty.edu/aat/300411733> .

cc:CC00144 a owl:NamedIndividual ;
    rdfs:label "cap sleeve"@en ;
    dcterms:identifier "CC00144" .

cc:CC00149 a owl:NamedIndividual ;
    rdfs:label "extra long sleeve"@en ;
    dcterms:identifier "CC00149" .

cc:CC00151 a owl:NamedIndividual ;
    rdfs:label "angled waistline"@en ;
    dcterms:identifier "CC00151" .

cc:CC00152 a owl:NamedIndividual ;
    rdfs:label "asymmetrical"@en ;
    dcterms:identifier "CC00152" .

cc:CC00153 a owl:NamedIndividual ;
    rdfs:label "bare midriff"@en ;
    dcterms:identifier "CC00153" .

cc:CC00155 a owl:NamedIndividual ;
    rdfs:label "bolero"@en ;
    dcterms:description [ rdfs:label "Waist-length or shorter jackets, with or without sleeves, usually collarless, and worn open in the front; originally worn by men in Spain."@en ;
            dcterms:creator "The J. Paul Getty Trust" ;
            dcterms:license <https://opendatacommons.org/licenses/by/1-0/> ;
            dcterms:rights <https://rightsstatements.org/vocab/InC/1.0/> ;
            dcterms:source <http://www.getty.edu/research/tools/vocabularies/aat/> ],
        "Waist-length or shorter jackets, with or without sleeves, usually collarless, and worn open in the front; originally worn by men in Spain."@en ;
    dcterms:identifier "CC00155" ;
    owl:sameAs <http://vocab.getty.edu/aat/300209876> .

cc:CC00157 a owl:NamedIndividual ;
    rdfs:label "dropped"@en ;
    dcterms:identifier "CC00157" .

cc:CC00158 a owl:NamedIndividual ;
    rdfs:label "high"@en ;
    dcterms:identifier "CC00158" .

cc:CC00159 a owl:NamedIndividual ;
    rdfs:label "hip-level"@en ;
    dcterms:identifier "CC00159" .

cc:CC00161 a owl:NamedIndividual ;
    rdfs:label "no waistline"@en ;
    dcterms:identifier "CC00161" .

cc:CC00163 a owl:NamedIndividual ;
    rdfs:label "accordion pleats"@en ;
    dcterms:description [ rdfs:label "Wide, sharply pressed pleats, arranged in a row, evenly spaced and all turned in the same direction. For narrow pleats of a similar nature, use \"knife pleats.\""@en ;
            dcterms:creator "The J. Paul Getty Trust" ;
            dcterms:license <https://opendatacommons.org/licenses/by/1-0/> ;
            dcterms:rights <https://rightsstatements.org/vocab/InC/1.0/> ;
            dcterms:source <http://www.getty.edu/research/tools/vocabularies/aat/> ],
        "Wide, sharply pressed pleats, arranged in a row, evenly spaced and all turned in the same direction. For narrow pleats of a similar nature, use \"knife pleats.\""@en ;
    dcterms:identifier "CC00163" ;
    owl:sameAs <http://vocab.getty.edu/aat/300228360> .

cc:CC00172 a owl:NamedIndividual ;
    rdfs:label "handkerchief"@en ;
    dcterms:description [ rdfs:label "Pieces of cloth, usually square, varying in size and material, carried for usefulness or as a costume accessory."@en ;
            dcterms:creator "The J. Paul Getty Trust" ;
            dcterms:license <https://opendatacommons.org/licenses/by/1-0/> ;
            dcterms:rights <https://rightsstatements.org/vocab/InC/1.0/> ;
            dcterms:source <http://www.getty.edu/research/tools/vocabularies/aat/> ],
        "Pieces of cloth, usually square, varying in size and material, carried for usefulness or as a costume accessory."@en ;
    dcterms:identifier "CC00172" ;
    owl:sameAs <http://vocab.getty.edu/aat/300216195> .

cc:CC00185 a owl:NamedIndividual ;
    rdfs:label "above knee"@en ;
    dcterms:identifier "CC00185" .

cc:CC00186 a owl:NamedIndividual ;
    rdfs:label "ankle length"@en ;
    dcterms:identifier "CC00186" .

cc:CC00187 a owl:NamedIndividual ;
    rdfs:label "floor length"@en ;
    dcterms:identifier "CC00187" .

cc:CC00188 a owl:NamedIndividual ;
    rdfs:label "hip length"@en ;
    dcterms:identifier "CC00188" .

cc:CC00189 a owl:NamedIndividual ;
    rdfs:label "knee length"@en ;
    dcterms:identifier "CC00189" .

cc:CC00190 a owl:NamedIndividual ;
    rdfs:label "maxi dress"@en ;
    dcterms:description [ rdfs:label "Dresses with long skirts."@en ;
            dcterms:creator "The J. Paul Getty Trust" ;
            dcterms:license <https://opendatacommons.org/licenses/by/1-0/> ;
            dcterms:rights <https://rightsstatements.org/vocab/InC/1.0/> ;
            dcterms:source <http://www.getty.edu/research/tools/vocabularies/aat/> ],
        "Dresses with long skirts."@en ;
    dcterms:identifier "CC00190" ;
    owl:sameAs <http://vocab.getty.edu/aat/300375298> .

cc:CC00191 a owl:NamedIndividual ;
    rdfs:label "mid calf length"@en ;
    dcterms:identifier "CC00191" .

cc:CC00192 a owl:NamedIndividual ;
    rdfs:label "mid-thigh length"@en ;
    dcterms:identifier "CC00192" .

cc:CC00193 a owl:NamedIndividual ;
    rdfs:label "midi dress"@en ;
    dcterms:description [ rdfs:label "Dresses of intermediate length. They are longer than mini dresses but shorter than maxi dresses, usually extending to mid-calf."@en ;
            dcterms:creator "The J. Paul Getty Trust" ;
            dcterms:license <https://opendatacommons.org/licenses/by/1-0/> ;
            dcterms:rights <https://rightsstatements.org/vocab/InC/1.0/> ;
            dcterms:source <http://www.getty.edu/research/tools/vocabularies/aat/> ],
        "Dresses of intermediate length. They are longer than mini dresses but shorter than maxi dresses, usually extending to mid-calf."@en ;
    dcterms:identifier "CC00193" ;
    owl:sameAs <http://vocab.getty.edu/aat/300375299> .

cc:CC00198 a owl:NamedIndividual ;
    rdfs:label "basket weave"@en ;
    dcterms:description [ rdfs:label "Weaving technique with a simple criss-cross checkerboard pattern in which two or more filling yarns, or a single heavier yarn, pass over and under two or more warp yarns."@en ;
            dcterms:creator "The J. Paul Getty Trust" ;
            dcterms:license <https://opendatacommons.org/licenses/by/1-0/> ;
            dcterms:rights <https://rightsstatements.org/vocab/InC/1.0/> ;
            dcterms:source <http://www.getty.edu/research/tools/vocabularies/aat/> ],
        "Weaving technique with a simple criss-cross checkerboard pattern in which two or more filling yarns, or a single heavier yarn, pass over and under two or more warp yarns."@en ;
    dcterms:identifier "CC00198" ;
    owl:sameAs <http://vocab.getty.edu/aat/300400693> .

cc:CC00207 a owl:NamedIndividual ;
    rdfs:label "crochet"@en ;
    dcterms:description [ rdfs:label "Needlework created by crocheting, which employs looped stitches made with a single cord or strand of yarn and a single hooked needle."@en ;
            dcterms:creator "The J. Paul Getty Trust" ;
            dcterms:license <https://opendatacommons.org/licenses/by/1-0/> ;
            dcterms:rights <https://rightsstatements.org/vocab/InC/1.0/> ;
            dcterms:source <http://www.getty.edu/research/tools/vocabularies/aat/> ],
        "Needlework created by crocheting, which employs looped stitches made with a single cord or strand of yarn and a single hooked needle."@en ;
    dcterms:identifier "CC00207" ;
    owl:sameAs <http://vocab.getty.edu/aat/300264038> .

cc:CC00209 a owl:NamedIndividual ;
    rdfs:label "dobby weave"@en ;
    dcterms:description [ rdfs:label "Dobby weave is an allover figured fabric made on looms having a dobby attachment, with narrow strips of wood instead of Jacquard cards. Dobby weaves are limited to simple, small geometric figures, with the design repeated frequently, and are fairly inexpensive to produce."@en ;
            dcterms:creator "The J. Paul Getty Trust" ;
            dcterms:license <https://opendatacommons.org/licenses/by/1-0/> ;
            dcterms:rights <https://rightsstatements.org/vocab/InC/1.0/> ;
            dcterms:source <http://www.getty.edu/research/tools/vocabularies/aat/> ],
        "Dobby weave is an allover figured fabric made on looms having a dobby attachment, with narrow strips of wood instead of Jacquard cards. Dobby weaves are limited to simple, small geometric figures, with the design repeated frequently, and are fairly inexpensive to produce."@en ;
    dcterms:identifier "CC00209" ;
    owl:sameAs <http://vocab.getty.edu/aat/300417868> .

cc:CC00223 a owl:NamedIndividual ;
    rdfs:label "matelasse"@en ;
    dcterms:description [ rdfs:label "A double-woven textile with a quilted appearance, utilizing a wadding weft to increase the relief."@en ;
            dcterms:creator "The J. Paul Getty Trust" ;
            dcterms:license <https://opendatacommons.org/licenses/by/1-0/> ;
            dcterms:rights <https://rightsstatements.org/vocab/InC/1.0/> ;
            dcterms:source <http://www.getty.edu/research/tools/vocabularies/aat/> ],
        "A double-woven textile with a quilted appearance, utilizing a wadding weft to increase the relief."@en ;
    dcterms:identifier "CC00223" ;
    owl:sameAs <http://vocab.getty.edu/aat/300227854> .

cc:CC00228 a owl:NamedIndividual ;
    rdfs:label "natural waistline"@en ;
    dcterms:identifier "CC00228" .

cc:CC00231 a owl:NamedIndividual ;
    rdfs:label "plain weave"@en ;
    dcterms:description [ rdfs:label "Textile in which warp/weft pathways are over/under every other thread. Tabby weave textiles are woven by a method based on a unit of two ends and two picks, in which each end passes over one and under one pick; the binding points are set over one end on successive picks."@en ;
            dcterms:creator "The J. Paul Getty Trust" ;
            dcterms:license <https://opendatacommons.org/licenses/by/1-0/> ;
            dcterms:rights <https://rightsstatements.org/vocab/InC/1.0/> ;
            dcterms:source <http://www.getty.edu/research/tools/vocabularies/aat/> ],
        "Textile in which warp/weft pathways are over/under every other thread. Tabby weave textiles are woven by a method based on a unit of two ends and two picks, in which each end passes over one and under one pick; the binding points are set over one end on successive picks."@en ;
    dcterms:identifier "CC00231" ;
    owl:sameAs <http://vocab.getty.edu/aat/300227906> .

cc:CC00237 a owl:NamedIndividual ;
    rdfs:label "rib weave"@en ;
    dcterms:description [ rdfs:label "Woven fabrics with ribbed or corded effects in either the warp or filling direction. Warp faced rib weave has a fine warp covering a thicker weft. In weft faced rib weave, a thin weft completely covers a thicker warp."@en ;
            dcterms:creator "The J. Paul Getty Trust" ;
            dcterms:license <https://opendatacommons.org/licenses/by/1-0/> ;
            dcterms:rights <https://rightsstatements.org/vocab/InC/1.0/> ;
            dcterms:source <http://www.getty.edu/research/tools/vocabularies/aat/> ],
        "Woven fabrics with ribbed or corded effects in either the warp or filling direction. Warp faced rib weave has a fine warp covering a thicker weft. In weft faced rib weave, a thin weft completely covers a thicker warp."@en ;
    dcterms:identifier "CC00237" ;
    owl:sameAs <http://vocab.getty.edu/aat/300417856> .

cc:CC00246 a owl:NamedIndividual ;
    rdfs:label "twill weave"@en ;
    dcterms:description [ rdfs:label "Refers to a woven textile characterized by parallel diagonal ridges or ribs, produced by passing the weft threads over one and under two or more threads of the warp, instead of over and under in regular succession, as in plain weaving. Regular twill features a diagonal line that is repeated regularly, usually running from the left to right at a 45-degree angle and upward. The weave may be varied in several ways, including changing the angle or direction of the twill line, as exemplified in herringbone twill."@en ;
            dcterms:creator "The J. Paul Getty Trust" ;
            dcterms:license <https://opendatacommons.org/licenses/by/1-0/> ;
            dcterms:rights <https://rightsstatements.org/vocab/InC/1.0/> ;
            dcterms:source <http://www.getty.edu/research/tools/vocabularies/aat/> ],
        "Refers to a woven textile characterized by parallel diagonal ridges or ribs, produced by passing the weft threads over one and under two or more threads of the warp, instead of over and under in regular succession, as in plain weaving. Regular twill features a diagonal line that is repeated regularly, usually running from the left to right at a 45-degree angle and upward. The weave may be varied in several ways, including changing the angle or direction of the twill line, as exemplified in herringbone twill."@en ;
    dcterms:identifier "CC00246" ;
    owl:sameAs <http://vocab.getty.edu/aat/300227915> .

cc:CC00252 a owl:NamedIndividual ;
    rdfs:label "chemise dress"@en ;
    dcterms:description [ rdfs:label "Dresses which hang straight from the shoulders, sometimes tapering slightly at hips."@en ;
            dcterms:creator "The J. Paul Getty Trust" ;
            dcterms:license <https://opendatacommons.org/licenses/by/1-0/> ;
            dcterms:rights <https://rightsstatements.org/vocab/InC/1.0/> ;
            dcterms:source <http://www.getty.edu/research/tools/vocabularies/aat/> ],
        "Dresses which hang straight from the shoulders, sometimes tapering slightly at hips."@en ;
    dcterms:identifier "CC00252" ;
    owl:sameAs <http://vocab.getty.edu/aat/300214100> .

cc:CC00265 a owl:NamedIndividual ;
    rdfs:label "brass"@en ;
    dcterms:description [ rdfs:label "Alloy of copper and zinc, usually with copper as the major alloying element and zinc up to 40% by weight."@en ;
            dcterms:creator "The J. Paul Getty Trust" ;
            dcterms:license <https://opendatacommons.org/licenses/by/1-0/> ;
            dcterms:rights <https://rightsstatements.org/vocab/InC/1.0/> ;
            dcterms:source <http://www.getty.edu/research/tools/vocabularies/aat/> ],
        "Alloy of copper and zinc, usually with copper as the major alloying element and zinc up to 40% by weight."@en ;
    dcterms:identifier "CC00265" ;
    owl:sameAs <http://vocab.getty.edu/aat/300010946> .

cc:CC00271 a owl:NamedIndividual ;
    rdfs:label "cloth"@en ;
    dcterms:description [ rdfs:label "Generally, textile that is woven, felted, knit, pounded, or otherwise made into a flat piece. For textile in the form of continuous strands made from filaments of fiber by reeling, spinning, twisting, or throwing, see \"yarn.\""@en ;
            dcterms:creator "The J. Paul Getty Trust" ;
            dcterms:license <https://opendatacommons.org/licenses/by/1-0/> ;
            dcterms:rights <https://rightsstatements.org/vocab/InC/1.0/> ;
            dcterms:source <http://www.getty.edu/research/tools/vocabularies/aat/> ],
        "Generally, textile that is woven, felted, knit, pounded, or otherwise made into a flat piece. For textile in the form of continuous strands made from filaments of fiber by reeling, spinning, twisting, or throwing, see \"yarn.\""@en ;
    dcterms:identifier "CC00271" ;
    owl:sameAs <http://vocab.getty.edu/aat/300162391> .

cc:CC00291 a owl:NamedIndividual ;
    rdfs:label "mink fur"@en ;
    dcterms:identifier "CC00291" ;
    owl:sameAs <http://www.wikidata.org/entity/Q1262096> .

cc:CC00301 a owl:NamedIndividual ;
    rdfs:label "pongee"@en ;
    dcterms:description [ rdfs:label "Soft, thin woven, and usually unbleached fabric woven from uneven threads of raw silk, cotton, or artificial fibers. It is often piece-dyed or printed. The term, of Chinese origin, means 'woven at home'."@en ;
            dcterms:creator "The J. Paul Getty Trust" ;
            dcterms:license <https://opendatacommons.org/licenses/by/1-0/> ;
            dcterms:rights <https://rightsstatements.org/vocab/InC/1.0/> ;
            dcterms:source <http://www.getty.edu/research/tools/vocabularies/aat/> ],
        "Soft, thin woven, and usually unbleached fabric woven from uneven threads of raw silk, cotton, or artificial fibers. It is often piece-dyed or printed. The term, of Chinese origin, means 'woven at home'."@en ;
    dcterms:identifier "CC00301" ;
    owl:sameAs <http://vocab.getty.edu/aat/300417854> .

cc:CC00309 a owl:NamedIndividual ;
    rdfs:label "starch"@en ;
    dcterms:description [ rdfs:label "Substance made of carbohydrate granules of varying sizes obtained from roots, bulbs, and seeds of most plants. Starch is primarily obtained from rice, wheat, corn, potatoes, cassava (tapioca), sago, and arrowroot. It is a mixture of the soluble straight-chain amylose molecules and the insoluble, branched-chain amylopectin molecules. When starch is heated, the granules swell and form a thick, tacky jelly upon cooling. Starchy adhesives have been used since at least 3500 BCE in Egypt. More recently starch has been used for sizing fabric, canvas, and paper, as an adhesive for paper cartons, bottle labels, gummed tape, and envelopes. Soluble starch has been used for priming canvas and as a binder in watercolor paints. Starch is sensitive to moisture and biodegradation. Starchy paste films become brittle with age."@en ;
            dcterms:creator "The J. Paul Getty Trust" ;
            dcterms:license <https://opendatacommons.org/licenses/by/1-0/> ;
            dcterms:rights <https://rightsstatements.org/vocab/InC/1.0/> ;
            dcterms:source <http://www.getty.edu/research/tools/vocabularies/aat/> ],
        "Substance made of carbohydrate granules of varying sizes obtained from roots, bulbs, and seeds of most plants. Starch is primarily obtained from rice, wheat, corn, potatoes, cassava (tapioca), sago, and arrowroot. It is a mixture of the soluble straight-chain amylose molecules and the insoluble, branched-chain amylopectin molecules. When starch is heated, the granules swell and form a thick, tacky jelly upon cooling. Starchy adhesives have been used since at least 3500 BCE in Egypt. More recently starch has been used for sizing fabric, canvas, and paper, as an adhesive for paper cartons, bottle labels, gummed tape, and envelopes. Soluble starch has been used for priming canvas and as a binder in watercolor paints. Starch is sensitive to moisture and biodegradation. Starchy paste films become brittle with age."@en ;
    dcterms:identifier "CC00309" ;
    owl:sameAs <http://vocab.getty.edu/aat/300012959> .

cc:CC00310 a owl:NamedIndividual ;
    rdfs:label "steel"@en ;
    dcterms:description [ rdfs:label "Any of various hard, strong, durable, malleable alloys of iron and carbon, often with other elements such as manganese, chromium, nickel, molybdenum, copper, tungsten, cobalt, or silicon; widely used as a structural material."@en ;
            dcterms:creator "The J. Paul Getty Trust" ;
            dcterms:license <https://opendatacommons.org/licenses/by/1-0/> ;
            dcterms:rights <https://rightsstatements.org/vocab/InC/1.0/> ;
            dcterms:source <http://www.getty.edu/research/tools/vocabularies/aat/> ],
        "Any of various hard, strong, durable, malleable alloys of iron and carbon, often with other elements such as manganese, chromium, nickel, molybdenum, copper, tungsten, cobalt, or silicon; widely used as a structural material."@en ;
    dcterms:identifier "CC00310" ;
    owl:sameAs <http://vocab.getty.edu/aat/300133751> .

cc:CC00320 a owl:NamedIndividual ;
    rdfs:label "weave"@en ;
    dcterms:identifier "CC00320" ;
    owl:sameAs <http://www.wikidata.org/entity/Q2862826> .

cc:CC00324 a owl:NamedIndividual ;
    rdfs:label "hoop skirt"@en ;
    dcterms:identifier "CC00324" ;
    owl:sameAs <http://vocab.getty.edu/aat/300426171> .

cc:CC00328 a owl:NamedIndividual ;
    rdfs:label "foresleeve"@en ;
    dcterms:description [ rdfs:label "decorative half-sleeve reaching generally from the elbow to the wrist, worn under trumpet sleeves in the 16th century"@en ;
            dcterms:creator "Wikidata contributors" ;
            dcterms:license <https://creativecommons.org/publicdomain/mark/1.0/> ;
            dcterms:rights <https://creativecommons.org/publicdomain/mark/1.0/> ;
            dcterms:source <https://www.wikidata.org/wiki/Wikidata:Data_access/en> ],
        "decorative half-sleeve reaching generally from the elbow to the wrist, worn under trumpet sleeves in the 16th century"@en ;
    dcterms:identifier "CC00328" ;
    owl:sameAs <http://www.wikidata.org/entity/Q73540794> .

cc:CC00334 a owl:NamedIndividual ;
    rdfs:label "dolman"@en ;
    dcterms:description [ rdfs:label "Mantles with a sleeve cut all in one with the side piece and hanging loose; sometimes made in the form of a sling."@en ;
            dcterms:creator "The J. Paul Getty Trust" ;
            dcterms:license <https://opendatacommons.org/licenses/by/1-0/> ;
            dcterms:rights <https://rightsstatements.org/vocab/InC/1.0/> ;
            dcterms:source <http://www.getty.edu/research/tools/vocabularies/aat/> ],
        "Mantles with a sleeve cut all in one with the side piece and hanging loose; sometimes made in the form of a sling."@en ;
    dcterms:identifier "CC00334" ;
    owl:sameAs <http://vocab.getty.edu/aat/300220742> .

cc:CC00336 a owl:NamedIndividual ;
    rdfs:label "bodice"@en ;
    dcterms:description [ rdfs:label "Originally, tight fitting, sleeveless garments for the torso and bust, quilted and strengthened with whalebone, worn chiefly by women, but also by men. Bodices were typically cross-laced at the side or back, and worn over a blouse or chemise. The term comes from \"a pair of bodies,\" the use of the plural referring to the fact that the garment was made in two pieces laced together. The term also now refers to the generally tight-fitting upper part of a woman's dress or to any tight-fitting outer vest or waistcoat"@en ;
            dcterms:creator "The J. Paul Getty Trust" ;
            dcterms:license <https://opendatacommons.org/licenses/by/1-0/> ;
            dcterms:rights <https://rightsstatements.org/vocab/InC/1.0/> ;
            dcterms:source <http://www.getty.edu/research/tools/vocabularies/aat/> ],
        "Originally, tight fitting, sleeveless garments for the torso and bust, quilted and strengthened with whalebone, worn chiefly by women, but also by men. Bodices were typically cross-laced at the side or back, and worn over a blouse or chemise. The term comes from \"a pair of bodies,\" the use of the plural referring to the fact that the garment was made in two pieces laced together. The term also now refers to the generally tight-fitting upper part of a woman's dress or to any tight-fitting outer vest or waistcoat"@en ;
    dcterms:identifier "CC00336" ;
    owl:sameAs <http://vocab.getty.edu/aat/300209874> .

cc:CC00337 a owl:NamedIndividual ;
    rdfs:label "blouse"@en ;
    dcterms:description [ rdfs:label "Main garments for the upper body, usually lightweight and loose-fitting, made with or without sleeves and worn over or tucked in the waistband of a skirt or trousers, especially by workmen, peasants and artists. Also, women's garments cut in the style of a man's classic, tailored-cut shirt, having a notch collar, collar band, front placket opening, and usually long sleeves with cuffs"@en ;
            dcterms:creator "The J. Paul Getty Trust" ;
            dcterms:license <https://opendatacommons.org/licenses/by/1-0/> ;
            dcterms:rights <https://rightsstatements.org/vocab/InC/1.0/> ;
            dcterms:source <http://www.getty.edu/research/tools/vocabularies/aat/> ],
        "Main garments for the upper body, usually lightweight and loose-fitting, made with or without sleeves and worn over or tucked in the waistband of a skirt or trousers, especially by workmen, peasants and artists. Also, women's garments cut in the style of a man's classic, tailored-cut shirt, having a notch collar, collar band, front placket opening, and usually long sleeves with cuffs"@en ;
    dcterms:identifier "CC00337" ;
    owl:sameAs <http://vocab.getty.edu/aat/300046133> .

cc:CC00338 a owl:NamedIndividual ;
    rdfs:label "forward sleeve"@en ;
    dcterms:description [ rdfs:label "sleeve in which the central axis is positioned forward of the lateral plane of the body, allowing increased range of motion"@en ;
            dcterms:creator "Wikidata contributors" ;
            dcterms:license <https://creativecommons.org/publicdomain/mark/1.0/> ;
            dcterms:rights <https://creativecommons.org/publicdomain/mark/1.0/> ;
            dcterms:source <https://www.wikidata.org/wiki/Wikidata:Data_access/en> ],
        "sleeve in which the central axis is positioned forward of the lateral plane of the body, allowing increased range of motion"@en ;
    dcterms:identifier "CC00338" ;
    owl:sameAs <http://www.wikidata.org/entity/Q67608772> .

cc:CC00340 a owl:NamedIndividual ;
    rdfs:label "shirt"@en ;
    dcterms:description [ rdfs:label "Generally refers to various types of main garments for the upper body, made with or without sleeves and worn over or tucked in the waistband of a skirt, trousers, or the like. Usually having a collar, which may be detachable, often a front opening, and sometimes pockets. Specifically often refers to an article of male attire with long sleeves terminating in wristbands or cuffs. It originally referred to undergarments for the upper part of the body, made of linen, calico, flannel, silk, or other washable material; originally always worn next to the skin."@en ;
            dcterms:creator "The J. Paul Getty Trust" ;
            dcterms:license <https://opendatacommons.org/licenses/by/1-0/> ;
            dcterms:rights <https://rightsstatements.org/vocab/InC/1.0/> ;
            dcterms:source <http://www.getty.edu/research/tools/vocabularies/aat/> ],
        "Generally refers to various types of main garments for the upper body, made with or without sleeves and worn over or tucked in the waistband of a skirt, trousers, or the like. Usually having a collar, which may be detachable, often a front opening, and sometimes pockets. Specifically often refers to an article of male attire with long sleeves terminating in wristbands or cuffs. It originally referred to undergarments for the upper part of the body, made of linen, calico, flannel, silk, or other washable material; originally always worn next to the skin."@en ;
    dcterms:identifier "CC00340" ;
    owl:sameAs <http://vocab.getty.edu/aat/300212499> .

cc:CC00348 a owl:NamedIndividual ;
    rdfs:label "center back closure"@en ;
    dcterms:identifier "CC00348" .

cc:CC00349 a owl:NamedIndividual ;
    rdfs:label "center front closure"@en ;
    dcterms:identifier "CC00349" .

cc:CC00351 a owl:NamedIndividual ;
    rdfs:label "neck closure"@en ;
    dcterms:identifier "CC00351" .

cc:CC00352 a owl:NamedIndividual ;
    rdfs:label "off-center back closure"@en ;
    dcterms:identifier "CC00352" .

cc:CC00353 a owl:NamedIndividual ;
    rdfs:label "off-center front closure"@en ;
    dcterms:identifier "CC00353" .

cc:CC00354 a owl:NamedIndividual ;
    rdfs:label "side closure"@en ;
    dcterms:identifier "CC00354" .

cc:CC00358 a owl:NamedIndividual ;
    rdfs:label "sleeve"@en ;
    dcterms:description [ rdfs:label "Shaped coverings for the arm. Originally made separate from the main garment and attached by lacing through eyelets at the shoulder; later, often made as component parts of garments."@en ;
            dcterms:creator "The J. Paul Getty Trust" ;
            dcterms:license <https://opendatacommons.org/licenses/by/1-0/> ;
            dcterms:rights <https://rightsstatements.org/vocab/InC/1.0/> ;
            dcterms:source <http://www.getty.edu/research/tools/vocabularies/aat/> ],
        "Shaped coverings for the arm. Originally made separate from the main garment and attached by lacing through eyelets at the shoulder; later, often made as component parts of garments."@en ;
    dcterms:identifier "CC00358" ;
    owl:sameAs <http://vocab.getty.edu/aat/300210530> .

cc:CC00363 a owl:NamedIndividual ;
    rdfs:label "trumpet sleeve"@en ;
    dcterms:description [ rdfs:label "long, wide, flaring sleeve worn turned back over a foresleeve and pinned near the shoulder, often fur-lined"@en ;
            dcterms:creator "Wikidata contributors" ;
            dcterms:license <https://creativecommons.org/publicdomain/mark/1.0/> ;
            dcterms:rights <https://creativecommons.org/publicdomain/mark/1.0/> ;
            dcterms:source <https://www.wikidata.org/wiki/Wikidata:Data_access/en> ],
        "long, wide, flaring sleeve worn turned back over a foresleeve and pinned near the shoulder, often fur-lined"@en ;
    dcterms:identifier "CC00363" ;
    owl:sameAs <http://www.wikidata.org/entity/Q73540348> .

cc:CC00369 a owl:NamedIndividual ;
    rdfs:label "dinner dress"@en ;
    dcterms:description [ rdfs:label "Mode of dress for a fashionable women in the 19th and 20th centuries; dinner dress is less formal than evening wear, ensembles often include sleeves, or open decolletage."@en ;
            dcterms:creator "The J. Paul Getty Trust" ;
            dcterms:license <https://opendatacommons.org/licenses/by/1-0/> ;
            dcterms:rights <https://rightsstatements.org/vocab/InC/1.0/> ;
            dcterms:source <http://www.getty.edu/research/tools/vocabularies/aat/> ],
        "Mode of dress for a fashionable women in the 19th and 20th centuries; dinner dress is less formal than evening wear, ensembles often include sleeves, or open decolletage."@en ;
    dcterms:identifier "CC00369" ;
    owl:sameAs <http://vocab.getty.edu/aat/300411766> .

cc:CC00373 a owl:NamedIndividual ;
    rdfs:label "morning dress"@en ;
    dcterms:description [ rdfs:label "Formal daytime dress for men; also, during the 19th century, women's dress appropriate for wear in the morning."@en ;
            dcterms:creator "The J. Paul Getty Trust" ;
            dcterms:license <https://opendatacommons.org/licenses/by/1-0/> ;
            dcterms:rights <https://rightsstatements.org/vocab/InC/1.0/> ;
            dcterms:source <http://www.getty.edu/research/tools/vocabularies/aat/> ],
        "Formal daytime dress for men; also, during the 19th century, women's dress appropriate for wear in the morning."@en ;
    dcterms:identifier "CC00373" ;
    owl:sameAs <http://vocab.getty.edu/aat/300255803> .

cc:CC00375 a owl:NamedIndividual ;
    rdfs:label "party dress"@en ;
    dcterms:identifier "CC00375" ;
    owl:sameAs <http://www.wikidata.org/entity/Q7140985> .

cc:CC00377 a owl:NamedIndividual ;
    rdfs:label "sports uniform"@en ;
    dcterms:description [ rdfs:label "Uniforms worn by sports teams and athletes."@en ;
            dcterms:creator "The J. Paul Getty Trust" ;
            dcterms:license <https://opendatacommons.org/licenses/by/1-0/> ;
            dcterms:rights <https://rightsstatements.org/vocab/InC/1.0/> ;
            dcterms:source <http://www.getty.edu/research/tools/vocabularies/aat/> ],
        "Uniforms worn by sports teams and athletes."@en ;
    dcterms:identifier "CC00377" ;
    owl:sameAs <http://vocab.getty.edu/aat/300266714> .

cc:CC00392 a owl:NamedIndividual ;
    rdfs:label "virago sleeve"@en ;
    dcterms:description [ rdfs:label "double-puffed, paned sleeve"@en ;
            dcterms:creator "Wikidata contributors" ;
            dcterms:license <https://creativecommons.org/publicdomain/mark/1.0/> ;
            dcterms:rights <https://creativecommons.org/publicdomain/mark/1.0/> ;
            dcterms:source <https://www.wikidata.org/wiki/Wikidata:Data_access/en> ],
        "double-puffed, paned sleeve"@en ;
    dcterms:identifier "CC00392" ;
    owl:sameAs <http://www.wikidata.org/entity/Q7933576> .

cc:CC00401 a owl:NamedIndividual ;
    rdfs:label "two piece tailored sleeve"@en ;
    dcterms:identifier "CC00401" .

cc:CC00402 a owl:NamedIndividual ;
    rdfs:label "main garment"@en ;
    dcterms:description [ rdfs:label "Main layer of dress, usually exclusive of accessories."@en ;
            dcterms:creator "The J. Paul Getty Trust" ;
            dcterms:license <https://opendatacommons.org/licenses/by/1-0/> ;
            dcterms:rights <https://rightsstatements.org/vocab/InC/1.0/> ;
            dcterms:source <http://www.getty.edu/research/tools/vocabularies/aat/> ],
        "Main layer of dress, usually exclusive of accessories."@en ;
    dcterms:identifier "CC00402" ;
    owl:sameAs <http://vocab.getty.edu/aat/300209263> .

cc:CC00403 a owl:NamedIndividual ;
    rdfs:label "Collection"@en ;
    dcterms:description [ rdfs:label "A collection is described as a group; its parts may also be separately described."@en ;
            dcterms:creator "Dublin Core Metadata Initiative (DCMI)" ;
            dcterms:license <https://creativecommons.org/licenses/by/3.0/> ;
            dcterms:rights <https://rightsstatements.org/vocab/InC/1.0/> ;
            dcterms:source <https://www.dublincore.org/specifications/dublin-core/dcmi-type-vocabulary/> ],
        "A collection is described as a group; its parts may also be separately described."@en ;
    dcterms:identifier "CC00403" .

cc:CC00404 a owl:NamedIndividual ;
    rdfs:label "Dataset"@en ;
    dcterms:description [ rdfs:label "Data encoded in a defined structure."@en ;
            dcterms:creator "Dublin Core Metadata Initiative (DCMI)" ;
            dcterms:license <https://creativecommons.org/licenses/by/3.0/> ;
            dcterms:rights <https://rightsstatements.org/vocab/InC/1.0/> ;
            dcterms:source <https://www.dublincore.org/specifications/dublin-core/dcmi-type-vocabulary/> ],
        "Data encoded in a defined structure."@en ;
    dcterms:identifier "CC00404" .

cc:CC00405 a owl:NamedIndividual ;
    rdfs:label "Event"@en ;
    dcterms:description [ rdfs:label "A non-persistent, time-based occurrence."@en ;
            dcterms:creator "Dublin Core Metadata Initiative (DCMI)" ;
            dcterms:license <https://creativecommons.org/licenses/by/3.0/> ;
            dcterms:rights <https://rightsstatements.org/vocab/InC/1.0/> ;
            dcterms:source <https://www.dublincore.org/specifications/dublin-core/dcmi-type-vocabulary/> ],
        "A non-persistent, time-based occurrence."@en ;
    dcterms:identifier "CC00405" .

cc:CC00406 a owl:NamedIndividual ;
    rdfs:label "Image"@en ;
    dcterms:description [ rdfs:label "A visual representation other than text."@en ;
            dcterms:creator "Dublin Core Metadata Initiative (DCMI)" ;
            dcterms:license <https://creativecommons.org/licenses/by/3.0/> ;
            dcterms:rights <https://rightsstatements.org/vocab/InC/1.0/> ;
            dcterms:source <https://www.dublincore.org/specifications/dublin-core/dcmi-type-vocabulary/> ],
        "A visual representation other than text."@en ;
    dcterms:identifier "CC00406" .

cc:CC00407 a owl:NamedIndividual ;
    rdfs:label "Interactive Resource"@en ;
    dcterms:description [ rdfs:label "A resource requiring interaction from the user to be understood, executed, or experienced."@en ;
            dcterms:creator "Dublin Core Metadata Initiative (DCMI)" ;
            dcterms:license <https://creativecommons.org/licenses/by/3.0/> ;
            dcterms:rights <https://rightsstatements.org/vocab/InC/1.0/> ;
            dcterms:source <https://www.dublincore.org/specifications/dublin-core/dcmi-type-vocabulary/> ],
        "A resource requiring interaction from the user to be understood, executed, or experienced."@en ;
    dcterms:identifier "CC00407" .

cc:CC00408 a owl:NamedIndividual ;
    rdfs:label "Moving Image"@en ;
    dcterms:description [ rdfs:label "A series of visual representations imparting an impression of motion when shown in succession."@en ;
            dcterms:creator "Dublin Core Metadata Initiative (DCMI)" ;
            dcterms:license <https://creativecommons.org/licenses/by/3.0/> ;
            dcterms:rights <https://rightsstatements.org/vocab/InC/1.0/> ;
            dcterms:source <https://www.dublincore.org/specifications/dublin-core/dcmi-type-vocabulary/> ],
        "A series of visual representations imparting an impression of motion when shown in succession."@en ;
    dcterms:identifier "CC00408" .

cc:CC00409 a owl:NamedIndividual ;
    rdfs:label "Physical Object"@en ;
    dcterms:description [ rdfs:label "An inanimate, three-dimensional object or substance."@en ;
            dcterms:creator "Dublin Core Metadata Initiative (DCMI)" ;
            dcterms:license <https://creativecommons.org/licenses/by/3.0/> ;
            dcterms:rights <https://rightsstatements.org/vocab/InC/1.0/> ;
            dcterms:source <https://www.dublincore.org/specifications/dublin-core/dcmi-type-vocabulary/> ],
        "An inanimate, three-dimensional object or substance."@en ;
    dcterms:identifier "CC00409" .

cc:CC00410 a owl:NamedIndividual ;
    rdfs:label "Service"@en ;
    dcterms:description [ rdfs:label "A system that provides one or more functions."@en ;
            dcterms:creator "Dublin Core Metadata Initiative (DCMI)" ;
            dcterms:license <https://creativecommons.org/licenses/by/3.0/> ;
            dcterms:rights <https://rightsstatements.org/vocab/InC/1.0/> ;
            dcterms:source <https://www.dublincore.org/specifications/dublin-core/dcmi-type-vocabulary/> ],
        "A system that provides one or more functions."@en ;
    dcterms:identifier "CC00410" .

cc:CC00411 a owl:NamedIndividual ;
    rdfs:label "Software"@en ;
    dcterms:description [ rdfs:label "A computer program in source or compiled form."@en ;
            dcterms:creator "Dublin Core Metadata Initiative (DCMI)" ;
            dcterms:license <https://creativecommons.org/licenses/by/3.0/> ;
            dcterms:rights <https://rightsstatements.org/vocab/InC/1.0/> ;
            dcterms:source <https://www.dublincore.org/specifications/dublin-core/dcmi-type-vocabulary/> ],
        "A computer program in source or compiled form."@en ;
    dcterms:identifier "CC00411" .

cc:CC00412 a owl:NamedIndividual ;
    rdfs:label "Sound"@en ;
    dcterms:description [ rdfs:label "A resource primarily intended to be heard."@en ;
            dcterms:creator "Dublin Core Metadata Initiative (DCMI)" ;
            dcterms:license <https://creativecommons.org/licenses/by/3.0/> ;
            dcterms:rights <https://rightsstatements.org/vocab/InC/1.0/> ;
            dcterms:source <https://www.dublincore.org/specifications/dublin-core/dcmi-type-vocabulary/> ],
        "A resource primarily intended to be heard."@en ;
    dcterms:identifier "CC00412" .

cc:CC00413 a owl:NamedIndividual ;
    rdfs:label "Still Image"@en ;
    dcterms:description [ rdfs:label "A static visual representation."@en ;
            dcterms:creator "Dublin Core Metadata Initiative (DCMI)" ;
            dcterms:license <https://creativecommons.org/licenses/by/3.0/> ;
            dcterms:rights <https://rightsstatements.org/vocab/InC/1.0/> ;
            dcterms:source <https://www.dublincore.org/specifications/dublin-core/dcmi-type-vocabulary/> ],
        "A static visual representation."@en ;
    dcterms:identifier "CC00413" .

cc:CC00414 a owl:NamedIndividual ;
    rdfs:label "Text"@en ;
    dcterms:description [ rdfs:label "A resource consisting primarily of words for reading."@en ;
            dcterms:creator "Dublin Core Metadata Initiative (DCMI)" ;
            dcterms:license <https://creativecommons.org/licenses/by/3.0/> ;
            dcterms:rights <https://rightsstatements.org/vocab/InC/1.0/> ;
            dcterms:source <https://www.dublincore.org/specifications/dublin-core/dcmi-type-vocabulary/> ],
        "A resource consisting primarily of words for reading."@en ;
    dcterms:identifier "CC00414" .

cc:CC00415 a owl:NamedIndividual ;
    rdfs:label "poor"@en ;
    dcterms:identifier "CC00415" .

cc:CC00416 a owl:NamedIndividual ;
    rdfs:label "fair"@en ;
    dcterms:identifier "CC00416" .

cc:CC00417 a owl:NamedIndividual ;
    rdfs:label "good"@en ;
    dcterms:identifier "CC00417" .

cc:CC00418 a owl:NamedIndividual ;
    rdfs:label "very good"@en ;
    dcterms:identifier "CC00418" .

cc:CC00419 a owl:NamedIndividual ;
    rdfs:label "excellent"@en ;
    dcterms:identifier "CC00419" .

cc:CC00421 a owl:NamedIndividual ;
    rdfs:label "braies"@en ;
    dcterms:identifier "CC00421" ;
    owl:sameAs <http://vocab.getty.edu/aat/300400621> .

cc:CC00430 a owl:NamedIndividual ;
    rdfs:label "pantaloons"@en ;
    dcterms:identifier "CC00430" ;
    owl:sameAs <http://vocab.getty.edu/aat/300046184> .

cc:CC00431 a owl:NamedIndividual ;
    rdfs:label "pedal pushers"@en ;
    dcterms:identifier "CC00431" ;
    owl:sameAs <http://vocab.getty.edu/aat/300209926> .

cc:CC00437 a owl:NamedIndividual ;
    rdfs:label "toreador pants"@en ;
    dcterms:identifier "CC00437" ;
    owl:sameAs <http://vocab.getty.edu/aat/300226607> .

cc:CC00438 a owl:NamedIndividual ;
    rdfs:label "athletic shorts"@en ;
    dcterms:identifier "CC00438" ;
    owl:sameAs <http://vocab.getty.edu/aat/300257544> .

cc:CC00439 a owl:NamedIndividual ;
    rdfs:label "Bermuda shorts"@en ;
    dcterms:identifier "CC00439" ;
    owl:sameAs <http://vocab.getty.edu/aat/300221453> .

cc:CC00440 a owl:NamedIndividual ;
    rdfs:label "short shorts"@en ;
    dcterms:identifier "CC00440" ;
    owl:sameAs <http://vocab.getty.edu/aat/300221447> .

cc:CC00442 a owl:NamedIndividual ;
    rdfs:label "aprons"@en ;
    dcterms:identifier "CC00442" .

cc:CC00466 a owl:NamedIndividual ;
    rdfs:label "face coverings and additions"@en ;
    dcterms:identifier "CC00466" .

cc:CC00472 a owl:NamedIndividual ;
    rdfs:label "accessories added to body or clothing for ornament"@en ;
    dcterms:identifier "CC00472" .

cc:CC00481 a owl:NamedIndividual ;
    rdfs:label "Containers"@en ;
    dcterms:description [ rdfs:label "The Containers hierarchy contains terms for objects used to hold substances or other objects. Included are terms for containers intended for culinary use, for horticultural use, for health care, hygiene, and similar personal needs as well as terms for containers associated with liturgical, funerary, and other ceremonial activities. A concept for a container is placed in the hierarchy either with respect to the item's earliest historical use or where the term has its broadest meaning. Ancient vase shapes, however, have been placed by their Classical meaning or context, even though in some instances the term may be applied to vessels dating to before or after the Classical period. Relation to other hierarchies: Terms for devices used to measure in terms of standard units or fixed amounts (e.g., \"measuring spoons\") are in the Measuring Devices hierarchy. Large- and small-scale appliances and similar culinary equipment (e.g., \"iceboxes,\" \"coffee makers\") are in the Tools and Equipment hierarchy. Terms for objects that may in some instances be considered types of container (e.g., \"chests of drawers\") but which more appropriately fall within the scope of other hierarchies, such as Furnishings or Tools and Equipment, are excluded here."@en ;
            dcterms:creator "The J. Paul Getty Trust" ;
            dcterms:license <https://opendatacommons.org/licenses/by/1-0/> ;
            dcterms:rights <https://rightsstatements.org/vocab/InC/1.0/> ;
            dcterms:source <http://www.getty.edu/research/tools/vocabularies/aat/> ],
        "The Containers hierarchy contains terms for objects used to hold substances or other objects. Included are terms for containers intended for culinary use, for horticultural use, for health care, hygiene, and similar personal needs as well as terms for containers associated with liturgical, funerary, and other ceremonial activities. A concept for a container is placed in the hierarchy either with respect to the item's earliest historical use or where the term has its broadest meaning. Ancient vase shapes, however, have been placed by their Classical meaning or context, even though in some instances the term may be applied to vessels dating to before or after the Classical period. Relation to other hierarchies: Terms for devices used to measure in terms of standard units or fixed amounts (e.g., \"measuring spoons\") are in the Measuring Devices hierarchy. Large- and small-scale appliances and similar culinary equipment (e.g., \"iceboxes,\" \"coffee makers\") are in the Tools and Equipment hierarchy. Terms for objects that may in some instances be considered types of container (e.g., \"chests of drawers\") but which more appropriately fall within the scope of other hierarchies, such as Furnishings or Tools and Equipment, are excluded here."@en ;
    dcterms:identifier "CC00481" ;
    owl:sameAs <http://vocab.getty.edu/aat/300045611> .

cc:CC00483 a owl:NamedIndividual ;
    rdfs:label "Furnishings"@en ;
    dcterms:description [ rdfs:label "The Furnishings hierarchy contains terms for objects that are primarily movable, provide comfort, convenience, or protection in dwellings, places or business, or other public or private spaces. They may be useful or ornamental and may be used in indoor or outdoor spaces. Former trade names for particular types of furnishing that have come to be used generically are included here. Relation to other hierarchies: Objects having the primary purpose is to serve as storage receptacles or other forms of container (e.g., \"candle boxes,\" \"footlockers\") appear in the Containers hierarchy. Permanent installations integrated into the fabric of buildings (e.g., \"altars,\" \"choir screens\") appear in the Components hierarchy. Timepieces and meteorological instruments (e.g., \"tall case clocks,\" \"barometers\") appear in the Measuring Devices hierarchy. Terms for the shapes of furniture pieces appear in the Attributes and Properties hierarchy (e.g., \"bomb\"). Terms for constituent parts of furnishings (e.g., \"footrests\") appear in the Components hierarchy; also in that hierarchy are terms for architectural elements that often appear on furnishings (e.g., \"arches,\" \"pediments\"). Abstract or stylized motifs and conventionalized patterns (e.g., \"gadrooning,\" \"trefoils\"), which represent a visual vocabulary used throughout the decorative arts, appear in the Design Elements hierarchy."@en ;
            dcterms:creator "The J. Paul Getty Trust" ;
            dcterms:license <https://opendatacommons.org/licenses/by/1-0/> ;
            dcterms:rights <https://rightsstatements.org/vocab/InC/1.0/> ;
            dcterms:source <http://www.getty.edu/research/tools/vocabularies/aat/> ],
        "The Furnishings hierarchy contains terms for objects that are primarily movable, provide comfort, convenience, or protection in dwellings, places or business, or other public or private spaces. They may be useful or ornamental and may be used in indoor or outdoor spaces. Former trade names for particular types of furnishing that have come to be used generically are included here. Relation to other hierarchies: Objects having the primary purpose is to serve as storage receptacles or other forms of container (e.g., \"candle boxes,\" \"footlockers\") appear in the Containers hierarchy. Permanent installations integrated into the fabric of buildings (e.g., \"altars,\" \"choir screens\") appear in the Components hierarchy. Timepieces and meteorological instruments (e.g., \"tall case clocks,\" \"barometers\") appear in the Measuring Devices hierarchy. Terms for the shapes of furniture pieces appear in the Attributes and Properties hierarchy (e.g., \"bomb\"). Terms for constituent parts of furnishings (e.g., \"footrests\") appear in the Components hierarchy; also in that hierarchy are terms for architectural elements that often appear on furnishings (e.g., \"arches,\" \"pediments\"). Abstract or stylized motifs and conventionalized patterns (e.g., \"gadrooning,\" \"trefoils\"), which represent a visual vocabulary used throughout the decorative arts, appear in the Design Elements hierarchy."@en ;
    dcterms:identifier "CC00483" ;
    owl:sameAs <http://vocab.getty.edu/aat/300037335> .

cc:CC00484 a owl:NamedIndividual ;
    rdfs:label "Information Forms"@en ;
    dcterms:description [ rdfs:label "The Information Forms hierarchy contains terms for textual, graphic, and physical objects having the primary and original purpose to record or convey specific information. Titles of particular texts are excluded, except where they are used to refer to a broad category of works (e.g., \"Bibles\" is included, but \"Tale of Two Cities\" is excluded). Relation to other hierarchies: Terms for typeface and scripts (e.g., \"Caroline minuscule\") are in the Components hierarchy; \"information forms components\" having a non-preferred partitive parent here. Terms for two- and three-dimensional works created to communicate primarily visually, especially to communicate expressive meaning rather than specific information, appear in the Visual Works hierarchy (e.g., \"still lifes\"). Types of prints used primarily to reproduce documents and technical drawings (e.g., \"blueprints (reprographic copies)\") which, though produced by light-sensitive processes are not considered photographs, appear here, while photographs and photomechanical prints are found in Visual Works. Terms for many types of financial documents are found here, while items that specifically are used in the exchange of goods or services or in the settlement of debts are found in the Exchange Media hierarchy."@en ;
            dcterms:creator "The J. Paul Getty Trust" ;
            dcterms:license <https://opendatacommons.org/licenses/by/1-0/> ;
            dcterms:rights <https://rightsstatements.org/vocab/InC/1.0/> ;
            dcterms:source <http://www.getty.edu/research/tools/vocabularies/aat/> ],
        "The Information Forms hierarchy contains terms for textual, graphic, and physical objects having the primary and original purpose to record or convey specific information. Titles of particular texts are excluded, except where they are used to refer to a broad category of works (e.g., \"Bibles\" is included, but \"Tale of Two Cities\" is excluded). Relation to other hierarchies: Terms for typeface and scripts (e.g., \"Caroline minuscule\") are in the Components hierarchy; \"information forms components\" having a non-preferred partitive parent here. Terms for two- and three-dimensional works created to communicate primarily visually, especially to communicate expressive meaning rather than specific information, appear in the Visual Works hierarchy (e.g., \"still lifes\"). Types of prints used primarily to reproduce documents and technical drawings (e.g., \"blueprints (reprographic copies)\") which, though produced by light-sensitive processes are not considered photographs, appear here, while photographs and photomechanical prints are found in Visual Works. Terms for many types of financial documents are found here, while items that specifically are used in the exchange of goods or services or in the settlement of debts are found in the Exchange Media hierarchy."@en ;
    dcterms:identifier "CC00484" ;
    owl:sameAs <http://vocab.getty.edu/aat/300026029> .

cc:CC00485 a owl:NamedIndividual ;
    rdfs:label "Recreational Artifacts"@en ;
    dcterms:description [ rdfs:label "The Recreational Artifacts hierarchy contains terms for equipment and accessories used in a large array of activities engaged in for personal satisfaction or amusement during leisure time. Included are terms for playthings, personal fitness equipment, and other devices used as pastimes or during competitive play. Relation to Other Hierarchies: Terms for sets of recreational artifacts (e.g., \"chess sets\") are found in the Object Groupings and Systems hierarchy. Terms for sports and athletic equipment worn on the body (e.g., \"crash helmets\") are found in the Costume hierarchy. Terms for objects used in sports but originally intended or based closely on offensive or defensive weapons (e.g.g., \"pes\", \"javelins\") are found in the Weapons and Ammunition hierarchy. Terms for objects that can be used in sports or play but are primarily or originally intended to carry people or goods over a distance (e.g.g., \"sleds\", \"canoes\") are found in the Transportation Vehicles hierarchy. Terms for types of figural representation not intended as toys are found in the Visual Works hierarchy (e.g., \"kachina dolls\"), with a high level node having a non-preferred parent here in Recreational Artifacts."@en ;
            dcterms:creator "The J. Paul Getty Trust" ;
            dcterms:license <https://opendatacommons.org/licenses/by/1-0/> ;
            dcterms:rights <https://rightsstatements.org/vocab/InC/1.0/> ;
            dcterms:source <http://www.getty.edu/research/tools/vocabularies/aat/> ],
        "The Recreational Artifacts hierarchy contains terms for equipment and accessories used in a large array of activities engaged in for personal satisfaction or amusement during leisure time. Included are terms for playthings, personal fitness equipment, and other devices used as pastimes or during competitive play. Relation to Other Hierarchies: Terms for sets of recreational artifacts (e.g., \"chess sets\") are found in the Object Groupings and Systems hierarchy. Terms for sports and athletic equipment worn on the body (e.g., \"crash helmets\") are found in the Costume hierarchy. Terms for objects used in sports but originally intended or based closely on offensive or defensive weapons (e.g.g., \"pes\", \"javelins\") are found in the Weapons and Ammunition hierarchy. Terms for objects that can be used in sports or play but are primarily or originally intended to carry people or goods over a distance (e.g.g., \"sleds\", \"canoes\") are found in the Transportation Vehicles hierarchy. Terms for types of figural representation not intended as toys are found in the Visual Works hierarchy (e.g., \"kachina dolls\"), with a high level node having a non-preferred parent here in Recreational Artifacts."@en ;
    dcterms:identifier "CC00485" ;
    owl:sameAs <http://vocab.getty.edu/aat/300136012> .

cc:CC00486 a owl:NamedIndividual ;
    rdfs:label "Tools and Equipment"@en ;
    dcterms:description [ rdfs:label "The Tools and Equipment hierarchy contains terms for equipment used in processing materials and fabricating objects, as well as terms associated with activities and disciplines in the construction industry, design professions, the fine and decorative arts, and other aspects of material culture. Excluded are terms for objects such as measuring devices and weapons, which may be considered equipment but fall into the scope of other hierarchies in the Furnishings and Equipment section of the Objects facet. Relation to other hierarchies: Terms for devices used to measure in terms of standard units or fixed amounts (e.g., \"gauges\") are in the Measuring Devices hierarchy. Terms for items that are necessary to anchor or join materials, objects, or components (e.g., \"nails,\" \"buckles\") appear in the Components hierarchy. Terms for constituent parts of equipment (e.g., \"handles\") are also in the Components hierarchy. HVAC systems can be found in the Object Groupings and Systems hierarchy, while the terms for HVAC equipment (e.g., \"air conditioners\") are found here."@en ;
            dcterms:creator "The J. Paul Getty Trust" ;
            dcterms:license <https://opendatacommons.org/licenses/by/1-0/> ;
            dcterms:rights <https://rightsstatements.org/vocab/InC/1.0/> ;
            dcterms:source <http://www.getty.edu/research/tools/vocabularies/aat/> ],
        "The Tools and Equipment hierarchy contains terms for equipment used in processing materials and fabricating objects, as well as terms associated with activities and disciplines in the construction industry, design professions, the fine and decorative arts, and other aspects of material culture. Excluded are terms for objects such as measuring devices and weapons, which may be considered equipment but fall into the scope of other hierarchies in the Furnishings and Equipment section of the Objects facet. Relation to other hierarchies: Terms for devices used to measure in terms of standard units or fixed amounts (e.g., \"gauges\") are in the Measuring Devices hierarchy. Terms for items that are necessary to anchor or join materials, objects, or components (e.g., \"nails,\" \"buckles\") appear in the Components hierarchy. Terms for constituent parts of equipment (e.g., \"handles\") are also in the Components hierarchy. HVAC systems can be found in the Object Groupings and Systems hierarchy, while the terms for HVAC equipment (e.g., \"air conditioners\") are found here."@en ;
    dcterms:identifier "CC00486" ;
    owl:sameAs <http://vocab.getty.edu/aat/300022238> .

cc:CC00487 a owl:NamedIndividual ;
    rdfs:label "Visual Works"@en ;
    dcterms:description [ rdfs:label "The Visual Works hierarchy contains terms for items, including works of art and any objects that occupy space, are perceived by the sense of sight, and are created, rather than naturally occurring. This hierarchy focuses especially on works conveying a symbolic or expressive meaning or an aesthetic experience, such as pictorial and sculptural works, and time-based works such as performance art. Relation to other hierarchies: In the Information Forms hierarchy are terms for items that communicate by visual, nonverbal means, but whose purpose is primarily informational (e.g., \"maps\"). Terms for decorative elements are in the Design Elements hierarchy (e.g., \"scrollwork\") and the Components hierarchy (e.g., \"acroteria\"); architectural forms that are primarily structural and secondarily sculptural (e.g., \"caryatids\") also appear in Components. Most terms used to create works are in the Materials hierarchy (e.g., \"canvas\"), although if found objects are used (e.g., \"dinner plates\"), these are considered components of the work, not materials. Terms for the methods used to create a work (e.g., \"wet collodion process,\" \"carving\") are in the Processes and Techniques hierarchy."@en ;
            dcterms:creator "The J. Paul Getty Trust" ;
            dcterms:license <https://opendatacommons.org/licenses/by/1-0/> ;
            dcterms:rights <https://rightsstatements.org/vocab/InC/1.0/> ;
            dcterms:source <http://www.getty.edu/research/tools/vocabularies/aat/> ],
        "The Visual Works hierarchy contains terms for items, including works of art and any objects that occupy space, are perceived by the sense of sight, and are created, rather than naturally occurring. This hierarchy focuses especially on works conveying a symbolic or expressive meaning or an aesthetic experience, such as pictorial and sculptural works, and time-based works such as performance art. Relation to other hierarchies: In the Information Forms hierarchy are terms for items that communicate by visual, nonverbal means, but whose purpose is primarily informational (e.g., \"maps\"). Terms for decorative elements are in the Design Elements hierarchy (e.g., \"scrollwork\") and the Components hierarchy (e.g., \"acroteria\"); architectural forms that are primarily structural and secondarily sculptural (e.g., \"caryatids\") also appear in Components. Most terms used to create works are in the Materials hierarchy (e.g., \"canvas\"), although if found objects are used (e.g., \"dinner plates\"), these are considered components of the work, not materials. Terms for the methods used to create a work (e.g., \"wet collodion process,\" \"carving\") are in the Processes and Techniques hierarchy."@en ;
    dcterms:identifier "CC00487" ;
    owl:sameAs <http://vocab.getty.edu/aat/300179869> .

cc:CC00488 a owl:NamedIndividual ;
    rdfs:label "Materials"@en ;
    dcterms:description [ rdfs:label "The Materials hierarchy contains terms for a broad range of substances, from natural and synthetic raw materials to material products. Material products are included here rather than in the Objects facet because they can be used in the construction of various objects (e.g., \"plank\" for floors or walls), and because they are not necessary constituent parts of objects (e.g., \"shingle\" is not essential to roofs in the same way as roof ridges or eaves). Relation to Other Hierarchies: Terms denoting activities performed on or with materials are found in the Processes and Techniques hierarchy (e.g., \"glassworking\"). Terms for generic object types are found in the Object Genres hierarchy (e.g., \"artifacts (object genres),\" \"images (object genres)\"), while terms for materials themselves are found here (e.g., \"metal,\" \"textile\"). Terms for tools used in the creation of images (e.g., \"charcoal sticks,\" \"pens\") are in the Tools and Equipment hierarchy, while terms for the materials of which they are made or which they use are found here (e.g., \"charcoal,\" \"ink\")."@en ;
            dcterms:creator "The J. Paul Getty Trust" ;
            dcterms:license <https://opendatacommons.org/licenses/by/1-0/> ;
            dcterms:rights <https://rightsstatements.org/vocab/InC/1.0/> ;
            dcterms:source <http://www.getty.edu/research/tools/vocabularies/aat/> ],
        "The Materials hierarchy contains terms for a broad range of substances, from natural and synthetic raw materials to material products. Material products are included here rather than in the Objects facet because they can be used in the construction of various objects (e.g., \"plank\" for floors or walls), and because they are not necessary constituent parts of objects (e.g., \"shingle\" is not essential to roofs in the same way as roof ridges or eaves). Relation to Other Hierarchies: Terms denoting activities performed on or with materials are found in the Processes and Techniques hierarchy (e.g., \"glassworking\"). Terms for generic object types are found in the Object Genres hierarchy (e.g., \"artifacts (object genres),\" \"images (object genres)\"), while terms for materials themselves are found here (e.g., \"metal,\" \"textile\"). Terms for tools used in the creation of images (e.g., \"charcoal sticks,\" \"pens\") are in the Tools and Equipment hierarchy, while terms for the materials of which they are made or which they use are found here (e.g., \"charcoal,\" \"ink\")."@en ;
    dcterms:identifier "CC00488" ;
    owl:sameAs <http://vocab.getty.edu/aat/300010357> .

cc:CC00495 a owl:NamedIndividual ;
    rdfs:label "Bodycon dress"@en ;
    dcterms:description [ rdfs:label "tight figure-hugging dress"@en ;
            dcterms:creator "Wikidata contributors" ;
            dcterms:license <https://creativecommons.org/publicdomain/mark/1.0/> ;
            dcterms:rights <https://creativecommons.org/publicdomain/mark/1.0/> ;
            dcterms:source <https://www.wikidata.org/wiki/Wikidata:Data_access/en> ],
        "tight figure-hugging dress"@en ;
    dcterms:identifier "CC00495" ;
    owl:sameAs <http://www.wikidata.org/entity/Q30588951> .

cc:CC00497 a owl:NamedIndividual ;
    rdfs:label "Delphos gown"@en ;
    dcterms:description [ rdfs:label "type of pleated woman's dress"@en ;
            dcterms:creator "Wikidata contributors" ;
            dcterms:license <https://creativecommons.org/publicdomain/mark/1.0/> ;
            dcterms:rights <https://creativecommons.org/publicdomain/mark/1.0/> ;
            dcterms:source <https://www.wikidata.org/wiki/Wikidata:Data_access/en> ],
        "type of pleated woman's dress"@en ;
    dcterms:identifier "CC00497" ;
    owl:sameAs <http://www.wikidata.org/entity/Q5254472> .

cc:CC00498 a owl:NamedIndividual ;
    rdfs:label "dirndl"@en ;
    dcterms:description [ rdfs:label "traditional dress worn in Germany,Switzerland, Liechtenstein, Austria and South Tyrol"@en ;
            dcterms:creator "The J. Paul Getty Trust" ;
            dcterms:license <https://opendatacommons.org/licenses/by/1-0/> ;
            dcterms:rights <https://rightsstatements.org/vocab/InC/1.0/> ;
            dcterms:source <http://www.getty.edu/research/tools/vocabularies/aat/> ],
        "traditional dress worn in Germany,Switzerland, Liechtenstein, Austria and South Tyrol"@en ;
    dcterms:identifier "CC00498" ;
    owl:sameAs <http://vocab.getty.edu/aat/300209912> .

cc:CC00499 a owl:NamedIndividual ;
    rdfs:label "mini dress"@en ;
    dcterms:description [ rdfs:label "dress ending well above the knee"@en ;
            dcterms:creator "Wikidata contributors" ;
            dcterms:license <https://creativecommons.org/publicdomain/mark/1.0/> ;
            dcterms:rights <https://creativecommons.org/publicdomain/mark/1.0/> ;
            dcterms:source <https://www.wikidata.org/wiki/Wikidata:Data_access/en> ],
        "dress ending well above the knee"@en ;
    dcterms:identifier "CC00499" ;
    owl:sameAs <http://www.wikidata.org/entity/Q11018285> .

cc:CC00500 a owl:NamedIndividual ;
    rdfs:label "Mother Hubbard"@en ;
    dcterms:description [ rdfs:label "long, loose dress with a high neckline and long sleeves, worn in 19th century America and introduced to Polynesia by missionaries"@en ;
            dcterms:creator "Wikidata contributors" ;
            dcterms:license <https://creativecommons.org/publicdomain/mark/1.0/> ;
            dcterms:rights <https://creativecommons.org/publicdomain/mark/1.0/> ;
            dcterms:source <https://www.wikidata.org/wiki/Wikidata:Data_access/en> ],
        "long, loose dress with a high neckline and long sleeves, worn in 19th century America and introduced to Polynesia by missionaries"@en ;
    dcterms:identifier "CC00500" ;
    owl:sameAs <http://www.wikidata.org/entity/Q3434328> .

cc:CC00503 a owl:NamedIndividual ;
    rdfs:label "redingote"@en ;
    dcterms:description [ rdfs:label "women's dress  open in front to show an underskirt or with a front gore of contrasting material, with collar and lapels and long sleeves; or a three-quarter length or full-length fitted overcoat with flared skirts"@en ;
            dcterms:creator "The J. Paul Getty Trust" ;
            dcterms:license <https://opendatacommons.org/licenses/by/1-0/> ;
            dcterms:rights <https://rightsstatements.org/vocab/InC/1.0/> ;
            dcterms:source <http://www.getty.edu/research/tools/vocabularies/aat/> ],
        "women's dress  open in front to show an underskirt or with a front gore of contrasting material, with collar and lapels and long sleeves; or a three-quarter length or full-length fitted overcoat with flared skirts"@en ;
    dcterms:identifier "CC00503" ;
    owl:sameAs <http://vocab.getty.edu/aat/300254632> .

cc:CC00504 a owl:NamedIndividual ;
    rdfs:label "robe de style"@en ;
    dcterms:description [ rdfs:label "full-skirted dress of the 1920s"@en ;
            dcterms:creator "Wikidata contributors" ;
            dcterms:license <https://creativecommons.org/publicdomain/mark/1.0/> ;
            dcterms:rights <https://creativecommons.org/publicdomain/mark/1.0/> ;
            dcterms:source <https://www.wikidata.org/wiki/Wikidata:Data_access/en> ],
        "full-skirted dress of the 1920s"@en ;
    dcterms:identifier "CC00504" ;
    owl:sameAs <http://www.wikidata.org/entity/Q7341111> .

cc:CC00505 a owl:NamedIndividual ;
    rdfs:label "afternoon dress"@en ;
    dcterms:description [ rdfs:label "woman's semiformal dress for afternoon social occasions"@en ;
            dcterms:creator "Wikidata contributors" ;
            dcterms:license <https://creativecommons.org/publicdomain/mark/1.0/> ;
            dcterms:rights <https://creativecommons.org/publicdomain/mark/1.0/> ;
            dcterms:source <https://www.wikidata.org/wiki/Wikidata:Data_access/en> ],
        "woman's semiformal dress for afternoon social occasions"@en ;
    dcterms:identifier "CC00505" ;
    owl:sameAs <http://www.wikidata.org/entity/Q11284623> .

cc:CC00506 a owl:NamedIndividual ;
    rdfs:label "court dress"@en ;
    dcterms:description [ rdfs:label "extremely formal woman's dress conforming to the regulations for attendance on or presentation to a monarch"@en ;
            dcterms:creator "Wikidata contributors" ;
            dcterms:license <https://creativecommons.org/publicdomain/mark/1.0/> ;
            dcterms:rights <https://creativecommons.org/publicdomain/mark/1.0/> ;
            dcterms:source <https://www.wikidata.org/wiki/Wikidata:Data_access/en> ],
        "extremely formal woman's dress conforming to the regulations for attendance on or presentation to a monarch"@en ;
    dcterms:identifier "CC00506" ;
    owl:sameAs <http://www.wikidata.org/entity/Q29405103> .

cc:CC00508 a owl:NamedIndividual ;
    rdfs:label "walking dress"@en ;
    dcterms:description [ rdfs:label "dress or ensemble for walking out-of-doors"@en ;
            dcterms:creator "Wikidata contributors" ;
            dcterms:license <https://creativecommons.org/publicdomain/mark/1.0/> ;
            dcterms:rights <https://creativecommons.org/publicdomain/mark/1.0/> ;
            dcterms:source <https://www.wikidata.org/wiki/Wikidata:Data_access/en> ],
        "dress or ensemble for walking out-of-doors"@en ;
    dcterms:identifier "CC00508" ;
    owl:sameAs <http://www.wikidata.org/entity/Q43299785> .

cc:CC00518 a owl:NamedIndividual ;
    rdfs:label "outerwear"@en ;
    dcterms:description [ rdfs:label "Garments worn over other garments as the outer layer, especially those worn for protection from the natural elements. For garments worn for protection from dirt or danger, use descriptors listed under \"<protective wear>.\""@en ;
            dcterms:creator "The J. Paul Getty Trust" ;
            dcterms:license <https://opendatacommons.org/licenses/by/1-0/> ;
            dcterms:rights <https://rightsstatements.org/vocab/InC/1.0/> ;
            dcterms:source <http://www.getty.edu/research/tools/vocabularies/aat/> ],
        "Garments worn over other garments as the outer layer, especially those worn for protection from the natural elements. For garments worn for protection from dirt or danger, use descriptors listed under \"<protective wear>.\""@en ;
    dcterms:identifier "CC00518" ;
    owl:sameAs <http://vocab.getty.edu/aat/300209265> .

cc:CC00521 a owl:NamedIndividual ;
    rdfs:label "a-line"@en ;
    dcterms:description [ rdfs:label "triangular or A-shaped silhouette in clothing, generally standing away from the body"@en ;
            dcterms:creator "Wikidata contributors" ;
            dcterms:license <https://creativecommons.org/publicdomain/mark/1.0/> ;
            dcterms:rights <https://creativecommons.org/publicdomain/mark/1.0/> ;
            dcterms:source <https://www.wikidata.org/wiki/Wikidata:Data_access/en> ],
        "triangular or A-shaped silhouette in clothing, generally standing away from the body"@en ;
    dcterms:identifier "CC00521" ;
    owl:sameAs <http://www.wikidata.org/entity/Q277835> .

cc:CC00523 a owl:NamedIndividual ;
    rdfs:label "trews"@en ;
    dcterms:identifier "CC00523" ;
    owl:sameAs <http://vocab.getty.edu/aat/300248711> .

cc:CC00526 a owl:NamedIndividual ;
    rdfs:label "skort"@en ;
    dcterms:description [ rdfs:label "full shorts made to look like a skirt, or shorts with a skirt-like panel in front and back"@en ;
            dcterms:creator "Wikidata contributors" ;
            dcterms:license <https://creativecommons.org/publicdomain/mark/1.0/> ;
            dcterms:rights <https://creativecommons.org/publicdomain/mark/1.0/> ;
            dcterms:source <https://www.wikidata.org/wiki/Wikidata:Data_access/en> ],
        "full shorts made to look like a skirt, or shorts with a skirt-like panel in front and back"@en ;
    dcterms:identifier "CC00526" ;
    owl:sameAs <http://www.wikidata.org/entity/Q363031> .

cc:CC00585 a owl:NamedIndividual ;
    rdfs:label "scroll"@en ;
    dcterms:description [ rdfs:label "General term for motifs consisting of a spirally wound band. For simple motifs of coiled lines, use \"spirals\"; for scroll-shaped architectural elements use other terms, such as \"consoles\" and \"volutes\"; for a series of scrolls, in running or allover patterns, use \"scrollwork.\""@en ;
            dcterms:creator "The J. Paul Getty Trust" ;
            dcterms:license <https://opendatacommons.org/licenses/by/1-0/> ;
            dcterms:rights <https://rightsstatements.org/vocab/InC/1.0/> ;
            dcterms:source <http://www.getty.edu/research/tools/vocabularies/aat/> ],
        "General term for motifs consisting of a spirally wound band. For simple motifs of coiled lines, use \"spirals\"; for scroll-shaped architectural elements use other terms, such as \"consoles\" and \"volutes\"; for a series of scrolls, in running or allover patterns, use \"scrollwork.\""@en ;
    dcterms:identifier "CC00585" .

cc:CC00595 a owl:NamedIndividual ;
    rdfs:label "geometric"@en ;
    dcterms:description [ rdfs:label "Design elements with geometrical themes."@en ;
            dcterms:creator "The J. Paul Getty Trust" ;
            dcterms:license <https://opendatacommons.org/licenses/by/1-0/> ;
            dcterms:rights <https://rightsstatements.org/vocab/InC/1.0/> ;
            dcterms:source <http://www.getty.edu/research/tools/vocabularies/aat/> ],
        "Design elements with geometrical themes."@en ;
    dcterms:identifier "CC00595" .

cc:CC00613 a owl:NamedIndividual ;
    rdfs:label "CNE"@en ;
    dcterms:description [ rdfs:label "Copyright Not Evaluated"@en ;
            dcterms:creator "RightsStatements.org" ;
            dcterms:license <https://creativecommons.org/publicdomain/zero/1.0/> ;
            dcterms:rights <https://creativecommons.org/publicdomain/zero/1.0/> ;
            dcterms:source <https://rightsstatements.org/page/1.0/> ],
        "Copyright Not Evaluated"@en ;
    dcterms:identifier "CC00613" .

cc:CC00614 a owl:NamedIndividual ;
    rdfs:label "UND"@en ;
    dcterms:description [ rdfs:label "Copyright Undetermined"@en ;
            dcterms:creator "RightsStatements.org" ;
            dcterms:license <https://creativecommons.org/publicdomain/zero/1.0/> ;
            dcterms:rights <https://creativecommons.org/publicdomain/zero/1.0/> ;
            dcterms:source <https://rightsstatements.org/page/1.0/> ],
        "Copyright Undetermined"@en ;
    dcterms:identifier "CC00614" .

cc:CC00615 a owl:NamedIndividual ;
    rdfs:label "InC"@en ;
    dcterms:description [ rdfs:label "In Copyright"@en ;
            dcterms:creator "RightsStatements.org" ;
            dcterms:license <https://creativecommons.org/publicdomain/zero/1.0/> ;
            dcterms:rights <https://creativecommons.org/publicdomain/zero/1.0/> ;
            dcterms:source <https://rightsstatements.org/page/1.0/> ],
        "In Copyright"@en ;
    dcterms:identifier "CC00615" .

cc:CC00616 a owl:NamedIndividual ;
    rdfs:label "InC-EDU"@en ;
    dcterms:description [ rdfs:label "In Copyright - Educational Use Permitted"@en ;
            dcterms:creator "RightsStatements.org" ;
            dcterms:license <https://creativecommons.org/publicdomain/zero/1.0/> ;
            dcterms:rights <https://creativecommons.org/publicdomain/zero/1.0/> ;
            dcterms:source <https://rightsstatements.org/page/1.0/> ],
        "In Copyright - Educational Use Permitted"@en ;
    dcterms:identifier "CC00616" .

cc:CC00617 a owl:NamedIndividual ;
    rdfs:label "InC-OW-EU"@en ;
    dcterms:description [ rdfs:label "In Copyright - EU Orphan Work"@en ;
            dcterms:creator "RightsStatements.org" ;
            dcterms:license <https://creativecommons.org/publicdomain/zero/1.0/> ;
            dcterms:rights <https://creativecommons.org/publicdomain/zero/1.0/> ;
            dcterms:source <https://rightsstatements.org/page/1.0/> ],
        "In Copyright - EU Orphan Work"@en ;
    dcterms:identifier "CC00617" .

cc:CC00618 a owl:NamedIndividual ;
    rdfs:label "InC-NC"@en ;
    dcterms:description [ rdfs:label "In Copyright - Non-Commercial Use Permitted"@en ;
            dcterms:creator "RightsStatements.org" ;
            dcterms:license <https://creativecommons.org/publicdomain/zero/1.0/> ;
            dcterms:rights <https://creativecommons.org/publicdomain/zero/1.0/> ;
            dcterms:source <https://rightsstatements.org/page/1.0/> ],
        "In Copyright - Non-Commercial Use Permitted"@en ;
    dcterms:identifier "CC00618" .

cc:CC00619 a owl:NamedIndividual ;
    rdfs:label "InC-RUU"@en ;
    dcterms:description [ rdfs:label "In Copyright - Rights-holders Unlocatable or Unidentificable"@en ;
            dcterms:creator "RightsStatements.org" ;
            dcterms:license <https://creativecommons.org/publicdomain/zero/1.0/> ;
            dcterms:rights <https://creativecommons.org/publicdomain/zero/1.0/> ;
            dcterms:source <https://rightsstatements.org/page/1.0/> ],
        "In Copyright - Rights-holders Unlocatable or Unidentificable"@en ;
    dcterms:identifier "CC00619" .

cc:CC00620 a owl:NamedIndividual ;
    rdfs:label "NoC-CR"@en ;
    dcterms:description [ rdfs:label "No Copyright - Contractual Restrictions"@en ;
            dcterms:creator "RightsStatements.org" ;
            dcterms:license <https://creativecommons.org/publicdomain/zero/1.0/> ;
            dcterms:rights <https://creativecommons.org/publicdomain/zero/1.0/> ;
            dcterms:source <https://rightsstatements.org/page/1.0/> ],
        "No Copyright - Contractual Restrictions"@en ;
    dcterms:identifier "CC00620" .

cc:CC00621 a owl:NamedIndividual ;
    rdfs:label "NoC-NC"@en ;
    dcterms:description [ rdfs:label "No Copyright - Non-Commercial Use Only"@en ;
            dcterms:creator "RightsStatements.org" ;
            dcterms:license <https://creativecommons.org/publicdomain/zero/1.0/> ;
            dcterms:rights <https://creativecommons.org/publicdomain/zero/1.0/> ;
            dcterms:source <https://rightsstatements.org/page/1.0/> ],
        "No Copyright - Non-Commercial Use Only"@en ;
    dcterms:identifier "CC00621" .

cc:CC00622 a owl:NamedIndividual ;
    rdfs:label "NoC-OKLR"@en ;
    dcterms:description [ rdfs:label "No Copyright - Other Known Legal Restrictions"@en ;
            dcterms:creator "RightsStatements.org" ;
            dcterms:license <https://creativecommons.org/publicdomain/zero/1.0/> ;
            dcterms:rights <https://creativecommons.org/publicdomain/zero/1.0/> ;
            dcterms:source <https://rightsstatements.org/page/1.0/> ],
        "No Copyright - Other Known Legal Restrictions"@en ;
    dcterms:identifier "CC00622" .

cc:CC00623 a owl:NamedIndividual ;
    rdfs:label "NoC-US"@en ;
    dcterms:description [ rdfs:label "No Copyright - United States"@en ;
            dcterms:creator "RightsStatements.org" ;
            dcterms:license <https://creativecommons.org/publicdomain/zero/1.0/> ;
            dcterms:rights <https://creativecommons.org/publicdomain/zero/1.0/> ;
            dcterms:source <https://rightsstatements.org/page/1.0/> ],
        "No Copyright - United States"@en ;
    dcterms:identifier "CC00623" .

cc:CC00624 a owl:NamedIndividual ;
    rdfs:label "NKC"@en ;
    dcterms:description [ rdfs:label "No Known Copyright Restrictions"@en ;
            dcterms:creator "RightsStatements.org" ;
            dcterms:license <https://creativecommons.org/publicdomain/zero/1.0/> ;
            dcterms:rights <https://creativecommons.org/publicdomain/zero/1.0/> ;
            dcterms:source <https://rightsstatements.org/page/1.0/> ],
        "No Known Copyright Restrictions"@en ;
    dcterms:identifier "CC00624" .

cc:CC00625 a owl:NamedIndividual ;
    rdfs:label "NoC"@en ;
    dcterms:description [ rdfs:label "Public Domain"@en ;
            dcterms:creator "Creative Commons" ;
            dcterms:license <https://creativecommons.org/publicdomain/zero/1.0/> ;
            dcterms:rights <https://creativecommons.org/publicdomain/zero/1.0/> ;
            dcterms:source <https://rightsstatements.org/page/1.0/> ],
        "Public Domain"@en ;
    dcterms:identifier "CC00625" .

cc:CC00626 a owl:NamedIndividual ;
    rdfs:label "waist length"@en ;
    dcterms:identifier "CC00626" .

cc:CC00627 a owl:NamedIndividual ;
    rdfs:label "above waist length"@en ;
    dcterms:identifier "CC00627" .

<http://vocab.getty.edu/aat/300209263> a owl:NamedIndividual ;
    owl:sameAs cc:CC00402,
        cc:CC00457 .

<http://vocab.getty.edu/aat/300209265> a owl:NamedIndividual ;
    owl:sameAs cc:CC00458,
        cc:CC00518 .

<http://vocab.getty.edu/aat/300209912> a owl:NamedIndividual ;
    owl:sameAs cc:CC00167,
        cc:CC00498 .

<http://vocab.getty.edu/aat/300211604> a owl:NamedIndividual ;
    owl:sameAs cc:CC00462,
        cc:CC00519 .

<http://vocab.getty.edu/aat/300214100> a owl:NamedIndividual ;
    owl:sameAs cc:CC00252,
        cc:CC00522 .

<http://vocab.getty.edu/aat/300227915> a owl:NamedIndividual ;
    owl:sameAs cc:CC00246,
        cc:CC00316 .

<http://vocab.getty.edu/aat/300253712> a owl:NamedIndividual ;
    owl:sameAs cc:CC00099,
        cc:CC00581 .

<http://www.wikidata.org/entity/Q2204140> a owl:NamedIndividual ;
    owl:sameAs cc:CC00099,
        cc:CC00581 .

<http://www.wikidata.org/entity/Q277835> a owl:NamedIndividual ;
    owl:sameAs cc:CC00102,
        cc:CC00521 .

cc:CC00001 a owl:NamedIndividual ;
    rdfs:label "buckle"@en ;
    dcterms:description [ rdfs:label "Devices used for fastening consisting of a usually open rectangular or rounded frame and a tongue or catch attached to one side or a vertical bar attached across the center. Sometimes used alone as an ornament."@en ;
            dcterms:creator "The J. Paul Getty Trust" ;
            dcterms:license <https://opendatacommons.org/licenses/by/1-0/> ;
            dcterms:rights <https://rightsstatements.org/vocab/InC/1.0/> ;
            dcterms:source <http://www.getty.edu/research/tools/vocabularies/aat/> ],
        "Devices used for fastening consisting of a usually open rectangular or rounded frame and a tongue or catch attached to one side or a vertical bar attached across the center. Sometimes used alone as an ornament."@en ;
    dcterms:identifier "CC00001" ;
    owl:sameAs <http://vocab.getty.edu/aat/300239260> .

cc:CC00002 a owl:NamedIndividual ;
    rdfs:label "buttons"@en ;
    dcterms:description [ rdfs:label "Disks, balls, or devices of other shape having holes or a shank by which they are sewn or secured to an article and that are used as fasteners by passing through a buttonhole or loop or a trimming."@en ;
            dcterms:creator "The J. Paul Getty Trust" ;
            dcterms:license <https://opendatacommons.org/licenses/by/1-0/> ;
            dcterms:rights <https://rightsstatements.org/vocab/InC/1.0/> ;
            dcterms:source <http://www.getty.edu/research/tools/vocabularies/aat/> ],
        "Disks, balls, or devices of other shape having holes or a shank by which they are sewn or secured to an article and that are used as fasteners by passing through a buttonhole or loop or a trimming."@en ;
    dcterms:identifier "CC00002" ;
    owl:sameAs <http://vocab.getty.edu/aat/300239261> .

cc:CC00003 a owl:NamedIndividual ;
    rdfs:label "frogs"@en ;
    dcterms:description [ rdfs:label "Two-part fasteners for a coat, jacket, or other garment usually made of a looped braid or cord in an ornamental design on one edge of the garment that attaches around a knot, toggle, or similar device on the other side. (AAT)"@en ;
            dcterms:creator "The J. Paul Getty Trust" ;
            dcterms:license <https://opendatacommons.org/licenses/by/1-0/> ;
            dcterms:rights <https://rightsstatements.org/vocab/InC/1.0/> ;
            dcterms:source <http://www.getty.edu/research/tools/vocabularies/aat/> ],
        "Two-part fasteners for a coat, jacket, or other garment usually made of a looped braid or cord in an ornamental design on one edge of the garment that attaches around a knot, toggle, or similar device on the other side. (AAT)"@en ;
    dcterms:identifier "CC00003" ;
    owl:sameAs <http://vocab.getty.edu/aat/300247475> .

cc:CC00004 a owl:NamedIndividual ;
    rdfs:label "hooks and eyes"@en ;
    dcterms:description [ rdfs:label "Two-part fastening devices, as on a garment or a door, consisting of a hook that catches over a bar or into a loop."@en ;
            dcterms:creator "The J. Paul Getty Trust" ;
            dcterms:license <https://opendatacommons.org/licenses/by/1-0/> ;
            dcterms:rights <https://rightsstatements.org/vocab/InC/1.0/> ;
            dcterms:source <http://www.getty.edu/research/tools/vocabularies/aat/> ],
        "Two-part fastening devices, as on a garment or a door, consisting of a hook that catches over a bar or into a loop."@en ;
    dcterms:identifier "CC00004" ;
    owl:sameAs <http://vocab.getty.edu/aat/300051508> .

cc:CC00005 a owl:NamedIndividual ;
    rdfs:label "lacing"@en ;
    dcterms:description [ rdfs:label "Cord, tape, or ribbon used for fastening by interlacing through holes in two garments or two sides of an opening. (EFT)"@en ;
            dcterms:creator "Wikidata contributors" ;
            dcterms:license <https://creativecommons.org/publicdomain/mark/1.0/> ;
            dcterms:rights <https://creativecommons.org/publicdomain/mark/1.0/> ;
            dcterms:source <https://www.wikidata.org/wiki/Wikidata:Data_access/en> ],
        "Cord, tape, or ribbon used for fastening by interlacing through holes in two garments or two sides of an opening. (EFT)"@en ;
    dcterms:identifier "CC00005" ;
    owl:sameAs <http://www.wikidata.org/entity/Q29514179> .

cc:CC00006 a owl:NamedIndividual ;
    rdfs:label "grommets"@en ;
    dcterms:description [ rdfs:label "Metal or plastic ringlike devices that provide a reinforced hole in a material, such as cloth or leather, that might otherwise tear from the stress on the hole when a fastener or other device is passed through it or attached to it."@en ;
            dcterms:creator "The J. Paul Getty Trust" ;
            dcterms:license <https://opendatacommons.org/licenses/by/1-0/> ;
            dcterms:rights <https://rightsstatements.org/vocab/InC/1.0/> ;
            dcterms:source <http://www.getty.edu/research/tools/vocabularies/aat/> ],
        "Metal or plastic ringlike devices that provide a reinforced hole in a material, such as cloth or leather, that might otherwise tear from the stress on the hole when a fastener or other device is passed through it or attached to it."@en ;
    dcterms:identifier "CC00006" ;
    owl:sameAs <http://vocab.getty.edu/aat/300080226> .

cc:CC00007 a owl:NamedIndividual ;
    rdfs:label "wrap dress"@en ;
    dcterms:description [ rdfs:label "Dresses constructed so that panels cross over each other and can be fastened. These are of varied design and may be in any length and have a variety of sleeve types and necklines."@en ;
            dcterms:creator "The J. Paul Getty Trust" ;
            dcterms:license <https://opendatacommons.org/licenses/by/1-0/> ;
            dcterms:rights <https://rightsstatements.org/vocab/InC/1.0/> ;
            dcterms:source <http://www.getty.edu/research/tools/vocabularies/aat/> ],
        "Dresses constructed so that panels cross over each other and can be fastened. These are of varied design and may be in any length and have a variety of sleeve types and necklines."@en ;
    dcterms:identifier "CC00007" ;
    owl:sameAs <http://vocab.getty.edu/aat/300417877> .

cc:CC00008 a owl:NamedIndividual ;
    rdfs:label "snaps"@en ;
    dcterms:description [ rdfs:label "Fastening devices that close with a click when the two parts are fitted tightly into each other."@en ;
            dcterms:creator "The J. Paul Getty Trust" ;
            dcterms:license <https://opendatacommons.org/licenses/by/1-0/> ;
            dcterms:rights <https://rightsstatements.org/vocab/InC/1.0/> ;
            dcterms:source <http://www.getty.edu/research/tools/vocabularies/aat/> ],
        "Fastening devices that close with a click when the two parts are fitted tightly into each other."@en ;
    dcterms:identifier "CC00008" ;
    owl:sameAs <http://vocab.getty.edu/aat/300239270> .

cc:CC00009 a owl:NamedIndividual ;
    rdfs:label "eyelets"@en ;
    dcterms:description [ rdfs:label "Small holes, usually round and finished along the edge, as in cloth or leather for the passage of a lace or cord or as in embroidery for ornamental effect."@en ;
            dcterms:creator "The J. Paul Getty Trust" ;
            dcterms:license <https://opendatacommons.org/licenses/by/1-0/> ;
            dcterms:rights <https://rightsstatements.org/vocab/InC/1.0/> ;
            dcterms:source <http://www.getty.edu/research/tools/vocabularies/aat/> ],
        "Small holes, usually round and finished along the edge, as in cloth or leather for the passage of a lace or cord or as in embroidery for ornamental effect."@en ;
    dcterms:identifier "CC00009" ;
    owl:sameAs <http://vocab.getty.edu/aat/300239342> .

cc:CC00010 a owl:NamedIndividual ;
    rdfs:label "ties"@en ;
    dcterms:description [ rdfs:label "Cords, bands, or similar flexible devices used for fastening, especially by interlacing, such as in a knot or bow."@en ;
            dcterms:creator "The J. Paul Getty Trust" ;
            dcterms:license <https://opendatacommons.org/licenses/by/1-0/> ;
            dcterms:rights <https://rightsstatements.org/vocab/InC/1.0/> ;
            dcterms:source <http://www.getty.edu/research/tools/vocabularies/aat/> ],
        "Cords, bands, or similar flexible devices used for fastening, especially by interlacing, such as in a knot or bow."@en ;
    dcterms:identifier "CC00010" ;
    owl:sameAs <http://vocab.getty.edu/aat/300239307> .

cc:CC00011 a owl:NamedIndividual ;
    rdfs:label "toggles"@en ;
    dcterms:description [ rdfs:label "Rodlike buttons of wood or other material, attached to cord, leather, or chain loops and designed to be passed through another loop as a fastener on a garment."@en ;
            dcterms:creator "The J. Paul Getty Trust" ;
            dcterms:license <https://opendatacommons.org/licenses/by/1-0/> ;
            dcterms:rights <https://rightsstatements.org/vocab/InC/1.0/> ;
            dcterms:source <http://www.getty.edu/research/tools/vocabularies/aat/> ],
        "Rodlike buttons of wood or other material, attached to cord, leather, or chain loops and designed to be passed through another loop as a fastener on a garment."@en ;
    dcterms:identifier "CC00011" ;
    owl:sameAs <http://vocab.getty.edu/aat/300254540> .

cc:CC00013 a owl:NamedIndividual ;
    rdfs:label "zipper"@en ;
    dcterms:description [ rdfs:label "Fasteners consisting usually of two rows of metal or plastic teeth on strips of tape for binding to the edges of an opening and having a sliding piece that closes the opening by drawing the teeth into interlocking position."@en ;
            dcterms:creator "The J. Paul Getty Trust" ;
            dcterms:license <https://opendatacommons.org/licenses/by/1-0/> ;
            dcterms:rights <https://rightsstatements.org/vocab/InC/1.0/> ;
            dcterms:source <http://www.getty.edu/research/tools/vocabularies/aat/> ],
        "Fasteners consisting usually of two rows of metal or plastic teeth on strips of tape for binding to the edges of an opening and having a sliding piece that closes the opening by drawing the teeth into interlocking position."@en ;
    dcterms:identifier "CC00013" ;
    owl:sameAs <http://vocab.getty.edu/aat/300239276> .

cc:CC00014 a owl:NamedIndividual ;
    rdfs:label "boat neck"@en ;
    dcterms:description [ rdfs:label "neckline cut straight or nearly straight across from should to shoulder"@en ;
            dcterms:creator "Wikidata contributors" ;
            dcterms:license <https://creativecommons.org/publicdomain/mark/1.0/> ;
            dcterms:rights <https://creativecommons.org/publicdomain/mark/1.0/> ;
            dcterms:source <https://www.wikidata.org/wiki/Wikidata:Data_access/en> ],
        "neckline cut straight or nearly straight across from should to shoulder"@en ;
    dcterms:identifier "CC00014" ;
    owl:sameAs <http://www.wikidata.org/entity/Q2466122> .

cc:CC00015 a owl:NamedIndividual ;
    rdfs:label "crew neck"@en ;
    dcterms:description [ rdfs:label "round neckline fitting close to the base of the neck, or a shiort or sweater with such a neckline"@en ;
            dcterms:creator "Wikidata contributors" ;
            dcterms:license <https://creativecommons.org/publicdomain/mark/1.0/> ;
            dcterms:rights <https://creativecommons.org/publicdomain/mark/1.0/> ;
            dcterms:source <https://www.wikidata.org/wiki/Wikidata:Data_access/en> ],
        "round neckline fitting close to the base of the neck, or a shiort or sweater with such a neckline"@en ;
    dcterms:identifier "CC00015" ;
    owl:sameAs <http://www.wikidata.org/entity/Q5184798> .

cc:CC00016 a owl:NamedIndividual ;
    rdfs:label "halterneck"@en ;
    dcterms:description [ rdfs:label "Garments having a strap encircling the neck and supporting the front of the bodice, leaving shoulders and most of the back bare."@en ;
            dcterms:creator "The J. Paul Getty Trust" ;
            dcterms:license <https://opendatacommons.org/licenses/by/1-0/> ;
            dcterms:rights <https://rightsstatements.org/vocab/InC/1.0/> ;
            dcterms:source <http://www.getty.edu/research/tools/vocabularies/aat/> ],
        "Garments having a strap encircling the neck and supporting the front of the bodice, leaving shoulders and most of the back bare."@en ;
    dcterms:identifier "CC00016" ;
    owl:sameAs <http://vocab.getty.edu/aat/300209885> .

cc:CC00017 a owl:NamedIndividual ;
    rdfs:label "henley neckline"@en ;
    dcterms:description [ rdfs:label "a round neckline with a button placket about 3 to 5 inches (8 to 13 cm) long, with 25 buttons"@en ;
            dcterms:creator "Wikidata contributors" ;
            dcterms:license <https://creativecommons.org/publicdomain/mark/1.0/> ;
            dcterms:rights <https://creativecommons.org/publicdomain/mark/1.0/> ;
            dcterms:source <https://www.wikidata.org/wiki/Wikidata:Data_access/en> ],
        "a round neckline with a button placket about 3 to 5 inches (8 to 13 cm) long, with 25 buttons"@en ;
    dcterms:identifier "CC00017" ;
    owl:sameAs <http://www.wikidata.org/entity/Q77004674> .

cc:CC00020 a owl:NamedIndividual ;
    rdfs:label "keyhole neckline"@en ;
    dcterms:identifier "CC00020" ;
    owl:sameAs <http://www.wikidata.org/entity/Q1751458> .

cc:CC00021 a owl:NamedIndividual ;
    rdfs:label "off-the-shoulder neckline"@en ;
    dcterms:identifier "CC00021" ;
    owl:sameAs <http://www.wikidata.org/entity/Q1043590> .

cc:CC00024 a owl:NamedIndividual ;
    rdfs:label "square neck"@en ;
    dcterms:identifier "CC00024" ;
    owl:sameAs <http://www.wikidata.org/entity/Q29583222> .

cc:CC00025 a owl:NamedIndividual ;
    rdfs:label "strapless"@en ;
    dcterms:description [ rdfs:label "Upper edge of the garment is just above the bustline with nothing over the shoulders."@en ;
            dcterms:creator "Wikidata contributors" ;
            dcterms:license <https://creativecommons.org/publicdomain/mark/1.0/> ;
            dcterms:rights <https://creativecommons.org/publicdomain/mark/1.0/> ;
            dcterms:source <https://www.wikidata.org/wiki/Wikidata:Data_access/en> ],
        "Upper edge of the garment is just above the bustline with nothing over the shoulders."@en ;
    dcterms:identifier "CC00025" ;
    owl:sameAs <http://www.wikidata.org/entity/Q83329964> .

cc:CC00026 a owl:NamedIndividual ;
    rdfs:label "sweetheart neckline"@en ;
    dcterms:identifier "CC00026" ;
    owl:sameAs <http://www.wikidata.org/entity/Q73419282> .

cc:CC00027 a owl:NamedIndividual ;
    rdfs:label "v-neck"@en ;
    dcterms:identifier "CC00027" ;
    owl:sameAs <http://www.wikidata.org/entity/Q29583212> .

cc:CC00030 a owl:NamedIndividual ;
    rdfs:label "bertha"@en ;
    dcterms:description [ rdfs:label "Deep, capelike collars, often of lace or silk, worn about the shoulders by women."@en ;
            dcterms:creator "The J. Paul Getty Trust" ;
            dcterms:license <https://opendatacommons.org/licenses/by/1-0/> ;
            dcterms:rights <https://rightsstatements.org/vocab/InC/1.0/> ;
            dcterms:source <http://www.getty.edu/research/tools/vocabularies/aat/> ],
        "Deep, capelike collars, often of lace or silk, worn about the shoulders by women."@en ;
    dcterms:identifier "CC00030" ;
    owl:sameAs <http://vocab.getty.edu/aat/300210054>,
        <http://www.wikidata.org/entity/Q64780667> .

cc:CC00034 a owl:NamedIndividual ;
    rdfs:label "cowl neck"@en ;
    dcterms:description [ rdfs:label "has fabric that drapes loosely around the neck, sometimes cut or knit in one with the torso, sometimes as an added a foldover collar"@en ;
            dcterms:creator "Wikidata contributors" ;
            dcterms:license <https://creativecommons.org/publicdomain/mark/1.0/> ;
            dcterms:rights <https://creativecommons.org/publicdomain/mark/1.0/> ;
            dcterms:source <https://www.wikidata.org/wiki/Wikidata:Data_access/en> ],
        "has fabric that drapes loosely around the neck, sometimes cut or knit in one with the torso, sometimes as an added a foldover collar"@en ;
    dcterms:identifier "CC00034" ;
    owl:sameAs <http://www.wikidata.org/entity/Q83328363> .

cc:CC00035 a owl:NamedIndividual ;
    rdfs:label "funnel neck"@en ;
    dcterms:description [ rdfs:label "a neckline with fabric standing high and close to the neck, cut or knit in one piece with the torso rather than as an added collar"@en ;
            dcterms:creator "Wikidata contributors" ;
            dcterms:license <https://creativecommons.org/publicdomain/mark/1.0/> ;
            dcterms:rights <https://creativecommons.org/publicdomain/mark/1.0/> ;
            dcterms:source <https://www.wikidata.org/wiki/Wikidata:Data_access/en> ],
        "a neckline with fabric standing high and close to the neck, cut or knit in one piece with the torso rather than as an added collar"@en ;
    dcterms:identifier "CC00035" ;
    owl:sameAs <http://www.wikidata.org/entity/Q83328663> .

cc:CC00037 a owl:NamedIndividual ;
    rdfs:label "Mandarin collar"@en ;
    dcterms:description [ rdfs:label "upright collar for a coat or waistcoat, without a turn-down"@en ;
            dcterms:creator "Wikidata contributors" ;
            dcterms:license <https://creativecommons.org/publicdomain/mark/1.0/> ;
            dcterms:rights <https://creativecommons.org/publicdomain/mark/1.0/> ;
            dcterms:source <https://www.wikidata.org/wiki/Wikidata:Data_access/en> ],
        "upright collar for a coat or waistcoat, without a turn-down"@en ;
    dcterms:identifier "CC00037" ;
    owl:sameAs <http://www.wikidata.org/entity/Q1045372> .

cc:CC00039 a owl:NamedIndividual ;
    rdfs:label "tailored collar"@en ;
    dcterms:description [ rdfs:label "collar constructed like a traditional men's coat collar, with a stand and fall"@en ;
            dcterms:creator "Wikidata contributors" ;
            dcterms:license <https://creativecommons.org/publicdomain/mark/1.0/> ;
            dcterms:rights <https://creativecommons.org/publicdomain/mark/1.0/> ;
            dcterms:source <https://www.wikidata.org/wiki/Wikidata:Data_access/en> ],
        "collar constructed like a traditional men's coat collar, with a stand and fall"@en ;
    dcterms:identifier "CC00039" ;
    owl:sameAs <http://www.wikidata.org/entity/Q29473272> .

cc:CC00040 a owl:NamedIndividual ;
    rdfs:label "Peter Pan collar"@en ;
    dcterms:description [ rdfs:label "small, soft, flat collar with rounded corners"@en ;
            dcterms:creator "Wikidata contributors" ;
            dcterms:license <https://creativecommons.org/publicdomain/mark/1.0/> ;
            dcterms:rights <https://creativecommons.org/publicdomain/mark/1.0/> ;
            dcterms:source <https://www.wikidata.org/wiki/Wikidata:Data_access/en> ],
        "small, soft, flat collar with rounded corners"@en ;
    dcterms:identifier "CC00040" ;
    owl:sameAs <http://www.wikidata.org/entity/Q997545> .

cc:CC00043 a owl:NamedIndividual ;
    rdfs:label "Puritan collar"@en ;
    dcterms:description [ rdfs:label "A wide, square collar often reaching to the shoulders, with a squared off opening at the center front"@en ;
            dcterms:creator "Wikidata contributors" ;
            dcterms:license <https://creativecommons.org/publicdomain/mark/1.0/> ;
            dcterms:rights <https://creativecommons.org/publicdomain/mark/1.0/> ;
            dcterms:source <https://www.wikidata.org/wiki/Wikidata:Data_access/en> ],
        "A wide, square collar often reaching to the shoulders, with a squared off opening at the center front"@en ;
    dcterms:identifier "CC00043" ;
    owl:sameAs <http://www.wikidata.org/entity/Q83329279> .

cc:CC00045 a owl:NamedIndividual ;
    rdfs:label "sailor collar"@en ;
    dcterms:description [ rdfs:label "collar with a V-opening in front and a broad, square, flat back, copied from sailor's unform"@en ;
            dcterms:creator "Wikidata contributors" ;
            dcterms:license <https://creativecommons.org/publicdomain/mark/1.0/> ;
            dcterms:rights <https://creativecommons.org/publicdomain/mark/1.0/> ;
            dcterms:source <https://www.wikidata.org/wiki/Wikidata:Data_access/en> ],
        "collar with a V-opening in front and a broad, square, flat back, copied from sailor's unform"@en ;
    dcterms:identifier "CC00045" ;
    owl:sameAs <http://www.wikidata.org/entity/Q23301561> .

cc:CC00046 a owl:NamedIndividual ;
    rdfs:label "shawl"@en ;
    dcterms:description [ rdfs:label "Large pieces of square, oblong, or triangular cloth worn over main garments as a covering for the shoulders and arms."@en ;
            dcterms:creator "The J. Paul Getty Trust" ;
            dcterms:license <https://opendatacommons.org/licenses/by/1-0/> ;
            dcterms:rights <https://rightsstatements.org/vocab/InC/1.0/> ;
            dcterms:source <http://www.getty.edu/research/tools/vocabularies/aat/> ],
        "Large pieces of square, oblong, or triangular cloth worn over main garments as a covering for the shoulders and arms."@en ;
    dcterms:identifier "CC00046" ;
    owl:sameAs <http://vocab.getty.edu/aat/300209991> .

cc:CC00047 a owl:NamedIndividual ;
    rdfs:label "turtleneck"@en ;
    dcterms:description [ rdfs:label "tall, snug, fold over neckline"@en ;
            dcterms:creator "Wikidata contributors" ;
            dcterms:license <https://creativecommons.org/publicdomain/mark/1.0/> ;
            dcterms:rights <https://creativecommons.org/publicdomain/mark/1.0/> ;
            dcterms:source <https://www.wikidata.org/wiki/Wikidata:Data_access/en> ],
        "tall, snug, fold over neckline"@en ;
    dcterms:identifier "CC00047" ;
    owl:sameAs <http://www.wikidata.org/entity/Q1544262> .

cc:CC00048 a owl:NamedIndividual ;
    rdfs:label "wingtip collar"@en ;
    dcterms:description [ rdfs:label "A small standing collar with the points pressed to stick out horizontally, resembling \"wings,\" worn with men's evening dress (white tie or black tie)"@en ;
            dcterms:creator "Wikipedia" ;
            dcterms:license <https://creativecommons.org/publicdomain/mark/1.0/> ;
            dcterms:rights <https://creativecommons.org/publicdomain/mark/1.0/> ;
            dcterms:source <https://en.wikipedia.org/wiki/Collar_(clothing)> ],
        "A small standing collar with the points pressed to stick out horizontally, resembling \"wings,\" worn with men's evening dress (white tie or black tie)"@en ;
    dcterms:identifier "CC00048" ;
    owl:sameAs <http://www.wikidata.org/entity/Q83328891> .

cc:CC00062 a owl:NamedIndividual ;
    rdfs:label "multicolored"@en ;
    dcterms:description [ rdfs:label "Refers generally to the use of many colors."@en ;
            dcterms:creator "The J. Paul Getty Trust" ;
            dcterms:license <https://opendatacommons.org/licenses/by/1-0/> ;
            dcterms:rights <https://rightsstatements.org/vocab/InC/1.0/> ;
            dcterms:source <http://www.getty.edu/research/tools/vocabularies/aat/> ],
        "Refers generally to the use of many colors."@en ;
    dcterms:identifier "CC00062" .

cc:CC00074 a owl:NamedIndividual ;
    rdfs:label "applique"@en ;
    dcterms:description [ rdfs:label "Technique of forming a design by applying cut out pieces of a material to a ground material; generally associated with needleworking, but also used in ceramics, leatherworking, woodworking, and metalworking."@en ;
            dcterms:creator "The J. Paul Getty Trust" ;
            dcterms:license <https://opendatacommons.org/licenses/by/1-0/> ;
            dcterms:rights <https://rightsstatements.org/vocab/InC/1.0/> ;
            dcterms:source <http://www.getty.edu/research/tools/vocabularies/aat/> ],
        "Technique of forming a design by applying cut out pieces of a material to a ground material; generally associated with needleworking, but also used in ceramics, leatherworking, woodworking, and metalworking."@en ;
    dcterms:identifier "CC00074" ;
    owl:sameAs <http://vocab.getty.edu/aat/300053646> .

cc:CC00075 a owl:NamedIndividual ;
    rdfs:label "beading"@en ;
    dcterms:description [ rdfs:label "Trimming, furnishing, adorning, or covering textiles or objects with beads, or creating jewelry by stringing beads."@en ;
            dcterms:creator "The J. Paul Getty Trust" ;
            dcterms:license <https://opendatacommons.org/licenses/by/1-0/> ;
            dcterms:rights <https://rightsstatements.org/vocab/InC/1.0/> ;
            dcterms:source <http://www.getty.edu/research/tools/vocabularies/aat/> ],
        "Trimming, furnishing, adorning, or covering textiles or objects with beads, or creating jewelry by stringing beads."@en ;
    dcterms:identifier "CC00075" ;
    owl:sameAs <http://vocab.getty.edu/aat/300235440> .

cc:CC00076 a owl:NamedIndividual ;
    rdfs:label "braiding"@en ;
    dcterms:description [ rdfs:label "Flat over-and-under oblique interlacing using the undifferentiated elements of a single set of strands, characterized by the oblique crossings of the elements and their common directional trend."@en ;
            dcterms:creator "The J. Paul Getty Trust" ;
            dcterms:license <https://opendatacommons.org/licenses/by/1-0/> ;
            dcterms:rights <https://rightsstatements.org/vocab/InC/1.0/> ;
            dcterms:source <http://www.getty.edu/research/tools/vocabularies/aat/> ],
        "Flat over-and-under oblique interlacing using the undifferentiated elements of a single set of strands, characterized by the oblique crossings of the elements and their common directional trend."@en ;
    dcterms:identifier "CC00076" ;
    owl:sameAs <http://vocab.getty.edu/aat/300053638> .

cc:CC00078 a owl:NamedIndividual ;
    rdfs:label "crocheting"@en ;
    dcterms:description [ rdfs:label "Textile construction involving the interlocking of looped stitches, employing a single cord or strand of yarn and a single hooked needle."@en ;
            dcterms:creator "The J. Paul Getty Trust" ;
            dcterms:license <https://opendatacommons.org/licenses/by/1-0/> ;
            dcterms:rights <https://rightsstatements.org/vocab/InC/1.0/> ;
            dcterms:source <http://www.getty.edu/research/tools/vocabularies/aat/> ],
        "Textile construction involving the interlocking of looped stitches, employing a single cord or strand of yarn and a single hooked needle."@en ;
    dcterms:identifier "CC00078" ;
    owl:sameAs <http://vocab.getty.edu/aat/300053632> .

cc:CC00080 a owl:NamedIndividual ;
    rdfs:label "embossing"@en ;
    dcterms:description [ rdfs:label "Producing raised letters or designs on a surface, typically by means of stamping or molding."@en ;
            dcterms:creator "The J. Paul Getty Trust" ;
            dcterms:license <https://opendatacommons.org/licenses/by/1-0/> ;
            dcterms:rights <https://rightsstatements.org/vocab/InC/1.0/> ;
            dcterms:source <http://www.getty.edu/research/tools/vocabularies/aat/> ],
        "Producing raised letters or designs on a surface, typically by means of stamping or molding."@en ;
    dcterms:identifier "CC00080" ;
    owl:sameAs <http://vocab.getty.edu/aat/300053826> .

cc:CC00082 a owl:NamedIndividual ;
    rdfs:label "flocking"@en ;
    dcterms:description [ rdfs:label "Creating a textured effect similar to suede or felt by blowing fibers of cotton, silk, nylon, or other material onto a tacky surface, usually paper."@en ;
            dcterms:creator "The J. Paul Getty Trust" ;
            dcterms:license <https://opendatacommons.org/licenses/by/1-0/> ;
            dcterms:rights <https://rightsstatements.org/vocab/InC/1.0/> ;
            dcterms:source <http://www.getty.edu/research/tools/vocabularies/aat/> ],
        "Creating a textured effect similar to suede or felt by blowing fibers of cotton, silk, nylon, or other material onto a tacky surface, usually paper."@en ;
    dcterms:identifier "CC00082" ;
    owl:sameAs <http://vocab.getty.edu/aat/300053786> .

cc:CC00083 a owl:NamedIndividual ;
    rdfs:label "glazing"@en ;
    dcterms:description [ rdfs:label "Overlaying or covering with a smooth and lustrous coating, or polishing and burnishing to create a smooth, shiney surface. To refer specifically to glazing paintings, use the narrower concept \"glazing (painting technique).\" To refer specifically to glazing ceramics, use the narrower concept \"pottery glazing (process).\""@en ;
            dcterms:creator "The J. Paul Getty Trust" ;
            dcterms:license <https://opendatacommons.org/licenses/by/1-0/> ;
            dcterms:rights <https://rightsstatements.org/vocab/InC/1.0/> ;
            dcterms:source <http://www.getty.edu/research/tools/vocabularies/aat/> ],
        "Overlaying or covering with a smooth and lustrous coating, or polishing and burnishing to create a smooth, shiney surface. To refer specifically to glazing paintings, use the narrower concept \"glazing (painting technique).\" To refer specifically to glazing ceramics, use the narrower concept \"pottery glazing (process).\""@en ;
    dcterms:identifier "CC00083" ;
    owl:sameAs <http://vocab.getty.edu/aat/300053914> .

cc:CC00084 a owl:NamedIndividual ;
    rdfs:label "hand sewing"@en ;
    dcterms:description [ rdfs:label "Sewing by hand, as distinct from sewing by machine."@en ;
            dcterms:creator "The J. Paul Getty Trust" ;
            dcterms:license <https://opendatacommons.org/licenses/by/1-0/> ;
            dcterms:rights <https://rightsstatements.org/vocab/InC/1.0/> ;
            dcterms:source <http://www.getty.edu/research/tools/vocabularies/aat/> ],
        "Sewing by hand, as distinct from sewing by machine."@en ;
    dcterms:identifier "CC00084" ;
    owl:sameAs <http://vocab.getty.edu/aat/300257459> .

cc:CC00085 a owl:NamedIndividual ;
    rdfs:label "hand weaving"@en ;
    dcterms:description [ rdfs:label "Weaving on a loom or other device operated wholly or partly by hand or foot power."@en ;
            dcterms:creator "The J. Paul Getty Trust" ;
            dcterms:license <https://opendatacommons.org/licenses/by/1-0/> ;
            dcterms:rights <https://rightsstatements.org/vocab/InC/1.0/> ;
            dcterms:source <http://www.getty.edu/research/tools/vocabularies/aat/> ],
        "Weaving on a loom or other device operated wholly or partly by hand or foot power."@en ;
    dcterms:identifier "CC00085" ;
    owl:sameAs <http://vocab.getty.edu/aat/300053643> .

cc:CC00086 a owl:NamedIndividual ;
    rdfs:label "knitting"@en ;
    dcterms:description [ rdfs:label "The forming and interlacing of loops by means of needles according to a prescribed manner or pattern, either by machine or by hand; most often used for textiles or costume."@en ;
            dcterms:creator "The J. Paul Getty Trust" ;
            dcterms:license <https://opendatacommons.org/licenses/by/1-0/> ;
            dcterms:rights <https://rightsstatements.org/vocab/InC/1.0/> ;
            dcterms:source <http://www.getty.edu/research/tools/vocabularies/aat/> ],
        "The forming and interlacing of loops by means of needles according to a prescribed manner or pattern, either by machine or by hand; most often used for textiles or costume."@en ;
    dcterms:identifier "CC00086" ;
    owl:sameAs <http://vocab.getty.edu/aat/300053634> .

cc:CC00088 a owl:NamedIndividual ;
    rdfs:label "machine sewing"@en ;
    dcterms:description [ rdfs:label "Sewing by machine, as distinct from sewing by hand."@en ;
            dcterms:creator "The J. Paul Getty Trust" ;
            dcterms:license <https://opendatacommons.org/licenses/by/1-0/> ;
            dcterms:rights <https://rightsstatements.org/vocab/InC/1.0/> ;
            dcterms:source <http://www.getty.edu/research/tools/vocabularies/aat/> ],
        "Sewing by machine, as distinct from sewing by hand."@en ;
    dcterms:identifier "CC00088" ;
    owl:sameAs <http://vocab.getty.edu/aat/300257463> .

cc:CC00089 a owl:NamedIndividual ;
    rdfs:label "mercerizing"@en ;
    dcterms:description [ rdfs:label "Treatment of cotton yarn or fabric by immersion in a caustic solution of sodium hydroxide or other chemical base. Fibers so treated swell permanently, and the cotton is made stronger and more lustrous. Named after Alexander Mercer (1791-1866), who perfected the process."@en ;
            dcterms:creator "The J. Paul Getty Trust" ;
            dcterms:license <https://opendatacommons.org/licenses/by/1-0/> ;
            dcterms:rights <https://rightsstatements.org/vocab/InC/1.0/> ;
            dcterms:source <http://www.getty.edu/research/tools/vocabularies/aat/> ],
        "Treatment of cotton yarn or fabric by immersion in a caustic solution of sodium hydroxide or other chemical base. Fibers so treated swell permanently, and the cotton is made stronger and more lustrous. Named after Alexander Mercer (1791-1866), who perfected the process."@en ;
    dcterms:identifier "CC00089" ;
    owl:sameAs <http://vocab.getty.edu/aat/300379924> .

cc:CC00090 a owl:NamedIndividual ;
    rdfs:label "needleworking"@en ;
    dcterms:identifier "CC00090" ;
    owl:sameAs <http://vocab.getty.edu/aat/300053652> .

cc:CC00092 a owl:NamedIndividual ;
    rdfs:label "painting"@en ;
    dcterms:description [ rdfs:label "The art and practice of applying pigments suspended in water, oil, egg yolk, molten wax, or other liquid to a surface to create an expressive or communicative image. Paint is usually, but not always, applied with a brush. For the application of paint primarily to protect a surface or add a general color, use \"painting (coating).\""@en ;
            dcterms:creator "The J. Paul Getty Trust" ;
            dcterms:license <https://opendatacommons.org/licenses/by/1-0/> ;
            dcterms:rights <https://rightsstatements.org/vocab/InC/1.0/> ;
            dcterms:source <http://www.getty.edu/research/tools/vocabularies/aat/> ],
        "The art and practice of applying pigments suspended in water, oil, egg yolk, molten wax, or other liquid to a surface to create an expressive or communicative image. Paint is usually, but not always, applied with a brush. For the application of paint primarily to protect a surface or add a general color, use \"painting (coating).\""@en ;
    dcterms:identifier "CC00092" ;
    owl:sameAs <http://vocab.getty.edu/aat/300054216> .

cc:CC00093 a owl:NamedIndividual ;
    rdfs:label "piecing"@en ;
    dcterms:description [ rdfs:label "Joining small pieces of cloth together with a seam to form an overall pattern."@en ;
            dcterms:creator "The J. Paul Getty Trust" ;
            dcterms:license <https://opendatacommons.org/licenses/by/1-0/> ;
            dcterms:rights <https://rightsstatements.org/vocab/InC/1.0/> ;
            dcterms:source <http://www.getty.edu/research/tools/vocabularies/aat/> ],
        "Joining small pieces of cloth together with a seam to form an overall pattern."@en ;
    dcterms:identifier "CC00093" ;
    owl:sameAs <http://vocab.getty.edu/aat/300231250> .

cc:CC00094 a owl:NamedIndividual ;
    rdfs:label "piping"@en ;
    dcterms:description [ rdfs:label "Tubular strip of textile, usually bias-cut, which may or may not enclose a cord, used for trimming the edges and seams of costume, coverings, and hangings. May be of matching or contrasting fabric, sometimes also in leather."@en ;
            dcterms:creator "The J. Paul Getty Trust" ;
            dcterms:license <https://opendatacommons.org/licenses/by/1-0/> ;
            dcterms:rights <https://rightsstatements.org/vocab/InC/1.0/> ;
            dcterms:source <http://www.getty.edu/research/tools/vocabularies/aat/> ],
        "Tubular strip of textile, usually bias-cut, which may or may not enclose a cord, used for trimming the edges and seams of costume, coverings, and hangings. May be of matching or contrasting fabric, sometimes also in leather."@en ;
    dcterms:identifier "CC00094" ;
    owl:sameAs <http://vocab.getty.edu/aat/300232162> .

cc:CC00095 a owl:NamedIndividual ;
    rdfs:label "pleating"@en ;
    dcterms:description [ rdfs:label "Double folding a definite, even width of fabric and fixing it in place by sewing or pressing or both."@en ;
            dcterms:creator "The J. Paul Getty Trust" ;
            dcterms:license <https://opendatacommons.org/licenses/by/1-0/> ;
            dcterms:rights <https://rightsstatements.org/vocab/InC/1.0/> ;
            dcterms:source <http://www.getty.edu/research/tools/vocabularies/aat/> ],
        "Double folding a definite, even width of fabric and fixing it in place by sewing or pressing or both."@en ;
    dcterms:identifier "CC00095" ;
    owl:sameAs <http://vocab.getty.edu/aat/300227874> .

cc:CC00096 a owl:NamedIndividual ;
    rdfs:label "polishing"@en ;
    dcterms:description [ rdfs:label "Process of rubbing a surface to make it smooth or shiny."@en ;
            dcterms:creator "The J. Paul Getty Trust" ;
            dcterms:license <https://opendatacommons.org/licenses/by/1-0/> ;
            dcterms:rights <https://rightsstatements.org/vocab/InC/1.0/> ;
            dcterms:source <http://www.getty.edu/research/tools/vocabularies/aat/> ],
        "Process of rubbing a surface to make it smooth or shiny."@en ;
    dcterms:identifier "CC00096" ;
    owl:sameAs <http://vocab.getty.edu/aat/300053867> .

cc:CC00097 a owl:NamedIndividual ;
    rdfs:label "printing"@en ;
    dcterms:description [ rdfs:label "Various means of reproducing identical copies of graphic matter in a fixed form. Processes by which an image, pictorial or textual, is transferred, usually to paper or cloth, most often by means of a plate, block, stone, or screen. Use also for the making of photographic prints and, with computers, for the production of a paper copy of stored data. For the production of prints in a fine arts context, prefer \"printmaking.\""@en ;
            dcterms:creator "The J. Paul Getty Trust" ;
            dcterms:license <https://opendatacommons.org/licenses/by/1-0/> ;
            dcterms:rights <https://rightsstatements.org/vocab/InC/1.0/> ;
            dcterms:source <http://www.getty.edu/research/tools/vocabularies/aat/> ],
        "Various means of reproducing identical copies of graphic matter in a fixed form. Processes by which an image, pictorial or textual, is transferred, usually to paper or cloth, most often by means of a plate, block, stone, or screen. Use also for the making of photographic prints and, with computers, for the production of a paper copy of stored data. For the production of prints in a fine arts context, prefer \"printmaking.\""@en ;
    dcterms:identifier "CC00097" ;
    owl:sameAs <http://vocab.getty.edu/aat/300053319> .

cc:CC00098 a owl:NamedIndividual ;
    rdfs:label "quilting"@en ;
    dcterms:description [ rdfs:label "Stitching together two or more layers of cloth, usually working the stitches into designs."@en ;
            dcterms:creator "The J. Paul Getty Trust" ;
            dcterms:license <https://opendatacommons.org/licenses/by/1-0/> ;
            dcterms:rights <https://rightsstatements.org/vocab/InC/1.0/> ;
            dcterms:source <http://www.getty.edu/research/tools/vocabularies/aat/> ],
        "Stitching together two or more layers of cloth, usually working the stitches into designs."@en ;
    dcterms:identifier "CC00098" ;
    owl:sameAs <http://vocab.getty.edu/aat/300053656> .

cc:CC00099 a owl:NamedIndividual ;
    rdfs:label "ruffle"@en ;
    dcterms:description [ rdfs:label "strip of fabric, lace, or ribbon gathered on one edge and applied as trimming"@en ;
            dcterms:creator "The J. Paul Getty Trust" ;
            dcterms:license <https://opendatacommons.org/licenses/by/1-0/> ;
            dcterms:rights <https://rightsstatements.org/vocab/InC/1.0/> ;
            dcterms:source <http://www.getty.edu/research/tools/vocabularies/aat/> ],
        "strip of fabric, lace, or ribbon gathered on one edge and applied as trimming"@en ;
    dcterms:identifier "CC00099" ;
    owl:sameAs <http://vocab.getty.edu/aat/300253712>,
        <http://www.wikidata.org/entity/Q2204140> .

cc:CC00100 a owl:NamedIndividual ;
    rdfs:label "smocking"@en ;
    dcterms:description [ rdfs:label "Refers to the process applied to a garment or other piece of fabric, comprising gathering tucks and working the tucks with a simple or decorative stitch."@en ;
            dcterms:creator "The J. Paul Getty Trust" ;
            dcterms:license <https://opendatacommons.org/licenses/by/1-0/> ;
            dcterms:rights <https://rightsstatements.org/vocab/InC/1.0/> ;
            dcterms:source <http://www.getty.edu/research/tools/vocabularies/aat/> ],
        "Refers to the process applied to a garment or other piece of fabric, comprising gathering tucks and working the tucks with a simple or decorative stitch."@en ;
    dcterms:identifier "CC00100" ;
    owl:sameAs <http://vocab.getty.edu/aat/300264622> .

cc:CC00101 a owl:NamedIndividual ;
    rdfs:label "weaving"@en ;
    dcterms:description [ rdfs:label "Generally, the process of interlacing strands or strips of various materials, such as cane, textile, or twigs, to make materials or objects such as wicker, cloth, baskets, or wreaths. Specifically used for the process of making textile on a loom or other weaving device by interlacing warp and weft in a particular order."@en ;
            dcterms:creator "The J. Paul Getty Trust" ;
            dcterms:license <https://opendatacommons.org/licenses/by/1-0/> ;
            dcterms:rights <https://rightsstatements.org/vocab/InC/1.0/> ;
            dcterms:source <http://www.getty.edu/research/tools/vocabularies/aat/> ],
        "Generally, the process of interlacing strands or strips of various materials, such as cane, textile, or twigs, to make materials or objects such as wicker, cloth, baskets, or wreaths. Specifically used for the process of making textile on a loom or other weaving device by interlacing warp and weft in a particular order."@en ;
    dcterms:identifier "CC00101" ;
    owl:sameAs <http://vocab.getty.edu/aat/300053642> .

cc:CC00102 a owl:NamedIndividual ;
    rdfs:label "a-line skirt"@en ;
    dcterms:description [ rdfs:label "a skirt with a slight flare, roughly in the shape of a capital letter A"@en ;
            dcterms:creator "Wikidata contributors" ;
            dcterms:license <https://creativecommons.org/publicdomain/mark/1.0/> ;
            dcterms:rights <https://creativecommons.org/publicdomain/mark/1.0/> ;
            dcterms:source <https://en.wikipedia.org/wiki/Skirt> ],
        "a skirt with a slight flare, roughly in the shape of a capital letter A"@en ;
    dcterms:identifier "CC00102" ;
    owl:sameAs <http://www.wikidata.org/entity/Q277835> .

cc:CC00106 a owl:NamedIndividual ;
    rdfs:label "coat"@en ;
    dcterms:description [ rdfs:label "Main garments usually fitted to the upper body, extending below the hip line, open at the front or side and generally having sleeves. Also, similar outer garments worn for warmth or protection from the weather."@en ;
            dcterms:creator "The J. Paul Getty Trust" ;
            dcterms:license <https://opendatacommons.org/licenses/by/1-0/> ;
            dcterms:rights <https://rightsstatements.org/vocab/InC/1.0/> ;
            dcterms:source <http://www.getty.edu/research/tools/vocabularies/aat/> ],
        "Main garments usually fitted to the upper body, extending below the hip line, open at the front or side and generally having sleeves. Also, similar outer garments worn for warmth or protection from the weather."@en ;
    dcterms:identifier "CC00106" ;
    owl:sameAs <http://vocab.getty.edu/aat/300046143> .

cc:CC00109 a owl:NamedIndividual ;
    rdfs:label "Empire silhouette"@en ;
    dcterms:description [ rdfs:label "woman's dress style with a high waist and narrow skirt"@en ;
            dcterms:creator "Wikidata contributors" ;
            dcterms:license <https://creativecommons.org/publicdomain/mark/1.0/> ;
            dcterms:rights <https://creativecommons.org/publicdomain/mark/1.0/> ;
            dcterms:source <https://www.wikidata.org/wiki/Wikidata:Data_access/en> ],
        "woman's dress style with a high waist and narrow skirt"@en ;
    dcterms:identifier "CC00109" ;
    owl:sameAs <http://www.wikidata.org/entity/Q3603737> .

cc:CC00112 a owl:NamedIndividual ;
    rdfs:label "jumper"@en ;
    dcterms:description [ rdfs:label "Sleeveless dresses or skirts with straps and a partial or full bodice, usually worn over a shirt or blouse by women and children."@en ;
            dcterms:creator "The J. Paul Getty Trust" ;
            dcterms:license <https://opendatacommons.org/licenses/by/1-0/> ;
            dcterms:rights <https://rightsstatements.org/vocab/InC/1.0/> ;
            dcterms:source <http://www.getty.edu/research/tools/vocabularies/aat/> ],
        "Sleeveless dresses or skirts with straps and a partial or full bodice, usually worn over a shirt or blouse by women and children."@en ;
    dcterms:identifier "CC00112" ;
    owl:sameAs <http://vocab.getty.edu/aat/300046164> .

cc:CC00116 a owl:NamedIndividual ;
    rdfs:label "princess seams"@en ;
    dcterms:description [ rdfs:label "Long rounded seams sewn into women's blouses or shirts to add shaping or a tailored fit to closely follow a woman's shape"@en ;
            dcterms:creator "Wikidata contributors" ;
            dcterms:license <https://creativecommons.org/publicdomain/mark/1.0/> ;
            dcterms:rights <https://creativecommons.org/publicdomain/mark/1.0/> ;
            dcterms:source <https://www.wikidata.org/wiki/Wikidata:Data_access/en> ],
        "Long rounded seams sewn into women's blouses or shirts to add shaping or a tailored fit to closely follow a woman's shape"@en ;
    dcterms:identifier "CC00116" ;
    owl:sameAs <http://www.wikidata.org/entity/Q2569037> .

cc:CC00119 a owl:NamedIndividual ;
    rdfs:label "round neck"@en ;
    dcterms:description [ rdfs:label "Curved neckline fitting close to the base of the neck."@en ;
            dcterms:creator "Wikidata contributors" ;
            dcterms:license <https://creativecommons.org/publicdomain/mark/1.0/> ;
            dcterms:rights <https://creativecommons.org/publicdomain/mark/1.0/> ;
            dcterms:source <https://www.wikidata.org/wiki/Wikidata:Data_access/en> ],
        "Curved neckline fitting close to the base of the neck."@en ;
    dcterms:identifier "CC00119" ;
    owl:sameAs <http://www.wikidata.org/entity/Q29583217> .

cc:CC00121 a owl:NamedIndividual ;
    rdfs:label "sheath dress"@en ;
    dcterms:description [ rdfs:label "Close-fitting dresses with a tight, straight skirt."@en ;
            dcterms:creator "The J. Paul Getty Trust" ;
            dcterms:license <https://opendatacommons.org/licenses/by/1-0/> ;
            dcterms:rights <https://rightsstatements.org/vocab/InC/1.0/> ;
            dcterms:source <http://www.getty.edu/research/tools/vocabularies/aat/> ],
        "Close-fitting dresses with a tight, straight skirt."@en ;
    dcterms:identifier "CC00121" ;
    owl:sameAs <http://vocab.getty.edu/aat/300211788> .

cc:CC00123 a owl:NamedIndividual ;
    rdfs:label "slip dress"@en ;
    dcterms:description [ rdfs:label "Underwear usually made the length of the garment under which it is to be worn, thereby taking the place of a lining. Usually applied to full slips with a bodice and shoulder straps made in dress length. Prefer \"half slips\" for skirtlike underwear extending from the waist to near the hemline of the garment with which it is worn."@en ;
            dcterms:creator "The J. Paul Getty Trust" ;
            dcterms:license <https://opendatacommons.org/licenses/by/1-0/> ;
            dcterms:rights <https://rightsstatements.org/vocab/InC/1.0/> ;
            dcterms:source <http://www.getty.edu/research/tools/vocabularies/aat/> ],
        "Underwear usually made the length of the garment under which it is to be worn, thereby taking the place of a lining. Usually applied to full slips with a bodice and shoulder straps made in dress length. Prefer \"half slips\" for skirtlike underwear extending from the waist to near the hemline of the garment with which it is worn."@en ;
    dcterms:identifier "CC00123" ;
    owl:sameAs <http://vocab.getty.edu/aat/300210564> .

cc:CC00125 a owl:NamedIndividual ;
    rdfs:label "toga"@en ;
    dcterms:description [ rdfs:label "Loose mantles of undyed woolen cloth worn by men and women of ancient Rome. Also, similar loose wraps made of various fabrics and worn in various historical periods."@en ;
            dcterms:creator "The J. Paul Getty Trust" ;
            dcterms:license <https://opendatacommons.org/licenses/by/1-0/> ;
            dcterms:rights <https://rightsstatements.org/vocab/InC/1.0/> ;
            dcterms:source <http://www.getty.edu/research/tools/vocabularies/aat/> ],
        "Loose mantles of undyed woolen cloth worn by men and women of ancient Rome. Also, similar loose wraps made of various fabrics and worn in various historical periods."@en ;
    dcterms:identifier "CC00125" ;
    owl:sameAs <http://vocab.getty.edu/aat/300209868> .

cc:CC00126 a owl:NamedIndividual ;
    rdfs:label "tunic"@en ;
    dcterms:description [ rdfs:label "Simple slip-on garments made with or without sleeves and usually knee-length or longer and belted at the waist; especially those worn by men and women of ancient Greece and Rome. Also, garments extending from the neckline to the waist or longer, usually high-necked and worn over other garments."@en ;
            dcterms:creator "The J. Paul Getty Trust" ;
            dcterms:license <https://opendatacommons.org/licenses/by/1-0/> ;
            dcterms:rights <https://rightsstatements.org/vocab/InC/1.0/> ;
            dcterms:source <http://www.getty.edu/research/tools/vocabularies/aat/> ],
        "Simple slip-on garments made with or without sleeves and usually knee-length or longer and belted at the waist; especially those worn by men and women of ancient Greece and Rome. Also, garments extending from the neckline to the waist or longer, usually high-necked and worn over other garments."@en ;
    dcterms:identifier "CC00126" ;
    owl:sameAs <http://vocab.getty.edu/aat/300209869> .

cc:CC00128 a owl:NamedIndividual ;
    rdfs:label "batwing sleeve"@en ;
    dcterms:description [ rdfs:label "A long sleeve with a deep armhole, tapering towards the wrist. Also known as a \"magyar\" sleeve."@en ;
            dcterms:creator "Wikidata contributors" ;
            dcterms:license <https://creativecommons.org/publicdomain/mark/1.0/> ;
            dcterms:rights <https://creativecommons.org/publicdomain/mark/1.0/> ;
            dcterms:source <https://www.wikidata.org/wiki/Wikidata:Data_access/en> ],
        "A long sleeve with a deep armhole, tapering towards the wrist. Also known as a \"magyar\" sleeve."@en ;
    dcterms:identifier "CC00128" ;
    owl:sameAs <http://www.wikidata.org/entity/Q29125416> .

cc:CC00129 a owl:NamedIndividual ;
    rdfs:label "bell skirt"@en ;
    dcterms:description [ rdfs:label "flared noticeably from the waist but then, unlike a church bell, cylindrical for much of its length"@en ;
            dcterms:creator "Wikidata contributors" ;
            dcterms:license <https://creativecommons.org/publicdomain/mark/1.0/> ;
            dcterms:rights <https://creativecommons.org/publicdomain/mark/1.0/> ;
            dcterms:source <https://en.wikipedia.org/wiki/Skirt> ],
        "flared noticeably from the waist but then, unlike a church bell, cylindrical for much of its length"@en ;
    dcterms:identifier "CC00129" ;
    owl:sameAs <http://www.wikidata.org/entity/Q83333837> .

cc:CC00130 a owl:NamedIndividual ;
    rdfs:label "bishop sleeve"@en ;
    dcterms:description [ rdfs:label "A long sleeve, fuller at the bottom than the top, and gathered into a cuff"@en ;
            dcterms:creator "Wikidata contributors" ;
            dcterms:license <https://creativecommons.org/publicdomain/mark/1.0/> ;
            dcterms:rights <https://creativecommons.org/publicdomain/mark/1.0/> ;
            dcterms:source <https://www.wikidata.org/wiki/Wikidata:Data_access/en> ],
        "A long sleeve, fuller at the bottom than the top, and gathered into a cuff"@en ;
    dcterms:identifier "CC00130" ;
    owl:sameAs <http://www.wikidata.org/entity/Q73514132> .

cc:CC00135 a owl:NamedIndividual ;
    rdfs:label "leg-of-mutton sleeve"@en ;
    dcterms:description [ rdfs:label "A sleeve that is extremely wide over the upper arm and narrow from the elbow to the wrist."@en ;
            dcterms:creator "Wikidata contributors" ;
            dcterms:license <https://creativecommons.org/publicdomain/mark/1.0/> ;
            dcterms:rights <https://creativecommons.org/publicdomain/mark/1.0/> ;
            dcterms:source <https://www.wikidata.org/wiki/Wikidata:Data_access/en> ],
        "A sleeve that is extremely wide over the upper arm and narrow from the elbow to the wrist."@en ;
    dcterms:identifier "CC00135" ;
    owl:sameAs <http://www.wikidata.org/entity/Q20732506> .

cc:CC00137 a owl:NamedIndividual ;
    rdfs:label "puff sleeve"@en ;
    dcterms:description [ rdfs:label "Any sleeve gathered (and sometimes stiffened) so that it puffs out, especially at the shoulder."@en ;
            dcterms:creator "Wikidata contributors" ;
            dcterms:license <https://creativecommons.org/publicdomain/mark/1.0/> ;
            dcterms:rights <https://creativecommons.org/publicdomain/mark/1.0/> ;
            dcterms:source <https://www.wikidata.org/wiki/Wikidata:Data_access/en> ],
        "Any sleeve gathered (and sometimes stiffened) so that it puffs out, especially at the shoulder."@en ;
    dcterms:identifier "CC00137" ;
    owl:sameAs <http://www.wikidata.org/entity/Q2117537> .

cc:CC00138 a owl:NamedIndividual ;
    rdfs:label "raglan sleeve"@en ;
    dcterms:description [ rdfs:label "Sleeve that extends to the neckline with diagonal seams from neck to underarm front and back."@en ;
            dcterms:creator "Wikidata contributors" ;
            dcterms:license <https://creativecommons.org/publicdomain/mark/1.0/> ;
            dcterms:rights <https://creativecommons.org/publicdomain/mark/1.0/> ;
            dcterms:source <https://www.wikidata.org/wiki/Wikidata:Data_access/en> ],
        "Sleeve that extends to the neckline with diagonal seams from neck to underarm front and back."@en ;
    dcterms:identifier "CC00138" ;
    owl:sameAs <http://www.wikidata.org/entity/Q1333132> .

cc:CC00145 a owl:NamedIndividual ;
    rdfs:label "short sleeve"@en ;
    dcterms:description [ rdfs:label "Sleeve ending above the elbow."@en ;
            dcterms:creator "Wikidata contributors" ;
            dcterms:license <https://creativecommons.org/publicdomain/mark/1.0/> ;
            dcterms:rights <https://creativecommons.org/publicdomain/mark/1.0/> ;
            dcterms:source <https://www.wikidata.org/wiki/Wikidata:Data_access/en> ],
        "Sleeve ending above the elbow."@en ;
    dcterms:identifier "CC00145" ;
    owl:sameAs <http://www.wikidata.org/entity/Q29126275> .

cc:CC00146 a owl:NamedIndividual ;
    rdfs:label "elbow-length sleeve"@en ;
    dcterms:description [ rdfs:label "Sleeve ending at or near the elbow."@en ;
            dcterms:creator "Wikidata contributors" ;
            dcterms:license <https://creativecommons.org/publicdomain/mark/1.0/> ;
            dcterms:rights <https://creativecommons.org/publicdomain/mark/1.0/> ;
            dcterms:source <https://www.wikidata.org/wiki/Wikidata:Data_access/en> ],
        "Sleeve ending at or near the elbow."@en ;
    dcterms:identifier "CC00146" ;
    owl:sameAs <http://www.wikidata.org/entity/Q73545207> .

cc:CC00147 a owl:NamedIndividual ;
    rdfs:label "three quarter sleeve"@en ;
    dcterms:description [ rdfs:label "Sleeve reaching from the shoulder to the middle of the forearm."@en ;
            dcterms:creator "Wikidata contributors" ;
            dcterms:license <https://creativecommons.org/publicdomain/mark/1.0/> ;
            dcterms:rights <https://creativecommons.org/publicdomain/mark/1.0/> ;
            dcterms:source <https://www.wikidata.org/wiki/Wikidata:Data_access/en> ],
        "Sleeve reaching from the shoulder to the middle of the forearm."@en ;
    dcterms:identifier "CC00147" ;
    owl:sameAs <http://www.wikidata.org/entity/Q29126653> .

cc:CC00148 a owl:NamedIndividual ;
    rdfs:label "long sleeve"@en ;
    dcterms:description [ rdfs:label "Sleeve reaching from the shoulder to the wrist."@en ;
            dcterms:creator "Wikidata contributors" ;
            dcterms:license <https://creativecommons.org/publicdomain/mark/1.0/> ;
            dcterms:rights <https://creativecommons.org/publicdomain/mark/1.0/> ;
            dcterms:source <https://www.wikidata.org/wiki/Wikidata:Data_access/en> ],
        "Sleeve reaching from the shoulder to the wrist."@en ;
    dcterms:identifier "CC00148" ;
    owl:sameAs <http://www.wikidata.org/entity/Q29125938> .

cc:CC00156 a owl:NamedIndividual ;
    rdfs:label "curved"@en ;
    dcterms:description [ rdfs:label "Shapes that are bent or formed into a curve, which is a line deviating from the straight or plane form continuously, without angles."@en ;
            dcterms:creator "The J. Paul Getty Trust" ;
            dcterms:license <https://opendatacommons.org/licenses/by/1-0/> ;
            dcterms:rights <https://rightsstatements.org/vocab/InC/1.0/> ;
            dcterms:source <http://www.getty.edu/research/tools/vocabularies/aat/> ],
        "Shapes that are bent or formed into a curve, which is a line deviating from the straight or plane form continuously, without angles."@en ;
    dcterms:identifier "CC00156" ;
    owl:sameAs <http://vocab.getty.edu/aat/300010305> .

cc:CC00160 a owl:NamedIndividual ;
    rdfs:label "natural fiber"@en ;
    dcterms:identifier "CC00160" .

cc:CC00162 a owl:NamedIndividual ;
    rdfs:label "pointed"@en ;
    dcterms:description [ rdfs:label "Having a form or outline delimited on at least one end by two intersecting lines, that is, tapering to or ending in a point or apex."@en ;
            dcterms:creator "The J. Paul Getty Trust" ;
            dcterms:license <https://opendatacommons.org/licenses/by/1-0/> ;
            dcterms:rights <https://rightsstatements.org/vocab/InC/1.0/> ;
            dcterms:source <http://www.getty.edu/research/tools/vocabularies/aat/> ],
        "Having a form or outline delimited on at least one end by two intersecting lines, that is, tapering to or ending in a point or apex."@en ;
    dcterms:identifier "CC00162" ;
    owl:sameAs <http://vocab.getty.edu/aat/300078755> .

cc:CC00164 a owl:NamedIndividual ;
    rdfs:label "balloon skirt"@en ;
    dcterms:description [ rdfs:label "a voluminous skirt whose hem is tucked back under to create a balloon or bubble effect at the bottom."@en ;
            dcterms:creator "Wikidata contributors" ;
            dcterms:license <https://creativecommons.org/publicdomain/mark/1.0/> ;
            dcterms:rights <https://creativecommons.org/publicdomain/mark/1.0/> ;
            dcterms:source <https://en.wikipedia.org/wiki/Skirt> ],
        "a voluminous skirt whose hem is tucked back under to create a balloon or bubble effect at the bottom."@en ;
    dcterms:identifier "CC00164" ;
    owl:sameAs <http://www.wikidata.org/entity/Q83333769> .

cc:CC00166 a owl:NamedIndividual ;
    rdfs:label "circle skirt"@en ;
    dcterms:description [ rdfs:label "a skirt cut in sections to make one or more circles with a hole for the waist, so the skirt is very full but hangs smoothly from the waist without darts, pleats, or gathers"@en ;
            dcterms:creator "Wikidata contributors" ;
            dcterms:license <https://creativecommons.org/publicdomain/mark/1.0/> ;
            dcterms:rights <https://creativecommons.org/publicdomain/mark/1.0/> ;
            dcterms:source <https://en.wikipedia.org/wiki/Skirt> ],
        "a skirt cut in sections to make one or more circles with a hole for the waist, so the skirt is very full but hangs smoothly from the waist without darts, pleats, or gathers"@en ;
    dcterms:identifier "CC00166" ;
    owl:sameAs <http://www.wikidata.org/entity/Q83333946> .

cc:CC00167 a owl:NamedIndividual ;
    rdfs:label "dirndl skirt"@en ;
    dcterms:description [ rdfs:label "Fulls skirts gathered or pleated on a tight waistband.  Also, similar parts of dresses."@en ;
            dcterms:creator "The J. Paul Getty Trust" ;
            dcterms:license <https://opendatacommons.org/licenses/by/1-0/> ;
            dcterms:rights <https://rightsstatements.org/vocab/InC/1.0/> ;
            dcterms:source <http://www.getty.edu/research/tools/vocabularies/aat/> ],
        "Fulls skirts gathered or pleated on a tight waistband.  Also, similar parts of dresses."@en ;
    dcterms:identifier "CC00167" ;
    owl:sameAs <http://vocab.getty.edu/aat/300209912> .

cc:CC00168 a owl:NamedIndividual ;
    rdfs:label "flared skirt"@en ;
    dcterms:description [ rdfs:label "A skirt cut to be wider at the hem than at the waistline."@en ;
            dcterms:creator "Wikidata contributors" ;
            dcterms:license <https://creativecommons.org/publicdomain/mark/1.0/> ;
            dcterms:rights <https://creativecommons.org/publicdomain/mark/1.0/> ;
            dcterms:source <https://www.wikidata.org/wiki/Wikidata:Data_access/en> ],
        "A skirt cut to be wider at the hem than at the waistline."@en ;
    dcterms:identifier "CC00168" ;
    owl:sameAs <http://www.wikidata.org/entity/Q83333994> .

cc:CC00170 a owl:NamedIndividual ;
    rdfs:label "gathering"@en ;
    dcterms:description [ rdfs:label "Bunching folds of textile together by pulling on a thread stitched through it for this purpose or on one or more of its constituent filaments, to create fullness."@en ;
            dcterms:creator "The J. Paul Getty Trust" ;
            dcterms:license <https://opendatacommons.org/licenses/by/1-0/> ;
            dcterms:rights <https://rightsstatements.org/vocab/InC/1.0/> ;
            dcterms:source <http://www.getty.edu/research/tools/vocabularies/aat/> ],
        "Bunching folds of textile together by pulling on a thread stitched through it for this purpose or on one or more of its constituent filaments, to create fullness."@en ;
    dcterms:identifier "CC00170" ;
    owl:sameAs <http://vocab.getty.edu/aat/300231237> .

cc:CC00171 a owl:NamedIndividual ;
    rdfs:label "gored skirt"@en ;
    dcterms:description [ rdfs:label "A skirt cut in pieces that are triangular or wedge-shaped so that there is more fullness at the hem than at the waist."@en ;
            dcterms:creator "Wikidata contributors" ;
            dcterms:license <https://creativecommons.org/publicdomain/mark/1.0/> ;
            dcterms:rights <https://creativecommons.org/publicdomain/mark/1.0/> ;
            dcterms:source <https://www.wikidata.org/wiki/Wikidata:Data_access/en> ],
        "A skirt cut in pieces that are triangular or wedge-shaped so that there is more fullness at the hem than at the waist."@en ;
    dcterms:identifier "CC00171" ;
    owl:sameAs <http://www.wikidata.org/entity/Q83334145> .

cc:CC00173 a owl:NamedIndividual ;
    rdfs:label "layering"@en ;
    dcterms:description [ rdfs:label "Forming or arranging in layers."@en ;
            dcterms:creator "The J. Paul Getty Trust" ;
            dcterms:license <https://opendatacommons.org/licenses/by/1-0/> ;
            dcterms:rights <https://rightsstatements.org/vocab/InC/1.0/> ;
            dcterms:source <http://www.getty.edu/research/tools/vocabularies/aat/> ],
        "Forming or arranging in layers."@en ;
    dcterms:identifier "CC00173" ;
    owl:sameAs <http://vocab.getty.edu/aat/300123034> .

cc:CC00175 a owl:NamedIndividual ;
    rdfs:label "pegged skirt"@en ;
    dcterms:description [ rdfs:label "A skirt shaped with fullness at the waistline but no fullness at the hemline."@en ;
            dcterms:creator "Wikidata contributors" ;
            dcterms:license <https://creativecommons.org/publicdomain/mark/1.0/> ;
            dcterms:rights <https://creativecommons.org/publicdomain/mark/1.0/> ;
            dcterms:source <https://www.wikidata.org/wiki/Wikidata:Data_access/en> ],
        "A skirt shaped with fullness at the waistline but no fullness at the hemline."@en ;
    dcterms:identifier "CC00175" ;
    owl:sameAs <http://www.wikidata.org/entity/Q83332399> .

cc:CC00176 a owl:NamedIndividual ;
    rdfs:label "peplum"@en ;
    dcterms:description [ rdfs:label "Short, skirtlike sections of a costume attached at the waistline, such as on a bodice or jacket, and usually extending to cover the hips."@en ;
            dcterms:creator "The J. Paul Getty Trust" ;
            dcterms:license <https://opendatacommons.org/licenses/by/1-0/> ;
            dcterms:rights <https://rightsstatements.org/vocab/InC/1.0/> ;
            dcterms:source <http://www.getty.edu/research/tools/vocabularies/aat/> ],
        "Short, skirtlike sections of a costume attached at the waistline, such as on a bodice or jacket, and usually extending to cover the hips."@en ;
    dcterms:identifier "CC00176" ;
    owl:sameAs <http://vocab.getty.edu/aat/300248709> .

cc:CC00177 a owl:NamedIndividual ;
    rdfs:label "pleated skirt"@en ;
    dcterms:description [ rdfs:label "a skirt with fullness reduced to fit the waist by means of regular pleats ('plaits') or folds, which can be stitched flat to hip-level or free-hanging"@en ;
            dcterms:creator "Wikidata contributors" ;
            dcterms:license <https://creativecommons.org/publicdomain/mark/1.0/> ;
            dcterms:rights <https://creativecommons.org/publicdomain/mark/1.0/> ;
            dcterms:source <https://www.wikidata.org/wiki/Wikidata:Data_access/en> ],
        "a skirt with fullness reduced to fit the waist by means of regular pleats ('plaits') or folds, which can be stitched flat to hip-level or free-hanging"@en ;
    dcterms:identifier "CC00177" ;
    owl:sameAs <http://www.wikidata.org/entity/Q18121766> .

cc:CC00179 a owl:NamedIndividual ;
    rdfs:label "sarong"@en ;
    dcterms:description [ rdfs:label "Main garments formed by wrapping a strip of cloth around the lower part of the body. Worn chiefly by men and women of the Malay Archipelago and the Pacific Islands. Also, similar often preformed garments worn by Western women."@en ;
            dcterms:creator "The J. Paul Getty Trust" ;
            dcterms:license <https://opendatacommons.org/licenses/by/1-0/> ;
            dcterms:rights <https://rightsstatements.org/vocab/InC/1.0/> ;
            dcterms:source <http://www.getty.edu/research/tools/vocabularies/aat/> ],
        "Main garments formed by wrapping a strip of cloth around the lower part of the body. Worn chiefly by men and women of the Malay Archipelago and the Pacific Islands. Also, similar often preformed garments worn by Western women."@en ;
    dcterms:identifier "CC00179" ;
    owl:sameAs <http://vocab.getty.edu/aat/300209928> .

cc:CC00180 a owl:NamedIndividual ;
    rdfs:label "pencil skirt"@en ;
    dcterms:description [ rdfs:label "Close-fitting straight-cut skirts, usually with the hemline at or below the knee."@en ;
            dcterms:creator "The J. Paul Getty Trust" ;
            dcterms:license <https://opendatacommons.org/licenses/by/1-0/> ;
            dcterms:rights <https://rightsstatements.org/vocab/InC/1.0/> ;
            dcterms:source <http://www.getty.edu/research/tools/vocabularies/aat/> ],
        "Close-fitting straight-cut skirts, usually with the hemline at or below the knee."@en ;
    dcterms:identifier "CC00180" ;
    owl:sameAs <http://vocab.getty.edu/aat/300411738> .

cc:CC00182 a owl:NamedIndividual ;
    rdfs:label "tiered skirt"@en ;
    dcterms:description [ rdfs:label "made of several horizontal layers, each wider than the one above, and divided by stitching. Layers may look identical in solid-colored garments, or may differ when made of printed fabrics."@en ;
            dcterms:creator "Wikidata contributors" ;
            dcterms:license <https://creativecommons.org/publicdomain/mark/1.0/> ;
            dcterms:rights <https://creativecommons.org/publicdomain/mark/1.0/> ;
            dcterms:source <https://www.wikidata.org/wiki/Wikidata:Data_access/en> ],
        "made of several horizontal layers, each wider than the one above, and divided by stitching. Layers may look identical in solid-colored garments, or may differ when made of printed fabrics."@en ;
    dcterms:identifier "CC00182" ;
    owl:sameAs <http://www.wikidata.org/entity/Q83334198> .

cc:CC00183 a owl:NamedIndividual ;
    rdfs:label "trumpet skirt"@en ;
    dcterms:description [ rdfs:label "A straight skirt with a hem flounce that flares away from the body at the hem."@en ;
            dcterms:creator "Wikidata contributors" ;
            dcterms:license <https://creativecommons.org/publicdomain/mark/1.0/> ;
            dcterms:rights <https://creativecommons.org/publicdomain/mark/1.0/> ;
            dcterms:source <https://en.wikipedia.org/wiki/Contemporary_Western_wedding_dress> ],
        "A straight skirt with a hem flounce that flares away from the body at the hem."@en ;
    dcterms:identifier "CC00183" ;
    owl:sameAs <http://www.wikidata.org/entity/Q83332911> .

cc:CC00184 a owl:NamedIndividual ;
    rdfs:label "yoke"@en ;
    dcterms:description [ rdfs:label "fitted costume component for the upper hips or shoulders"@en ;
            dcterms:creator "Wikidata contributors" ;
            dcterms:license <https://creativecommons.org/publicdomain/mark/1.0/> ;
            dcterms:rights <https://creativecommons.org/publicdomain/mark/1.0/> ;
            dcterms:source <https://www.wikidata.org/wiki/Wikidata:Data_access/en> ],
        "fitted costume component for the upper hips or shoulders"@en ;
    dcterms:identifier "CC00184" ;
    owl:sameAs <http://www.wikidata.org/entity/Q8054544> .

cc:CC00194 a owl:NamedIndividual ;
    rdfs:label "train"@en ;
    dcterms:description [ rdfs:label "Extended parts of a skirt, gown, or state robe that lie on the floor and trail behind the wearer, either separate or attached. (AAT)"@en ;
            dcterms:creator "The J. Paul Getty Trust" ;
            dcterms:license <https://opendatacommons.org/licenses/by/1-0/> ;
            dcterms:rights <https://rightsstatements.org/vocab/InC/1.0/> ;
            dcterms:source <http://www.getty.edu/research/tools/vocabularies/aat/> ],
        "Extended parts of a skirt, gown, or state robe that lie on the floor and trail behind the wearer, either separate or attached. (AAT)"@en ;
    dcterms:identifier "CC00194" ;
    owl:sameAs <http://vocab.getty.edu/aat/300224243> .

cc:CC00213 a owl:NamedIndividual ;
    rdfs:label "fiber blend"@en ;
    dcterms:identifier "CC00213" .

cc:CC00218 a owl:NamedIndividual ;
    rdfs:label "knit"@en ;
    dcterms:identifier "CC00218" .

cc:CC00222 a owl:NamedIndividual ;
    rdfs:label "looped pile"@en ;
    dcterms:identifier "CC00222" .

cc:CC00225 a owl:NamedIndividual ;
    rdfs:label "microfiber"@en ;
    dcterms:identifier "CC00225" .

cc:CC00236 a owl:NamedIndividual ;
    rdfs:label "rib knit"@en ;
    dcterms:identifier "CC00236" .

cc:CC00251 a owl:NamedIndividual ;
    rdfs:label "bustle skirt"@en ;
    dcterms:description [ rdfs:label "A skirt shaped with much more fullness in the back than in the front, accomodating a bustle pad or petticoat for added fullness underneath"@en ;
            dcterms:creator "Wikidata contributors" ;
            dcterms:license <https://creativecommons.org/publicdomain/mark/1.0/> ;
            dcterms:rights <https://creativecommons.org/publicdomain/mark/1.0/> ;
            dcterms:source <https://www.wikidata.org/wiki/Wikidata:Data_access/en> ],
        "A skirt shaped with much more fullness in the back than in the front, accomodating a bustle pad or petticoat for added fullness underneath"@en ;
    dcterms:identifier "CC00251" ;
    owl:sameAs <http://www.wikidata.org/entity/Q83333892> .

cc:CC00254 a owl:NamedIndividual ;
    rdfs:label "embroidering"@en ;
    dcterms:description [ rdfs:label "Refers to the process in which a needle and thread or fine wire are used to stitch decorative designs into cloth, leather, paper, or other material. It may also refer to the process used to create machine-made imitations of hand-made embroidery. For the weft patterning technique of weaving raised patterns on a woven textile, use \"brocading.\""@en ;
            dcterms:creator "The J. Paul Getty Trust" ;
            dcterms:license <https://opendatacommons.org/licenses/by/1-0/> ;
            dcterms:rights <https://rightsstatements.org/vocab/InC/1.0/> ;
            dcterms:source <http://www.getty.edu/research/tools/vocabularies/aat/> ],
        "Refers to the process in which a needle and thread or fine wire are used to stitch decorative designs into cloth, leather, paper, or other material. It may also refer to the process used to create machine-made imitations of hand-made embroidery. For the weft patterning technique of weaving raised patterns on a woven textile, use \"brocading.\""@en ;
    dcterms:identifier "CC00254" ;
    owl:sameAs <http://vocab.getty.edu/aat/300053653> .

cc:CC00255 a owl:NamedIndividual ;
    rdfs:label "handkerchief skirt"@en ;
    dcterms:description [ rdfs:label "Skirt with an asymmetric hem, resembling a handkerchief that is held by the centre so that its corners hang down as points."@en ;
            dcterms:creator "Wikidata contributors" ;
            dcterms:license <https://creativecommons.org/publicdomain/mark/1.0/> ;
            dcterms:rights <https://creativecommons.org/publicdomain/mark/1.0/> ;
            dcterms:source <https://www.wikidata.org/wiki/Wikidata:Data_access/en> ],
        "Skirt with an asymmetric hem, resembling a handkerchief that is held by the centre so that its corners hang down as points."@en ;
    dcterms:identifier "CC00255" ;
    owl:sameAs <http://www.wikidata.org/entity/Q5647451> .

cc:CC00256 a owl:NamedIndividual ;
    rdfs:label "kimono sleeve"@en ;
    dcterms:description [ rdfs:label "A sleeve cut in one with the bodice in a wide sloping shape, similar to that on traditional Chinese robes (not Japanese kimono whose sleeves are sewn separately)."@en ;
            dcterms:creator "Wikidata contributors" ;
            dcterms:license <https://creativecommons.org/publicdomain/mark/1.0/> ;
            dcterms:rights <https://creativecommons.org/publicdomain/mark/1.0/> ;
            dcterms:source <https://www.wikidata.org/wiki/Wikidata:Data_access/en> ],
        "A sleeve cut in one with the bodice in a wide sloping shape, similar to that on traditional Chinese robes (not Japanese kimono whose sleeves are sewn separately)."@en ;
    dcterms:identifier "CC00256" ;
    owl:sameAs <http://www.wikidata.org/entity/Q24016353> .

cc:CC00257 a owl:NamedIndividual ;
    rdfs:label "needlepoint"@en ;
    dcterms:description [ rdfs:label "Refers to the process of creating works with a needle and thread on fabric or a mesh of canvas, using the grid of the fabric to count out the desired position of varoius stitches or colors in the design."@en ;
            dcterms:creator "The J. Paul Getty Trust" ;
            dcterms:license <https://opendatacommons.org/licenses/by/1-0/> ;
            dcterms:rights <https://rightsstatements.org/vocab/InC/1.0/> ;
            dcterms:source <http://www.getty.edu/research/tools/vocabularies/aat/> ],
        "Refers to the process of creating works with a needle and thread on fabric or a mesh of canvas, using the grid of the fabric to count out the desired position of varoius stitches or colors in the design."@en ;
    dcterms:identifier "CC00257" ;
    owl:sameAs <http://vocab.getty.edu/aat/300061985> .

cc:CC00258 a owl:NamedIndividual ;
    rdfs:label "shawl collar"@en ;
    dcterms:description [ rdfs:label "soft, rounded collar of unbroken outline, usually following a surplice neckline, common on coats and some tuxedo jackets"@en ;
            dcterms:creator "Wikidata contributors" ;
            dcterms:license <https://creativecommons.org/publicdomain/mark/1.0/> ;
            dcterms:rights <https://creativecommons.org/publicdomain/mark/1.0/> ;
            dcterms:source <https://www.wikidata.org/wiki/Wikidata:Data_access/en> ],
        "soft, rounded collar of unbroken outline, usually following a surplice neckline, common on coats and some tuxedo jackets"@en ;
    dcterms:identifier "CC00258" ;
    owl:sameAs <http://www.wikidata.org/entity/Q29473093> .

cc:CC00277 a owl:NamedIndividual ;
    rdfs:label "floral patterns"@en ;
    dcterms:description [ rdfs:label "Patterns of or pertaining to flowers."@en ;
            dcterms:creator "The J. Paul Getty Trust" ;
            dcterms:license <https://opendatacommons.org/licenses/by/1-0/> ;
            dcterms:rights <https://rightsstatements.org/vocab/InC/1.0/> ;
            dcterms:source <http://www.getty.edu/research/tools/vocabularies/aat/> ],
        "Patterns of or pertaining to flowers."@en ;
    dcterms:identifier "CC00277" ;
    owl:sameAs <http://vocab.getty.edu/aat/300010135> .

cc:CC00287 a owl:NamedIndividual ;
    rdfs:label "lining"@en ;
    dcterms:description [ rdfs:label "Layer of material used to line the inner side or surface of something to reinforce or protect it."@en ;
            dcterms:creator "The J. Paul Getty Trust" ;
            dcterms:license <https://opendatacommons.org/licenses/by/1-0/> ;
            dcterms:rights <https://rightsstatements.org/vocab/InC/1.0/> ;
            dcterms:source <http://www.getty.edu/research/tools/vocabularies/aat/> ],
        "Layer of material used to line the inner side or surface of something to reinforce or protect it."@en ;
    dcterms:identifier "CC00287" ;
    owl:sameAs <http://vocab.getty.edu/aat/300227846> .

cc:CC00300 a owl:NamedIndividual ;
    rdfs:label "plaid (pattern)"@en ;
    dcterms:description [ rdfs:label "The characteristic pattern known from plaid textiles, consisting of bars or stripes of various colors crossing each other at right angles over a contrasting background color, whether or not the pattern exists on a textile or another material. Plaid patterns were known from ancient times in many cultures."@en ;
            dcterms:creator "The J. Paul Getty Trust" ;
            dcterms:license <https://opendatacommons.org/licenses/by/1-0/> ;
            dcterms:rights <https://rightsstatements.org/vocab/InC/1.0/> ;
            dcterms:source <http://www.getty.edu/research/tools/vocabularies/aat/> ],
        "The characteristic pattern known from plaid textiles, consisting of bars or stripes of various colors crossing each other at right angles over a contrasting background color, whether or not the pattern exists on a textile or another material. Plaid patterns were known from ancient times in many cultures."@en ;
    dcterms:identifier "CC00300" ;
    owl:sameAs <http://vocab.getty.edu/aat/300411863> .

cc:CC00314 a owl:NamedIndividual ;
    rdfs:label "trimming"@en ;
    dcterms:description [ rdfs:label "Collectively used for decorative or additional material serving to finish, decorate, or complete."@en ;
            dcterms:creator "The J. Paul Getty Trust" ;
            dcterms:license <https://opendatacommons.org/licenses/by/1-0/> ;
            dcterms:rights <https://rightsstatements.org/vocab/InC/1.0/> ;
            dcterms:source <http://www.getty.edu/research/tools/vocabularies/aat/> ],
        "Collectively used for decorative or additional material serving to finish, decorate, or complete."@en ;
    dcterms:identifier "CC00314" ;
    owl:sameAs <http://vocab.getty.edu/aat/300183798> .

cc:CC00317 a owl:NamedIndividual ;
    rdfs:label "twill tape"@en ;
    dcterms:identifier "CC00317" .

cc:CC00325 a owl:NamedIndividual ;
    rdfs:label "tucks"@en ;
    dcterms:description [ rdfs:label "In sewing, a tuck is a fold or pleat in fabric that is sewn in place."@en ;
            dcterms:creator "Wikidata contributors" ;
            dcterms:license <https://creativecommons.org/publicdomain/mark/1.0/> ;
            dcterms:rights <https://creativecommons.org/publicdomain/mark/1.0/> ;
            dcterms:source <https://www.wikidata.org/wiki/Wikidata:Data_access/en> ],
        "In sewing, a tuck is a fold or pleat in fabric that is sewn in place."@en ;
    dcterms:identifier "CC00325" ;
    owl:sameAs <http://www.wikidata.org/entity/Q858090> .

cc:CC00326 a owl:NamedIndividual ;
    rdfs:label "sleeveless"@en ;
    dcterms:description [ rdfs:label "Having a finished armhole but no sleeves."@en ;
            dcterms:creator "Wikidata contributors" ;
            dcterms:license <https://creativecommons.org/publicdomain/mark/1.0/> ;
            dcterms:rights <https://creativecommons.org/publicdomain/mark/1.0/> ;
            dcterms:source <https://www.wikidata.org/wiki/Wikidata:Data_access/en> ],
        "Having a finished armhole but no sleeves."@en ;
    dcterms:identifier "CC00326" ;
    owl:sameAs <http://www.wikidata.org/entity/Q29741669> .

cc:CC00335 a owl:NamedIndividual ;
    rdfs:label "dress"@en ;
    dcterms:description [ rdfs:label "Main garments for women, children, or infants consisting of a bodice and skirt made in one or more pieces"@en ;
            dcterms:creator "The J. Paul Getty Trust" ;
            dcterms:license <https://opendatacommons.org/licenses/by/1-0/> ;
            dcterms:rights <https://rightsstatements.org/vocab/InC/1.0/> ;
            dcterms:source <http://www.getty.edu/research/tools/vocabularies/aat/> ],
        "Main garments for women, children, or infants consisting of a bodice and skirt made in one or more pieces"@en ;
    dcterms:identifier "CC00335" ;
    owl:sameAs <http://vocab.getty.edu/aat/300046159> .

cc:CC00339 a owl:NamedIndividual ;
    rdfs:label "jacket"@en ;
    dcterms:description [ rdfs:label "A short coat for the upper body made in various forms and lengths but usually no lower than the waist; worn separately or as part of a suit. Also, similar outer garments worn for warmth or protection from the weather."@en ;
            dcterms:creator "The J. Paul Getty Trust" ;
            dcterms:license <https://opendatacommons.org/licenses/by/1-0/> ;
            dcterms:rights <https://rightsstatements.org/vocab/InC/1.0/> ;
            dcterms:source <http://www.getty.edu/research/tools/vocabularies/aat/> ],
        "A short coat for the upper body made in various forms and lengths but usually no lower than the waist; worn separately or as part of a suit. Also, similar outer garments worn for warmth or protection from the weather."@en ;
    dcterms:identifier "CC00339" ;
    owl:sameAs <http://vocab.getty.edu/aat/300046167> .

cc:CC00341 a owl:NamedIndividual ;
    rdfs:label "skirt"@en ;
    dcterms:description [ rdfs:label "Main garments of varying length extending from the waist or hip and covering a part of the lower body. Also, the lower part of a dress, coat, or other garment."@en ;
            dcterms:creator "The J. Paul Getty Trust" ;
            dcterms:license <https://opendatacommons.org/licenses/by/1-0/> ;
            dcterms:rights <https://rightsstatements.org/vocab/InC/1.0/> ;
            dcterms:source <http://www.getty.edu/research/tools/vocabularies/aat/> ],
        "Main garments of varying length extending from the waist or hip and covering a part of the lower body. Also, the lower part of a dress, coat, or other garment."@en ;
    dcterms:identifier "CC00341" ;
    owl:sameAs <http://vocab.getty.edu/aat/300209932> .

cc:CC00342 a owl:NamedIndividual ;
    rdfs:label "suit"@en ;
    dcterms:description [ rdfs:label "Sets of two or more garments made to harmonize or match in color. Also, any costume designed to be worn for a special purpose or under particular conditions, such as a space suit or a snowsuit"@en ;
            dcterms:creator "The J. Paul Getty Trust" ;
            dcterms:license <https://opendatacommons.org/licenses/by/1-0/> ;
            dcterms:rights <https://rightsstatements.org/vocab/InC/1.0/> ;
            dcterms:source <http://www.getty.edu/research/tools/vocabularies/aat/> ],
        "Sets of two or more garments made to harmonize or match in color. Also, any costume designed to be worn for a special purpose or under particular conditions, such as a space suit or a snowsuit"@en ;
    dcterms:identifier "CC00342" ;
    owl:sameAs <http://vocab.getty.edu/aat/300209863> .

cc:CC00343 a owl:NamedIndividual ;
    rdfs:label "sweater"@en ;
    dcterms:description [ rdfs:label "Knitted or crocheted garments worn on the upper body which extend to the waist or below."@en ;
            dcterms:creator "The J. Paul Getty Trust" ;
            dcterms:license <https://opendatacommons.org/licenses/by/1-0/> ;
            dcterms:rights <https://rightsstatements.org/vocab/InC/1.0/> ;
            dcterms:source <http://www.getty.edu/research/tools/vocabularies/aat/> ],
        "Knitted or crocheted garments worn on the upper body which extend to the waist or below."@en ;
    dcterms:identifier "CC00343" ;
    owl:sameAs <http://vocab.getty.edu/aat/300209900> .

cc:CC00344 a owl:NamedIndividual ;
    rdfs:label "pants"@en ;
    dcterms:description [ rdfs:label "Exposed bifurcated garments which extend from waist or hips to the ankle or sometimes to the knee or just below."@en ;
            dcterms:creator "The J. Paul Getty Trust" ;
            dcterms:license <https://opendatacommons.org/licenses/by/1-0/> ;
            dcterms:rights <https://rightsstatements.org/vocab/InC/1.0/> ;
            dcterms:source <http://www.getty.edu/research/tools/vocabularies/aat/> ],
        "Exposed bifurcated garments which extend from waist or hips to the ankle or sometimes to the knee or just below."@en ;
    dcterms:identifier "CC00344" ;
    owl:sameAs <http://vocab.getty.edu/aat/300209935> .

cc:CC00346 a owl:NamedIndividual ;
    rdfs:label "vest"@en ;
    dcterms:description [ rdfs:label "Close-fitting main garments extending to the waist or just below. Sleeveless and usually collarless, and often having buttons or pockets. For close-fitting main garments extending below the waistline that are usually front-buttoning and may have sleeves, that are worn over a shirt and under a coat or jacket, use \"waistcoats.\""@en ;
            dcterms:creator "The J. Paul Getty Trust" ;
            dcterms:license <https://opendatacommons.org/licenses/by/1-0/> ;
            dcterms:rights <https://rightsstatements.org/vocab/InC/1.0/> ;
            dcterms:source <http://www.getty.edu/research/tools/vocabularies/aat/> ],
        "Close-fitting main garments extending to the waist or just below. Sleeveless and usually collarless, and often having buttons or pockets. For close-fitting main garments extending below the waistline that are usually front-buttoning and may have sleeves, that are worn over a shirt and under a coat or jacket, use \"waistcoats.\""@en ;
    dcterms:identifier "CC00346" ;
    owl:sameAs <http://vocab.getty.edu/aat/300209904> .

cc:CC00350 a owl:NamedIndividual ;
    rdfs:label "double-breasted"@en ;
    dcterms:description [ rdfs:label "Describes a garment for which a wide section in the front overlaps the other side and has two rows of fasteners."@en ;
            dcterms:creator "Wikidata contributors" ;
            dcterms:license <https://creativecommons.org/publicdomain/mark/1.0/> ;
            dcterms:rights <https://creativecommons.org/publicdomain/mark/1.0/> ;
            dcterms:source <https://www.wikidata.org/wiki/Wikidata:Data_access/en> ],
        "Describes a garment for which a wide section in the front overlaps the other side and has two rows of fasteners."@en ;
    dcterms:identifier "CC00350" ;
    owl:sameAs <http://www.wikidata.org/entity/Q3037506> .

cc:CC00355 a owl:NamedIndividual ;
    rdfs:label "one sleeve"@en ;
    dcterms:description [ rdfs:label "single sleeve as part of garment"@en ;
            dcterms:creator "Wikidata contributors" ;
            dcterms:license <https://creativecommons.org/publicdomain/mark/1.0/> ;
            dcterms:rights <https://creativecommons.org/publicdomain/mark/1.0/> ;
            dcterms:source <https://www.wikidata.org/wiki/Wikidata:Data_access/en> ],
        "single sleeve as part of garment"@en ;
    dcterms:identifier "CC00355" ;
    owl:sameAs <http://www.wikidata.org/entity/Q29655994> .

cc:CC00362 a owl:NamedIndividual ;
    rdfs:label "water sleeve"@en ;
    dcterms:description [ rdfs:label "traditional trailing sleeve of Chinese opera costume"@en ;
            dcterms:creator "Wikidata contributors" ;
            dcterms:license <https://creativecommons.org/publicdomain/mark/1.0/> ;
            dcterms:rights <https://creativecommons.org/publicdomain/mark/1.0/> ;
            dcterms:source <https://www.wikidata.org/wiki/Wikidata:Data_access/en> ],
        "traditional trailing sleeve of Chinese opera costume"@en ;
    dcterms:identifier "CC00362" ;
    owl:sameAs <http://www.wikidata.org/entity/Q766204> .

cc:CC00364 a owl:NamedIndividual ;
    rdfs:label "womenswear"@en ;
    dcterms:description [ rdfs:label "Clothing designed for or worn by women; often used in commercial contexts."@en ;
            dcterms:creator "The J. Paul Getty Trust" ;
            dcterms:license <https://opendatacommons.org/licenses/by/1-0/> ;
            dcterms:rights <https://rightsstatements.org/vocab/InC/1.0/> ;
            dcterms:source <http://www.getty.edu/research/tools/vocabularies/aat/> ],
        "Clothing designed for or worn by women; often used in commercial contexts."@en ;
    dcterms:identifier "CC00364" ;
    owl:sameAs <http://vocab.getty.edu/aat/300379344> .

cc:CC00365 a owl:NamedIndividual ;
    rdfs:label "menswear"@en ;
    dcterms:description [ rdfs:label "Clothing designed for or worn by men; often used in commercial contexts."@en ;
            dcterms:creator "The J. Paul Getty Trust" ;
            dcterms:license <https://opendatacommons.org/licenses/by/1-0/> ;
            dcterms:rights <https://rightsstatements.org/vocab/InC/1.0/> ;
            dcterms:source <http://www.getty.edu/research/tools/vocabularies/aat/> ],
        "Clothing designed for or worn by men; often used in commercial contexts."@en ;
    dcterms:identifier "CC00365" ;
    owl:sameAs <http://vocab.getty.edu/aat/300379341> .

cc:CC00366 a owl:NamedIndividual ;
    rdfs:label "unisex clothing"@en ;
    dcterms:description [ rdfs:label "General term for clothing designed for or suitable for either males or females."@en ;
            dcterms:creator "The J. Paul Getty Trust" ;
            dcterms:license <https://opendatacommons.org/licenses/by/1-0/> ;
            dcterms:rights <https://rightsstatements.org/vocab/InC/1.0/> ;
            dcterms:source <http://www.getty.edu/research/tools/vocabularies/aat/> ],
        "General term for clothing designed for or suitable for either males or females."@en ;
    dcterms:identifier "CC00366" ;
    owl:sameAs <http://vocab.getty.edu/aat/300411750> .

cc:CC00368 a owl:NamedIndividual ;
    rdfs:label "day wear"@en ;
    dcterms:description [ rdfs:label "Articles of clothing suitable for casual wear during the day, in contrast to formal wear suitable for evening events."@en ;
            dcterms:creator "The J. Paul Getty Trust" ;
            dcterms:license <https://opendatacommons.org/licenses/by/1-0/> ;
            dcterms:rights <https://rightsstatements.org/vocab/InC/1.0/> ;
            dcterms:source <http://www.getty.edu/research/tools/vocabularies/aat/> ],
        "Articles of clothing suitable for casual wear during the day, in contrast to formal wear suitable for evening events."@en ;
    dcterms:identifier "CC00368" ;
    owl:sameAs <http://vocab.getty.edu/aat/300403910> .

cc:CC00370 a owl:NamedIndividual ;
    rdfs:label "evening dress"@en ;
    dcterms:description [ rdfs:label "Manner of dressing required by custom or etiquette for formal or semiformal evening occasions."@en ;
            dcterms:creator "The J. Paul Getty Trust" ;
            dcterms:license <https://opendatacommons.org/licenses/by/1-0/> ;
            dcterms:rights <https://rightsstatements.org/vocab/InC/1.0/> ;
            dcterms:source <http://www.getty.edu/research/tools/vocabularies/aat/> ],
        "Manner of dressing required by custom or etiquette for formal or semiformal evening occasions."@en ;
    dcterms:identifier "CC00370" ;
    owl:sameAs <http://vocab.getty.edu/aat/300224227> .

cc:CC00372 a owl:NamedIndividual ;
    rdfs:label "military uniform"@en ;
    dcterms:description [ rdfs:label "Uniforms intended for those in the armed forces."@en ;
            dcterms:creator "The J. Paul Getty Trust" ;
            dcterms:license <https://opendatacommons.org/licenses/by/1-0/> ;
            dcterms:rights <https://rightsstatements.org/vocab/InC/1.0/> ;
            dcterms:source <http://www.getty.edu/research/tools/vocabularies/aat/> ],
        "Uniforms intended for those in the armed forces."@en ;
    dcterms:identifier "CC00372" ;
    owl:sameAs <http://vocab.getty.edu/aat/300248030> .

cc:CC00374 a owl:NamedIndividual ;
    rdfs:label "mourning dress"@en ;
    dcterms:description [ rdfs:label "Clothes or draperies customarily indicative of bereavement, often donned during a period designated for the conventional or ceremonial manifestation of sorrow."@en ;
            dcterms:creator "The J. Paul Getty Trust" ;
            dcterms:license <https://opendatacommons.org/licenses/by/1-0/> ;
            dcterms:rights <https://rightsstatements.org/vocab/InC/1.0/> ;
            dcterms:source <http://www.getty.edu/research/tools/vocabularies/aat/> ],
        "Clothes or draperies customarily indicative of bereavement, often donned during a period designated for the conventional or ceremonial manifestation of sorrow."@en ;
    dcterms:identifier "CC00374" ;
    owl:sameAs <http://vocab.getty.edu/aat/300375755> .

cc:CC00376 a owl:NamedIndividual ;
    rdfs:label "school uniform"@en ;
    dcterms:description [ rdfs:label "Uniforms for school children, which are often made mandatory. School uniform designs vary, but may consist of a jacket and a skirt or a pair of pants, a collared shirt and a type of neckwear. Originally these may have been inspired by formal wear, military, or marine uniforms."@en ;
            dcterms:creator "The J. Paul Getty Trust" ;
            dcterms:license <https://opendatacommons.org/licenses/by/1-0/> ;
            dcterms:rights <https://rightsstatements.org/vocab/InC/1.0/> ;
            dcterms:source <http://www.getty.edu/research/tools/vocabularies/aat/> ],
        "Uniforms for school children, which are often made mandatory. School uniform designs vary, but may consist of a jacket and a skirt or a pair of pants, a collared shirt and a type of neckwear. Originally these may have been inspired by formal wear, military, or marine uniforms."@en ;
    dcterms:identifier "CC00376" ;
    owl:sameAs <http://vocab.getty.edu/aat/300417888> .

cc:CC00378 a owl:NamedIndividual ;
    rdfs:label "uniform"@en ;
    dcterms:description [ rdfs:label "Identifying garments or styles of dress worn by the members of a given profession, organization, or rank."@en ;
            dcterms:creator "The J. Paul Getty Trust" ;
            dcterms:license <https://opendatacommons.org/licenses/by/1-0/> ;
            dcterms:rights <https://rightsstatements.org/vocab/InC/1.0/> ;
            dcterms:source <http://www.getty.edu/research/tools/vocabularies/aat/> ],
        "Identifying garments or styles of dress worn by the members of a given profession, organization, or rank."@en ;
    dcterms:identifier "CC00378" ;
    owl:sameAs <http://vocab.getty.edu/aat/300212393> .

cc:CC00379 a owl:NamedIndividual ;
    rdfs:label "wedding dress"@en ;
    dcterms:description [ rdfs:label "Dresses worn by brides during the wedding ceremony, in many styles and colors, often having a train."@en ;
            dcterms:creator "The J. Paul Getty Trust" ;
            dcterms:license <https://opendatacommons.org/licenses/by/1-0/> ;
            dcterms:rights <https://rightsstatements.org/vocab/InC/1.0/> ;
            dcterms:source <http://www.getty.edu/research/tools/vocabularies/aat/> ],
        "Dresses worn by brides during the wedding ceremony, in many styles and colors, often having a train."@en ;
    dcterms:identifier "CC00379" ;
    owl:sameAs <http://vocab.getty.edu/aat/300255177> .

cc:CC00380 a owl:NamedIndividual ;
    rdfs:label "work clothes"@en ;
    dcterms:description [ rdfs:label "Clothing designed for or worn while working, differing in style depending upon the job, such as manual labor, crafts, or office work."@en ;
            dcterms:creator "The J. Paul Getty Trust" ;
            dcterms:license <https://opendatacommons.org/licenses/by/1-0/> ;
            dcterms:rights <https://rightsstatements.org/vocab/InC/1.0/> ;
            dcterms:source <http://www.getty.edu/research/tools/vocabularies/aat/> ],
        "Clothing designed for or worn while working, differing in style depending upon the job, such as manual labor, crafts, or office work."@en ;
    dcterms:identifier "CC00380" ;
    owl:sameAs <http://vocab.getty.edu/aat/300411756> .

cc:CC00382 a owl:NamedIndividual ;
    rdfs:label "childhood"@en ;
    dcterms:description [ rdfs:label "The earliest developmental stage of a living being."@en ;
            dcterms:creator "The J. Paul Getty Trust" ;
            dcterms:license <https://opendatacommons.org/licenses/by/1-0/> ;
            dcterms:rights <https://rightsstatements.org/vocab/InC/1.0/> ;
            dcterms:source <http://www.getty.edu/research/tools/vocabularies/aat/> ],
        "The earliest developmental stage of a living being."@en ;
    dcterms:identifier "CC00382" ;
    owl:sameAs <http://vocab.getty.edu/aat/300189588> .

cc:CC00383 a owl:NamedIndividual ;
    rdfs:label "infancy"@en ;
    dcterms:description [ rdfs:label "Stage of early childhood, commonly considered to be the period before being able to walk."@en ;
            dcterms:creator "The J. Paul Getty Trust" ;
            dcterms:license <https://opendatacommons.org/licenses/by/1-0/> ;
            dcterms:rights <https://rightsstatements.org/vocab/InC/1.0/> ;
            dcterms:source <http://www.getty.edu/research/tools/vocabularies/aat/> ],
        "Stage of early childhood, commonly considered to be the period before being able to walk."@en ;
    dcterms:identifier "CC00383" ;
    owl:sameAs <http://vocab.getty.edu/aat/300189590> .

cc:CC00384 a owl:NamedIndividual ;
    rdfs:label "adolescence"@en ;
    dcterms:description [ rdfs:label "Transitional stage between childhood and adulthood in the physical and emotional development of a living being; in humans, it extends mainly over the teen years and terminates legally when the official age of majority is reached."@en ;
            dcterms:creator "The J. Paul Getty Trust" ;
            dcterms:license <https://opendatacommons.org/licenses/by/1-0/> ;
            dcterms:rights <https://rightsstatements.org/vocab/InC/1.0/> ;
            dcterms:source <http://www.getty.edu/research/tools/vocabularies/aat/> ],
        "Transitional stage between childhood and adulthood in the physical and emotional development of a living being; in humans, it extends mainly over the teen years and terminates legally when the official age of majority is reached."@en ;
    dcterms:identifier "CC00384" ;
    owl:sameAs <http://vocab.getty.edu/aat/300189595> .

cc:CC00385 a owl:NamedIndividual ;
    rdfs:label "adulthood"@en ;
    dcterms:description [ rdfs:label "Stage at which a living being is fully grown or developed."@en ;
            dcterms:creator "The J. Paul Getty Trust" ;
            dcterms:license <https://opendatacommons.org/licenses/by/1-0/> ;
            dcterms:rights <https://rightsstatements.org/vocab/InC/1.0/> ;
            dcterms:source <http://www.getty.edu/research/tools/vocabularies/aat/> ],
        "Stage at which a living being is fully grown or developed."@en ;
    dcterms:identifier "CC00385" ;
    owl:sameAs <http://vocab.getty.edu/aat/300189598> .

cc:CC00386 a owl:NamedIndividual ;
    rdfs:label "middle age"@en ;
    dcterms:description [ rdfs:label "Stage of adult life between young adulthood and old age; in humans, commonly defined as extending from 45 to 65."@en ;
            dcterms:creator "The J. Paul Getty Trust" ;
            dcterms:license <https://opendatacommons.org/licenses/by/1-0/> ;
            dcterms:rights <https://rightsstatements.org/vocab/InC/1.0/> ;
            dcterms:source <http://www.getty.edu/research/tools/vocabularies/aat/> ],
        "Stage of adult life between young adulthood and old age; in humans, commonly defined as extending from 45 to 65."@en ;
    dcterms:identifier "CC00386" ;
    owl:sameAs <http://vocab.getty.edu/aat/300189599> .

cc:CC00387 a owl:NamedIndividual ;
    rdfs:label "old age"@en ;
    dcterms:description [ rdfs:label "Final stage of the normal life span, now commonly considered to be the years after 65."@en ;
            dcterms:creator "The J. Paul Getty Trust" ;
            dcterms:license <https://opendatacommons.org/licenses/by/1-0/> ;
            dcterms:rights <https://rightsstatements.org/vocab/InC/1.0/> ;
            dcterms:source <http://www.getty.edu/research/tools/vocabularies/aat/> ],
        "Final stage of the normal life span, now commonly considered to be the years after 65."@en ;
    dcterms:identifier "CC00387" ;
    owl:sameAs <http://vocab.getty.edu/aat/300189603> .

cc:CC00389 a owl:NamedIndividual ;
    rdfs:label "working class"@en ;
    dcterms:description [ rdfs:label "Class of persons employed for wages, usually at manual labor."@en ;
            dcterms:creator "The J. Paul Getty Trust" ;
            dcterms:license <https://opendatacommons.org/licenses/by/1-0/> ;
            dcterms:rights <https://rightsstatements.org/vocab/InC/1.0/> ;
            dcterms:source <http://www.getty.edu/research/tools/vocabularies/aat/> ],
        "Class of persons employed for wages, usually at manual labor."@en ;
    dcterms:identifier "CC00389" ;
    owl:sameAs <http://vocab.getty.edu/aat/300055485> .

cc:CC00390 a owl:NamedIndividual ;
    rdfs:label "middle class"@en ;
    dcterms:description [ rdfs:label "Social class ranking between upper and lower classes."@en ;
            dcterms:creator "The J. Paul Getty Trust" ;
            dcterms:license <https://opendatacommons.org/licenses/by/1-0/> ;
            dcterms:rights <https://rightsstatements.org/vocab/InC/1.0/> ;
            dcterms:source <http://www.getty.edu/research/tools/vocabularies/aat/> ],
        "Social class ranking between upper and lower classes."@en ;
    dcterms:identifier "CC00390" ;
    owl:sameAs <http://vocab.getty.edu/aat/300055481> .

cc:CC00391 a owl:NamedIndividual ;
    rdfs:label "upper class"@en ;
    dcterms:description [ rdfs:label "That social and economic class that ranks above the middle class."@en ;
            dcterms:creator "The J. Paul Getty Trust" ;
            dcterms:license <https://opendatacommons.org/licenses/by/1-0/> ;
            dcterms:rights <https://rightsstatements.org/vocab/InC/1.0/> ;
            dcterms:source <http://www.getty.edu/research/tools/vocabularies/aat/> ],
        "That social and economic class that ranks above the middle class."@en ;
    dcterms:identifier "CC00391" ;
    owl:sameAs <http://vocab.getty.edu/aat/300055483> .

cc:CC00393 a owl:NamedIndividual ;
    rdfs:label "darts"@en ;
    dcterms:description [ rdfs:label "in sewing, a pointed fold used to take up ease or shape a garment"@en ;
            dcterms:creator "Wikidata contributors" ;
            dcterms:license <https://creativecommons.org/publicdomain/mark/1.0/> ;
            dcterms:rights <https://creativecommons.org/publicdomain/mark/1.0/> ;
            dcterms:source <https://www.wikidata.org/wiki/Wikidata:Data_access/en> ],
        "in sewing, a pointed fold used to take up ease or shape a garment"@en ;
    dcterms:identifier "CC00393" ;
    owl:sameAs <http://www.wikidata.org/entity/Q5225562> .

cc:CC00394 a owl:NamedIndividual ;
    rdfs:label "cuff"@en ;
    dcterms:description [ rdfs:label "Any of various folds or bands that serve as a finish or trimming on items of costume or costume accessories, such as on trousers, gloves, or boots. In a military context, sleeve cuffs may be employed to designate unit or rank. Includes those made as separate items in addition to those made as component parts of garments or costume accessories."@en ;
            dcterms:creator "The J. Paul Getty Trust" ;
            dcterms:license <https://opendatacommons.org/licenses/by/1-0/> ;
            dcterms:rights <https://rightsstatements.org/vocab/InC/1.0/> ;
            dcterms:source <http://www.getty.edu/research/tools/vocabularies/aat/> ],
        "Any of various folds or bands that serve as a finish or trimming on items of costume or costume accessories, such as on trousers, gloves, or boots. In a military context, sleeve cuffs may be employed to designate unit or rank. Includes those made as separate items in addition to those made as component parts of garments or costume accessories."@en ;
    dcterms:identifier "CC00394" ;
    owl:sameAs <http://vocab.getty.edu/aat/300210488> .

cc:CC00395 a owl:NamedIndividual ;
    rdfs:label "epaulette"@en ;
    dcterms:description [ rdfs:label "Cloth straps, usually with fringe, worn at the shoulder on military uniforms to indicate rank, service, or unit and sometimes to retain shoulder belts or sashes. Also, similar ornamental straps adapted for civilian use."@en ;
            dcterms:creator "The J. Paul Getty Trust" ;
            dcterms:license <https://opendatacommons.org/licenses/by/1-0/> ;
            dcterms:rights <https://rightsstatements.org/vocab/InC/1.0/> ;
            dcterms:source <http://www.getty.edu/research/tools/vocabularies/aat/> ],
        "Cloth straps, usually with fringe, worn at the shoulder on military uniforms to indicate rank, service, or unit and sometimes to retain shoulder belts or sashes. Also, similar ornamental straps adapted for civilian use."@en ;
    dcterms:identifier "CC00395" ;
    owl:sameAs <http://vocab.getty.edu/aat/300224235> .

cc:CC00396 a owl:NamedIndividual ;
    rdfs:label "facing"@en ;
    dcterms:description [ rdfs:label "Linings applied to the edge of a garment for ornament or strengthening."@en ;
            dcterms:creator "The J. Paul Getty Trust" ;
            dcterms:license <https://opendatacommons.org/licenses/by/1-0/> ;
            dcterms:rights <https://rightsstatements.org/vocab/InC/1.0/> ;
            dcterms:source <http://www.getty.edu/research/tools/vocabularies/aat/> ],
        "Linings applied to the edge of a garment for ornament or strengthening."@en ;
    dcterms:identifier "CC00396" ;
    owl:sameAs <http://vocab.getty.edu/aat/300224429> .

cc:CC00397 a owl:NamedIndividual ;
    rdfs:label "pocket"@en ;
    dcterms:description [ rdfs:label "Flat pouchlike components stitched into or onto a garment, accessible through a finished opening typically convenient to the hand."@en ;
            dcterms:creator "The J. Paul Getty Trust" ;
            dcterms:license <https://opendatacommons.org/licenses/by/1-0/> ;
            dcterms:rights <https://rightsstatements.org/vocab/InC/1.0/> ;
            dcterms:source <http://www.getty.edu/research/tools/vocabularies/aat/> ],
        "Flat pouchlike components stitched into or onto a garment, accessible through a finished opening typically convenient to the hand."@en ;
    dcterms:identifier "CC00397" ;
    owl:sameAs <http://vocab.getty.edu/aat/300210517> .

cc:CC00398 a owl:NamedIndividual ;
    rdfs:label "shoulder pad"@en ;
    dcterms:description [ rdfs:label "Pads, usually semicircular or triangular in shape, stitched or otherwise attached to the inside of a garment to shape, raise, or widen the shoulders."@en ;
            dcterms:creator "The J. Paul Getty Trust" ;
            dcterms:license <https://opendatacommons.org/licenses/by/1-0/> ;
            dcterms:rights <https://rightsstatements.org/vocab/InC/1.0/> ;
            dcterms:source <http://www.getty.edu/research/tools/vocabularies/aat/> ],
        "Pads, usually semicircular or triangular in shape, stitched or otherwise attached to the inside of a garment to shape, raise, or widen the shoulders."@en ;
    dcterms:identifier "CC00398" ;
    owl:sameAs <http://vocab.getty.edu/aat/300210527> .

cc:CC00399 a owl:NamedIndividual ;
    rdfs:label "waistband"@en ;
    dcterms:description [ rdfs:label "Bands encircling the waist, especially as a part of a skirt or pair of trousers."@en ;
            dcterms:creator "The J. Paul Getty Trust" ;
            dcterms:license <https://opendatacommons.org/licenses/by/1-0/> ;
            dcterms:rights <https://rightsstatements.org/vocab/InC/1.0/> ;
            dcterms:source <http://www.getty.edu/research/tools/vocabularies/aat/> ],
        "Bands encircling the waist, especially as a part of a skirt or pair of trousers."@en ;
    dcterms:identifier "CC00399" ;
    owl:sameAs <http://vocab.getty.edu/aat/300224244> .

cc:CC00400 a owl:NamedIndividual ;
    rdfs:label "wristband"@en ;
    dcterms:description [ rdfs:label "Bands on a sleeve, especially on a shirt sleeve, that cover the wrist."@en ;
            dcterms:creator "The J. Paul Getty Trust" ;
            dcterms:license <https://opendatacommons.org/licenses/by/1-0/> ;
            dcterms:rights <https://rightsstatements.org/vocab/InC/1.0/> ;
            dcterms:source <http://www.getty.edu/research/tools/vocabularies/aat/> ],
        "Bands on a sleeve, especially on a shirt sleeve, that cover the wrist."@en ;
    dcterms:identifier "CC00400" ;
    owl:sameAs <http://vocab.getty.edu/aat/300210017> .

cc:CC00420 a owl:NamedIndividual ;
    rdfs:label "bell-bottoms"@en ;
    dcterms:identifier "CC00420" ;
    owl:sameAs <http://vocab.getty.edu/aat/300262720> .

cc:CC00422 a owl:NamedIndividual ;
    rdfs:label "breeches"@en ;
    dcterms:identifier "CC00422" ;
    owl:sameAs <http://vocab.getty.edu/aat/300046135> .

cc:CC00423 a owl:NamedIndividual ;
    rdfs:label "Capri pants"@en ;
    dcterms:identifier "CC00423" ;
    owl:sameAs <http://vocab.getty.edu/aat/300221449> .

cc:CC00424 a owl:NamedIndividual ;
    rdfs:label "drop-front pants"@en ;
    dcterms:identifier "CC00424" ;
    owl:sameAs <http://vocab.getty.edu/aat/300411740> .

cc:CC00425 a owl:NamedIndividual ;
    rdfs:label "hiphuggers"@en ;
    dcterms:identifier "CC00425" ;
    owl:sameAs <http://vocab.getty.edu/aat/300221446> .

cc:CC00426 a owl:NamedIndividual ;
    rdfs:label "jeans"@en ;
    dcterms:identifier "CC00426" ;
    owl:sameAs <http://vocab.getty.edu/aat/300209918> .

cc:CC00427 a owl:NamedIndividual ;
    rdfs:label "jodhpurs"@en ;
    dcterms:identifier "CC00427" ;
    owl:sameAs <http://vocab.getty.edu/aat/300209919> .

cc:CC00429 a owl:NamedIndividual ;
    rdfs:label "overtrousers"@en ;
    dcterms:identifier "CC00429" ;
    owl:sameAs <http://vocab.getty.edu/aat/300391016> .

cc:CC00432 a owl:NamedIndividual ;
    rdfs:label "puffed pants"@en ;
    dcterms:identifier "CC00432" ;
    owl:sameAs <http://vocab.getty.edu/aat/300411741> .

cc:CC00433 a owl:NamedIndividual ;
    rdfs:label "riding breeches"@en ;
    dcterms:identifier "CC00433" ;
    owl:sameAs <http://vocab.getty.edu/aat/300256819> .

cc:CC00434 a owl:NamedIndividual ;
    rdfs:label "shalwar"@en ;
    dcterms:identifier "CC00434" ;
    owl:sameAs <http://vocab.getty.edu/aat/300216954> .

cc:CC00435 a owl:NamedIndividual ;
    rdfs:label "slacks"@en ;
    dcterms:identifier "CC00435" ;
    owl:sameAs <http://vocab.getty.edu/aat/300209934> .

cc:CC00436 a owl:NamedIndividual ;
    rdfs:label "sweat pants"@en ;
    dcterms:identifier "CC00436" ;
    owl:sameAs <http://vocab.getty.edu/aat/300245257> .

cc:CC00441 a owl:NamedIndividual ;
    rdfs:label "antependia"@en ;
    dcterms:description [ rdfs:label "Panels or hangings for the front of a Christian altar, pulpit, or lectern; may be carved, painted, embroidered, or otherwise decorated. Antependia are of various materials including wood, ivory, precious metals, and embroidered textiles. The exposed position of precious antependia meant that they were sometimes moved on top of the altar for safety, thus becoming retables. If the coverings are continued around the sides and back they are called \"paraments\" or paliotti."@en ;
            dcterms:creator "The J. Paul Getty Trust" ;
            dcterms:license <https://opendatacommons.org/licenses/by/1-0/> ;
            dcterms:rights <https://rightsstatements.org/vocab/InC/1.0/> ;
            dcterms:source <http://www.getty.edu/research/tools/vocabularies/aat/> ],
        "Panels or hangings for the front of a Christian altar, pulpit, or lectern; may be carved, painted, embroidered, or otherwise decorated. Antependia are of various materials including wood, ivory, precious metals, and embroidered textiles. The exposed position of precious antependia meant that they were sometimes moved on top of the altar for safety, thus becoming retables. If the coverings are continued around the sides and back they are called \"paraments\" or paliotti."@en ;
    dcterms:identifier "CC00441" ;
    owl:sameAs <http://vocab.getty.edu/aat/300265255> .

cc:CC00443 a owl:NamedIndividual ;
    rdfs:label "burses (corporal)"@en ;
    dcterms:description [ rdfs:label "Envelope-like cases formed from two squares of stiffened material or of cardboard lined with fabric; used to carry and hold the folded corporal (altar cloth). In Roman form the burse is ordinarily made of two juxtaposed pieces about twenty-five centimeters (or ten inches) square, bound together at three edges, leaving the fourth open to receive the corporal. The fabric of the case is of the liturgical color appropriate to the liturgical calendar. The use of the burse is relatively recent. When the corporal reached its present small dimensions, it was carried to the altar in the Missal or in a bag (burse) or box. For the larger box-like containers used to carry or store corporals, use \"corporal cases.\""@en ;
            dcterms:creator "The J. Paul Getty Trust" ;
            dcterms:license <https://opendatacommons.org/licenses/by/1-0/> ;
            dcterms:rights <https://rightsstatements.org/vocab/InC/1.0/> ;
            dcterms:source <http://www.getty.edu/research/tools/vocabularies/aat/> ],
        "Envelope-like cases formed from two squares of stiffened material or of cardboard lined with fabric; used to carry and hold the folded corporal (altar cloth). In Roman form the burse is ordinarily made of two juxtaposed pieces about twenty-five centimeters (or ten inches) square, bound together at three edges, leaving the fourth open to receive the corporal. The fabric of the case is of the liturgical color appropriate to the liturgical calendar. The use of the burse is relatively recent. When the corporal reached its present small dimensions, it was carried to the altar in the Missal or in a bag (burse) or box. For the larger box-like containers used to carry or store corporals, use \"corporal cases.\""@en ;
    dcterms:identifier "CC00443" ;
    owl:sameAs <http://vocab.getty.edu/aat/300197322> .

cc:CC00444 a owl:NamedIndividual ;
    rdfs:label "cassocks (liturgical costume)"@en ;
    dcterms:description [ rdfs:label "Ankle-length garments of various types, but usually having long, narrow sleeves; worn especially members of the clergy and others participating in church services."@en ;
            dcterms:creator "The J. Paul Getty Trust" ;
            dcterms:license <https://opendatacommons.org/licenses/by/1-0/> ;
            dcterms:rights <https://rightsstatements.org/vocab/InC/1.0/> ;
            dcterms:source <http://www.getty.edu/research/tools/vocabularies/aat/> ],
        "Ankle-length garments of various types, but usually having long, narrow sleeves; worn especially members of the clergy and others participating in church services."@en ;
    dcterms:identifier "CC00444" ;
    owl:sameAs <http://vocab.getty.edu/aat/300210423> .

cc:CC00445 a owl:NamedIndividual ;
    rdfs:label "chasubles (liturgical vestments)"@en ;
    dcterms:description [ rdfs:label "Sleeveless outer vestments in the form of a wide cloak or mantle that slips over the wearer's head and remains open at the sides. Chasubles are worn over the alb and stole by the celebrant at Mass."@en ;
            dcterms:creator "The J. Paul Getty Trust" ;
            dcterms:license <https://opendatacommons.org/licenses/by/1-0/> ;
            dcterms:rights <https://rightsstatements.org/vocab/InC/1.0/> ;
            dcterms:source <http://www.getty.edu/research/tools/vocabularies/aat/> ],
        "Sleeveless outer vestments in the form of a wide cloak or mantle that slips over the wearer's head and remains open at the sides. Chasubles are worn over the alb and stole by the celebrant at Mass."@en ;
    dcterms:identifier "CC00445" ;
    owl:sameAs <http://vocab.getty.edu/aat/300210424> .

cc:CC00446 a owl:NamedIndividual ;
    rdfs:label "chalice veils"@en ;
    dcterms:description [ rdfs:label "Square textile coverings used to cover both chalice and paten before and after communion. A chalice veil is placed over the chalice, paten, and purificator when the vessels are prepared for the Eucharist and placed on the altar; it is removed before the Consecration. It may be embellished and of the same color as the liturgical vestments. For stiff squares covering just the top of the chalice, use \"palls (chalice covers).\""@en ;
            dcterms:creator "The J. Paul Getty Trust" ;
            dcterms:license <https://opendatacommons.org/licenses/by/1-0/> ;
            dcterms:rights <https://rightsstatements.org/vocab/InC/1.0/> ;
            dcterms:source <http://www.getty.edu/research/tools/vocabularies/aat/> ],
        "Square textile coverings used to cover both chalice and paten before and after communion. A chalice veil is placed over the chalice, paten, and purificator when the vessels are prepared for the Eucharist and placed on the altar; it is removed before the Consecration. It may be embellished and of the same color as the liturgical vestments. For stiff squares covering just the top of the chalice, use \"palls (chalice covers).\""@en ;
    dcterms:identifier "CC00446" ;
    owl:sameAs <http://vocab.getty.edu/aat/300204872> .

cc:CC00447 a owl:NamedIndividual ;
    rdfs:label "collets"@en ;
    dcterms:description [ rdfs:label "Casings or sockets which hold a drill or other tool."@en ;
            dcterms:creator "The J. Paul Getty Trust" ;
            dcterms:license <https://opendatacommons.org/licenses/by/1-0/> ;
            dcterms:rights <https://rightsstatements.org/vocab/InC/1.0/> ;
            dcterms:source <http://www.getty.edu/research/tools/vocabularies/aat/> ],
        "Casings or sockets which hold a drill or other tool."@en ;
    dcterms:identifier "CC00447" ;
    owl:sameAs <http://vocab.getty.edu/aat/300024967> .

cc:CC00448 a owl:NamedIndividual ;
    rdfs:label "copes"@en ;
    dcterms:description [ rdfs:label "Long, semi-circular cloaklike garments fastened at the neck with a morse; worn by ecclesiastics in processions and on other ceremonial occasions. Also, similar garments worn as coronation or processional robes by laymen."@en ;
            dcterms:creator "The J. Paul Getty Trust" ;
            dcterms:license <https://opendatacommons.org/licenses/by/1-0/> ;
            dcterms:rights <https://rightsstatements.org/vocab/InC/1.0/> ;
            dcterms:source <http://www.getty.edu/research/tools/vocabularies/aat/> ],
        "Long, semi-circular cloaklike garments fastened at the neck with a morse; worn by ecclesiastics in processions and on other ceremonial occasions. Also, similar garments worn as coronation or processional robes by laymen."@en ;
    dcterms:identifier "CC00448" ;
    owl:sameAs <http://vocab.getty.edu/aat/300210429> .

cc:CC00449 a owl:NamedIndividual ;
    rdfs:label "dalmatics"@en ;
    dcterms:description [ rdfs:label "Long, wide-sleeved tunics of the type worn as Christian liturgical vestments, or as secular dress in earlier periods, with or without a belt. In modern times it has been sometimes worn by kings or emperors. In the western church, the dalmatic is the outer liturgical vestment of the deacon, worn by bishops under the chasuble at solemn pontifical Masses, and by priests only with permission and on certain occasions; normally priests wear chasubles and subdeacons wear tunicles. "@en ;
            dcterms:creator "The J. Paul Getty Trust" ;
            dcterms:license <https://opendatacommons.org/licenses/by/1-0/> ;
            dcterms:rights <https://rightsstatements.org/vocab/InC/1.0/> ;
            dcterms:source <http://www.getty.edu/research/tools/vocabularies/aat/> ],
        "Long, wide-sleeved tunics of the type worn as Christian liturgical vestments, or as secular dress in earlier periods, with or without a belt. In modern times it has been sometimes worn by kings or emperors. In the western church, the dalmatic is the outer liturgical vestment of the deacon, worn by bishops under the chasuble at solemn pontifical Masses, and by priests only with permission and on certain occasions; normally priests wear chasubles and subdeacons wear tunicles. "@en ;
    dcterms:identifier "CC00449" ;
    owl:sameAs <http://vocab.getty.edu/aat/300210431> .

cc:CC00450 a owl:NamedIndividual ;
    rdfs:label "stoles (vestments)"@en ;
    dcterms:description [ rdfs:label "Ecclesiastical vestments worn by bishops and priests consisting of a long narrow cloth band worn around the neck and falling from the shoulders. In the Western church, the sides of the stole are crossed over the chest."@en ;
            dcterms:creator "The J. Paul Getty Trust" ;
            dcterms:license <https://opendatacommons.org/licenses/by/1-0/> ;
            dcterms:rights <https://rightsstatements.org/vocab/InC/1.0/> ;
            dcterms:source <http://www.getty.edu/research/tools/vocabularies/aat/> ],
        "Ecclesiastical vestments worn by bishops and priests consisting of a long narrow cloth band worn around the neck and falling from the shoulders. In the Western church, the sides of the stole are crossed over the chest."@en ;
    dcterms:identifier "CC00450" ;
    owl:sameAs <http://vocab.getty.edu/aat/300221756> .

cc:CC00451 a owl:NamedIndividual ;
    rdfs:label "tabernacle veils"@en ;
    dcterms:description [ rdfs:label "Textile coverings for the tabernacle, which holds the consecrated host and is located in, on, or near the high altar of a church. The tabernacle veil is often of a prescribed liturgical color, based on the period of the church calendar."@en ;
            dcterms:creator "The J. Paul Getty Trust" ;
            dcterms:license <https://opendatacommons.org/licenses/by/1-0/> ;
            dcterms:rights <https://rightsstatements.org/vocab/InC/1.0/> ;
            dcterms:source <http://www.getty.edu/research/tools/vocabularies/aat/> ],
        "Textile coverings for the tabernacle, which holds the consecrated host and is located in, on, or near the high altar of a church. The tabernacle veil is often of a prescribed liturgical color, based on the period of the church calendar."@en ;
    dcterms:identifier "CC00451" ;
    owl:sameAs <http://vocab.getty.edu/aat/300204880> .

cc:CC00452 a owl:NamedIndividual ;
    rdfs:label "tunicles"@en ;
    dcterms:description [ rdfs:label "Vestments resembling dalmatics worn by subdeacons over the alb (and also by bishops between the alb and dalmatic) at celebrations of the Eucharist."@en ;
            dcterms:creator "The J. Paul Getty Trust" ;
            dcterms:license <https://opendatacommons.org/licenses/by/1-0/> ;
            dcterms:rights <https://rightsstatements.org/vocab/InC/1.0/> ;
            dcterms:source <http://www.getty.edu/research/tools/vocabularies/aat/> ],
        "Vestments resembling dalmatics worn by subdeacons over the alb (and also by bishops between the alb and dalmatic) at celebrations of the Eucharist."@en ;
    dcterms:identifier "CC00452" ;
    owl:sameAs <http://vocab.getty.edu/aat/300221685> .

cc:CC00453 a owl:NamedIndividual ;
    rdfs:label "diamonds (motifs)"@en ;
    dcterms:identifier "CC00453" ;
    owl:sameAs <http://vocab.getty.edu/aat/300009791> .

cc:CC00454 a owl:NamedIndividual ;
    rdfs:label "stripes"@en ;
    dcterms:identifier "CC00454" ;
    owl:sameAs <http://vocab.getty.edu/aat/300010230> .

cc:CC00455 a owl:NamedIndividual ;
    rdfs:label "stars (motifs)"@en ;
    dcterms:identifier "CC00455" ;
    owl:sameAs <http://vocab.getty.edu/aat/300009811> .

cc:CC00456 a owl:NamedIndividual ;
    rdfs:label "shells (motifs)"@en ;
    dcterms:identifier "CC00456" ;
    owl:sameAs <http://vocab.getty.edu/aat/300010128> .

cc:CC00457 a owl:NamedIndividual ;
    rdfs:label "main garments"@en ;
    dcterms:description [ rdfs:label "Main layer of dress, usually exclusive of accessories."@en ;
            dcterms:creator "The J. Paul Getty Trust" ;
            dcterms:license <https://opendatacommons.org/licenses/by/1-0/> ;
            dcterms:rights <https://rightsstatements.org/vocab/InC/1.0/> ;
            dcterms:source <http://www.getty.edu/research/tools/vocabularies/aat/> ],
        "Main layer of dress, usually exclusive of accessories."@en ;
    dcterms:identifier "CC00457" ;
    owl:sameAs <http://vocab.getty.edu/aat/300209263> .

cc:CC00459 a owl:NamedIndividual ;
    rdfs:label "protective wear"@en ;
    dcterms:description [ rdfs:label "Garments worn for protection against dirt or danger. For garments worn for protection from weather, use \"outerwear\" or its narrower terms."@en ;
            dcterms:creator "The J. Paul Getty Trust" ;
            dcterms:license <https://opendatacommons.org/licenses/by/1-0/> ;
            dcterms:rights <https://rightsstatements.org/vocab/InC/1.0/> ;
            dcterms:source <http://www.getty.edu/research/tools/vocabularies/aat/> ],
        "Garments worn for protection against dirt or danger. For garments worn for protection from weather, use \"outerwear\" or its narrower terms."@en ;
    dcterms:identifier "CC00459" ;
    owl:sameAs <http://vocab.getty.edu/aat/300209266> .

cc:CC00461 a owl:NamedIndividual ;
    rdfs:label "underwear and accessories for shaping and supporting"@en ;
    dcterms:identifier "CC00461" ;
    owl:sameAs <http://vocab.getty.edu/aat/300209268> .

cc:CC00462 a owl:NamedIndividual ;
    rdfs:label "nightwear"@en ;
    dcterms:description [ rdfs:label "Clothing worn at night, especially garments worn to bed. For dress clothing intended to be worn to evening events, use \"evening wear.\""@en ;
            dcterms:creator "The J. Paul Getty Trust" ;
            dcterms:license <https://opendatacommons.org/licenses/by/1-0/> ;
            dcterms:rights <https://rightsstatements.org/vocab/InC/1.0/> ;
            dcterms:source <http://www.getty.edu/research/tools/vocabularies/aat/> ],
        "Clothing worn at night, especially garments worn to bed. For dress clothing intended to be worn to evening events, use \"evening wear.\""@en ;
    dcterms:identifier "CC00462" ;
    owl:sameAs <http://vocab.getty.edu/aat/300211604> .

cc:CC00463 a owl:NamedIndividual ;
    rdfs:label "worn costume accessories"@en ;
    dcterms:description [ rdfs:label "Items that do not form the primary articles of clothing, but are instead the smaller articles of dress, and that are worn on the body, as opposed to being carried."@en ;
            dcterms:creator "The J. Paul Getty Trust" ;
            dcterms:license <https://opendatacommons.org/licenses/by/1-0/> ;
            dcterms:rights <https://rightsstatements.org/vocab/InC/1.0/> ;
            dcterms:source <http://www.getty.edu/research/tools/vocabularies/aat/> ],
        "Items that do not form the primary articles of clothing, but are instead the smaller articles of dress, and that are worn on the body, as opposed to being carried."@en ;
    dcterms:identifier "CC00463" ;
    owl:sameAs <http://vocab.getty.edu/aat/300209274> .

cc:CC00464 a owl:NamedIndividual ;
    rdfs:label "accessories by location on the head"@en ;
    dcterms:description [ rdfs:label "Costume accessories specifically worn on the head, such as hats."@en ;
            dcterms:creator "The J. Paul Getty Trust" ;
            dcterms:license <https://opendatacommons.org/licenses/by/1-0/> ;
            dcterms:rights <https://rightsstatements.org/vocab/InC/1.0/> ;
            dcterms:source <http://www.getty.edu/research/tools/vocabularies/aat/> ],
        "Costume accessories specifically worn on the head, such as hats."@en ;
    dcterms:identifier "CC00464" ;
    owl:sameAs <http://vocab.getty.edu/aat/300211601> .

cc:CC00465 a owl:NamedIndividual ;
    rdfs:label "hair accessories"@en ;
    dcterms:description [ rdfs:label "Costume accessories worn in conjunction with hair on the head."@en ;
            dcterms:creator "The J. Paul Getty Trust" ;
            dcterms:license <https://opendatacommons.org/licenses/by/1-0/> ;
            dcterms:rights <https://rightsstatements.org/vocab/InC/1.0/> ;
            dcterms:source <http://www.getty.edu/research/tools/vocabularies/aat/> ],
        "Costume accessories worn in conjunction with hair on the head."@en ;
    dcterms:identifier "CC00465" ;
    owl:sameAs <http://vocab.getty.edu/aat/300225910> .

cc:CC00467 a owl:NamedIndividual ;
    rdfs:label "accessories by location above the waist"@en ;
    dcterms:description [ rdfs:label "Costume accessories specifically worn above the waist, such as boutonnieres."@en ;
            dcterms:creator "The J. Paul Getty Trust" ;
            dcterms:license <https://opendatacommons.org/licenses/by/1-0/> ;
            dcterms:rights <https://rightsstatements.org/vocab/InC/1.0/> ;
            dcterms:source <http://www.getty.edu/research/tools/vocabularies/aat/> ],
        "Costume accessories specifically worn above the waist, such as boutonnieres."@en ;
    dcterms:identifier "CC00467" ;
    owl:sameAs <http://vocab.getty.edu/aat/300211602> .

cc:CC00468 a owl:NamedIndividual ;
    rdfs:label "accessories by location at the waist or below"@en ;
    dcterms:description [ rdfs:label "Costume accessories specifically worn at the waist or below."@en ;
            dcterms:creator "The J. Paul Getty Trust" ;
            dcterms:license <https://opendatacommons.org/licenses/by/1-0/> ;
            dcterms:rights <https://rightsstatements.org/vocab/InC/1.0/> ;
            dcterms:source <http://www.getty.edu/research/tools/vocabularies/aat/> ],
        "Costume accessories specifically worn at the waist or below."@en ;
    dcterms:identifier "CC00468" ;
    owl:sameAs <http://vocab.getty.edu/aat/300209283> .

cc:CC00469 a owl:NamedIndividual ;
    rdfs:label "accessories by location on arms or hands"@en ;
    dcterms:description [ rdfs:label "Costume accessories specifically worn on the arms or hands."@en ;
            dcterms:creator "The J. Paul Getty Trust" ;
            dcterms:license <https://opendatacommons.org/licenses/by/1-0/> ;
            dcterms:rights <https://rightsstatements.org/vocab/InC/1.0/> ;
            dcterms:source <http://www.getty.edu/research/tools/vocabularies/aat/> ],
        "Costume accessories specifically worn on the arms or hands."@en ;
    dcterms:identifier "CC00469" ;
    owl:sameAs <http://vocab.getty.edu/aat/300209282> .

cc:CC00470 a owl:NamedIndividual ;
    rdfs:label "accessories by location on the legs or feet"@en ;
    dcterms:description [ rdfs:label "Costume accessories specifically worn on the legs, such as stockings, or the feet, such as footwear."@en ;
            dcterms:creator "The J. Paul Getty Trust" ;
            dcterms:license <https://opendatacommons.org/licenses/by/1-0/> ;
            dcterms:rights <https://rightsstatements.org/vocab/InC/1.0/> ;
            dcterms:source <http://www.getty.edu/research/tools/vocabularies/aat/> ],
        "Costume accessories specifically worn on the legs, such as stockings, or the feet, such as footwear."@en ;
    dcterms:identifier "CC00470" ;
    owl:sameAs <http://vocab.getty.edu/aat/300211599> .

cc:CC00471 a owl:NamedIndividual ;
    rdfs:label "costume accessories carried"@en ;
    dcterms:description [ rdfs:label "Items that do not form the primary articles of clothing, but are instead the smaller articles of dress, and that are carried, as opposed to worn on the body."@en ;
            dcterms:creator "The J. Paul Getty Trust" ;
            dcterms:license <https://opendatacommons.org/licenses/by/1-0/> ;
            dcterms:rights <https://rightsstatements.org/vocab/InC/1.0/> ;
            dcterms:source <http://www.getty.edu/research/tools/vocabularies/aat/> ],
        "Items that do not form the primary articles of clothing, but are instead the smaller articles of dress, and that are carried, as opposed to worn on the body."@en ;
    dcterms:identifier "CC00471" ;
    owl:sameAs <http://vocab.getty.edu/aat/300209275> .

cc:CC00473 a owl:NamedIndividual ;
    rdfs:label "equipment for grooming, hygiene and health care"@en ;
    dcterms:identifier "CC00473" ;
    owl:sameAs <http://vocab.getty.edu/aat/300236656> .

cc:CC00474 a owl:NamedIndividual ;
    rdfs:label "equipment for costume"@en ;
    dcterms:identifier "CC00474" ;
    owl:sameAs <http://vocab.getty.edu/aat/300236657> .

cc:CC00475 a owl:NamedIndividual ;
    rdfs:label "textile working equipment"@en ;
    dcterms:description [ rdfs:label "Equipment used in the making of, or the working with, textiles."@en ;
            dcterms:creator "The J. Paul Getty Trust" ;
            dcterms:license <https://opendatacommons.org/licenses/by/1-0/> ;
            dcterms:rights <https://rightsstatements.org/vocab/InC/1.0/> ;
            dcterms:source <http://www.getty.edu/research/tools/vocabularies/aat/> ],
        "Equipment used in the making of, or the working with, textiles."@en ;
    dcterms:identifier "CC00475" ;
    owl:sameAs <http://vocab.getty.edu/aat/300163224> .

cc:CC00476 a owl:NamedIndividual ;
    rdfs:label "main garments for the lower body"@en ;
    dcterms:identifier "CC00476" ;
    owl:sameAs <http://vocab.getty.edu/aat/300209279> .

cc:CC00477 a owl:NamedIndividual ;
    rdfs:label "main garments for the upper body"@en ;
    dcterms:identifier "CC00477" ;
    owl:sameAs <http://vocab.getty.edu/aat/300209278> .

cc:CC00478 a owl:NamedIndividual ;
    rdfs:label "sports clothing"@en ;
    dcterms:description [ rdfs:label "Garments and accessories designed to be worn while engaged in a specific active sport."@en ;
            dcterms:creator "The J. Paul Getty Trust" ;
            dcterms:license <https://opendatacommons.org/licenses/by/1-0/> ;
            dcterms:rights <https://rightsstatements.org/vocab/InC/1.0/> ;
            dcterms:source <http://www.getty.edu/research/tools/vocabularies/aat/> ],
        "Garments and accessories designed to be worn while engaged in a specific active sport."@en ;
    dcterms:identifier "CC00478" ;
    owl:sameAs <http://vocab.getty.edu/aat/300221269> .

cc:CC00479 a owl:NamedIndividual ;
    rdfs:label "boys' wear"@en ;
    dcterms:description [ rdfs:label "General term for clothing designed for or worn by young males."@en ;
            dcterms:creator "The J. Paul Getty Trust" ;
            dcterms:license <https://opendatacommons.org/licenses/by/1-0/> ;
            dcterms:rights <https://rightsstatements.org/vocab/InC/1.0/> ;
            dcterms:source <http://www.getty.edu/research/tools/vocabularies/aat/> ],
        "General term for clothing designed for or worn by young males."@en ;
    dcterms:identifier "CC00479" ;
    owl:sameAs <http://vocab.getty.edu/aat/300411417> .

cc:CC00480 a owl:NamedIndividual ;
    rdfs:label "girls' wear"@en ;
    dcterms:description [ rdfs:label "General term for clothing designed for or worn by young females."@en ;
            dcterms:creator "The J. Paul Getty Trust" ;
            dcterms:license <https://opendatacommons.org/licenses/by/1-0/> ;
            dcterms:rights <https://rightsstatements.org/vocab/InC/1.0/> ;
            dcterms:source <http://www.getty.edu/research/tools/vocabularies/aat/> ],
        "General term for clothing designed for or worn by young females."@en ;
    dcterms:identifier "CC00480" ;
    owl:sameAs <http://vocab.getty.edu/aat/300411405> .

cc:CC00482 a owl:NamedIndividual ;
    rdfs:label "Costume"@en ;
    dcterms:description [ rdfs:label "The Costume hierarchy contains terms for objects worn or carried for warmth, protection, embellishment, or for symbolic purposes. It includes descriptors for garments considered as the main item of dress (e.g., \"shirts,\" \"trousers\"), terms for garments worn under the main garments (e.g., \"undershirts\"), and terms for garments worn over the main garments (e.g., \"parkas\"). Also included are terms for protective wear, including types of armor; vestments and other ceremonial garments; uniforms; and an extensive listing of accessories, including those worn on the body (e.g., \"headgear,\" \"footwear\") and those carried on the person (e.g., \"evening bags,\" \"parasols\"). Relation to other hierarchies: Terms for accessories that involve measuring (e.g., \"pocket watches\" and \"wrist watches\") are in the Measuring Devices hierarchy. Terms for accessories that are weapons (e.g., \"pocket pistols\" and \"dress swords\") appear with other forms of weapons in the Weapons and Ammunition hierarchy. Terms for objects that may be used in the grooming and care of costume or the person (e.g., \"clothes brushes,\" \"nail clippers\") are in the Tools and Equipment hierarchy. Terms for objects used to store or transport costume or other personal effects (e.g., \"glove boxes,\" \"suitcases\") appear in the Containers hierarchy. Constituent parts of costume (e.g., \"busks,\" \"waistbands\") appear in the Components hierarchy, which has a non-preferred, partitive hierarchical relationship to the Costume hierarchy."@en ;
            dcterms:creator "The J. Paul Getty Trust" ;
            dcterms:license <https://opendatacommons.org/licenses/by/1-0/> ;
            dcterms:rights <https://rightsstatements.org/vocab/InC/1.0/> ;
            dcterms:source <http://www.getty.edu/research/tools/vocabularies/aat/> ],
        "The Costume hierarchy contains terms for objects worn or carried for warmth, protection, embellishment, or for symbolic purposes. It includes descriptors for garments considered as the main item of dress (e.g., \"shirts,\" \"trousers\"), terms for garments worn under the main garments (e.g., \"undershirts\"), and terms for garments worn over the main garments (e.g., \"parkas\"). Also included are terms for protective wear, including types of armor; vestments and other ceremonial garments; uniforms; and an extensive listing of accessories, including those worn on the body (e.g., \"headgear,\" \"footwear\") and those carried on the person (e.g., \"evening bags,\" \"parasols\"). Relation to other hierarchies: Terms for accessories that involve measuring (e.g., \"pocket watches\" and \"wrist watches\") are in the Measuring Devices hierarchy. Terms for accessories that are weapons (e.g., \"pocket pistols\" and \"dress swords\") appear with other forms of weapons in the Weapons and Ammunition hierarchy. Terms for objects that may be used in the grooming and care of costume or the person (e.g., \"clothes brushes,\" \"nail clippers\") are in the Tools and Equipment hierarchy. Terms for objects used to store or transport costume or other personal effects (e.g., \"glove boxes,\" \"suitcases\") appear in the Containers hierarchy. Constituent parts of costume (e.g., \"busks,\" \"waistbands\") appear in the Components hierarchy, which has a non-preferred, partitive hierarchical relationship to the Costume hierarchy."@en ;
    dcterms:identifier "CC00482" ;
    owl:sameAs <http://vocab.getty.edu/aat/300209261> .

cc:CC00489 a owl:NamedIndividual ;
    rdfs:label "ballerina neckline"@en ;
    dcterms:description [ rdfs:label "wide, shallowly-curved neckline"@en ;
            dcterms:creator "Wikidata contributors" ;
            dcterms:license <https://creativecommons.org/publicdomain/mark/1.0/> ;
            dcterms:rights <https://creativecommons.org/publicdomain/mark/1.0/> ;
            dcterms:source <https://www.wikidata.org/wiki/Wikidata:Data_access/en> ],
        "wide, shallowly-curved neckline"@en ;
    dcterms:identifier "CC00489" ;
    owl:sameAs <http://www.wikidata.org/entity/Q4851616> .

cc:CC00490 a owl:NamedIndividual ;
    rdfs:label "dcolletage"@en ;
    dcterms:description [ rdfs:label "a low neckline on a woman's dress, especially one that reveals or emphasizes her cleavage"@en ;
            dcterms:creator "Wikidata contributors" ;
            dcterms:license <https://creativecommons.org/publicdomain/mark/1.0/> ;
            dcterms:rights <https://creativecommons.org/publicdomain/mark/1.0/> ;
            dcterms:source <https://www.wikidata.org/wiki/Wikidata:Data_access/en> ],
        "a low neckline on a woman's dress, especially one that reveals or emphasizes her cleavage"@en ;
    dcterms:identifier "CC00490" ;
    owl:sameAs <http://www.wikidata.org/entity/Q116887> .

cc:CC00491 a owl:NamedIndividual ;
    rdfs:label "surplice neckline"@en ;
    dcterms:description [ rdfs:label "V-shaped neckline resulting from overlapping left and right sides of a wrapped garment"@en ;
            dcterms:creator "Wikidata contributors" ;
            dcterms:license <https://creativecommons.org/publicdomain/mark/1.0/> ;
            dcterms:rights <https://creativecommons.org/publicdomain/mark/1.0/> ;
            dcterms:source <https://www.wikidata.org/wiki/Wikidata:Data_access/en> ],
        "V-shaped neckline resulting from overlapping left and right sides of a wrapped garment"@en ;
    dcterms:identifier "CC00491" ;
    owl:sameAs <http://www.wikidata.org/entity/Q29583224> .

cc:CC00492 a owl:NamedIndividual ;
    rdfs:label "patch"@en ;
    dcterms:description [ rdfs:label "piece of textile or leather applied to clothing as a reinforcement against wear or to mend a damaged spot"@en ;
            dcterms:creator "Wikidata contributors" ;
            dcterms:license <https://creativecommons.org/publicdomain/mark/1.0/> ;
            dcterms:rights <https://creativecommons.org/publicdomain/mark/1.0/> ;
            dcterms:source <https://www.wikidata.org/wiki/Wikidata:Data_access/en> ],
        "piece of textile or leather applied to clothing as a reinforcement against wear or to mend a damaged spot"@en ;
    dcterms:identifier "CC00492" ;
    owl:sameAs <http://www.wikidata.org/entity/Q2058306> .

cc:CC00494 a owl:NamedIndividual ;
    rdfs:label "ball gown"@en ;
    dcterms:description [ rdfs:label "most formal style of full-length woman's evening dress"@en ;
            dcterms:creator "Wikidata contributors" ;
            dcterms:license <https://creativecommons.org/publicdomain/mark/1.0/> ;
            dcterms:rights <https://creativecommons.org/publicdomain/mark/1.0/> ;
            dcterms:source <https://www.wikidata.org/wiki/Wikidata:Data_access/en> ],
        "most formal style of full-length woman's evening dress"@en ;
    dcterms:identifier "CC00494" ;
    owl:sameAs <http://www.wikidata.org/entity/Q635784> .

cc:CC00496 a owl:NamedIndividual ;
    rdfs:label "cheongsam"@en ;
    dcterms:description [ rdfs:label "fitted dress in Chinese culture"@en ;
            dcterms:creator "Wikidata contributors" ;
            dcterms:license <https://creativecommons.org/publicdomain/mark/1.0/> ;
            dcterms:rights <https://creativecommons.org/publicdomain/mark/1.0/> ;
            dcterms:source <https://www.wikidata.org/wiki/Wikidata:Data_access/en> ],
        "fitted dress in Chinese culture"@en ;
    dcterms:identifier "CC00496" ;
    owl:sameAs <http://www.wikidata.org/entity/Q836934> .

cc:CC00501 a owl:NamedIndividual ;
    rdfs:label "muumuu"@en ;
    dcterms:description [ rdfs:label "loose dress, usually brightly colored or patterned, worn especially by Hawaiian women, or as a housecoat"@en ;
            dcterms:creator "The J. Paul Getty Trust" ;
            dcterms:license <https://opendatacommons.org/licenses/by/1-0/> ;
            dcterms:rights <https://rightsstatements.org/vocab/InC/1.0/> ;
            dcterms:source <http://www.getty.edu/research/tools/vocabularies/aat/> ],
        "loose dress, usually brightly colored or patterned, worn especially by Hawaiian women, or as a housecoat"@en ;
    dcterms:identifier "CC00501" ;
    owl:sameAs <http://vocab.getty.edu/aat/300046174> .

cc:CC00502 a owl:NamedIndividual ;
    rdfs:label "princess line"@en ;
    dcterms:description [ rdfs:label "woman's fitted dress cut without a waist seam, the bodice and skirt being cut in one"@en ;
            dcterms:creator "Wikidata contributors" ;
            dcterms:license <https://creativecommons.org/publicdomain/mark/1.0/> ;
            dcterms:rights <https://creativecommons.org/publicdomain/mark/1.0/> ;
            dcterms:source <https://www.wikidata.org/wiki/Wikidata:Data_access/en> ],
        "woman's fitted dress cut without a waist seam, the bodice and skirt being cut in one"@en ;
    dcterms:identifier "CC00502" ;
    owl:sameAs <http://www.wikidata.org/entity/Q10638846> .

cc:CC00507 a owl:NamedIndividual ;
    rdfs:label "maternity clothes"@en ;
    dcterms:description [ rdfs:label "Womenswear designed to be worn during pregnancy."@en ;
            dcterms:creator "The J. Paul Getty Trust" ;
            dcterms:license <https://opendatacommons.org/licenses/by/1-0/> ;
            dcterms:rights <https://rightsstatements.org/vocab/InC/1.0/> ;
            dcterms:source <http://www.getty.edu/research/tools/vocabularies/aat/> ],
        "Womenswear designed to be worn during pregnancy."@en ;
    dcterms:identifier "CC00507" ;
    owl:sameAs <http://vocab.getty.edu/aat/300411755> .

cc:CC00509 a owl:NamedIndividual ;
    rdfs:label "wedding clothes"@en ;
    dcterms:description [ rdfs:label "Clothing designed or worn for a wedding."@en ;
            dcterms:creator "The J. Paul Getty Trust" ;
            dcterms:license <https://opendatacommons.org/licenses/by/1-0/> ;
            dcterms:rights <https://rightsstatements.org/vocab/InC/1.0/> ;
            dcterms:source <http://www.getty.edu/research/tools/vocabularies/aat/> ],
        "Clothing designed or worn for a wedding."@en ;
    dcterms:identifier "CC00509" ;
    owl:sameAs <http://vocab.getty.edu/aat/300411762> .

cc:CC00510 a owl:NamedIndividual ;
    rdfs:label "hobble skirt"@en ;
    dcterms:description [ rdfs:label "skirt that is narrower at the gen than the knee"@en ;
            dcterms:creator "Wikidata contributors" ;
            dcterms:license <https://creativecommons.org/publicdomain/mark/1.0/> ;
            dcterms:rights <https://creativecommons.org/publicdomain/mark/1.0/> ;
            dcterms:source <https://www.wikidata.org/wiki/Wikidata:Data_access/en> ],
        "skirt that is narrower at the gen than the knee"@en ;
    dcterms:identifier "CC00510" ;
    owl:sameAs <http://www.wikidata.org/entity/Q1637220> .

cc:CC00511 a owl:NamedIndividual ;
    rdfs:label "kilt"@en ;
    dcterms:description [ rdfs:label "knee-length garment of Celtic and Scottish origin"@en ;
            dcterms:creator "Wikidata contributors" ;
            dcterms:license <https://creativecommons.org/publicdomain/mark/1.0/> ;
            dcterms:rights <https://creativecommons.org/publicdomain/mark/1.0/> ;
            dcterms:source <https://www.wikidata.org/wiki/Wikidata:Data_access/en> ],
        "knee-length garment of Celtic and Scottish origin"@en ;
    dcterms:identifier "CC00511" ;
    owl:sameAs <http://www.wikidata.org/entity/Q151948> .

cc:CC00512 a owl:NamedIndividual ;
    rdfs:label "overskirt"@en ;
    dcterms:description [ rdfs:label "skirt worn draped over a dress, underskirt or petticoat"@en ;
            dcterms:creator "Wikidata contributors" ;
            dcterms:license <https://creativecommons.org/publicdomain/mark/1.0/> ;
            dcterms:rights <https://creativecommons.org/publicdomain/mark/1.0/> ;
            dcterms:source <https://www.wikidata.org/wiki/Wikidata:Data_access/en> ],
        "skirt worn draped over a dress, underskirt or petticoat"@en ;
    dcterms:identifier "CC00512" ;
    owl:sameAs <http://www.wikidata.org/entity/Q22921095> .

cc:CC00513 a owl:NamedIndividual ;
    rdfs:label "wrap skirt"@en ;
    dcterms:description [ rdfs:label "a skirt that wraps around the waist with an overlap of material"@en ;
            dcterms:creator "Wikidata contributors" ;
            dcterms:license <https://creativecommons.org/publicdomain/mark/1.0/> ;
            dcterms:rights <https://creativecommons.org/publicdomain/mark/1.0/> ;
            dcterms:source <https://www.wikidata.org/wiki/Wikidata:Data_access/en> ],
        "a skirt that wraps around the waist with an overlap of material"@en ;
    dcterms:identifier "CC00513" ;
    owl:sameAs <http://www.wikidata.org/entity/Q1485316> .

cc:CC00515 a owl:NamedIndividual ;
    rdfs:label "clasp"@en ;
    dcterms:description [ rdfs:label "Fasteners made of two or more parts, often of metal, and consisting of separate interlocking hooking and catching elements that hold together two or more objects or complimentary parts of the same object."@en ;
            dcterms:creator "The J. Paul Getty Trust" ;
            dcterms:license <https://opendatacommons.org/licenses/by/1-0/> ;
            dcterms:rights <https://rightsstatements.org/vocab/InC/1.0/> ;
            dcterms:source <http://www.getty.edu/research/tools/vocabularies/aat/> ],
        "Fasteners made of two or more parts, often of metal, and consisting of separate interlocking hooking and catching elements that hold together two or more objects or complimentary parts of the same object."@en ;
    dcterms:identifier "CC00515" ;
    owl:sameAs <http://vocab.getty.edu/aat/300239507> .

cc:CC00517 a owl:NamedIndividual ;
    rdfs:label "knickerbockers"@en ;
    dcterms:description [ rdfs:label "Loose-cut breeches banded at the knee."@en ;
            dcterms:creator "The J. Paul Getty Trust" ;
            dcterms:license <https://opendatacommons.org/licenses/by/1-0/> ;
            dcterms:rights <https://rightsstatements.org/vocab/InC/1.0/> ;
            dcterms:source <http://www.getty.edu/research/tools/vocabularies/aat/> ],
        "Loose-cut breeches banded at the knee."@en ;
    dcterms:identifier "CC00517" ;
    owl:sameAs <http://vocab.getty.edu/aat/300214558> .

cc:CC00519 a owl:NamedIndividual ;
    rdfs:label "nightwear"@en ;
    dcterms:description [ rdfs:label "Clothing worn at night, especially garments worn to bed. For dress clothing intended to be worn to evening events, use \"evening wear.\""@en ;
            dcterms:creator "The J. Paul Getty Trust" ;
            dcterms:license <https://opendatacommons.org/licenses/by/1-0/> ;
            dcterms:rights <https://rightsstatements.org/vocab/InC/1.0/> ;
            dcterms:source <http://www.getty.edu/research/tools/vocabularies/aat/> ],
        "Clothing worn at night, especially garments worn to bed. For dress clothing intended to be worn to evening events, use \"evening wear.\""@en ;
    dcterms:identifier "CC00519" ;
    owl:sameAs <http://vocab.getty.edu/aat/300211604> .

cc:CC00520 a owl:NamedIndividual ;
    rdfs:label "tent"@en ;
    dcterms:description [ rdfs:label "dress that hangs loose from shoulder to below the hips, with no waistline"@en ;
            dcterms:creator "Wikidata contributors" ;
            dcterms:license <https://creativecommons.org/publicdomain/mark/1.0/> ;
            dcterms:rights <https://creativecommons.org/publicdomain/mark/1.0/> ;
            dcterms:source <https://www.wikidata.org/wiki/Wikidata:Data_access/en> ],
        "dress that hangs loose from shoulder to below the hips, with no waistline"@en ;
    dcterms:identifier "CC00520" ;
    owl:sameAs <http://www.wikidata.org/entity/Q10707950> .

cc:CC00522 a owl:NamedIndividual ;
    rdfs:label "shift"@en ;
    dcterms:description [ rdfs:label "Dresses which hang straight from the shoulders, sometimes tapering slightly at hips."@en ;
            dcterms:creator "The J. Paul Getty Trust" ;
            dcterms:license <https://opendatacommons.org/licenses/by/1-0/> ;
            dcterms:rights <https://rightsstatements.org/vocab/InC/1.0/> ;
            dcterms:source <http://www.getty.edu/research/tools/vocabularies/aat/> ],
        "Dresses which hang straight from the shoulders, sometimes tapering slightly at hips."@en ;
    dcterms:identifier "CC00522" ;
    owl:sameAs <http://vocab.getty.edu/aat/300214100> .

cc:CC00524 a owl:NamedIndividual ;
    rdfs:label "bloomers"@en ;
    dcterms:description [ rdfs:label "Drawers with full, loose legs gathered above or below the knee; worn by women and children."@en ;
            dcterms:creator "The J. Paul Getty Trust" ;
            dcterms:license <https://opendatacommons.org/licenses/by/1-0/> ;
            dcterms:rights <https://rightsstatements.org/vocab/InC/1.0/> ;
            dcterms:source <http://www.getty.edu/research/tools/vocabularies/aat/> ],
        "Drawers with full, loose legs gathered above or below the knee; worn by women and children."@en ;
    dcterms:identifier "CC00524" ;
    owl:sameAs <http://vocab.getty.edu/aat/300210537> .

cc:CC00527 a owl:NamedIndividual ;
    rdfs:label "1500s"@en ;
    dcterms:description [ rdfs:label "decade"@en ;
            dcterms:creator "Wikidata contributors" ;
            dcterms:license <https://creativecommons.org/publicdomain/mark/1.0/> ;
            dcterms:rights <https://creativecommons.org/publicdomain/mark/1.0/> ;
            dcterms:source <https://www.wikidata.org/wiki/Wikidata:Data_access/en> ],
        "decade"@en ;
    dcterms:identifier "CC00527" ;
    owl:sameAs <http://www.wikidata.org/entity/Q44140> .

cc:CC00528 a owl:NamedIndividual ;
    rdfs:label "1510s"@en ;
    dcterms:description [ rdfs:label "decade"@en ;
            dcterms:creator "Wikidata contributors" ;
            dcterms:license <https://creativecommons.org/publicdomain/mark/1.0/> ;
            dcterms:rights <https://creativecommons.org/publicdomain/mark/1.0/> ;
            dcterms:source <https://www.wikidata.org/wiki/Wikidata:Data_access/en> ],
        "decade"@en ;
    dcterms:identifier "CC00528" ;
    owl:sameAs <http://www.wikidata.org/entity/Q46245> .

cc:CC00529 a owl:NamedIndividual ;
    rdfs:label "1520s"@en ;
    dcterms:description [ rdfs:label "decade"@en ;
            dcterms:creator "Wikidata contributors" ;
            dcterms:license <https://creativecommons.org/publicdomain/mark/1.0/> ;
            dcterms:rights <https://creativecommons.org/publicdomain/mark/1.0/> ;
            dcterms:source <https://www.wikidata.org/wiki/Wikidata:Data_access/en> ],
        "decade"@en ;
    dcterms:identifier "CC00529" ;
    owl:sameAs <http://www.wikidata.org/entity/Q192244> .

cc:CC00530 a owl:NamedIndividual ;
    rdfs:label "1530s"@en ;
    dcterms:description [ rdfs:label "decade"@en ;
            dcterms:creator "Wikidata contributors" ;
            dcterms:license <https://creativecommons.org/publicdomain/mark/1.0/> ;
            dcterms:rights <https://creativecommons.org/publicdomain/mark/1.0/> ;
            dcterms:source <https://www.wikidata.org/wiki/Wikidata:Data_access/en> ],
        "decade"@en ;
    dcterms:identifier "CC00530" ;
    owl:sameAs <http://www.wikidata.org/entity/Q192500> .

cc:CC00531 a owl:NamedIndividual ;
    rdfs:label "1540s"@en ;
    dcterms:description [ rdfs:label "decade"@en ;
            dcterms:creator "Wikidata contributors" ;
            dcterms:license <https://creativecommons.org/publicdomain/mark/1.0/> ;
            dcterms:rights <https://creativecommons.org/publicdomain/mark/1.0/> ;
            dcterms:source <https://www.wikidata.org/wiki/Wikidata:Data_access/en> ],
        "decade"@en ;
    dcterms:identifier "CC00531" ;
    owl:sameAs <http://www.wikidata.org/entity/Q48158> .

cc:CC00532 a owl:NamedIndividual ;
    rdfs:label "1550s"@en ;
    dcterms:description [ rdfs:label "decade"@en ;
            dcterms:creator "Wikidata contributors" ;
            dcterms:license <https://creativecommons.org/publicdomain/mark/1.0/> ;
            dcterms:rights <https://creativecommons.org/publicdomain/mark/1.0/> ;
            dcterms:source <https://www.wikidata.org/wiki/Wikidata:Data_access/en> ],
        "decade"@en ;
    dcterms:identifier "CC00532" ;
    owl:sameAs <http://www.wikidata.org/entity/Q193242> .

cc:CC00533 a owl:NamedIndividual ;
    rdfs:label "1560s"@en ;
    dcterms:description [ rdfs:label "decade"@en ;
            dcterms:creator "Wikidata contributors" ;
            dcterms:license <https://creativecommons.org/publicdomain/mark/1.0/> ;
            dcterms:rights <https://creativecommons.org/publicdomain/mark/1.0/> ;
            dcterms:source <https://www.wikidata.org/wiki/Wikidata:Data_access/en> ],
        "decade"@en ;
    dcterms:identifier "CC00533" ;
    owl:sameAs <http://www.wikidata.org/entity/Q193480> .

cc:CC00534 a owl:NamedIndividual ;
    rdfs:label "1570s"@en ;
    dcterms:description [ rdfs:label "decade"@en ;
            dcterms:creator "Wikidata contributors" ;
            dcterms:license <https://creativecommons.org/publicdomain/mark/1.0/> ;
            dcterms:rights <https://creativecommons.org/publicdomain/mark/1.0/> ;
            dcterms:source <https://www.wikidata.org/wiki/Wikidata:Data_access/en> ],
        "decade"@en ;
    dcterms:identifier "CC00534" ;
    owl:sameAs <http://www.wikidata.org/entity/Q193679> .

cc:CC00535 a owl:NamedIndividual ;
    rdfs:label "1580s"@en ;
    dcterms:description [ rdfs:label "decade"@en ;
            dcterms:creator "Wikidata contributors" ;
            dcterms:license <https://creativecommons.org/publicdomain/mark/1.0/> ;
            dcterms:rights <https://creativecommons.org/publicdomain/mark/1.0/> ;
            dcterms:source <https://www.wikidata.org/wiki/Wikidata:Data_access/en> ],
        "decade"@en ;
    dcterms:identifier "CC00535" ;
    owl:sameAs <http://www.wikidata.org/entity/Q48563> .

cc:CC00536 a owl:NamedIndividual ;
    rdfs:label "1590s"@en ;
    dcterms:description [ rdfs:label "decade"@en ;
            dcterms:creator "Wikidata contributors" ;
            dcterms:license <https://creativecommons.org/publicdomain/mark/1.0/> ;
            dcterms:rights <https://creativecommons.org/publicdomain/mark/1.0/> ;
            dcterms:source <https://www.wikidata.org/wiki/Wikidata:Data_access/en> ],
        "decade"@en ;
    dcterms:identifier "CC00536" ;
    owl:sameAs <http://www.wikidata.org/entity/Q48595> .

cc:CC00537 a owl:NamedIndividual ;
    rdfs:label "1600s"@en ;
    dcterms:description [ rdfs:label "decade"@en ;
            dcterms:creator "Wikidata contributors" ;
            dcterms:license <https://creativecommons.org/publicdomain/mark/1.0/> ;
            dcterms:rights <https://creativecommons.org/publicdomain/mark/1.0/> ;
            dcterms:source <https://www.wikidata.org/wiki/Wikidata:Data_access/en> ],
        "decade"@en ;
    dcterms:identifier "CC00537" ;
    owl:sameAs <http://www.wikidata.org/entity/Q42995> .

cc:CC00538 a owl:NamedIndividual ;
    rdfs:label "1610s"@en ;
    dcterms:description [ rdfs:label "decade"@en ;
            dcterms:creator "Wikidata contributors" ;
            dcterms:license <https://creativecommons.org/publicdomain/mark/1.0/> ;
            dcterms:rights <https://creativecommons.org/publicdomain/mark/1.0/> ;
            dcterms:source <https://www.wikidata.org/wiki/Wikidata:Data_access/en> ],
        "decade"@en ;
    dcterms:identifier "CC00538" ;
    owl:sameAs <http://www.wikidata.org/entity/Q46050> .

cc:CC00539 a owl:NamedIndividual ;
    rdfs:label "1620s"@en ;
    dcterms:description [ rdfs:label "decade"@en ;
            dcterms:creator "Wikidata contributors" ;
            dcterms:license <https://creativecommons.org/publicdomain/mark/1.0/> ;
            dcterms:rights <https://creativecommons.org/publicdomain/mark/1.0/> ;
            dcterms:source <https://www.wikidata.org/wiki/Wikidata:Data_access/en> ],
        "decade"@en ;
    dcterms:identifier "CC00539" ;
    owl:sameAs <http://www.wikidata.org/entity/Q195923> .

cc:CC00540 a owl:NamedIndividual ;
    rdfs:label "1630s"@en ;
    dcterms:description [ rdfs:label "decade"@en ;
            dcterms:creator "Wikidata contributors" ;
            dcterms:license <https://creativecommons.org/publicdomain/mark/1.0/> ;
            dcterms:rights <https://creativecommons.org/publicdomain/mark/1.0/> ;
            dcterms:source <https://www.wikidata.org/wiki/Wikidata:Data_access/en> ],
        "decade"@en ;
    dcterms:identifier "CC00540" ;
    owl:sameAs <http://www.wikidata.org/entity/Q196292> .

cc:CC00541 a owl:NamedIndividual ;
    rdfs:label "1640s"@en ;
    dcterms:description [ rdfs:label "decade"@en ;
            dcterms:creator "Wikidata contributors" ;
            dcterms:license <https://creativecommons.org/publicdomain/mark/1.0/> ;
            dcterms:rights <https://creativecommons.org/publicdomain/mark/1.0/> ;
            dcterms:source <https://www.wikidata.org/wiki/Wikidata:Data_access/en> ],
        "decade"@en ;
    dcterms:identifier "CC00541" ;
    owl:sameAs <http://www.wikidata.org/entity/Q196375> .

cc:CC00542 a owl:NamedIndividual ;
    rdfs:label "1650s"@en ;
    dcterms:description [ rdfs:label "decade"@en ;
            dcterms:creator "Wikidata contributors" ;
            dcterms:license <https://creativecommons.org/publicdomain/mark/1.0/> ;
            dcterms:rights <https://creativecommons.org/publicdomain/mark/1.0/> ;
            dcterms:source <https://www.wikidata.org/wiki/Wikidata:Data_access/en> ],
        "decade"@en ;
    dcterms:identifier "CC00542" ;
    owl:sameAs <http://www.wikidata.org/entity/Q196467> .

cc:CC00543 a owl:NamedIndividual ;
    rdfs:label "1660s"@en ;
    dcterms:description [ rdfs:label "decade"@en ;
            dcterms:creator "Wikidata contributors" ;
            dcterms:license <https://creativecommons.org/publicdomain/mark/1.0/> ;
            dcterms:rights <https://creativecommons.org/publicdomain/mark/1.0/> ;
            dcterms:source <https://www.wikidata.org/wiki/Wikidata:Data_access/en> ],
        "decade"@en ;
    dcterms:identifier "CC00543" ;
    owl:sameAs <http://www.wikidata.org/entity/Q196549> .

cc:CC00544 a owl:NamedIndividual ;
    rdfs:label "1670s"@en ;
    dcterms:description [ rdfs:label "decade"@en ;
            dcterms:creator "Wikidata contributors" ;
            dcterms:license <https://creativecommons.org/publicdomain/mark/1.0/> ;
            dcterms:rights <https://creativecommons.org/publicdomain/mark/1.0/> ;
            dcterms:source <https://www.wikidata.org/wiki/Wikidata:Data_access/en> ],
        "decade"@en ;
    dcterms:identifier "CC00544" ;
    owl:sameAs <http://www.wikidata.org/entity/Q196647> .

cc:CC00545 a owl:NamedIndividual ;
    rdfs:label "1680s"@en ;
    dcterms:description [ rdfs:label "decade"@en ;
            dcterms:creator "Wikidata contributors" ;
            dcterms:license <https://creativecommons.org/publicdomain/mark/1.0/> ;
            dcterms:rights <https://creativecommons.org/publicdomain/mark/1.0/> ;
            dcterms:source <https://www.wikidata.org/wiki/Wikidata:Data_access/en> ],
        "decade"@en ;
    dcterms:identifier "CC00545" ;
    owl:sameAs <http://www.wikidata.org/entity/Q46011> .

cc:CC00546 a owl:NamedIndividual ;
    rdfs:label "1690s"@en ;
    dcterms:description [ rdfs:label "decade"@en ;
            dcterms:creator "Wikidata contributors" ;
            dcterms:license <https://creativecommons.org/publicdomain/mark/1.0/> ;
            dcterms:rights <https://creativecommons.org/publicdomain/mark/1.0/> ;
            dcterms:source <https://www.wikidata.org/wiki/Wikidata:Data_access/en> ],
        "decade"@en ;
    dcterms:identifier "CC00546" ;
    owl:sameAs <http://www.wikidata.org/entity/Q197012> .

cc:CC00547 a owl:NamedIndividual ;
    rdfs:label "1700s"@en ;
    dcterms:description [ rdfs:label "decade"@en ;
            dcterms:creator "Wikidata contributors" ;
            dcterms:license <https://creativecommons.org/publicdomain/mark/1.0/> ;
            dcterms:rights <https://creativecommons.org/publicdomain/mark/1.0/> ;
            dcterms:source <https://www.wikidata.org/wiki/Wikidata:Data_access/en> ],
        "decade"@en ;
    dcterms:identifier "CC00547" ;
    owl:sameAs <http://www.wikidata.org/entity/Q43370> .

cc:CC00548 a owl:NamedIndividual ;
    rdfs:label "1710s"@en ;
    dcterms:description [ rdfs:label "decade"@en ;
            dcterms:creator "Wikidata contributors" ;
            dcterms:license <https://creativecommons.org/publicdomain/mark/1.0/> ;
            dcterms:rights <https://creativecommons.org/publicdomain/mark/1.0/> ;
            dcterms:source <https://www.wikidata.org/wiki/Wikidata:Data_access/en> ],
        "decade"@en ;
    dcterms:identifier "CC00548" ;
    owl:sameAs <http://www.wikidata.org/entity/Q198144> .

cc:CC00549 a owl:NamedIndividual ;
    rdfs:label "1720s"@en ;
    dcterms:description [ rdfs:label "decade"@en ;
            dcterms:creator "Wikidata contributors" ;
            dcterms:license <https://creativecommons.org/publicdomain/mark/1.0/> ;
            dcterms:rights <https://creativecommons.org/publicdomain/mark/1.0/> ;
            dcterms:source <https://www.wikidata.org/wiki/Wikidata:Data_access/en> ],
        "decade"@en ;
    dcterms:identifier "CC00549" ;
    owl:sameAs <http://www.wikidata.org/entity/Q198469> .

cc:CC00550 a owl:NamedIndividual ;
    rdfs:label "1730s"@en ;
    dcterms:description [ rdfs:label "decade"@en ;
            dcterms:creator "Wikidata contributors" ;
            dcterms:license <https://creativecommons.org/publicdomain/mark/1.0/> ;
            dcterms:rights <https://creativecommons.org/publicdomain/mark/1.0/> ;
            dcterms:source <https://www.wikidata.org/wiki/Wikidata:Data_access/en> ],
        "decade"@en ;
    dcterms:identifier "CC00550" ;
    owl:sameAs <http://www.wikidata.org/entity/Q48121> .

cc:CC00551 a owl:NamedIndividual ;
    rdfs:label "1740s"@en ;
    dcterms:description [ rdfs:label "decade"@en ;
            dcterms:creator "Wikidata contributors" ;
            dcterms:license <https://creativecommons.org/publicdomain/mark/1.0/> ;
            dcterms:rights <https://creativecommons.org/publicdomain/mark/1.0/> ;
            dcterms:source <https://www.wikidata.org/wiki/Wikidata:Data_access/en> ],
        "decade"@en ;
    dcterms:identifier "CC00551" ;
    owl:sameAs <http://www.wikidata.org/entity/Q43970> .

cc:CC00552 a owl:NamedIndividual ;
    rdfs:label "1750s"@en ;
    dcterms:description [ rdfs:label "decade"@en ;
            dcterms:creator "Wikidata contributors" ;
            dcterms:license <https://creativecommons.org/publicdomain/mark/1.0/> ;
            dcterms:rights <https://creativecommons.org/publicdomain/mark/1.0/> ;
            dcterms:source <https://www.wikidata.org/wiki/Wikidata:Data_access/en> ],
        "decade"@en ;
    dcterms:identifier "CC00552" ;
    owl:sameAs <http://www.wikidata.org/entity/Q48528> .

cc:CC00553 a owl:NamedIndividual ;
    rdfs:label "1760s"@en ;
    dcterms:description [ rdfs:label "decade"@en ;
            dcterms:creator "Wikidata contributors" ;
            dcterms:license <https://creativecommons.org/publicdomain/mark/1.0/> ;
            dcterms:rights <https://creativecommons.org/publicdomain/mark/1.0/> ;
            dcterms:source <https://www.wikidata.org/wiki/Wikidata:Data_access/en> ],
        "decade"@en ;
    dcterms:identifier "CC00553" ;
    owl:sameAs <http://www.wikidata.org/entity/Q199545> .

cc:CC00554 a owl:NamedIndividual ;
    rdfs:label "1770s"@en ;
    dcterms:description [ rdfs:label "decade"@en ;
            dcterms:creator "Wikidata contributors" ;
            dcterms:license <https://creativecommons.org/publicdomain/mark/1.0/> ;
            dcterms:rights <https://creativecommons.org/publicdomain/mark/1.0/> ;
            dcterms:source <https://www.wikidata.org/wiki/Wikidata:Data_access/en> ],
        "decade"@en ;
    dcterms:identifier "CC00554" ;
    owl:sameAs <http://www.wikidata.org/entity/Q44859> .

cc:CC00555 a owl:NamedIndividual ;
    rdfs:label "1780s"@en ;
    dcterms:description [ rdfs:label "decade"@en ;
            dcterms:creator "Wikidata contributors" ;
            dcterms:license <https://creativecommons.org/publicdomain/mark/1.0/> ;
            dcterms:rights <https://creativecommons.org/publicdomain/mark/1.0/> ;
            dcterms:source <https://www.wikidata.org/wiki/Wikidata:Data_access/en> ],
        "decade"@en ;
    dcterms:identifier "CC00555" ;
    owl:sameAs <http://www.wikidata.org/entity/Q48058> .

cc:CC00556 a owl:NamedIndividual ;
    rdfs:label "1790s"@en ;
    dcterms:description [ rdfs:label "decade"@en ;
            dcterms:creator "Wikidata contributors" ;
            dcterms:license <https://creativecommons.org/publicdomain/mark/1.0/> ;
            dcterms:rights <https://creativecommons.org/publicdomain/mark/1.0/> ;
            dcterms:source <https://www.wikidata.org/wiki/Wikidata:Data_access/en> ],
        "decade"@en ;
    dcterms:identifier "CC00556" ;
    owl:sameAs <http://www.wikidata.org/entity/Q199912> .

cc:CC00557 a owl:NamedIndividual ;
    rdfs:label "1800s"@en ;
    dcterms:description [ rdfs:label "decade"@en ;
            dcterms:creator "Wikidata contributors" ;
            dcterms:license <https://creativecommons.org/publicdomain/mark/1.0/> ;
            dcterms:rights <https://creativecommons.org/publicdomain/mark/1.0/> ;
            dcterms:source <https://www.wikidata.org/wiki/Wikidata:Data_access/en> ],
        "decade"@en ;
    dcterms:identifier "CC00557" ;
    owl:sameAs <http://www.wikidata.org/entity/Q39577> .

cc:CC00558 a owl:NamedIndividual ;
    rdfs:label "1810s"@en ;
    dcterms:description [ rdfs:label "decade"@en ;
            dcterms:creator "Wikidata contributors" ;
            dcterms:license <https://creativecommons.org/publicdomain/mark/1.0/> ;
            dcterms:rights <https://creativecommons.org/publicdomain/mark/1.0/> ;
            dcterms:source <https://www.wikidata.org/wiki/Wikidata:Data_access/en> ],
        "decade"@en ;
    dcterms:identifier "CC00558" ;
    owl:sameAs <http://www.wikidata.org/entity/Q40196> .

cc:CC00559 a owl:NamedIndividual ;
    rdfs:label "1820s"@en ;
    dcterms:description [ rdfs:label "decade"@en ;
            dcterms:creator "Wikidata contributors" ;
            dcterms:license <https://creativecommons.org/publicdomain/mark/1.0/> ;
            dcterms:rights <https://creativecommons.org/publicdomain/mark/1.0/> ;
            dcterms:source <https://www.wikidata.org/wiki/Wikidata:Data_access/en> ],
        "decade"@en ;
    dcterms:identifier "CC00559" ;
    owl:sameAs <http://www.wikidata.org/entity/Q44659> .

cc:CC00560 a owl:NamedIndividual ;
    rdfs:label "1830s"@en ;
    dcterms:description [ rdfs:label "decade"@en ;
            dcterms:creator "Wikidata contributors" ;
            dcterms:license <https://creativecommons.org/publicdomain/mark/1.0/> ;
            dcterms:rights <https://creativecommons.org/publicdomain/mark/1.0/> ;
            dcterms:source <https://www.wikidata.org/wiki/Wikidata:Data_access/en> ],
        "decade"@en ;
    dcterms:identifier "CC00560" ;
    owl:sameAs <http://www.wikidata.org/entity/Q39484> .

cc:CC00561 a owl:NamedIndividual ;
    rdfs:label "1840s"@en ;
    dcterms:description [ rdfs:label "decade"@en ;
            dcterms:creator "Wikidata contributors" ;
            dcterms:license <https://creativecommons.org/publicdomain/mark/1.0/> ;
            dcterms:rights <https://creativecommons.org/publicdomain/mark/1.0/> ;
            dcterms:source <https://www.wikidata.org/wiki/Wikidata:Data_access/en> ],
        "decade"@en ;
    dcterms:identifier "CC00561" ;
    owl:sameAs <http://www.wikidata.org/entity/Q38324> .

cc:CC00562 a owl:NamedIndividual ;
    rdfs:label "1850s"@en ;
    dcterms:description [ rdfs:label "decade"@en ;
            dcterms:creator "Wikidata contributors" ;
            dcterms:license <https://creativecommons.org/publicdomain/mark/1.0/> ;
            dcterms:rights <https://creativecommons.org/publicdomain/mark/1.0/> ;
            dcterms:source <https://www.wikidata.org/wiki/Wikidata:Data_access/en> ],
        "decade"@en ;
    dcterms:identifier "CC00562" ;
    owl:sameAs <http://www.wikidata.org/entity/Q40927> .

cc:CC00563 a owl:NamedIndividual ;
    rdfs:label "1860s"@en ;
    dcterms:description [ rdfs:label "decade"@en ;
            dcterms:creator "Wikidata contributors" ;
            dcterms:license <https://creativecommons.org/publicdomain/mark/1.0/> ;
            dcterms:rights <https://creativecommons.org/publicdomain/mark/1.0/> ;
            dcterms:source <https://www.wikidata.org/wiki/Wikidata:Data_access/en> ],
        "decade"@en ;
    dcterms:identifier "CC00563" ;
    owl:sameAs <http://www.wikidata.org/entity/Q39844> .

cc:CC00564 a owl:NamedIndividual ;
    rdfs:label "1870s"@en ;
    dcterms:description [ rdfs:label "decade"@en ;
            dcterms:creator "Wikidata contributors" ;
            dcterms:license <https://creativecommons.org/publicdomain/mark/1.0/> ;
            dcterms:rights <https://creativecommons.org/publicdomain/mark/1.0/> ;
            dcterms:source <https://www.wikidata.org/wiki/Wikidata:Data_access/en> ],
        "decade"@en ;
    dcterms:identifier "CC00564" ;
    owl:sameAs <http://www.wikidata.org/entity/Q39847> .

cc:CC00565 a owl:NamedIndividual ;
    rdfs:label "1880s"@en ;
    dcterms:description [ rdfs:label "decade"@en ;
            dcterms:creator "Wikidata contributors" ;
            dcterms:license <https://creativecommons.org/publicdomain/mark/1.0/> ;
            dcterms:rights <https://creativecommons.org/publicdomain/mark/1.0/> ;
            dcterms:source <https://www.wikidata.org/wiki/Wikidata:Data_access/en> ],
        "decade"@en ;
    dcterms:identifier "CC00565" ;
    owl:sameAs <http://www.wikidata.org/entity/Q38674> .

cc:CC00566 a owl:NamedIndividual ;
    rdfs:label "1890s"@en ;
    dcterms:description [ rdfs:label "decade"@en ;
            dcterms:creator "Wikidata contributors" ;
            dcterms:license <https://creativecommons.org/publicdomain/mark/1.0/> ;
            dcterms:rights <https://creativecommons.org/publicdomain/mark/1.0/> ;
            dcterms:source <https://www.wikidata.org/wiki/Wikidata:Data_access/en> ],
        "decade"@en ;
    dcterms:identifier "CC00566" ;
    owl:sameAs <http://www.wikidata.org/entity/Q38971> .

cc:CC00567 a owl:NamedIndividual ;
    rdfs:label "1900s"@en ;
    dcterms:description [ rdfs:label "decade"@en ;
            dcterms:creator "Wikidata contributors" ;
            dcterms:license <https://creativecommons.org/publicdomain/mark/1.0/> ;
            dcterms:rights <https://creativecommons.org/publicdomain/mark/1.0/> ;
            dcterms:source <https://www.wikidata.org/wiki/Wikidata:Data_access/en> ],
        "decade"@en ;
    dcterms:identifier "CC00567" ;
    owl:sameAs <http://www.wikidata.org/entity/Q36574> .

cc:CC00568 a owl:NamedIndividual ;
    rdfs:label "1910s"@en ;
    dcterms:description [ rdfs:label "decade"@en ;
            dcterms:creator "Wikidata contributors" ;
            dcterms:license <https://creativecommons.org/publicdomain/mark/1.0/> ;
            dcterms:rights <https://creativecommons.org/publicdomain/mark/1.0/> ;
            dcterms:source <https://www.wikidata.org/wiki/Wikidata:Data_access/en> ],
        "decade"@en ;
    dcterms:identifier "CC00568" ;
    owl:sameAs <http://www.wikidata.org/entity/Q36585> .

cc:CC00569 a owl:NamedIndividual ;
    rdfs:label "1920s"@en ;
    dcterms:description [ rdfs:label "decade"@en ;
            dcterms:creator "Wikidata contributors" ;
            dcterms:license <https://creativecommons.org/publicdomain/mark/1.0/> ;
            dcterms:rights <https://creativecommons.org/publicdomain/mark/1.0/> ;
            dcterms:source <https://www.wikidata.org/wiki/Wikidata:Data_access/en> ],
        "decade"@en ;
    dcterms:identifier "CC00569" ;
    owl:sameAs <http://www.wikidata.org/entity/Q35736> .

cc:CC00570 a owl:NamedIndividual ;
    rdfs:label "1930s"@en ;
    dcterms:description [ rdfs:label "decade"@en ;
            dcterms:creator "Wikidata contributors" ;
            dcterms:license <https://creativecommons.org/publicdomain/mark/1.0/> ;
            dcterms:rights <https://creativecommons.org/publicdomain/mark/1.0/> ;
            dcterms:source <https://www.wikidata.org/wiki/Wikidata:Data_access/en> ],
        "decade"@en ;
    dcterms:identifier "CC00570" ;
    owl:sameAs <http://www.wikidata.org/entity/Q35702> .

cc:CC00571 a owl:NamedIndividual ;
    rdfs:label "1940s"@en ;
    dcterms:description [ rdfs:label "decade"@en ;
            dcterms:creator "Wikidata contributors" ;
            dcterms:license <https://creativecommons.org/publicdomain/mark/1.0/> ;
            dcterms:rights <https://creativecommons.org/publicdomain/mark/1.0/> ;
            dcterms:source <https://www.wikidata.org/wiki/Wikidata:Data_access/en> ],
        "decade"@en ;
    dcterms:identifier "CC00571" ;
    owl:sameAs <http://www.wikidata.org/entity/Q36561> .

cc:CC00572 a owl:NamedIndividual ;
    rdfs:label "1950s"@en ;
    dcterms:description [ rdfs:label "decade"@en ;
            dcterms:creator "Wikidata contributors" ;
            dcterms:license <https://creativecommons.org/publicdomain/mark/1.0/> ;
            dcterms:rights <https://creativecommons.org/publicdomain/mark/1.0/> ;
            dcterms:source <https://www.wikidata.org/wiki/Wikidata:Data_access/en> ],
        "decade"@en ;
    dcterms:identifier "CC00572" ;
    owl:sameAs <http://www.wikidata.org/entity/Q36297> .

cc:CC00573 a owl:NamedIndividual ;
    rdfs:label "1960s"@en ;
    dcterms:description [ rdfs:label "decade"@en ;
            dcterms:creator "Wikidata contributors" ;
            dcterms:license <https://creativecommons.org/publicdomain/mark/1.0/> ;
            dcterms:rights <https://creativecommons.org/publicdomain/mark/1.0/> ;
            dcterms:source <https://www.wikidata.org/wiki/Wikidata:Data_access/en> ],
        "decade"@en ;
    dcterms:identifier "CC00573" ;
    owl:sameAs <http://www.wikidata.org/entity/Q35724> .

cc:CC00574 a owl:NamedIndividual ;
    rdfs:label "1970s"@en ;
    dcterms:description [ rdfs:label "decade"@en ;
            dcterms:creator "Wikidata contributors" ;
            dcterms:license <https://creativecommons.org/publicdomain/mark/1.0/> ;
            dcterms:rights <https://creativecommons.org/publicdomain/mark/1.0/> ;
            dcterms:source <https://www.wikidata.org/wiki/Wikidata:Data_access/en> ],
        "decade"@en ;
    dcterms:identifier "CC00574" ;
    owl:sameAs <http://www.wikidata.org/entity/Q35014> .

cc:CC00575 a owl:NamedIndividual ;
    rdfs:label "1980s"@en ;
    dcterms:description [ rdfs:label "decade"@en ;
            dcterms:creator "Wikidata contributors" ;
            dcterms:license <https://creativecommons.org/publicdomain/mark/1.0/> ;
            dcterms:rights <https://creativecommons.org/publicdomain/mark/1.0/> ;
            dcterms:source <https://www.wikidata.org/wiki/Wikidata:Data_access/en> ],
        "decade"@en ;
    dcterms:identifier "CC00575" ;
    owl:sameAs <http://www.wikidata.org/entity/Q34644> .

cc:CC00576 a owl:NamedIndividual ;
    rdfs:label "1990s"@en ;
    dcterms:description [ rdfs:label "decade"@en ;
            dcterms:creator "Wikidata contributors" ;
            dcterms:license <https://creativecommons.org/publicdomain/mark/1.0/> ;
            dcterms:rights <https://creativecommons.org/publicdomain/mark/1.0/> ;
            dcterms:source <https://www.wikidata.org/wiki/Wikidata:Data_access/en> ],
        "decade"@en ;
    dcterms:identifier "CC00576" ;
    owl:sameAs <http://www.wikidata.org/entity/Q34653> .

cc:CC00577 a owl:NamedIndividual ;
    rdfs:label "2000s"@en ;
    dcterms:description [ rdfs:label "decade"@en ;
            dcterms:creator "Wikidata contributors" ;
            dcterms:license <https://creativecommons.org/publicdomain/mark/1.0/> ;
            dcterms:rights <https://creativecommons.org/publicdomain/mark/1.0/> ;
            dcterms:source <https://www.wikidata.org/wiki/Wikidata:Data_access/en> ],
        "decade"@en ;
    dcterms:identifier "CC00577" ;
    owl:sameAs <http://www.wikidata.org/entity/Q35024> .

cc:CC00578 a owl:NamedIndividual ;
    rdfs:label "2010s"@en ;
    dcterms:description [ rdfs:label "decade"@en ;
            dcterms:creator "Wikidata contributors" ;
            dcterms:license <https://creativecommons.org/publicdomain/mark/1.0/> ;
            dcterms:rights <https://creativecommons.org/publicdomain/mark/1.0/> ;
            dcterms:source <https://www.wikidata.org/wiki/Wikidata:Data_access/en> ],
        "decade"@en ;
    dcterms:identifier "CC00578" ;
    owl:sameAs <http://www.wikidata.org/entity/Q19022> .

cc:CC00579 a owl:NamedIndividual ;
    rdfs:label "2020s"@en ;
    dcterms:description [ rdfs:label "decade"@en ;
            dcterms:creator "Wikidata contributors" ;
            dcterms:license <https://creativecommons.org/publicdomain/mark/1.0/> ;
            dcterms:rights <https://creativecommons.org/publicdomain/mark/1.0/> ;
            dcterms:source <https://www.wikidata.org/wiki/Wikidata:Data_access/en> ],
        "decade"@en ;
    dcterms:identifier "CC00579" ;
    owl:sameAs <http://www.wikidata.org/entity/Q534495> .

cc:CC00582 a owl:NamedIndividual ;
    rdfs:label "ceremonial costume"@en ;
    dcterms:description [ rdfs:label "Clothing or other apparel having a primarily ceremonial or ritual purpose."@en ;
            dcterms:creator "The J. Paul Getty Trust" ;
            dcterms:license <https://opendatacommons.org/licenses/by/1-0/> ;
            dcterms:rights <https://rightsstatements.org/vocab/InC/1.0/> ;
            dcterms:source <http://www.getty.edu/research/tools/vocabularies/aat/> ],
        "Clothing or other apparel having a primarily ceremonial or ritual purpose."@en ;
    dcterms:identifier "CC00582" ;
    owl:sameAs <http://www.wikidata.org/entity/Q5064153> .

cc:CC00583 a owl:NamedIndividual ;
    rdfs:label "costume"@en ;
    dcterms:description [ rdfs:label "The dress of an actor or actress who is representing a character on stage or in film, or of any other person who is playing a role or impersonating a character, as during Carnevale or Halloween."@en ;
            dcterms:creator "The J. Paul Getty Trust" ;
            dcterms:license <https://opendatacommons.org/licenses/by/1-0/> ;
            dcterms:rights <https://rightsstatements.org/vocab/InC/1.0/> ;
            dcterms:source <http://www.getty.edu/research/tools/vocabularies/aat/> ],
        "The dress of an actor or actress who is representing a character on stage or in film, or of any other person who is playing a role or impersonating a character, as during Carnevale or Halloween."@en ;
    dcterms:identifier "CC00583" ;
    owl:sameAs <http://www.wikidata.org/entity/Q1410477> .

cc:CC00584 a owl:NamedIndividual ;
    rdfs:label "moir"@en ;
    dcterms:description [ rdfs:label "Patterns having a watered or rippled look. To refer to the optical illusion of movement caused by intersecting lines, use \"moir effect.\""@en ;
            dcterms:creator "The J. Paul Getty Trust" ;
            dcterms:license <https://opendatacommons.org/licenses/by/1-0/> ;
            dcterms:rights <https://rightsstatements.org/vocab/InC/1.0/> ;
            dcterms:source <http://www.getty.edu/research/tools/vocabularies/aat/> ],
        "Patterns having a watered or rippled look. To refer to the optical illusion of movement caused by intersecting lines, use \"moir effect.\""@en ;
    dcterms:identifier "CC00584" ;
    owl:sameAs <http://www.wikidata.org/entity/Q26468> .

cc:CC00586 a owl:NamedIndividual ;
    rdfs:label "paisley"@en ;
    dcterms:description [ rdfs:label "Motif derived from the the boteh, copied from Kashmiri shawls by the woollen manufacturers of Paisley, Scotland in the 19th century, and becoming popular in Britain, France, and North America. It occurs in many variations and with numerous ancillary motifs, particularly in textile patterns."@en ;
            dcterms:creator "The J. Paul Getty Trust" ;
            dcterms:license <https://opendatacommons.org/licenses/by/1-0/> ;
            dcterms:rights <https://rightsstatements.org/vocab/InC/1.0/> ;
            dcterms:source <http://www.getty.edu/research/tools/vocabularies/aat/> ],
        "Motif derived from the the boteh, copied from Kashmiri shawls by the woollen manufacturers of Paisley, Scotland in the 19th century, and becoming popular in Britain, France, and North America. It occurs in many variations and with numerous ancillary motifs, particularly in textile patterns."@en ;
    dcterms:identifier "CC00586" ;
    owl:sameAs <http://www.wikidata.org/entity/Q937704> .

cc:CC00587 a owl:NamedIndividual ;
    rdfs:label "chevron"@en ;
    dcterms:description [ rdfs:label "Simple geometric forms composed of Vs used singly, in a vertical series, or in a string to form a zigzag."@en ;
            dcterms:creator "The J. Paul Getty Trust" ;
            dcterms:license <https://opendatacommons.org/licenses/by/1-0/> ;
            dcterms:rights <https://rightsstatements.org/vocab/InC/1.0/> ;
            dcterms:source <http://www.getty.edu/research/tools/vocabularies/aat/> ],
        "Simple geometric forms composed of Vs used singly, in a vertical series, or in a string to form a zigzag."@en ;
    dcterms:identifier "CC00587" ;
    owl:sameAs <http://vocab.getty.edu/aat/300009766> .

cc:CC00588 a owl:NamedIndividual ;
    rdfs:label "houndstooth"@en ;
    dcterms:description [ rdfs:label "An irregular check pattern, most commonly appearing in woven fabric."@en ;
            dcterms:creator "The J. Paul Getty Trust" ;
            dcterms:license <https://opendatacommons.org/licenses/by/1-0/> ;
            dcterms:rights <https://rightsstatements.org/vocab/InC/1.0/> ;
            dcterms:source <http://www.getty.edu/research/tools/vocabularies/aat/> ],
        "An irregular check pattern, most commonly appearing in woven fabric."@en ;
    dcterms:identifier "CC00588" ;
    owl:sameAs <http://www.wikidata.org/entity/Q911389> .

cc:CC00589 a owl:NamedIndividual ;
    rdfs:label "check"@en ;
    dcterms:description [ rdfs:label "pattern of intersecting vertical and horizontal lines"@en ;
            dcterms:creator "Wikidata contributors" ;
            dcterms:license <https://creativecommons.org/publicdomain/mark/1.0/> ;
            dcterms:rights <https://creativecommons.org/publicdomain/mark/1.0/> ;
            dcterms:source <https://www.wikidata.org/wiki/Wikidata:Data_access/en> ],
        "pattern of intersecting vertical and horizontal lines"@en ;
    dcterms:identifier "CC00589" ;
    owl:sameAs <http://www.wikidata.org/entity/Q14290457> .

cc:CC00590 a owl:NamedIndividual ;
    rdfs:label "polka dots"@en ;
    dcterms:description [ rdfs:label "Round dots of uniform size repeated at regular intervals so as to form a pattern, usually designated as a pattern for fabric, or otherwise applied to planographic surfaces."@en ;
            dcterms:creator "The J. Paul Getty Trust" ;
            dcterms:license <https://opendatacommons.org/licenses/by/1-0/> ;
            dcterms:rights <https://rightsstatements.org/vocab/InC/1.0/> ;
            dcterms:source <http://www.getty.edu/research/tools/vocabularies/aat/> ],
        "Round dots of uniform size repeated at regular intervals so as to form a pattern, usually designated as a pattern for fabric, or otherwise applied to planographic surfaces."@en ;
    dcterms:identifier "CC00590" ;
    owl:sameAs <http://www.wikidata.org/entity/Q2429962> .

cc:CC00591 a owl:NamedIndividual ;
    rdfs:label "ikat"@en ;
    dcterms:description [ rdfs:label "Technique of resist dyeing in which hanks of thread are bound and dyed before being woven into fabric."@en ;
            dcterms:creator "The J. Paul Getty Trust" ;
            dcterms:license <https://opendatacommons.org/licenses/by/1-0/> ;
            dcterms:rights <https://rightsstatements.org/vocab/InC/1.0/> ;
            dcterms:source <http://www.getty.edu/research/tools/vocabularies/aat/> ],
        "Technique of resist dyeing in which hanks of thread are bound and dyed before being woven into fabric."@en ;
    dcterms:identifier "CC00591" ;
    owl:sameAs <http://www.wikidata.org/entity/Q140101> .

cc:CC00592 a owl:NamedIndividual ;
    rdfs:label "camouflage"@en ;
    dcterms:description [ rdfs:label "The technique of disguising the appearance of beings or things so as to make them blend into their surroundings."@en ;
            dcterms:creator "The J. Paul Getty Trust" ;
            dcterms:license <https://opendatacommons.org/licenses/by/1-0/> ;
            dcterms:rights <https://rightsstatements.org/vocab/InC/1.0/> ;
            dcterms:source <http://www.getty.edu/research/tools/vocabularies/aat/> ],
        "The technique of disguising the appearance of beings or things so as to make them blend into their surroundings."@en ;
    dcterms:identifier "CC00592" ;
    owl:sameAs <http://www.wikidata.org/entity/Q196113> .

cc:CC00593 a owl:NamedIndividual ;
    rdfs:label "animal print"@en ;
    dcterms:description [ rdfs:label "A print made to resemble the pattern of the skin and fur of an animal such as a leopard, cheetah, jaguar, zebra, tiger, giraffe, or snake."@en ;
            dcterms:creator "The J. Paul Getty Trust" ;
            dcterms:license <https://opendatacommons.org/licenses/by/1-0/> ;
            dcterms:rights <https://rightsstatements.org/vocab/InC/1.0/> ;
            dcterms:source <http://www.getty.edu/research/tools/vocabularies/aat/> ],
        "A print made to resemble the pattern of the skin and fur of an animal such as a leopard, cheetah, jaguar, zebra, tiger, giraffe, or snake."@en ;
    dcterms:identifier "CC00593" ;
    owl:sameAs <http://www.wikidata.org/entity/Q4764964> .

cc:CC00596 a owl:NamedIndividual ;
    rdfs:label "bird's-eye twill"@en ;
    dcterms:description [ rdfs:label "A lozenge twill with a small weave unit which has an interlacing forming a spot in the center of each lozenge."@en ;
            dcterms:creator "The J. Paul Getty Trust" ;
            dcterms:license <https://opendatacommons.org/licenses/by/1-0/> ;
            dcterms:rights <https://rightsstatements.org/vocab/InC/1.0/> ;
            dcterms:source <http://www.getty.edu/research/tools/vocabularies/aat/> ],
        "A lozenge twill with a small weave unit which has an interlacing forming a spot in the center of each lozenge."@en ;
    dcterms:identifier "CC00596" ;
    owl:sameAs <http://www.wikidata.org/entity/Q2553036> .

cc:CC00597 a owl:NamedIndividual ;
    rdfs:label "ombr"@en ;
    dcterms:description [ rdfs:label "The effect of graduated or shaded color in textiles, created through the weave or by dyeing. The effect may be monochromatic or polychromatic. The term is most often used for textiles, but may also be extended to painted or colored surfaces that display a graduated shading effect."@en ;
            dcterms:creator "The J. Paul Getty Trust" ;
            dcterms:license <https://opendatacommons.org/licenses/by/1-0/> ;
            dcterms:rights <https://rightsstatements.org/vocab/InC/1.0/> ;
            dcterms:source <http://www.getty.edu/research/tools/vocabularies/aat/> ],
        "The effect of graduated or shaded color in textiles, created through the weave or by dyeing. The effect may be monochromatic or polychromatic. The term is most often used for textiles, but may also be extended to painted or colored surfaces that display a graduated shading effect."@en ;
    dcterms:identifier "CC00597" ;
    owl:sameAs <http://www.wikidata.org/entity/Q1700971> .

cc:CC00598 a owl:NamedIndividual ;
    rdfs:label "dress shield"@en ;
    dcterms:description [ rdfs:label "Shaped pieces of absorbent and rubberized or plastic-coated materials often padded or occasionally filled with deodorizing herbs; attached to or placed inside a garment, as in the underarm of a dress or blouse, to prevent the garment from being soiled by perspiration."@en ;
            dcterms:creator "The J. Paul Getty Trust" ;
            dcterms:license <https://opendatacommons.org/licenses/by/1-0/> ;
            dcterms:rights <https://rightsstatements.org/vocab/InC/1.0/> ;
            dcterms:source <http://www.getty.edu/research/tools/vocabularies/aat/> ],
        "Shaped pieces of absorbent and rubberized or plastic-coated materials often padded or occasionally filled with deodorizing herbs; attached to or placed inside a garment, as in the underarm of a dress or blouse, to prevent the garment from being soiled by perspiration."@en ;
    dcterms:identifier "CC00598" ;
    owl:sameAs <http://www.wikidata.org/entity/Q63505185> .

cc:CC00599 a owl:NamedIndividual ;
    rdfs:label "bow"@en ;
    dcterms:description [ rdfs:label "Applied clothing accessories that may be made of rope, ribbon or fabric. These consist of knots with two loops and two ends, fixed into decorative elements attached to clothing or other objects."@en ;
            dcterms:creator "The J. Paul Getty Trust" ;
            dcterms:license <https://opendatacommons.org/licenses/by/1-0/> ;
            dcterms:rights <https://rightsstatements.org/vocab/InC/1.0/> ;
            dcterms:source <http://www.getty.edu/research/tools/vocabularies/aat/> ],
        "Applied clothing accessories that may be made of rope, ribbon or fabric. These consist of knots with two loops and two ends, fixed into decorative elements attached to clothing or other objects."@en ;
    dcterms:identifier "CC00599" ;
    owl:sameAs <http://www.wikidata.org/entity/Q2238808> .

cc:CC00601 a owl:NamedIndividual ;
    rdfs:label "bodysuit"@en ;
    dcterms:description [ rdfs:label "One-piece form-fitting garment that covers the torso and the crotch"@en ;
            dcterms:creator "Wikidata contributors" ;
            dcterms:license <https://creativecommons.org/publicdomain/mark/1.0/> ;
            dcterms:rights <https://creativecommons.org/publicdomain/mark/1.0/> ;
            dcterms:source <https://www.wikidata.org/wiki/Wikidata:Data_access/en> ],
        "One-piece form-fitting garment that covers the torso and the crotch"@en ;
    dcterms:identifier "CC00601" ;
    owl:sameAs <http://www.wikidata.org/entity/Q890119> .

cc:CC00609 a owl:NamedIndividual ;
    rdfs:label "underpants"@en ;
    dcterms:description [ rdfs:label "Garments worn next to the body and under main garments having leg openings or short or long legs."@en ;
            dcterms:creator "The J. Paul Getty Trust" ;
            dcterms:license <https://opendatacommons.org/licenses/by/1-0/> ;
            dcterms:rights <https://rightsstatements.org/vocab/InC/1.0/> ;
            dcterms:source <http://www.getty.edu/research/tools/vocabularies/aat/> ],
        "Garments worn next to the body and under main garments having leg openings or short or long legs."@en ;
    dcterms:identifier "CC00609" ;
    owl:sameAs <http://vocab.getty.edu/aat/300220740>,
        <http://www.wikidata.org/entity/Q39908> .

cc:CC00612 a owl:NamedIndividual ;
    rdfs:label "bag"@en ;
    dcterms:description [ rdfs:label "Small, medium, or large-sized soft or rigid receptacles, intended for carrying personal articles and usually used as ladies' costume accessories. A bag is closed in on all sides except at the top, where also it generally can be closed, and usually having handles or straps for carrying on the shoulder or in the hand."@en ;
            dcterms:creator "The J. Paul Getty Trust" ;
            dcterms:license <https://opendatacommons.org/licenses/by/1-0/> ;
            dcterms:rights <https://rightsstatements.org/vocab/InC/1.0/> ;
            dcterms:source <http://www.getty.edu/research/tools/vocabularies/aat/> ],
        "Small, medium, or large-sized soft or rigid receptacles, intended for carrying personal articles and usually used as ladies' costume accessories. A bag is closed in on all sides except at the top, where also it generally can be closed, and usually having handles or straps for carrying on the shoulder or in the hand."@en ;
    dcterms:identifier "CC00612" ;
    owl:sameAs <http://vocab.getty.edu/aat/300198926>,
        <http://www.wikidata.org/entity/Q1323314> .

cc:CC00629 a owl:NamedIndividual ;
    rdfs:label "shirt collar"@en ;
    dcterms:description [ rdfs:label "collar like that of a dress shirt, with a small stand"@en ;
            dcterms:creator "Wikidata contributors" ;
            dcterms:license <https://creativecommons.org/publicdomain/mark/1.0/> ;
            dcterms:rights <https://creativecommons.org/publicdomain/mark/1.0/> ;
            dcterms:source <https://www.wikidata.org/wiki/Wikidata:Data_access/en> ],
        "collar like that of a dress shirt, with a small stand"@en ;
    dcterms:identifier "CC00629" ;
    owl:sameAs <http://www.wikidata.org/entity/Q29473382> .

cc:CC00012 a owl:NamedIndividual ;
    rdfs:label "velcro"@en ;
    dcterms:description [ rdfs:label "Trademark name for fastening material consisting of opposing pieces of fabric, one with a dense arrangement of tiny nylon hooks and the other with a dense nylon pile, that interlock when pressed together."@en ;
            dcterms:creator "The J. Paul Getty Trust" ;
            dcterms:license <https://opendatacommons.org/licenses/by/1-0/> ;
            dcterms:rights <https://rightsstatements.org/vocab/InC/1.0/> ;
            dcterms:source <http://www.getty.edu/research/tools/vocabularies/aat/> ],
        "Trademark name for fastening material consisting of opposing pieces of fabric, one with a dense arrangement of tiny nylon hooks and the other with a dense nylon pile, that interlock when pressed together."@en ;
    dcterms:identifier "CC00012" ;
    owl:sameAs <http://vocab.getty.edu/aat/300239275>,
        <http://www.wikidata.org/entity/Q15411420> .

cc:CC00029 a owl:NamedIndividual ;
    rdfs:label "band collar"@en ;
    dcterms:description [ rdfs:label "Flat, stand-up collars, starched, wired, or otherwise stiffened, especially those commonly worn by men and women in the 17th century."@en ;
            dcterms:creator "The J. Paul Getty Trust" ;
            dcterms:license <https://opendatacommons.org/licenses/by/1-0/> ;
            dcterms:rights <https://rightsstatements.org/vocab/InC/1.0/> ;
            dcterms:source <http://www.getty.edu/vow/AATFullDisplay?find=band&logic=AND&note=&english=N&prev_page=1&subjectid=300217242> ],
        "Flat, stand-up collars, starched, wired, or otherwise stiffened, especially those commonly worn by men and women in the 17th century."@en ;
    dcterms:identifier "CC00029" ;
    owl:sameAs <http://vocab.getty.edu/aat/300217242>,
        <http://www.wikidata.org/entity/Q4854234> .

cc:CC00049 a owl:NamedIndividual ;
    rdfs:label "beige"@en ;
    dcterms:description [ rdfs:label "A variable color generally light grayish-yellowish brown, originally referring to the color of unbleached wool. (AAT)"@en ;
            dcterms:creator "The J. Paul Getty Trust" ;
            dcterms:license <https://opendatacommons.org/licenses/by/1-0/> ;
            dcterms:rights <https://rightsstatements.org/vocab/InC/1.0/> ;
            dcterms:source <http://www.getty.edu/research/tools/vocabularies/aat/> ],
        "A variable color generally light grayish-yellowish brown, originally referring to the color of unbleached wool. (AAT)"@en ;
    dcterms:identifier "CC00049" ;
    owl:sameAs <http://vocab.getty.edu/aat/300266234> .

cc:CC00050 a owl:NamedIndividual ;
    rdfs:label "black"@en ;
    dcterms:description [ rdfs:label "UCL (Universal Color Language) standard color name identifying a range of blackish colors. More specifically, black is an achromatic color of maximum darkness, referring to objects having little or no hue owing to the absorption of almost all light in the visible spectrum. In the context of pigments, black is theoretically the mixture of all colors. In the context of colors of light, black is the absence of light. (AAT)"@en ;
            dcterms:creator "The J. Paul Getty Trust" ;
            dcterms:license <https://opendatacommons.org/licenses/by/1-0/> ;
            dcterms:rights <https://rightsstatements.org/vocab/InC/1.0/> ;
            dcterms:source <http://www.getty.edu/research/tools/vocabularies/aat/> ],
        "UCL (Universal Color Language) standard color name identifying a range of blackish colors. More specifically, black is an achromatic color of maximum darkness, referring to objects having little or no hue owing to the absorption of almost all light in the visible spectrum. In the context of pigments, black is theoretically the mixture of all colors. In the context of colors of light, black is the absence of light. (AAT)"@en ;
    dcterms:identifier "CC00050" ;
    owl:sameAs <http://vocab.getty.edu/aat/300130920> .

cc:CC00051 a owl:NamedIndividual ;
    rdfs:label "blue"@en ;
    dcterms:description [ rdfs:label "Hue name for one of the three primary additive colors; that portion of the spectrum lying between green and violet, with a wavelength of about 420 to 490 nanometers, which is the shortest wavelength range of the three primary colors. The term may refer to any of this group of colors that vary in lightness and saturation. An example of blue color in nature is that of a clear sky during the day. (AAT)"@en ;
            dcterms:creator "The J. Paul Getty Trust" ;
            dcterms:license <https://opendatacommons.org/licenses/by/1-0/> ;
            dcterms:rights <https://rightsstatements.org/vocab/InC/1.0/> ;
            dcterms:source <http://www.getty.edu/research/tools/vocabularies/aat/> ],
        "Hue name for one of the three primary additive colors; that portion of the spectrum lying between green and violet, with a wavelength of about 420 to 490 nanometers, which is the shortest wavelength range of the three primary colors. The term may refer to any of this group of colors that vary in lightness and saturation. An example of blue color in nature is that of a clear sky during the day. (AAT)"@en ;
    dcterms:identifier "CC00051" ;
    owl:sameAs <http://vocab.getty.edu/aat/300129361> .

cc:CC00052 a owl:NamedIndividual ;
    rdfs:label "brown"@en ;
    dcterms:description [ rdfs:label "Hue name for any dull reddish-yellowish or orangish color of low brightness and saturation, resembling the color of wood or earth. Brown is a low luminance color that is typically produced by adding black or their complementary colors to red, orange, or yellow paint. It is considered an earth tone and has an unlimited numbers of shades. (AAT)"@en ;
            dcterms:creator "The J. Paul Getty Trust" ;
            dcterms:license <https://opendatacommons.org/licenses/by/1-0/> ;
            dcterms:rights <https://rightsstatements.org/vocab/InC/1.0/> ;
            dcterms:source <http://www.getty.edu/research/tools/vocabularies/aat/> ],
        "Hue name for any dull reddish-yellowish or orangish color of low brightness and saturation, resembling the color of wood or earth. Brown is a low luminance color that is typically produced by adding black or their complementary colors to red, orange, or yellow paint. It is considered an earth tone and has an unlimited numbers of shades. (AAT)"@en ;
    dcterms:identifier "CC00052" ;
    owl:sameAs <http://vocab.getty.edu/aat/300127490> .

cc:CC00053 a owl:NamedIndividual ;
    rdfs:label "burgundy"@en ;
    dcterms:description [ rdfs:label "dark red color associated with the Burgundy wine"@en ;
            dcterms:creator "Wikidata contributors" ;
            dcterms:license <https://creativecommons.org/publicdomain/mark/1.0/> ;
            dcterms:rights <https://creativecommons.org/publicdomain/mark/1.0/> ;
            dcterms:source <https://www.wikidata.org/wiki/Wikidata:Data_access/en> ],
        "dark red color associated with the Burgundy wine"@en ;
    dcterms:identifier "CC00053" ;
    owl:sameAs <http://www.wikidata.org/entity/Q797446> .

cc:CC00054 a owl:NamedIndividual ;
    rdfs:label "coral"@en ;
    dcterms:description [ rdfs:label "Color of coral."@en ;
            dcterms:creator "Wikidata contributors" ;
            dcterms:license <https://creativecommons.org/publicdomain/mark/1.0/> ;
            dcterms:rights <https://creativecommons.org/publicdomain/mark/1.0/> ;
            dcterms:source <https://www.wikidata.org/wiki/Wikidata:Data_access/en> ],
        "Color of coral."@en ;
    dcterms:identifier "CC00054" ;
    owl:sameAs <http://www.wikidata.org/entity/Q2411228> .

cc:CC00055 a owl:NamedIndividual ;
    rdfs:label "cream"@en ;
    dcterms:description [ rdfs:label "Refers to a warm off-white color of various shades, reminiscent of the color of cream, which is the whitish-yellowish fatty thick material in milk that floats to the top."@en ;
            dcterms:creator "The J. Paul Getty Trust" ;
            dcterms:license <https://opendatacommons.org/licenses/by/1-0/> ;
            dcterms:rights <https://rightsstatements.org/vocab/InC/1.0/> ;
            dcterms:source <http://www.getty.edu/research/tools/vocabularies/aat/> ],
        "Refers to a warm off-white color of various shades, reminiscent of the color of cream, which is the whitish-yellowish fatty thick material in milk that floats to the top."@en ;
    dcterms:identifier "CC00055" ;
    owl:sameAs <http://vocab.getty.edu/aat/300266242> .

cc:CC00056 a owl:NamedIndividual ;
    rdfs:label "fuchsia"@en ;
    dcterms:description [ rdfs:label "Variable color name referring to bright pinkish colors similar to those of blooms of the fuchsia plant."@en ;
            dcterms:creator "The J. Paul Getty Trust" ;
            dcterms:license <https://opendatacommons.org/licenses/by/1-0/> ;
            dcterms:rights <https://rightsstatements.org/vocab/InC/1.0/> ;
            dcterms:source <http://www.getty.edu/research/tools/vocabularies/aat/> ],
        "Variable color name referring to bright pinkish colors similar to those of blooms of the fuchsia plant."@en ;
    dcterms:identifier "CC00056" ;
    owl:sameAs <http://vocab.getty.edu/aat/300311477> .

cc:CC00057 a owl:NamedIndividual ;
    rdfs:label "gold"@en ;
    dcterms:description [ rdfs:label "A range of yellowish colors, typically with undertones of red or brown, resembling the color of the lustrous metal, gold. (AAT)"@en ;
            dcterms:creator "The J. Paul Getty Trust" ;
            dcterms:license <https://opendatacommons.org/licenses/by/1-0/> ;
            dcterms:rights <https://rightsstatements.org/vocab/InC/1.0/> ;
            dcterms:source <http://www.getty.edu/research/tools/vocabularies/aat/> ],
        "A range of yellowish colors, typically with undertones of red or brown, resembling the color of the lustrous metal, gold. (AAT)"@en ;
    dcterms:identifier "CC00057" ;
    owl:sameAs <http://vocab.getty.edu/aat/300311191> .

cc:CC00059 a owl:NamedIndividual ;
    rdfs:label "green"@en ;
    dcterms:description [ rdfs:label "Hue name for the color representing that portion of the spectrum that is intermediate between blue and yellow, with wavelengths between 520 and 570 nanometers. The term may refer to any of this group of colors that vary in lightness and saturation. An example of green color in nature is that of growing grass. It is a secondary pigment color (made by combining yellow and blue) and one of the three additive primary colors."@en ;
            dcterms:creator "The J. Paul Getty Trust" ;
            dcterms:license <https://opendatacommons.org/licenses/by/1-0/> ;
            dcterms:rights <https://rightsstatements.org/vocab/InC/1.0/> ;
            dcterms:source <http://www.getty.edu/research/tools/vocabularies/aat/> ],
        "Hue name for the color representing that portion of the spectrum that is intermediate between blue and yellow, with wavelengths between 520 and 570 nanometers. The term may refer to any of this group of colors that vary in lightness and saturation. An example of green color in nature is that of growing grass. It is a secondary pigment color (made by combining yellow and blue) and one of the three additive primary colors."@en ;
    dcterms:identifier "CC00059" ;
    owl:sameAs <http://vocab.getty.edu/aat/300128438> .

cc:CC00060 a owl:NamedIndividual ;
    rdfs:label "lavender"@en ;
    dcterms:description [ rdfs:label "A range of purplish or bluish colors resembling the color of flower of the lavender plant, which is a Mediterranean mint widely cultivated for its narrow aromatic leaves and spikes of flowers that are dried and used in sachets."@en ;
            dcterms:creator "The J. Paul Getty Trust" ;
            dcterms:license <https://opendatacommons.org/licenses/by/1-0/> ;
            dcterms:rights <https://rightsstatements.org/vocab/InC/1.0/> ;
            dcterms:source <http://www.getty.edu/research/tools/vocabularies/aat/> ],
        "A range of purplish or bluish colors resembling the color of flower of the lavender plant, which is a Mediterranean mint widely cultivated for its narrow aromatic leaves and spikes of flowers that are dried and used in sachets."@en ;
    dcterms:identifier "CC00060" ;
    owl:sameAs <http://vocab.getty.edu/aat/300311131> .

cc:CC00061 a owl:NamedIndividual ;
    rdfs:label "maroon"@en ;
    dcterms:description [ rdfs:label "A range of dark reddish or purplish brown colors resembling the color of dyes or colorants made from chestnut bark, derived from trees or shrubs of the genus Castanea of the beech family; from the Italian word for chestnut, \"marrone.\""@en ;
            dcterms:creator "The J. Paul Getty Trust" ;
            dcterms:license <https://opendatacommons.org/licenses/by/1-0/> ;
            dcterms:rights <https://rightsstatements.org/vocab/InC/1.0/> ;
            dcterms:source <http://www.getty.edu/research/tools/vocabularies/aat/> ],
        "A range of dark reddish or purplish brown colors resembling the color of dyes or colorants made from chestnut bark, derived from trees or shrubs of the genus Castanea of the beech family; from the Italian word for chestnut, \"marrone.\""@en ;
    dcterms:identifier "CC00061" ;
    owl:sameAs <http://vocab.getty.edu/aat/300311173> .

cc:CC00063 a owl:NamedIndividual ;
    rdfs:label "navy blue"@en ;
    dcterms:description [ rdfs:label "Range of deep grayish blues, originally named for the color of the British naval uniform."@en ;
            dcterms:creator "The J. Paul Getty Trust" ;
            dcterms:license <https://opendatacommons.org/licenses/by/1-0/> ;
            dcterms:rights <https://rightsstatements.org/vocab/InC/1.0/> ;
            dcterms:source <http://www.getty.edu/research/tools/vocabularies/aat/> ],
        "Range of deep grayish blues, originally named for the color of the British naval uniform."@en ;
    dcterms:identifier "CC00063" ;
    owl:sameAs <http://vocab.getty.edu/aat/300311067> .

cc:CC00064 a owl:NamedIndividual ;
    rdfs:label "orange"@en ;
    dcterms:description [ rdfs:label "Hue name for the color representing that portion of the spectrum that is intermediate between red and yellow, with wavelengths between 585 and 620 nanometers. The term may refer to any of this group of colors that vary in lightness and saturation. An example of orange color in nature is that of the citrus fruit orange, for which the color is named in modern English. It is a secondary pigment color (made by combining yellow and red). (AAT)"@en ;
            dcterms:creator "The J. Paul Getty Trust" ;
            dcterms:license <https://opendatacommons.org/licenses/by/1-0/> ;
            dcterms:rights <https://rightsstatements.org/vocab/InC/1.0/> ;
            dcterms:source <http://www.getty.edu/research/tools/vocabularies/aat/> ],
        "Hue name for the color representing that portion of the spectrum that is intermediate between red and yellow, with wavelengths between 585 and 620 nanometers. The term may refer to any of this group of colors that vary in lightness and saturation. An example of orange color in nature is that of the citrus fruit orange, for which the color is named in modern English. It is a secondary pigment color (made by combining yellow and red). (AAT)"@en ;
    dcterms:identifier "CC00064" ;
    owl:sameAs <http://vocab.getty.edu/aat/300126734> .

cc:CC00065 a owl:NamedIndividual ;
    rdfs:label "pink"@en ;
    dcterms:description [ rdfs:label "Hue name for the range of colors intermediate between red and white, often a pale red, sometimes with a slight purple or yellow tinge. (AAT)"@en ;
            dcterms:creator "The J. Paul Getty Trust" ;
            dcterms:license <https://opendatacommons.org/licenses/by/1-0/> ;
            dcterms:rights <https://rightsstatements.org/vocab/InC/1.0/> ;
            dcterms:source <http://www.getty.edu/research/tools/vocabularies/aat/> ],
        "Hue name for the range of colors intermediate between red and white, often a pale red, sometimes with a slight purple or yellow tinge. (AAT)"@en ;
    dcterms:identifier "CC00065" ;
    owl:sameAs <http://vocab.getty.edu/aat/300124707> .

cc:CC00066 a owl:NamedIndividual ;
    rdfs:label "purple"@en ;
    dcterms:description [ rdfs:label "Hue name for the colors intermediate between red and blue, originally the colors derived from a crimson mollusk dye. (AAT)"@en ;
            dcterms:creator "The J. Paul Getty Trust" ;
            dcterms:license <https://opendatacommons.org/licenses/by/1-0/> ;
            dcterms:rights <https://rightsstatements.org/vocab/InC/1.0/> ;
            dcterms:source <http://www.getty.edu/research/tools/vocabularies/aat/> ],
        "Hue name for the colors intermediate between red and blue, originally the colors derived from a crimson mollusk dye. (AAT)"@en ;
    dcterms:identifier "CC00066" ;
    owl:sameAs <http://vocab.getty.edu/aat/300130257> .

cc:CC00067 a owl:NamedIndividual ;
    rdfs:label "red"@en ;
    dcterms:description [ rdfs:label "Hue name for one of the three primary additive colors; that portion of the spectrum lying at the lowest frequencies of light discernible by the human eye, with a wavelength range between 630 and 760 nanometers. The term may refer to any of this group of colors that vary in lightness and saturation. Examples of red color in nature are that of blood and ripe cherries."@en ;
            dcterms:creator "The J. Paul Getty Trust" ;
            dcterms:license <https://opendatacommons.org/licenses/by/1-0/> ;
            dcterms:rights <https://rightsstatements.org/vocab/InC/1.0/> ;
            dcterms:source <http://www.getty.edu/research/tools/vocabularies/aat/> ],
        "Hue name for one of the three primary additive colors; that portion of the spectrum lying at the lowest frequencies of light discernible by the human eye, with a wavelength range between 630 and 760 nanometers. The term may refer to any of this group of colors that vary in lightness and saturation. Examples of red color in nature are that of blood and ripe cherries."@en ;
    dcterms:identifier "CC00067" ;
    owl:sameAs <http://vocab.getty.edu/aat/300126225> .

cc:CC00068 a owl:NamedIndividual ;
    rdfs:label "rust"@en ;
    dcterms:description [ rdfs:label "red-orange-brown-color resembling iron oxide"@en ;
            dcterms:creator "Wikidata contributors" ;
            dcterms:license <https://creativecommons.org/publicdomain/mark/1.0/> ;
            dcterms:rights <https://creativecommons.org/publicdomain/mark/1.0/> ;
            dcterms:source <https://www.wikidata.org/wiki/Wikidata:Data_access/en> ],
        "red-orange-brown-color resembling iron oxide"@en ;
    dcterms:identifier "CC00068" ;
    owl:sameAs <http://www.wikidata.org/entity/Q543923> .

cc:CC00069 a owl:NamedIndividual ;
    rdfs:label "tan"@en ;
    dcterms:description [ rdfs:label "A light to moderate brownish tawny color. The term originally referred to the color of crushed oak bark or tannin that is employed to tan leather."@en ;
            dcterms:creator "The J. Paul Getty Trust" ;
            dcterms:license <https://opendatacommons.org/licenses/by/1-0/> ;
            dcterms:rights <https://rightsstatements.org/vocab/InC/1.0/> ;
            dcterms:source <http://www.getty.edu/research/tools/vocabularies/aat/> ],
        "A light to moderate brownish tawny color. The term originally referred to the color of crushed oak bark or tannin that is employed to tan leather."@en ;
    dcterms:identifier "CC00069" ;
    owl:sameAs <http://vocab.getty.edu/aat/300266248> .

cc:CC00070 a owl:NamedIndividual ;
    rdfs:label "teal"@en ;
    dcterms:description [ rdfs:label "Colors in a range of a bluish grayish green, resembling the color of certain patches feathers of the teal (a river duck)."@en ;
            dcterms:creator "The J. Paul Getty Trust" ;
            dcterms:license <https://opendatacommons.org/licenses/by/1-0/> ;
            dcterms:rights <https://rightsstatements.org/vocab/InC/1.0/> ;
            dcterms:source <http://www.getty.edu/research/tools/vocabularies/aat/> ],
        "Colors in a range of a bluish grayish green, resembling the color of certain patches feathers of the teal (a river duck)."@en ;
    dcterms:identifier "CC00070" ;
    owl:sameAs <http://vocab.getty.edu/aat/300311051> .

cc:CC00071 a owl:NamedIndividual ;
    rdfs:label "turquoise"@en ;
    dcterms:description [ rdfs:label "Refers to a range of bluish and greenish colors resembling the turquoise mineral, typically a light to moderate greenish blue."@en ;
            dcterms:creator "The J. Paul Getty Trust" ;
            dcterms:license <https://opendatacommons.org/licenses/by/1-0/> ;
            dcterms:rights <https://rightsstatements.org/vocab/InC/1.0/> ;
            dcterms:source <http://www.getty.edu/research/tools/vocabularies/aat/> ],
        "Refers to a range of bluish and greenish colors resembling the turquoise mineral, typically a light to moderate greenish blue."@en ;
    dcterms:identifier "CC00071" ;
    owl:sameAs <http://vocab.getty.edu/aat/300311024> .

cc:CC00072 a owl:NamedIndividual ;
    rdfs:label "white"@en ;
    dcterms:description [ rdfs:label "UCL (Universal Color Language) standard color name identifying whitish colors, such as the color of snow or milk. More specifically, white is the absence of color. It is the color produced by reflection, transmission, or emission of all kinds of light in the proportion in which they exist in the complete visible spectrum, without sensible absorption, being thus fully luminous and devoid of any distinctive hue."@en ;
            dcterms:creator "The J. Paul Getty Trust" ;
            dcterms:license <https://opendatacommons.org/licenses/by/1-0/> ;
            dcterms:rights <https://rightsstatements.org/vocab/InC/1.0/> ;
            dcterms:source <http://www.getty.edu/research/tools/vocabularies/aat/> ],
        "UCL (Universal Color Language) standard color name identifying whitish colors, such as the color of snow or milk. More specifically, white is the absence of color. It is the color produced by reflection, transmission, or emission of all kinds of light in the proportion in which they exist in the complete visible spectrum, without sensible absorption, being thus fully luminous and devoid of any distinctive hue."@en ;
    dcterms:identifier "CC00072" ;
    owl:sameAs <http://vocab.getty.edu/aat/300129784> .

cc:CC00073 a owl:NamedIndividual ;
    rdfs:label "yellow"@en ;
    dcterms:description [ rdfs:label "Hue name for one of the three primary subtractive colors. Represents that portion of the spectrum lying between green and orange, with a wavelength range between 565 and 590 nanometers. The term may refer to any of this group of colors that vary in lightness and saturation. Examples of yellow color in nature are that of a ripe lemon and the yolk of an egg."@en ;
            dcterms:creator "The J. Paul Getty Trust" ;
            dcterms:license <https://opendatacommons.org/licenses/by/1-0/> ;
            dcterms:rights <https://rightsstatements.org/vocab/InC/1.0/> ;
            dcterms:source <http://www.getty.edu/research/tools/vocabularies/aat/> ],
        "Hue name for one of the three primary subtractive colors. Represents that portion of the spectrum lying between green and orange, with a wavelength range between 565 and 590 nanometers. The term may refer to any of this group of colors that vary in lightness and saturation. Examples of yellow color in nature are that of a ripe lemon and the yolk of an egg."@en ;
    dcterms:identifier "CC00073" ;
    owl:sameAs <http://vocab.getty.edu/aat/300127794> .

cc:CC00077 a owl:NamedIndividual ;
    rdfs:label "devor "@en ;
    dcterms:description [ rdfs:label "technique of creating a pattern on fabric, especially velvet, by burning out the pile with acid"@en ;
            dcterms:creator "The J. Paul Getty Trust" ;
            dcterms:license <https://opendatacommons.org/licenses/by/1-0/> ;
            dcterms:rights <https://rightsstatements.org/vocab/InC/1.0/> ;
            dcterms:source <http://www.getty.edu/research/tools/vocabularies/aat/> ],
        "technique of creating a pattern on fabric, especially velvet, by burning out the pile with acid"@en ;
    dcterms:identifier "CC00077" ;
    owl:sameAs <http://vocab.getty.edu/aat/300386429>,
        <http://www.wikidata.org/entity/Q778180> .

cc:CC00087 a owl:NamedIndividual ;
    rdfs:label "lace making"@en ;
    dcterms:description [ rdfs:label "Refers to the process of creating lace, which is a textile work made of thread, comprising a ground of netting with patterns worked in or embroidered on the mesh."@en ;
            dcterms:creator "The J. Paul Getty Trust" ;
            dcterms:license <https://opendatacommons.org/licenses/by/1-0/> ;
            dcterms:rights <https://rightsstatements.org/vocab/InC/1.0/> ;
            dcterms:source <http://www.getty.edu/research/tools/vocabularies/aat/> ],
        "Refers to the process of creating lace, which is a textile work made of thread, comprising a ground of netting with patterns worked in or embroidered on the mesh."@en ;
    dcterms:identifier "CC00087" ;
    owl:sameAs <http://vocab.getty.edu/aat/300053651>,
        <http://www.wikidata.org/entity/Q43065851> .

cc:CC00114 a owl:NamedIndividual ;
    rdfs:label "pinafore"@en ;
    dcterms:description [ rdfs:label "Sleeveless apronlike garments which have a skirt and a bodice portion and which cover the front, sides, and a portion of the back. Worn over main garments for protection or ornamentation."@en ;
            dcterms:creator "The J. Paul Getty Trust" ;
            dcterms:license <https://opendatacommons.org/licenses/by/1-0/> ;
            dcterms:rights <https://rightsstatements.org/vocab/InC/1.0/> ;
            dcterms:source <http://www.getty.edu/research/tools/vocabularies/aat/> ],
        "Sleeveless apronlike garments which have a skirt and a bodice portion and which cover the front, sides, and a portion of the back. Worn over main garments for protection or ornamentation."@en ;
    dcterms:identifier "CC00114" ;
    owl:sameAs <http://vocab.getty.edu/aat/300046186>,
        <http://www.wikidata.org/entity/Q3247116> .

cc:CC00142 a owl:NamedIndividual ;
    rdfs:label "shoulder strap"@en ;
    dcterms:description [ rdfs:label "Strips of leather, cloth, or other material that pass over the shoulder and from which an article is suspended or a garment is held up. For strips used for fastening, use \"straps.\""@en ;
            dcterms:creator "The J. Paul Getty Trust" ;
            dcterms:license <https://opendatacommons.org/licenses/by/1-0/> ;
            dcterms:rights <https://rightsstatements.org/vocab/InC/1.0/> ;
            dcterms:source <http://www.getty.edu/research/tools/vocabularies/aat/> ],
        "Strips of leather, cloth, or other material that pass over the shoulder and from which an article is suspended or a garment is held up. For strips used for fastening, use \"straps.\""@en ;
    dcterms:identifier "CC00142" ;
    owl:sameAs <http://vocab.getty.edu/aat/300259717>,
        <http://www.wikidata.org/entity/#N/A> .

cc:CC00150 a owl:NamedIndividual ;
    rdfs:label "hanging sleeve"@en ;
    dcterms:description [ rdfs:label "Long loose sleeves with a slit through which the arm can emerge. Also, long false decorative sleeves attached to the back of the armhole. Worn by men, women, or children especially from the 15th through the 18th century."@en ;
            dcterms:creator "The J. Paul Getty Trust" ;
            dcterms:license <https://opendatacommons.org/licenses/by/1-0/> ;
            dcterms:rights <https://rightsstatements.org/vocab/InC/1.0/> ;
            dcterms:source <http://www.getty.edu/research/tools/vocabularies/aat/> ],
        "Long loose sleeves with a slit through which the arm can emerge. Also, long false decorative sleeves attached to the back of the armhole. Worn by men, women, or children especially from the 15th through the 18th century."@en ;
    dcterms:identifier "CC00150" ;
    owl:sameAs <http://vocab.getty.edu/aat/300253738>,
        <http://www.wikidata.org/entity/http://www.wikidata.org/entity/Q29129637> .

cc:CC00195 a owl:NamedIndividual ;
    rdfs:label "acetate"@en ;
    dcterms:description [ rdfs:label "fiber made from acetylcellulose"@en ;
            dcterms:creator "Wikidata contributors" ;
            dcterms:license <https://creativecommons.org/publicdomain/mark/1.0/> ;
            dcterms:rights <https://creativecommons.org/publicdomain/mark/1.0/> ;
            dcterms:source <https://www.wikidata.org/wiki/Wikidata:Data_access/en> ],
        "fiber made from acetylcellulose"@en ;
    dcterms:identifier "CC00195" ;
    owl:sameAs <http://www.wikidata.org/entity/Q212527> .

cc:CC00196 a owl:NamedIndividual ;
    rdfs:label "acrylic"@en ;
    dcterms:description [ rdfs:label "Synthetic fiber in which the fiber forming substance is composed of at least 85% acrylic resin."@en ;
            dcterms:creator "The J. Paul Getty Trust" ;
            dcterms:license <https://opendatacommons.org/licenses/by/1-0/> ;
            dcterms:rights <https://rightsstatements.org/vocab/InC/1.0/> ;
            dcterms:source <http://www.getty.edu/research/tools/vocabularies/aat/> ],
        "Synthetic fiber in which the fiber forming substance is composed of at least 85% acrylic resin."@en ;
    dcterms:identifier "CC00196" ;
    owl:sameAs <http://vocab.getty.edu/aat/300386559> .

cc:CC00197 a owl:NamedIndividual ;
    rdfs:label "angora"@en ;
    dcterms:description [ rdfs:label "The long, fine hair from any breed of Angora rabbit. The white French rabbit is favored for its high-quality, soft hair. Angora dyes readily, but is difficult to spin because of its fine texture and it does not felt like common rabbit hair. It is usually mixed with sheep wool or other fibers for weaving."@en ;
            dcterms:creator "The J. Paul Getty Trust" ;
            dcterms:license <https://opendatacommons.org/licenses/by/1-0/> ;
            dcterms:rights <https://rightsstatements.org/vocab/InC/1.0/> ;
            dcterms:source <http://www.getty.edu/research/tools/vocabularies/aat/> ],
        "The long, fine hair from any breed of Angora rabbit. The white French rabbit is favored for its high-quality, soft hair. Angora dyes readily, but is difficult to spin because of its fine texture and it does not felt like common rabbit hair. It is usually mixed with sheep wool or other fibers for weaving."@en ;
    dcterms:identifier "CC00197" ;
    owl:sameAs <http://vocab.getty.edu/aat/300386672> .

cc:CC00200 a owl:NamedIndividual ;
    rdfs:label "brocade"@en ;
    dcterms:description [ rdfs:label "Textile produced by brocading, typically richly figured and incorporating metal thread. (AAT)"@en ;
            dcterms:creator "The J. Paul Getty Trust" ;
            dcterms:license <https://opendatacommons.org/licenses/by/1-0/> ;
            dcterms:rights <https://rightsstatements.org/vocab/InC/1.0/> ;
            dcterms:source <http://www.getty.edu/research/tools/vocabularies/aat/> ],
        "Textile produced by brocading, typically richly figured and incorporating metal thread. (AAT)"@en ;
    dcterms:identifier "CC00200" ;
    owl:sameAs <http://vocab.getty.edu/aat/300227779> .

cc:CC00201 a owl:NamedIndividual ;
    rdfs:label "camel hair"@en ;
    dcterms:description [ rdfs:label "Fine body hair, or camel wool, used as a textile fiber."@en ;
            dcterms:creator "The J. Paul Getty Trust" ;
            dcterms:license <https://opendatacommons.org/licenses/by/1-0/> ;
            dcterms:rights <https://rightsstatements.org/vocab/InC/1.0/> ;
            dcterms:source <http://www.getty.edu/research/tools/vocabularies/aat/> ],
        "Fine body hair, or camel wool, used as a textile fiber."@en ;
    dcterms:identifier "CC00201" ;
    owl:sameAs <http://vocab.getty.edu/aat/300011816> .

cc:CC00202 a owl:NamedIndividual ;
    rdfs:label "cashmere"@en ;
    dcterms:description [ rdfs:label "Yarn or fabric made from the fine, soft, light wool from the undercoat of the Kashmir goat."@en ;
            dcterms:creator "The J. Paul Getty Trust" ;
            dcterms:license <https://opendatacommons.org/licenses/by/1-0/> ;
            dcterms:rights <https://rightsstatements.org/vocab/InC/1.0/> ;
            dcterms:source <http://www.getty.edu/research/tools/vocabularies/aat/> ],
        "Yarn or fabric made from the fine, soft, light wool from the undercoat of the Kashmir goat."@en ;
    dcterms:identifier "CC00202" ;
    owl:sameAs <http://vocab.getty.edu/aat/300403905> .

cc:CC00203 a owl:NamedIndividual ;
    rdfs:label "chiffon"@en ;
    dcterms:description [ rdfs:label "Sheer, lightweight plain-woven textile of fine, tightly-twisted yarn, originally of silk now also of various synthetic fibers, used, for example, for scarves, dresses, blouses, underwear, and veils. (AAT)"@en ;
            dcterms:creator "The J. Paul Getty Trust" ;
            dcterms:license <https://opendatacommons.org/licenses/by/1-0/> ;
            dcterms:rights <https://rightsstatements.org/vocab/InC/1.0/> ;
            dcterms:source <http://www.getty.edu/research/tools/vocabularies/aat/> ],
        "Sheer, lightweight plain-woven textile of fine, tightly-twisted yarn, originally of silk now also of various synthetic fibers, used, for example, for scarves, dresses, blouses, underwear, and veils. (AAT)"@en ;
    dcterms:identifier "CC00203" ;
    owl:sameAs <http://vocab.getty.edu/aat/300249449> .

cc:CC00204 a owl:NamedIndividual ;
    rdfs:label "corduroy"@en ;
    dcterms:description [ rdfs:label "Weft pile weave with cut pile ribbed in the direction of the warp, usually made of cotton."@en ;
            dcterms:creator "The J. Paul Getty Trust" ;
            dcterms:license <https://opendatacommons.org/licenses/by/1-0/> ;
            dcterms:rights <https://rightsstatements.org/vocab/InC/1.0/> ;
            dcterms:source <http://www.getty.edu/research/tools/vocabularies/aat/> ],
        "Weft pile weave with cut pile ribbed in the direction of the warp, usually made of cotton."@en ;
    dcterms:identifier "CC00204" ;
    owl:sameAs <http://vocab.getty.edu/aat/300014080> .

cc:CC00205 a owl:NamedIndividual ;
    rdfs:label "cotton"@en ;
    dcterms:description [ rdfs:label "Textile made from cotton fiber."@en ;
            dcterms:creator "The J. Paul Getty Trust" ;
            dcterms:license <https://opendatacommons.org/licenses/by/1-0/> ;
            dcterms:rights <https://rightsstatements.org/vocab/InC/1.0/> ;
            dcterms:source <http://www.getty.edu/research/tools/vocabularies/aat/> ],
        "Textile made from cotton fiber."@en ;
    dcterms:identifier "CC00205" ;
    owl:sameAs <http://vocab.getty.edu/aat/300014067> .

cc:CC00206 a owl:NamedIndividual ;
    rdfs:label "crepe"@en ;
    dcterms:description [ rdfs:label "Lightweight textile made of various types of fiber, having a crinkled surface obtained by using hard twisted thread or yarn, by printing with caustic soda, by weaving with varied tensions, or by embossing. (AAT)"@en ;
            dcterms:creator "The J. Paul Getty Trust" ;
            dcterms:license <https://opendatacommons.org/licenses/by/1-0/> ;
            dcterms:rights <https://rightsstatements.org/vocab/InC/1.0/> ;
            dcterms:source <http://www.getty.edu/research/tools/vocabularies/aat/> ],
        "Lightweight textile made of various types of fiber, having a crinkled surface obtained by using hard twisted thread or yarn, by printing with caustic soda, by weaving with varied tensions, or by embossing. (AAT)"@en ;
    dcterms:identifier "CC00206" ;
    owl:sameAs <http://vocab.getty.edu/aat/300183741> .

cc:CC00208 a owl:NamedIndividual ;
    rdfs:label "damask"@en ;
    dcterms:description [ rdfs:label "Woven figured textile with one warp and one weft in which the pattern is formed by a contrast of binding systems, and appears on the face and the back in reverse positions."@en ;
            dcterms:creator "The J. Paul Getty Trust" ;
            dcterms:license <https://opendatacommons.org/licenses/by/1-0/> ;
            dcterms:rights <https://rightsstatements.org/vocab/InC/1.0/> ;
            dcterms:source <http://www.getty.edu/research/tools/vocabularies/aat/> ],
        "Woven figured textile with one warp and one weft in which the pattern is formed by a contrast of binding systems, and appears on the face and the back in reverse positions."@en ;
    dcterms:identifier "CC00208" ;
    owl:sameAs <http://vocab.getty.edu/aat/300163295> .

cc:CC00211 a owl:NamedIndividual ;
    rdfs:label "elastic"@en ;
    dcterms:description [ rdfs:label "Textile having the characteristic that it can be stretched without permanent alteration of size or shape. Examples include yardage or strips of textile material comprising threads or thin strips of rubber or other another elastic substance covered by a woven material."@en ;
            dcterms:creator "The J. Paul Getty Trust" ;
            dcterms:license <https://opendatacommons.org/licenses/by/1-0/> ;
            dcterms:rights <https://rightsstatements.org/vocab/InC/1.0/> ;
            dcterms:source <http://www.getty.edu/research/tools/vocabularies/aat/> ],
        "Textile having the characteristic that it can be stretched without permanent alteration of size or shape. Examples include yardage or strips of textile material comprising threads or thin strips of rubber or other another elastic substance covered by a woven material."@en ;
    dcterms:identifier "CC00211" ;
    owl:sameAs <http://vocab.getty.edu/aat/300404361> .

cc:CC00212 a owl:NamedIndividual ;
    rdfs:label "felt"@en ;
    dcterms:description [ rdfs:label "Textile constructed usually of wool and fur fiber often mixed with natural or synthetic fiber by the interlocking of the loose fiber through the action of heat, moisture, chemicals, and pressure without spinning, weaving, or knitting."@en ;
            dcterms:creator "The J. Paul Getty Trust" ;
            dcterms:license <https://opendatacommons.org/licenses/by/1-0/> ;
            dcterms:rights <https://rightsstatements.org/vocab/InC/1.0/> ;
            dcterms:source <http://www.getty.edu/research/tools/vocabularies/aat/> ],
        "Textile constructed usually of wool and fur fiber often mixed with natural or synthetic fiber by the interlocking of the loose fiber through the action of heat, moisture, chemicals, and pressure without spinning, weaving, or knitting."@en ;
    dcterms:identifier "CC00212" ;
    owl:sameAs <http://vocab.getty.edu/aat/300014107> .

cc:CC00214 a owl:NamedIndividual ;
    rdfs:label "georgette"@en ;
    dcterms:description [ rdfs:label "A semi-transparent artificial fiber or natural silk fabric woven in plain weave with undeterred chain and weft threads, alternately two right and two left twisted."@en ;
            dcterms:creator "The J. Paul Getty Trust" ;
            dcterms:license <https://opendatacommons.org/licenses/by/1-0/> ;
            dcterms:rights <https://rightsstatements.org/vocab/InC/1.0/> ;
            dcterms:source <http://www.getty.edu/research/tools/vocabularies/aat/> ],
        "A semi-transparent artificial fiber or natural silk fabric woven in plain weave with undeterred chain and weft threads, alternately two right and two left twisted."@en ;
    dcterms:identifier "CC00214" ;
    owl:sameAs <http://vocab.getty.edu/aat/300417883> .

cc:CC00215 a owl:NamedIndividual ;
    rdfs:label "glass"@en ;
    dcterms:description [ rdfs:label "An amorphous, inorganic substance made by fusing silica (silicon dioxide) with a basic oxide; generally transparent but often translucent or opaque. Its characteristic properties are its hardness and rigidity at ordinary temperatures, its capacity for plastic working at elevated temperatures, and its resistance to weathering and to most chemicals except hydrofluoric acid. Used for both utilitarian and decorative purposes, it can be formed into various shapes, colored or decorated. Glass originated as a glaze in Mesopotamia in about 3500 BCE and the first objects made wholly of glass date to about 2500 BCE."@en ;
            dcterms:creator "The J. Paul Getty Trust" ;
            dcterms:license <https://opendatacommons.org/licenses/by/1-0/> ;
            dcterms:rights <https://rightsstatements.org/vocab/InC/1.0/> ;
            dcterms:source <http://www.getty.edu/research/tools/vocabularies/aat/> ],
        "An amorphous, inorganic substance made by fusing silica (silicon dioxide) with a basic oxide; generally transparent but often translucent or opaque. Its characteristic properties are its hardness and rigidity at ordinary temperatures, its capacity for plastic working at elevated temperatures, and its resistance to weathering and to most chemicals except hydrofluoric acid. Used for both utilitarian and decorative purposes, it can be formed into various shapes, colored or decorated. Glass originated as a glaze in Mesopotamia in about 3500 BCE and the first objects made wholly of glass date to about 2500 BCE."@en ;
    dcterms:identifier "CC00215" ;
    owl:sameAs <http://vocab.getty.edu/aat/300010797> .

cc:CC00216 a owl:NamedIndividual ;
    rdfs:label "hemp"@en ;
    dcterms:description [ rdfs:label "Fiber derived from the stalk of the species Cannabis sativa. Fibers range from 1-2 m in length and are yellow to brown in color. They have a high cellulose content with little lignin. Hemp is lustrous, strong, and durable with good resistance to water, salts, light, and insects; used for cordage, fish lines, sailcloth, canvas, burlap, packing, and as a fiber for paper or for plastic filler."@en ;
            dcterms:creator "The J. Paul Getty Trust" ;
            dcterms:license <https://opendatacommons.org/licenses/by/1-0/> ;
            dcterms:rights <https://rightsstatements.org/vocab/InC/1.0/> ;
            dcterms:source <http://www.getty.edu/research/tools/vocabularies/aat/> ],
        "Fiber derived from the stalk of the species Cannabis sativa. Fibers range from 1-2 m in length and are yellow to brown in color. They have a high cellulose content with little lignin. Hemp is lustrous, strong, and durable with good resistance to water, salts, light, and insects; used for cordage, fish lines, sailcloth, canvas, burlap, packing, and as a fiber for paper or for plastic filler."@en ;
    dcterms:identifier "CC00216" ;
    owl:sameAs <http://vocab.getty.edu/aat/300014043> .

cc:CC00217 a owl:NamedIndividual ;
    rdfs:label "jacquard"@en ;
    dcterms:description [ rdfs:label "Any woven figured textile produced on a Jacquard loom."@en ;
            dcterms:creator "The J. Paul Getty Trust" ;
            dcterms:license <https://opendatacommons.org/licenses/by/1-0/> ;
            dcterms:rights <https://rightsstatements.org/vocab/InC/1.0/> ;
            dcterms:source <http://www.getty.edu/research/tools/vocabularies/aat/> ],
        "Any woven figured textile produced on a Jacquard loom."@en ;
    dcterms:identifier "CC00217" ;
    owl:sameAs <http://vocab.getty.edu/aat/300256616> .

cc:CC00219 a owl:NamedIndividual ;
    rdfs:label "lace"@en ;
    dcterms:description [ rdfs:label "Refers to a fine, openwork ornamental textile work formed by looping, interlacing, twisting, plaiting, or braiding threads of linen, cotton, silk, hair, metal, or another fiber to form designs or patterns. Lace may be made with a needle or with bobbins. Embroidery may be added. Modern lace may be made by machine. Openwork fabrics made on a loom and ornamental openwork knitting are generally not classified as lace. Lace is often white or monochromatic. True lace developed in the fourteenth century in Europe and the Middle East, although ornamented openwork fabrics were known in ancient cultures, including the Egyptian culture. Lace may be used as a border, edging, or insert on linens or apparel; it is also formed into large pieces of cloth used for hangings, draperies, apparel, or other items. (AAT)"@en ;
            dcterms:creator "The J. Paul Getty Trust" ;
            dcterms:license <https://opendatacommons.org/licenses/by/1-0/> ;
            dcterms:rights <https://rightsstatements.org/vocab/InC/1.0/> ;
            dcterms:source <http://www.getty.edu/research/tools/vocabularies/aat/> ],
        "Refers to a fine, openwork ornamental textile work formed by looping, interlacing, twisting, plaiting, or braiding threads of linen, cotton, silk, hair, metal, or another fiber to form designs or patterns. Lace may be made with a needle or with bobbins. Embroidery may be added. Modern lace may be made by machine. Openwork fabrics made on a loom and ornamental openwork knitting are generally not classified as lace. Lace is often white or monochromatic. True lace developed in the fourteenth century in Europe and the Middle East, although ornamented openwork fabrics were known in ancient cultures, including the Egyptian culture. Lace may be used as a border, edging, or insert on linens or apparel; it is also formed into large pieces of cloth used for hangings, draperies, apparel, or other items. (AAT)"@en ;
    dcterms:identifier "CC00219" ;
    owl:sameAs <http://vocab.getty.edu/aat/300132861> .

cc:CC00220 a owl:NamedIndividual ;
    rdfs:label "leather"@en ;
    dcterms:description [ rdfs:label "The skin or hide of an animal that has been tanned to render it resistant to putrefication and relatively soft and flexible when dry. For composite material made from scrap leather pieces, use maril. (AAT)"@en ;
            dcterms:creator "The J. Paul Getty Trust" ;
            dcterms:license <https://opendatacommons.org/licenses/by/1-0/> ;
            dcterms:rights <https://rightsstatements.org/vocab/InC/1.0/> ;
            dcterms:source <http://www.getty.edu/research/tools/vocabularies/aat/> ],
        "The skin or hide of an animal that has been tanned to render it resistant to putrefication and relatively soft and flexible when dry. For composite material made from scrap leather pieces, use maril. (AAT)"@en ;
    dcterms:identifier "CC00220" ;
    owl:sameAs <http://vocab.getty.edu/aat/300011845> .

cc:CC00221 a owl:NamedIndividual ;
    rdfs:label "linen"@en ;
    dcterms:description [ rdfs:label "General name for textile woven from the spun fiber of the flax plant."@en ;
            dcterms:creator "The J. Paul Getty Trust" ;
            dcterms:license <https://opendatacommons.org/licenses/by/1-0/> ;
            dcterms:rights <https://rightsstatements.org/vocab/InC/1.0/> ;
            dcterms:source <http://www.getty.edu/research/tools/vocabularies/aat/> ],
        "General name for textile woven from the spun fiber of the flax plant."@en ;
    dcterms:identifier "CC00221" ;
    owl:sameAs <http://vocab.getty.edu/aat/300014069> .

cc:CC00224 a owl:NamedIndividual ;
    rdfs:label "metal"@en ;
    dcterms:description [ rdfs:label "Any of a large group of substances that typically show a characteristic luster, are good conductors of electricity and heat, are opaque, can be fused, and are usually malleable or ductile. (AAT)"@en ;
            dcterms:creator "The J. Paul Getty Trust" ;
            dcterms:license <https://opendatacommons.org/licenses/by/1-0/> ;
            dcterms:rights <https://rightsstatements.org/vocab/InC/1.0/> ;
            dcterms:source <http://www.getty.edu/research/tools/vocabularies/aat/> ],
        "Any of a large group of substances that typically show a characteristic luster, are good conductors of electricity and heat, are opaque, can be fused, and are usually malleable or ductile. (AAT)"@en ;
    dcterms:identifier "CC00224" ;
    owl:sameAs <http://vocab.getty.edu/aat/300010900> .

cc:CC00226 a owl:NamedIndividual ;
    rdfs:label "mohair"@en ;
    dcterms:description [ rdfs:label "Long, lustrous hair of the Angora goat, valued for its strength and excellent spinning qualities."@en ;
            dcterms:creator "The J. Paul Getty Trust" ;
            dcterms:license <https://opendatacommons.org/licenses/by/1-0/> ;
            dcterms:rights <https://rightsstatements.org/vocab/InC/1.0/> ;
            dcterms:source <http://www.getty.edu/research/tools/vocabularies/aat/> ],
        "Long, lustrous hair of the Angora goat, valued for its strength and excellent spinning qualities."@en ;
    dcterms:identifier "CC00226" ;
    owl:sameAs <http://vocab.getty.edu/aat/300192989> .

cc:CC00227 a owl:NamedIndividual ;
    rdfs:label "moire"@en ;
    dcterms:description [ rdfs:label "Patterns having a watered or rippled look. Where this produces an illusion of movement, use moir effect. (AAT)"@en ;
            dcterms:creator "The J. Paul Getty Trust" ;
            dcterms:license <https://opendatacommons.org/licenses/by/1-0/> ;
            dcterms:rights <https://rightsstatements.org/vocab/InC/1.0/> ;
            dcterms:source <http://www.getty.edu/research/tools/vocabularies/aat/> ],
        "Patterns having a watered or rippled look. Where this produces an illusion of movement, use moir effect. (AAT)"@en ;
    dcterms:identifier "CC00227" ;
    owl:sameAs <http://vocab.getty.edu/aat/300400593> .

cc:CC00229 a owl:NamedIndividual ;
    rdfs:label "net"@en ;
    dcterms:description [ rdfs:label "Refers to an open weave textile made of thread, twine, yarn, or cord, usually of silk, cotton, nylon, or rayon, with fine to coarse meshes of fixed dimension. It is characterized by being a simple mesh joined by knots; it may be made by hand or by machine. It may be used to make various items from veils and trimming on clothing to tennis nets and fishing nets. Fine net that is used in lace, headwear, and other apparel is often referred to as netting rather than as net. For the objects consisting of meshed arrangements of threads, cords, or ropes that have been twisted, knotted, or woven together at regular intervals, use nets (objects). (AAT)"@en ;
            dcterms:creator "The J. Paul Getty Trust" ;
            dcterms:license <https://opendatacommons.org/licenses/by/1-0/> ;
            dcterms:rights <https://rightsstatements.org/vocab/InC/1.0/> ;
            dcterms:source <http://www.getty.edu/research/tools/vocabularies/aat/> ],
        "Refers to an open weave textile made of thread, twine, yarn, or cord, usually of silk, cotton, nylon, or rayon, with fine to coarse meshes of fixed dimension. It is characterized by being a simple mesh joined by knots; it may be made by hand or by machine. It may be used to make various items from veils and trimming on clothing to tennis nets and fishing nets. Fine net that is used in lace, headwear, and other apparel is often referred to as netting rather than as net. For the objects consisting of meshed arrangements of threads, cords, or ropes that have been twisted, knotted, or woven together at regular intervals, use nets (objects). (AAT)"@en ;
    dcterms:identifier "CC00229" ;
    owl:sameAs <http://vocab.getty.edu/aat/300249438> .

cc:CC00230 a owl:NamedIndividual ;
    rdfs:label "nylon"@en ;
    dcterms:description [ rdfs:label "Any of a variety of thermoplastic polymers originally developed as textile fibers and used in fabrics. They have a straight-chain polyamide structure and are largely heat-resistant."@en ;
            dcterms:creator "The J. Paul Getty Trust" ;
            dcterms:license <https://opendatacommons.org/licenses/by/1-0/> ;
            dcterms:rights <https://rightsstatements.org/vocab/InC/1.0/> ;
            dcterms:source <http://www.getty.edu/research/tools/vocabularies/aat/> ],
        "Any of a variety of thermoplastic polymers originally developed as textile fibers and used in fabrics. They have a straight-chain polyamide structure and are largely heat-resistant."@en ;
    dcterms:identifier "CC00230" ;
    owl:sameAs <http://vocab.getty.edu/aat/300014462> .

cc:CC00232 a owl:NamedIndividual ;
    rdfs:label "plastic"@en ;
    dcterms:description [ rdfs:label "A general term for any of a large and varied class of natural or synthetic organic materials that can be molded, extruded, or cast when soft or liquid, and then set into a rigid or slightly elastic form. Natural plastics include tree resins, beeswax, gutta-percha, horn, and clay. Synthetic plastics were first made in the 19th century. Plastics are used widely in manufacturing."@en ;
            dcterms:creator "The J. Paul Getty Trust" ;
            dcterms:license <https://opendatacommons.org/licenses/by/1-0/> ;
            dcterms:rights <https://rightsstatements.org/vocab/InC/1.0/> ;
            dcterms:source <http://www.getty.edu/research/tools/vocabularies/aat/> ],
        "A general term for any of a large and varied class of natural or synthetic organic materials that can be molded, extruded, or cast when soft or liquid, and then set into a rigid or slightly elastic form. Natural plastics include tree resins, beeswax, gutta-percha, horn, and clay. Synthetic plastics were first made in the 19th century. Plastics are used widely in manufacturing."@en ;
    dcterms:identifier "CC00232" ;
    owl:sameAs <http://vocab.getty.edu/aat/300014570> .

cc:CC00233 a owl:NamedIndividual ;
    rdfs:label "polyester"@en ;
    dcterms:description [ rdfs:label "Refers to polyester polymers used as fibers woven into fabrics. (AAT)"@en ;
            dcterms:creator "The J. Paul Getty Trust" ;
            dcterms:license <https://opendatacommons.org/licenses/by/1-0/> ;
            dcterms:rights <https://rightsstatements.org/vocab/InC/1.0/> ;
            dcterms:source <http://www.getty.edu/research/tools/vocabularies/aat/> ],
        "Refers to polyester polymers used as fibers woven into fabrics. (AAT)"@en ;
    dcterms:identifier "CC00233" ;
    owl:sameAs <http://vocab.getty.edu/aat/300379829> .

cc:CC00234 a owl:NamedIndividual ;
    rdfs:label "ramie"@en ;
    dcterms:description [ rdfs:label "Bast fiber obtained from the stems of several varieties of the species Boehmeria nivea, native to tropical Asia but cultivated in China, Japan, Europe, South America, and the United States. The Ramie has been used in China for paper and fabric since prehistoric times. Its use spread through Europe in the Middle Ages. It is white or green in color, depending upon the variety. It is soft, fine, and durable fiber that is very lustrous and dyes well, used for twine, fishnets, sewing thread, and fabric for clothing, summer suits, dresses, canvas, tablecloths, and upholstery. Ramie has also been used to produce strong paper for linings, banknotes, and cigarettes."@en ;
            dcterms:creator "The J. Paul Getty Trust" ;
            dcterms:license <https://opendatacommons.org/licenses/by/1-0/> ;
            dcterms:rights <https://rightsstatements.org/vocab/InC/1.0/> ;
            dcterms:source <http://www.getty.edu/research/tools/vocabularies/aat/> ],
        "Bast fiber obtained from the stems of several varieties of the species Boehmeria nivea, native to tropical Asia but cultivated in China, Japan, Europe, South America, and the United States. The Ramie has been used in China for paper and fabric since prehistoric times. Its use spread through Europe in the Middle Ages. It is white or green in color, depending upon the variety. It is soft, fine, and durable fiber that is very lustrous and dyes well, used for twine, fishnets, sewing thread, and fabric for clothing, summer suits, dresses, canvas, tablecloths, and upholstery. Ramie has also been used to produce strong paper for linings, banknotes, and cigarettes."@en ;
    dcterms:identifier "CC00234" ;
    owl:sameAs <http://vocab.getty.edu/aat/300014071> .

cc:CC00235 a owl:NamedIndividual ;
    rdfs:label "rayon"@en ;
    dcterms:description [ rdfs:label "Synthetic fiber made from regenerated cellulose."@en ;
            dcterms:creator "The J. Paul Getty Trust" ;
            dcterms:license <https://opendatacommons.org/licenses/by/1-0/> ;
            dcterms:rights <https://rightsstatements.org/vocab/InC/1.0/> ;
            dcterms:source <http://www.getty.edu/research/tools/vocabularies/aat/> ],
        "Synthetic fiber made from regenerated cellulose."@en ;
    dcterms:identifier "CC00235" ;
    owl:sameAs <http://vocab.getty.edu/aat/300014059> .

cc:CC00238 a owl:NamedIndividual ;
    rdfs:label "ribbon"@en ;
    dcterms:description [ rdfs:label "Strips of fine textile, such as silk, satin, or velvet, often with a cord finish along both edges instead of selvage, forming a narrow strip or band, used for decorative trimming of a garment or for fastening or attaching something. May also refer to anything that resembles such objects, that is, any long, thin, flat, flexible strips of any material. (AAT)"@en ;
            dcterms:creator "The J. Paul Getty Trust" ;
            dcterms:license <https://opendatacommons.org/licenses/by/1-0/> ;
            dcterms:rights <https://rightsstatements.org/vocab/InC/1.0/> ;
            dcterms:source <http://www.getty.edu/research/tools/vocabularies/aat/> ],
        "Strips of fine textile, such as silk, satin, or velvet, often with a cord finish along both edges instead of selvage, forming a narrow strip or band, used for decorative trimming of a garment or for fastening or attaching something. May also refer to anything that resembles such objects, that is, any long, thin, flat, flexible strips of any material. (AAT)"@en ;
    dcterms:identifier "CC00238" ;
    owl:sameAs <http://vocab.getty.edu/aat/300014668> .

cc:CC00239 a owl:NamedIndividual ;
    rdfs:label "satin"@en ;
    dcterms:description [ rdfs:label "Woven textile characterized by a basic binding system or weave with smooth, shiny surface formed by long warp floats. Generally, each warp end passes over four or more adjacent weft picks and under the next one. (AAT)"@en ;
            dcterms:creator "The J. Paul Getty Trust" ;
            dcterms:license <https://opendatacommons.org/licenses/by/1-0/> ;
            dcterms:rights <https://rightsstatements.org/vocab/InC/1.0/> ;
            dcterms:source <http://www.getty.edu/research/tools/vocabularies/aat/> ],
        "Woven textile characterized by a basic binding system or weave with smooth, shiny surface formed by long warp floats. Generally, each warp end passes over four or more adjacent weft picks and under the next one. (AAT)"@en ;
    dcterms:identifier "CC00239" ;
    owl:sameAs <http://vocab.getty.edu/aat/300132902> .

cc:CC00241 a owl:NamedIndividual ;
    rdfs:label "shell"@en ;
    dcterms:description [ rdfs:label "Hard outer covering of invertebrate creatures, composed of calcareous or chitinous material."@en ;
            dcterms:creator "The J. Paul Getty Trust" ;
            dcterms:license <https://opendatacommons.org/licenses/by/1-0/> ;
            dcterms:rights <https://rightsstatements.org/vocab/InC/1.0/> ;
            dcterms:source <http://www.getty.edu/research/tools/vocabularies/aat/> ],
        "Hard outer covering of invertebrate creatures, composed of calcareous or chitinous material."@en ;
    dcterms:identifier "CC00241" ;
    owl:sameAs <http://vocab.getty.edu/aat/300011829> .

cc:CC00242 a owl:NamedIndividual ;
    rdfs:label "silk"@en ;
    dcterms:description [ rdfs:label "Textile made from silk fiber, which is a fiber derived from the cocoon of the silkworm moth."@en ;
            dcterms:creator "The J. Paul Getty Trust" ;
            dcterms:license <https://opendatacommons.org/licenses/by/1-0/> ;
            dcterms:rights <https://rightsstatements.org/vocab/InC/1.0/> ;
            dcterms:source <http://www.getty.edu/research/tools/vocabularies/aat/> ],
        "Textile made from silk fiber, which is a fiber derived from the cocoon of the silkworm moth."@en ;
    dcterms:identifier "CC00242" ;
    owl:sameAs <http://vocab.getty.edu/aat/300243428> .

cc:CC00243 a owl:NamedIndividual ;
    rdfs:label "spandex"@en ;
    dcterms:description [ rdfs:label "Synthetic elastomeric fiber or fabric composed largely of alternating rigid and flexible segments of polyurethane. It is used in the clothing industry, especially for hosiery, underwear, swimwear, and other close-fitting garments. Spandex is the generic name in the United States and Canada. Elastane is the generic name used elsewhere. Lycra is a proprietary name for this material."@en ;
            dcterms:creator "The J. Paul Getty Trust" ;
            dcterms:license <https://opendatacommons.org/licenses/by/1-0/> ;
            dcterms:rights <https://rightsstatements.org/vocab/InC/1.0/> ;
            dcterms:source <http://www.getty.edu/research/tools/vocabularies/aat/> ],
        "Synthetic elastomeric fiber or fabric composed largely of alternating rigid and flexible segments of polyurethane. It is used in the clothing industry, especially for hosiery, underwear, swimwear, and other close-fitting garments. Spandex is the generic name in the United States and Canada. Elastane is the generic name used elsewhere. Lycra is a proprietary name for this material."@en ;
    dcterms:identifier "CC00243" ;
    owl:sameAs <http://vocab.getty.edu/aat/300310125> .

cc:CC00245 a owl:NamedIndividual ;
    rdfs:label "taffeta"@en ;
    dcterms:description [ rdfs:label "Crisp textile, typically in plain weave, sometimes with a fine crosswise rib and a smooth lustrous surface on both sides, originally of silk, now of various fibers."@en ;
            dcterms:creator "The J. Paul Getty Trust" ;
            dcterms:license <https://opendatacommons.org/licenses/by/1-0/> ;
            dcterms:rights <https://rightsstatements.org/vocab/InC/1.0/> ;
            dcterms:source <http://www.getty.edu/research/tools/vocabularies/aat/> ],
        "Crisp textile, typically in plain weave, sometimes with a fine crosswise rib and a smooth lustrous surface on both sides, originally of silk, now of various fibers."@en ;
    dcterms:identifier "CC00245" ;
    owl:sameAs <http://vocab.getty.edu/aat/300249434> .

cc:CC00247 a owl:NamedIndividual ;
    rdfs:label "velvet"@en ;
    dcterms:description [ rdfs:label "Warp pile weave, typically silk, with a short, soft dense pile produced by a supplementary warp that is raised in loops above the surface of the textile through the introduction of rods during the weaving; the loops may be cut or left uncut."@en ;
            dcterms:creator "The J. Paul Getty Trust" ;
            dcterms:license <https://opendatacommons.org/licenses/by/1-0/> ;
            dcterms:rights <https://rightsstatements.org/vocab/InC/1.0/> ;
            dcterms:source <http://www.getty.edu/research/tools/vocabularies/aat/> ],
        "Warp pile weave, typically silk, with a short, soft dense pile produced by a supplementary warp that is raised in loops above the surface of the textile through the introduction of rods during the weaving; the loops may be cut or left uncut."@en ;
    dcterms:identifier "CC00247" ;
    owl:sameAs <http://vocab.getty.edu/aat/300133711> .

cc:CC00248 a owl:NamedIndividual ;
    rdfs:label "wax"@en ;
    dcterms:description [ rdfs:label "Any solid or semi-solid substance that is slightly greasy to touch, usually solid, translucent, and has a low melting point; waxes are not a chemically homogeneous group. Waxes are composed of long chain hydrocarbon compounds, and may contain esters of fatty acids and alcohols, are thermoplastic and melt at low temperatures of between 40 and 100 C. In general, waxes are water-repellent, smooth, soluble in organic solvents, and classified as animal (e.g., beeswax), vegetable (e.g., bayberry), mineral (e.g., paraffin), or synthetic (e.g., polyethylene). Waxes are used for polishes, candles, crayons, sealants, coatings, adhesives, waterproofing, carbon paper, media in encaustic and wax emulsion paintings, and as repellents in wax-resist watercolor paintings."@en ;
            dcterms:creator "The J. Paul Getty Trust" ;
            dcterms:license <https://opendatacommons.org/licenses/by/1-0/> ;
            dcterms:rights <https://rightsstatements.org/vocab/InC/1.0/> ;
            dcterms:source <http://www.getty.edu/research/tools/vocabularies/aat/> ],
        "Any solid or semi-solid substance that is slightly greasy to touch, usually solid, translucent, and has a low melting point; waxes are not a chemically homogeneous group. Waxes are composed of long chain hydrocarbon compounds, and may contain esters of fatty acids and alcohols, are thermoplastic and melt at low temperatures of between 40 and 100 C. In general, waxes are water-repellent, smooth, soluble in organic solvents, and classified as animal (e.g., beeswax), vegetable (e.g., bayberry), mineral (e.g., paraffin), or synthetic (e.g., polyethylene). Waxes are used for polishes, candles, crayons, sealants, coatings, adhesives, waterproofing, carbon paper, media in encaustic and wax emulsion paintings, and as repellents in wax-resist watercolor paintings."@en ;
    dcterms:identifier "CC00248" ;
    owl:sameAs <http://vocab.getty.edu/aat/300014585> .

cc:CC00249 a owl:NamedIndividual ;
    rdfs:label "wood"@en ;
    dcterms:description [ rdfs:label "The principal tissue of trees and other plants that provides both strength and a means of conducting nutrients. Wood is one of the most versatile materials known."@en ;
            dcterms:creator "The J. Paul Getty Trust" ;
            dcterms:license <https://opendatacommons.org/licenses/by/1-0/> ;
            dcterms:rights <https://rightsstatements.org/vocab/InC/1.0/> ;
            dcterms:source <http://www.getty.edu/research/tools/vocabularies/aat/> ],
        "The principal tissue of trees and other plants that provides both strength and a means of conducting nutrients. Wood is one of the most versatile materials known."@en ;
    dcterms:identifier "CC00249" ;
    owl:sameAs <http://vocab.getty.edu/aat/300011914> .

cc:CC00250 a owl:NamedIndividual ;
    rdfs:label "wool"@en ;
    dcterms:description [ rdfs:label "Textile made from the animal hair wool. (AAT)"@en ;
            dcterms:creator "The J. Paul Getty Trust" ;
            dcterms:license <https://opendatacommons.org/licenses/by/1-0/> ;
            dcterms:rights <https://rightsstatements.org/vocab/InC/1.0/> ;
            dcterms:source <http://www.getty.edu/research/tools/vocabularies/aat/> ],
        "Textile made from the animal hair wool. (AAT)"@en ;
    dcterms:identifier "CC00250" ;
    owl:sameAs <http://vocab.getty.edu/aat/300243430> .

cc:CC00259 a owl:NamedIndividual ;
    rdfs:label "adhesive"@en ;
    dcterms:description [ rdfs:label "A substance, in the form of a liquid, paste, powder, or dry film; used for sticking or adhering one surface to another. A substance capable of holding materials together by a surface attachment."@en ;
            dcterms:creator "The J. Paul Getty Trust" ;
            dcterms:license <https://opendatacommons.org/licenses/by/1-0/> ;
            dcterms:rights <https://rightsstatements.org/vocab/InC/1.0/> ;
            dcterms:source <http://www.getty.edu/research/tools/vocabularies/aat/> ],
        "A substance, in the form of a liquid, paste, powder, or dry film; used for sticking or adhering one surface to another. A substance capable of holding materials together by a surface attachment."@en ;
    dcterms:identifier "CC00259" ;
    owl:sameAs <http://vocab.getty.edu/aat/300014801> .

cc:CC00260 a owl:NamedIndividual ;
    rdfs:label "batiste"@en ;
    dcterms:description [ rdfs:label "Fine, soft, sheer cloth of plain weave made of any of the principal types of fiber, such as cotton, linen, rayon, silk, or wool."@en ;
            dcterms:creator "The J. Paul Getty Trust" ;
            dcterms:license <https://opendatacommons.org/licenses/by/1-0/> ;
            dcterms:rights <https://rightsstatements.org/vocab/InC/1.0/> ;
            dcterms:source <http://www.getty.edu/research/tools/vocabularies/aat/> ],
        "Fine, soft, sheer cloth of plain weave made of any of the principal types of fiber, such as cotton, linen, rayon, silk, or wool."@en ;
    dcterms:identifier "CC00260" ;
    owl:sameAs <http://vocab.getty.edu/aat/300183634> .

cc:CC00261 a owl:NamedIndividual ;
    rdfs:label "batting"@en ;
    dcterms:description [ rdfs:label "A soft cushion of loosely matted fibers of cotton, polyester, or wool, often distributed in a roll, used in upholstered furniture, cushions, packing, dollmaking, padding, and interlining in quilting."@en ;
            dcterms:creator "The J. Paul Getty Trust" ;
            dcterms:license <https://opendatacommons.org/licenses/by/1-0/> ;
            dcterms:rights <https://rightsstatements.org/vocab/InC/1.0/> ;
            dcterms:source <http://www.getty.edu/research/tools/vocabularies/aat/> ],
        "A soft cushion of loosely matted fibers of cotton, polyester, or wool, often distributed in a roll, used in upholstered furniture, cushions, packing, dollmaking, padding, and interlining in quilting."@en ;
    dcterms:identifier "CC00261" ;
    owl:sameAs <http://vocab.getty.edu/aat/300227771> .

cc:CC00262 a owl:NamedIndividual ;
    rdfs:label "beads"@en ;
    dcterms:description [ rdfs:label "Refers to small objects, of any shape or material, pierced so that they may be strung or hung or attached, as by sewing."@en ;
            dcterms:creator "The J. Paul Getty Trust" ;
            dcterms:license <https://opendatacommons.org/licenses/by/1-0/> ;
            dcterms:rights <https://rightsstatements.org/vocab/InC/1.0/> ;
            dcterms:source <http://www.getty.edu/research/tools/vocabularies/aat/> ],
        "Refers to small objects, of any shape or material, pierced so that they may be strung or hung or attached, as by sewing."@en ;
    dcterms:identifier "CC00262" ;
    owl:sameAs <http://vocab.getty.edu/aat/300234006> .

cc:CC00264 a owl:NamedIndividual ;
    rdfs:label "braid"@en ;
    dcterms:description [ rdfs:label "A narrow trimming made by a variety of techniques such as tablet weaving or braiding. It comes in a variety of fibers and weights, but is heavier than ribbon and flatter than cord."@en ;
            dcterms:creator "The J. Paul Getty Trust" ;
            dcterms:license <https://opendatacommons.org/licenses/by/1-0/> ;
            dcterms:rights <https://rightsstatements.org/vocab/InC/1.0/> ;
            dcterms:source <http://www.getty.edu/research/tools/vocabularies/aat/> ],
        "A narrow trimming made by a variety of techniques such as tablet weaving or braiding. It comes in a variety of fibers and weights, but is heavier than ribbon and flatter than cord."@en ;
    dcterms:identifier "CC00264" ;
    owl:sameAs <http://vocab.getty.edu/aat/300232186> .

cc:CC00266 a owl:NamedIndividual ;
    rdfs:label "buckram"@en ;
    dcterms:description [ rdfs:label "Heavy weave cotton, jute, or linen textile stiffened with glue, size, or starch and used for interlinings in garments, box making, bookbinding, etc."@en ;
            dcterms:creator "The J. Paul Getty Trust" ;
            dcterms:license <https://opendatacommons.org/licenses/by/1-0/> ;
            dcterms:rights <https://rightsstatements.org/vocab/InC/1.0/> ;
            dcterms:source <http://www.getty.edu/research/tools/vocabularies/aat/> ],
        "Heavy weave cotton, jute, or linen textile stiffened with glue, size, or starch and used for interlinings in garments, box making, bookbinding, etc."@en ;
    dcterms:identifier "CC00266" ;
    owl:sameAs <http://vocab.getty.edu/aat/300253474> .

cc:CC00267 a owl:NamedIndividual ;
    rdfs:label "cardboard"@en ;
    dcterms:description [ rdfs:label "A type of stiff pasteboard that is thicker than 0.006 inches, typically consisting of good-quality chemical pulp or rag pasteboard, and varying greatly in type and stability. High quality archival cardboard is made from rag pulp and has a low acid content, used for mounting prints, drawings and watercolors. Other grades of cardboard is used for cards, signs, printed materials, and high-quality boxes. Inferior grades of cardboard, such as corrugated board, are made from coarsely ground sulfite treated wood pulp; for this board, use \"corrugated board.\" The first carboard box was produced in England in 1817. Corrugated cardboard was patented in 1871."@en ;
            dcterms:creator "The J. Paul Getty Trust" ;
            dcterms:license <https://opendatacommons.org/licenses/by/1-0/> ;
            dcterms:rights <https://rightsstatements.org/vocab/InC/1.0/> ;
            dcterms:source <http://www.getty.edu/research/tools/vocabularies/aat/> ],
        "A type of stiff pasteboard that is thicker than 0.006 inches, typically consisting of good-quality chemical pulp or rag pasteboard, and varying greatly in type and stability. High quality archival cardboard is made from rag pulp and has a low acid content, used for mounting prints, drawings and watercolors. Other grades of cardboard is used for cards, signs, printed materials, and high-quality boxes. Inferior grades of cardboard, such as corrugated board, are made from coarsely ground sulfite treated wood pulp; for this board, use \"corrugated board.\" The first carboard box was produced in England in 1817. Corrugated cardboard was patented in 1871."@en ;
    dcterms:identifier "CC00267" ;
    owl:sameAs <http://vocab.getty.edu/aat/300014224> .

cc:CC00268 a owl:NamedIndividual ;
    rdfs:label "chenille"@en ;
    dcterms:description [ rdfs:label "Tufted cord, of silk or worsted, for the trimming of ladies' dresses, for embroidery and fringes, and for the weft of Chenillerugs. (Webster's)"@en ;
            dcterms:creator "The J. Paul Getty Trust" ;
            dcterms:license <https://opendatacommons.org/licenses/by/1-0/> ;
            dcterms:rights <https://rightsstatements.org/vocab/InC/1.0/> ;
            dcterms:source <http://www.getty.edu/research/tools/vocabularies/aat/> ],
        "Tufted cord, of silk or worsted, for the trimming of ladies' dresses, for embroidery and fringes, and for the weft of Chenillerugs. (Webster's)"@en ;
    dcterms:identifier "CC00268" ;
    owl:sameAs <http://vocab.getty.edu/aat/300227801> .

cc:CC00269 a owl:NamedIndividual ;
    rdfs:label "China silk"@en ;
    dcterms:description [ rdfs:label "Lightweight silk of plain weave."@en ;
            dcterms:creator "The J. Paul Getty Trust" ;
            dcterms:license <https://opendatacommons.org/licenses/by/1-0/> ;
            dcterms:rights <https://rightsstatements.org/vocab/InC/1.0/> ;
            dcterms:source <http://www.getty.edu/research/tools/vocabularies/aat/> ],
        "Lightweight silk of plain weave."@en ;
    dcterms:identifier "CC00269" ;
    owl:sameAs <http://vocab.getty.edu/aat/300132896> .

cc:CC00270 a owl:NamedIndividual ;
    rdfs:label "chintz"@en ;
    dcterms:description [ rdfs:label "Textile, usually cotton or linen, dyed in a number of colors and usually glazed."@en ;
            dcterms:creator "The J. Paul Getty Trust" ;
            dcterms:license <https://opendatacommons.org/licenses/by/1-0/> ;
            dcterms:rights <https://rightsstatements.org/vocab/InC/1.0/> ;
            dcterms:source <http://www.getty.edu/research/tools/vocabularies/aat/> ],
        "Textile, usually cotton or linen, dyed in a number of colors and usually glazed."@en ;
    dcterms:identifier "CC00270" ;
    owl:sameAs <http://vocab.getty.edu/aat/300132876> .

cc:CC00272 a owl:NamedIndividual ;
    rdfs:label "cord"@en ;
    dcterms:description [ rdfs:label "Long, slender, flexible, roughly cylindrical construction of fibrous material, usually made of several strands twisted together. Cord is typically made from a type of bast fiber such as cotton, jute, flax, ramie, hemp, sisal, olona, gravata, agel, widuri, caraguata, or others."@en ;
            dcterms:creator "The J. Paul Getty Trust" ;
            dcterms:license <https://opendatacommons.org/licenses/by/1-0/> ;
            dcterms:rights <https://rightsstatements.org/vocab/InC/1.0/> ;
            dcterms:source <http://www.getty.edu/research/tools/vocabularies/aat/> ],
        "Long, slender, flexible, roughly cylindrical construction of fibrous material, usually made of several strands twisted together. Cord is typically made from a type of bast fiber such as cotton, jute, flax, ramie, hemp, sisal, olona, gravata, agel, widuri, caraguata, or others."@en ;
    dcterms:identifier "CC00272" ;
    owl:sameAs <http://vocab.getty.edu/aat/300014247> .

cc:CC00273 a owl:NamedIndividual ;
    rdfs:label "Dacron"@en ;
    dcterms:description [ rdfs:label "Trademarked name for the textile fiber made of polyethylene terephthalate. Originally manufactured and developed by Du Pont."@en ;
            dcterms:creator "The J. Paul Getty Trust" ;
            dcterms:license <https://opendatacommons.org/licenses/by/1-0/> ;
            dcterms:rights <https://rightsstatements.org/vocab/InC/1.0/> ;
            dcterms:source <http://www.getty.edu/research/tools/vocabularies/aat/> ],
        "Trademarked name for the textile fiber made of polyethylene terephthalate. Originally manufactured and developed by Du Pont."@en ;
    dcterms:identifier "CC00273" ;
    owl:sameAs <http://vocab.getty.edu/aat/300132879> .

cc:CC00274 a owl:NamedIndividual ;
    rdfs:label "dupioni"@en ;
    dcterms:description [ rdfs:label "Irregular, rough silk reeled from double cocoons or cocoons spun side-by-side that have interlocked. The surface can be recognized by the irregular relief caused by the uneven width of the yarns, and this quality makes it difficult to distinguish from wild silk."@en ;
            dcterms:creator "The J. Paul Getty Trust" ;
            dcterms:license <https://opendatacommons.org/licenses/by/1-0/> ;
            dcterms:rights <https://rightsstatements.org/vocab/InC/1.0/> ;
            dcterms:source <http://www.getty.edu/research/tools/vocabularies/aat/> ],
        "Irregular, rough silk reeled from double cocoons or cocoons spun side-by-side that have interlocked. The surface can be recognized by the irregular relief caused by the uneven width of the yarns, and this quality makes it difficult to distinguish from wild silk."@en ;
    dcterms:identifier "CC00274" ;
    owl:sameAs <http://vocab.getty.edu/aat/300417880> .

cc:CC00275 a owl:NamedIndividual ;
    rdfs:label "faille"@en ;
    dcterms:description [ rdfs:label "Plain-woven textile, originally of silk, now made also of wool, cotton, and synthetic fibers, characterized by slight, flat ribs in the weft; used, for example, for women's suits and dresses, hats, trimmings, and interior furnishings."@en ;
            dcterms:creator "The J. Paul Getty Trust" ;
            dcterms:license <https://opendatacommons.org/licenses/by/1-0/> ;
            dcterms:rights <https://rightsstatements.org/vocab/InC/1.0/> ;
            dcterms:source <http://www.getty.edu/research/tools/vocabularies/aat/> ],
        "Plain-woven textile, originally of silk, now made also of wool, cotton, and synthetic fibers, characterized by slight, flat ribs in the weft; used, for example, for women's suits and dresses, hats, trimmings, and interior furnishings."@en ;
    dcterms:identifier "CC00275" ;
    owl:sameAs <http://vocab.getty.edu/aat/300249448> .

cc:CC00276 a owl:NamedIndividual ;
    rdfs:label "feathers"@en ;
    dcterms:description [ rdfs:label "Material comprising stiff, lightweight, often colorful, keratin structures that are the principal covering of birds."@en ;
            dcterms:creator "The J. Paul Getty Trust" ;
            dcterms:license <https://opendatacommons.org/licenses/by/1-0/> ;
            dcterms:rights <https://rightsstatements.org/vocab/InC/1.0/> ;
            dcterms:source <http://www.getty.edu/research/tools/vocabularies/aat/> ],
        "Material comprising stiff, lightweight, often colorful, keratin structures that are the principal covering of birds."@en ;
    dcterms:identifier "CC00276" ;
    owl:sameAs <http://vocab.getty.edu/aat/300011809> .

cc:CC00278 a owl:NamedIndividual ;
    rdfs:label "flowers"@en ;
    dcterms:description [ rdfs:label "Imitation flower, usually of silk or synthetic fabric, used as an ornament on clothing or hats."@en ;
            dcterms:creator "Wikidata contributors" ;
            dcterms:license <https://creativecommons.org/publicdomain/mark/1.0/> ;
            dcterms:rights <https://creativecommons.org/publicdomain/mark/1.0/> ;
            dcterms:source <https://www.wikidata.org/wiki/Wikidata:Data_access/en> ],
        "Imitation flower, usually of silk or synthetic fabric, used as an ornament on clothing or hats."@en ;
    dcterms:identifier "CC00278" ;
    owl:sameAs <http://www.wikidata.org/entity/Q44407651> .

cc:CC00279 a owl:NamedIndividual ;
    rdfs:label "fur"@en ;
    dcterms:description [ rdfs:label "Fine, soft, thick, hairy coat of a mammal, usually consisting of a double coat of hair that includes a layer of comparatively short, soft, curly barbed hair next to the skin, protected by longer, smoother, stiffer hair growing up through it."@en ;
            dcterms:creator "The J. Paul Getty Trust" ;
            dcterms:license <https://opendatacommons.org/licenses/by/1-0/> ;
            dcterms:rights <https://rightsstatements.org/vocab/InC/1.0/> ;
            dcterms:source <http://www.getty.edu/research/tools/vocabularies/aat/> ],
        "Fine, soft, thick, hairy coat of a mammal, usually consisting of a double coat of hair that includes a layer of comparatively short, soft, curly barbed hair next to the skin, protected by longer, smoother, stiffer hair growing up through it."@en ;
    dcterms:identifier "CC00279" ;
    owl:sameAs <http://vocab.getty.edu/aat/300011811> .

cc:CC00280 a owl:NamedIndividual ;
    rdfs:label "gabardine"@en ;
    dcterms:description [ rdfs:label "Variety of twill-woven cloth, usually of fine worsted yarn or thread."@en ;
            dcterms:creator "The J. Paul Getty Trust" ;
            dcterms:license <https://opendatacommons.org/licenses/by/1-0/> ;
            dcterms:rights <https://rightsstatements.org/vocab/InC/1.0/> ;
            dcterms:source <http://www.getty.edu/research/tools/vocabularies/aat/> ],
        "Variety of twill-woven cloth, usually of fine worsted yarn or thread."@en ;
    dcterms:identifier "CC00280" ;
    owl:sameAs <http://vocab.getty.edu/aat/300403912> .

cc:CC00281 a owl:NamedIndividual ;
    rdfs:label "gauze"@en ;
    dcterms:description [ rdfs:label "Woven textile in which the binding is achieved by a displacement of warp ends secured by the weft, resulting usually, though not always, in a very open weave; used particularly for surgical dressings and as backing for paper, especially maps."@en ;
            dcterms:creator "The J. Paul Getty Trust" ;
            dcterms:license <https://opendatacommons.org/licenses/by/1-0/> ;
            dcterms:rights <https://rightsstatements.org/vocab/InC/1.0/> ;
            dcterms:source <http://www.getty.edu/research/tools/vocabularies/aat/> ],
        "Woven textile in which the binding is achieved by a displacement of warp ends secured by the weft, resulting usually, though not always, in a very open weave; used particularly for surgical dressings and as backing for paper, especially maps."@en ;
    dcterms:identifier "CC00281" ;
    owl:sameAs <http://vocab.getty.edu/aat/300014083> .

cc:CC00282 a owl:NamedIndividual ;
    rdfs:label "horsehair"@en ;
    dcterms:description [ rdfs:label "Hair from the manes and tails of horses, used chiefly as a brush fiber, for musical instrument bows, and for making haircloth.(AAT)"@en ;
            dcterms:creator "The J. Paul Getty Trust" ;
            dcterms:license <https://opendatacommons.org/licenses/by/1-0/> ;
            dcterms:rights <https://rightsstatements.org/vocab/InC/1.0/> ;
            dcterms:source <http://www.getty.edu/research/tools/vocabularies/aat/> ],
        "Hair from the manes and tails of horses, used chiefly as a brush fiber, for musical instrument bows, and for making haircloth.(AAT)"@en ;
    dcterms:identifier "CC00282" ;
    owl:sameAs <http://vocab.getty.edu/aat/300011819> .

cc:CC00283 a owl:NamedIndividual ;
    rdfs:label "jersey"@en ;
    dcterms:description [ rdfs:label "Plain knit fabric."@en ;
            dcterms:creator "Wikidata contributors" ;
            dcterms:license <https://creativecommons.org/publicdomain/mark/1.0/> ;
            dcterms:rights <https://creativecommons.org/publicdomain/mark/1.0/> ;
            dcterms:source <https://www.wikidata.org/wiki/Wikidata:Data_access/en> ],
        "Plain knit fabric."@en ;
    dcterms:identifier "CC00283" ;
    owl:sameAs <http://www.wikidata.org/entity/Q1348773> .

cc:CC00284 a owl:NamedIndividual ;
    rdfs:label "jet"@en ;
    dcterms:description [ rdfs:label "A dense, black, semiprecious form of lignite that takes a brilliant polish and is used ornamentally, particularly in Victorian mourning jewelry."@en ;
            dcterms:creator "The J. Paul Getty Trust" ;
            dcterms:license <https://opendatacommons.org/licenses/by/1-0/> ;
            dcterms:rights <https://rightsstatements.org/vocab/InC/1.0/> ;
            dcterms:source <http://www.getty.edu/research/tools/vocabularies/aat/> ],
        "A dense, black, semiprecious form of lignite that takes a brilliant polish and is used ornamentally, particularly in Victorian mourning jewelry."@en ;
    dcterms:identifier "CC00284" ;
    owl:sameAs <http://vocab.getty.edu/aat/300045514> .

cc:CC00285 a owl:NamedIndividual ;
    rdfs:label "lawn"@en ;
    dcterms:description [ rdfs:label "Sheer, lightweight plain-woven textile, originally of linen now also of fine combed cotton yarn, filled with starch or sizing. often used for handkerchiefs, aprons, and curtains."@en ;
            dcterms:creator "The J. Paul Getty Trust" ;
            dcterms:license <https://opendatacommons.org/licenses/by/1-0/> ;
            dcterms:rights <https://rightsstatements.org/vocab/InC/1.0/> ;
            dcterms:source <http://www.getty.edu/research/tools/vocabularies/aat/> ],
        "Sheer, lightweight plain-woven textile, originally of linen now also of fine combed cotton yarn, filled with starch or sizing. often used for handkerchiefs, aprons, and curtains."@en ;
    dcterms:identifier "CC00285" ;
    owl:sameAs <http://vocab.getty.edu/aat/300249444> .

cc:CC00286 a owl:NamedIndividual ;
    rdfs:label "leaves"@en ;
    dcterms:description [ rdfs:label "Outgrowths, usually green and flattened, that extend from the stem of a vascular plant. Botanically, leaves are an integral part of the stem system, and they are initiated in the apical bud along with the tissues of the stem itself. Leaves manufacture food for plants, which in turn ultimately nourish and sustain all land animals, directly or indirectly."@en ;
            dcterms:creator "The J. Paul Getty Trust" ;
            dcterms:license <https://opendatacommons.org/licenses/by/1-0/> ;
            dcterms:rights <https://rightsstatements.org/vocab/InC/1.0/> ;
            dcterms:source <http://www.getty.edu/research/tools/vocabularies/aat/> ],
        "Outgrowths, usually green and flattened, that extend from the stem of a vascular plant. Botanically, leaves are an integral part of the stem system, and they are initiated in the apical bud along with the tissues of the stem itself. Leaves manufacture food for plants, which in turn ultimately nourish and sustain all land animals, directly or indirectly."@en ;
    dcterms:identifier "CC00286" ;
    owl:sameAs <http://vocab.getty.edu/aat/300400479> .

cc:CC00288 a owl:NamedIndividual ;
    rdfs:label "merino"@en ;
    dcterms:description [ rdfs:label "Fine, soft, light wool from merino sheep resembling cashmere; also yarn or fabric made from the wool, sometimes in combination with cotton. By extension any fine woolen yarn used in knitwear."@en ;
            dcterms:creator "The J. Paul Getty Trust" ;
            dcterms:license <https://opendatacommons.org/licenses/by/1-0/> ;
            dcterms:rights <https://rightsstatements.org/vocab/InC/1.0/> ;
            dcterms:source <http://www.getty.edu/research/tools/vocabularies/aat/> ],
        "Fine, soft, light wool from merino sheep resembling cashmere; also yarn or fabric made from the wool, sometimes in combination with cotton. By extension any fine woolen yarn used in knitwear."@en ;
    dcterms:identifier "CC00288" ;
    owl:sameAs <http://vocab.getty.edu/aat/300380171> .

cc:CC00289 a owl:NamedIndividual ;
    rdfs:label "mesh"@en ;
    dcterms:description [ rdfs:label "Fabric with open spaces between the yarn or wire. A mesh fabric may be knit, woven, or knotted."@en ;
            dcterms:creator "The J. Paul Getty Trust" ;
            dcterms:license <https://opendatacommons.org/licenses/by/1-0/> ;
            dcterms:rights <https://rightsstatements.org/vocab/InC/1.0/> ;
            dcterms:source <http://www.getty.edu/research/tools/vocabularies/aat/> ],
        "Fabric with open spaces between the yarn or wire. A mesh fabric may be knit, woven, or knotted."@en ;
    dcterms:identifier "CC00289" ;
    owl:sameAs <http://vocab.getty.edu/aat/300410339> .

cc:CC00290 a owl:NamedIndividual ;
    rdfs:label "metallic"@en ;
    dcterms:description [ rdfs:label "Of or pertaining to a metal; of the nature of metal; resembling metal; as, a metallic appearance (Webster's)"@en ;
            dcterms:creator "The J. Paul Getty Trust" ;
            dcterms:license <https://opendatacommons.org/licenses/by/1-0/> ;
            dcterms:rights <https://rightsstatements.org/vocab/InC/1.0/> ;
            dcterms:source <http://www.getty.edu/research/tools/vocabularies/aat/> ],
        "Of or pertaining to a metal; of the nature of metal; resembling metal; as, a metallic appearance (Webster's)"@en ;
    dcterms:identifier "CC00290" ;
    owl:sameAs <http://vocab.getty.edu/aat/300311171> .

cc:CC00292 a owl:NamedIndividual ;
    rdfs:label "mother of pearl"@en ;
    dcterms:description [ rdfs:label "Hard, pearly, iridescent internal layer of various kinds of mollusk shell, extensively used for making small articles and inlays."@en ;
            dcterms:creator "The J. Paul Getty Trust" ;
            dcterms:license <https://opendatacommons.org/licenses/by/1-0/> ;
            dcterms:rights <https://rightsstatements.org/vocab/InC/1.0/> ;
            dcterms:source <http://www.getty.edu/research/tools/vocabularies/aat/> ],
        "Hard, pearly, iridescent internal layer of various kinds of mollusk shell, extensively used for making small articles and inlays."@en ;
    dcterms:identifier "CC00292" ;
    owl:sameAs <http://vocab.getty.edu/aat/300011835> .

cc:CC00293 a owl:NamedIndividual ;
    rdfs:label "muslin"@en ;
    dcterms:description [ rdfs:label "Very fine plain weave white cotton made in a great variety of qualities; originally from India, it has been extensively produced and used in Europe and North America for costume, and sometimes as an artist's support."@en ;
            dcterms:creator "The J. Paul Getty Trust" ;
            dcterms:license <https://opendatacommons.org/licenses/by/1-0/> ;
            dcterms:rights <https://rightsstatements.org/vocab/InC/1.0/> ;
            dcterms:source <http://www.getty.edu/research/tools/vocabularies/aat/> ],
        "Very fine plain weave white cotton made in a great variety of qualities; originally from India, it has been extensively produced and used in Europe and North America for costume, and sometimes as an artist's support."@en ;
    dcterms:identifier "CC00293" ;
    owl:sameAs <http://vocab.getty.edu/aat/300014087> .

cc:CC00294 a owl:NamedIndividual ;
    rdfs:label "organza"@en ;
    dcterms:description [ rdfs:label "Sheer, crisp fabric made with a loose plain weave; usually made from silk or synthetics such as rayon, nylon, acrylic or polyester. It is fine to leightweight, strong, stable, and durable. It is distinct from organdy, which is made from cotton."@en ;
            dcterms:creator "The J. Paul Getty Trust" ;
            dcterms:license <https://opendatacommons.org/licenses/by/1-0/> ;
            dcterms:rights <https://rightsstatements.org/vocab/InC/1.0/> ;
            dcterms:source <http://www.getty.edu/research/tools/vocabularies/aat/> ],
        "Sheer, crisp fabric made with a loose plain weave; usually made from silk or synthetics such as rayon, nylon, acrylic or polyester. It is fine to leightweight, strong, stable, and durable. It is distinct from organdy, which is made from cotton."@en ;
    dcterms:identifier "CC00294" ;
    owl:sameAs <http://vocab.getty.edu/aat/300310123> .

cc:CC00295 a owl:NamedIndividual ;
    rdfs:label "paint"@en ;
    dcterms:description [ rdfs:label "Any dispersion of pigment in a liquid binder. Paint is applied with a brush, roller, sprayer, or by dipping and dries to form a decorative or protective film."@en ;
            dcterms:creator "The J. Paul Getty Trust" ;
            dcterms:license <https://opendatacommons.org/licenses/by/1-0/> ;
            dcterms:rights <https://rightsstatements.org/vocab/InC/1.0/> ;
            dcterms:source <http://www.getty.edu/research/tools/vocabularies/aat/> ],
        "Any dispersion of pigment in a liquid binder. Paint is applied with a brush, roller, sprayer, or by dipping and dries to form a decorative or protective film."@en ;
    dcterms:identifier "CC00295" ;
    owl:sameAs <http://vocab.getty.edu/aat/300015029> .

cc:CC00296 a owl:NamedIndividual ;
    rdfs:label "paper"@en ;
    dcterms:description [ rdfs:label "Refers generally to all types of thin matted or felted sheets or webs of fiber formed and dried on a fine screen from a pulpy water suspension. The fibers may be animal, such as hair, silk or wool, or mineral, such as asbestos, or synthetic. However most paper is made from cellulosic plant fiber, such as from wood pulp, grass, cotton, linen, and straw."@en ;
            dcterms:creator "The J. Paul Getty Trust" ;
            dcterms:license <https://opendatacommons.org/licenses/by/1-0/> ;
            dcterms:rights <https://rightsstatements.org/vocab/InC/1.0/> ;
            dcterms:source <http://www.getty.edu/research/tools/vocabularies/aat/> ],
        "Refers generally to all types of thin matted or felted sheets or webs of fiber formed and dried on a fine screen from a pulpy water suspension. The fibers may be animal, such as hair, silk or wool, or mineral, such as asbestos, or synthetic. However most paper is made from cellulosic plant fiber, such as from wood pulp, grass, cotton, linen, and straw."@en ;
    dcterms:identifier "CC00296" ;
    owl:sameAs <http://vocab.getty.edu/aat/300014109> .

cc:CC00297 a owl:NamedIndividual ;
    rdfs:label "pearl"@en ;
    dcterms:description [ rdfs:label "A smooth round bead formed primarily within the shells of two distantly related groups of molluscan bivalves or clams, including the ocean-dwelling pearl oysters and the freshwater river mussels. Pearls are used in jewelry and for other ornamental puposes; they are considered a gem."@en ;
            dcterms:creator "The J. Paul Getty Trust" ;
            dcterms:license <https://opendatacommons.org/licenses/by/1-0/> ;
            dcterms:rights <https://rightsstatements.org/vocab/InC/1.0/> ;
            dcterms:source <http://www.getty.edu/research/tools/vocabularies/aat/> ],
        "A smooth round bead formed primarily within the shells of two distantly related groups of molluscan bivalves or clams, including the ocean-dwelling pearl oysters and the freshwater river mussels. Pearls are used in jewelry and for other ornamental puposes; they are considered a gem."@en ;
    dcterms:identifier "CC00297" ;
    owl:sameAs <http://vocab.getty.edu/aat/300011827> .

cc:CC00298 a owl:NamedIndividual ;
    rdfs:label "pia cloth"@en ;
    dcterms:description [ rdfs:label "Fine, lustrous, soft, sheer cloth originating in the Philippines, woven from pia fibers, from the pineapple plant. It is used for decorative handkerchiefs, trimmings, lingerie, accessories, and home furnishings."@en ;
            dcterms:creator "The J. Paul Getty Trust" ;
            dcterms:license <https://opendatacommons.org/licenses/by/1-0/> ;
            dcterms:rights <https://rightsstatements.org/vocab/InC/1.0/> ;
            dcterms:source <http://www.getty.edu/research/tools/vocabularies/aat/> ],
        "Fine, lustrous, soft, sheer cloth originating in the Philippines, woven from pia fibers, from the pineapple plant. It is used for decorative handkerchiefs, trimmings, lingerie, accessories, and home furnishings."@en ;
    dcterms:identifier "CC00298" ;
    owl:sameAs <http://vocab.getty.edu/aat/300263386> .

cc:CC00299 a owl:NamedIndividual ;
    rdfs:label "pineapple fiber"@en ;
    dcterms:description [ rdfs:label "Long bast fibers obtained from the leaves of the species Ananas comosus, native to tropical America. The fibers are fine, soft, lustrous, and light cream in color. They are resistant to salt water, strong, wear resistant, and easy to clean; used for fabric, rope, twine, and paper."@en ;
            dcterms:creator "The J. Paul Getty Trust" ;
            dcterms:license <https://opendatacommons.org/licenses/by/1-0/> ;
            dcterms:rights <https://rightsstatements.org/vocab/InC/1.0/> ;
            dcterms:source <http://www.getty.edu/research/tools/vocabularies/aat/> ],
        "Long bast fibers obtained from the leaves of the species Ananas comosus, native to tropical America. The fibers are fine, soft, lustrous, and light cream in color. They are resistant to salt water, strong, wear resistant, and easy to clean; used for fabric, rope, twine, and paper."@en ;
    dcterms:identifier "CC00299" ;
    owl:sameAs <http://vocab.getty.edu/aat/300375581> .

cc:CC00302 a owl:NamedIndividual ;
    rdfs:label "porcelain"@en ;
    dcterms:description [ rdfs:label "A material comprising white clay, or \"kaolin,\" and a feldspathic rock, that react when fired so the clay serves to hold the shape of the object and the rock fuses into a natural glass. In China, it includes any such ware that is highly fired enough to produce a ringing sound when struck. In Europe, it is limited to hard-fired ceramic that is translucent."@en ;
            dcterms:creator "The J. Paul Getty Trust" ;
            dcterms:license <https://opendatacommons.org/licenses/by/1-0/> ;
            dcterms:rights <https://rightsstatements.org/vocab/InC/1.0/> ;
            dcterms:source <http://www.getty.edu/research/tools/vocabularies/aat/> ],
        "A material comprising white clay, or \"kaolin,\" and a feldspathic rock, that react when fired so the clay serves to hold the shape of the object and the rock fuses into a natural glass. In China, it includes any such ware that is highly fired enough to produce a ringing sound when struck. In Europe, it is limited to hard-fired ceramic that is translucent."@en ;
    dcterms:identifier "CC00302" ;
    owl:sameAs <http://vocab.getty.edu/aat/300010662> .

cc:CC00303 a owl:NamedIndividual ;
    rdfs:label "raffia"@en ;
    dcterms:description [ rdfs:label "Strong fiber from leafstalks of palms of the genus Raphia, native to Africa and other places. Raffia fibers are used in their natural state by splitting apart thick sections and knotting the ends together. The fibers are a pale cream color and are often dyed to bright colors. Raffia is used to make skirts, woven into baskets, hats, bags, and mats. It is also used to make a fine grade of paper similar to Japanese papers."@en ;
            dcterms:creator "The J. Paul Getty Trust" ;
            dcterms:license <https://opendatacommons.org/licenses/by/1-0/> ;
            dcterms:rights <https://rightsstatements.org/vocab/InC/1.0/> ;
            dcterms:source <http://www.getty.edu/research/tools/vocabularies/aat/> ],
        "Strong fiber from leafstalks of palms of the genus Raphia, native to Africa and other places. Raffia fibers are used in their natural state by splitting apart thick sections and knotting the ends together. The fibers are a pale cream color and are often dyed to bright colors. Raffia is used to make skirts, woven into baskets, hats, bags, and mats. It is also used to make a fine grade of paper similar to Japanese papers."@en ;
    dcterms:identifier "CC00303" ;
    owl:sameAs <http://vocab.getty.edu/aat/300014051> .

cc:CC00304 a owl:NamedIndividual ;
    rdfs:label "rhinestones"@en ;
    dcterms:description [ rdfs:label "A colorless artificial gem of paste or glass, often with facets that sparkle in imitation of a diamond. Also refers to foil-backed or silvered cut glass used to imitate diamonds. Rhinestones were originally quartz pebbles found in the Rhine River, thus the name."@en ;
            dcterms:creator "The J. Paul Getty Trust" ;
            dcterms:license <https://opendatacommons.org/licenses/by/1-0/> ;
            dcterms:rights <https://rightsstatements.org/vocab/InC/1.0/> ;
            dcterms:source <http://www.getty.edu/research/tools/vocabularies/aat/> ],
        "A colorless artificial gem of paste or glass, often with facets that sparkle in imitation of a diamond. Also refers to foil-backed or silvered cut glass used to imitate diamonds. Rhinestones were originally quartz pebbles found in the Rhine River, thus the name."@en ;
    dcterms:identifier "CC00304" ;
    owl:sameAs <http://vocab.getty.edu/aat/300010806> .

cc:CC00305 a owl:NamedIndividual ;
    rdfs:label "rope"@en ;
    dcterms:description [ rdfs:label "Heavy cord, at least 1/4 inch in diameter, formed by twisting or braiding three to six yarns of natural or artificial fiber. In ancient Egypt, ropes were made from reeds or date palm fibers. Ancient ropes were also made from flax, grass, esparto grass, hemp, sisal, coir, cotton, jute, papyrus, and camel hair. Up to 1850, most ropes were made from hemp or sisal. After this point, abaca and agave became the fibers of choice. By the 1950s, synthetic fibers (nylon, rayon, saran, polyester, etc.) became predominant. Glass and metallic fibers have also been incorporated into ropes for added strength and resistance to fire and chemicals."@en ;
            dcterms:creator "The J. Paul Getty Trust" ;
            dcterms:license <https://opendatacommons.org/licenses/by/1-0/> ;
            dcterms:rights <https://rightsstatements.org/vocab/InC/1.0/> ;
            dcterms:source <http://www.getty.edu/research/tools/vocabularies/aat/> ],
        "Heavy cord, at least 1/4 inch in diameter, formed by twisting or braiding three to six yarns of natural or artificial fiber. In ancient Egypt, ropes were made from reeds or date palm fibers. Ancient ropes were also made from flax, grass, esparto grass, hemp, sisal, coir, cotton, jute, papyrus, and camel hair. Up to 1850, most ropes were made from hemp or sisal. After this point, abaca and agave became the fibers of choice. By the 1950s, synthetic fibers (nylon, rayon, saran, polyester, etc.) became predominant. Glass and metallic fibers have also been incorporated into ropes for added strength and resistance to fire and chemicals."@en ;
    dcterms:identifier "CC00305" ;
    owl:sameAs <http://vocab.getty.edu/aat/300014248> .

cc:CC00306 a owl:NamedIndividual ;
    rdfs:label "rubber"@en ;
    dcterms:description [ rdfs:label "A natural hydrocarbon polymer formed from the resinous latex of trees of the Hevea and Parthenium genera. To prepare natural rubber, the latex is collected from a cut in the bark, precipitated with acid, then washed and dried. Rubber is very elastic and was used for bowls, shoe soles, adhesives, and bouncy balls. However, when cooled, rubber becomes brittle and when warmed it becomes sweaty and tacky. Prior to the development of synthetic resins, unvulcanized rubber was used for adhesive tapes and crepe shoe soles. In 1839, Charles Goodyear discovered that rubber can be hardened with the vulcanization process in which sulfur is used to initiate crosslinking of the hydrocarbon strands. Higher sulfur content produces a harder, denser material. Vulcanized rubber is used to make rubber bands, foams, fabric coatings, small objects, combs, pens, and musical instruments. Vulcanized rubber, however, will emit sulfur when exposed to light or heat causing the rubber to degrade and become brittle. Since the 19th century, small amounts of wax have been added to the rubber during vulcanization. The wax slowly migrates to the surface and provides a thin layer of protection from oxidation."@en ;
            dcterms:creator "The J. Paul Getty Trust" ;
            dcterms:license <https://opendatacommons.org/licenses/by/1-0/> ;
            dcterms:rights <https://rightsstatements.org/vocab/InC/1.0/> ;
            dcterms:source <http://www.getty.edu/research/tools/vocabularies/aat/> ],
        "A natural hydrocarbon polymer formed from the resinous latex of trees of the Hevea and Parthenium genera. To prepare natural rubber, the latex is collected from a cut in the bark, precipitated with acid, then washed and dried. Rubber is very elastic and was used for bowls, shoe soles, adhesives, and bouncy balls. However, when cooled, rubber becomes brittle and when warmed it becomes sweaty and tacky. Prior to the development of synthetic resins, unvulcanized rubber was used for adhesive tapes and crepe shoe soles. In 1839, Charles Goodyear discovered that rubber can be hardened with the vulcanization process in which sulfur is used to initiate crosslinking of the hydrocarbon strands. Higher sulfur content produces a harder, denser material. Vulcanized rubber is used to make rubber bands, foams, fabric coatings, small objects, combs, pens, and musical instruments. Vulcanized rubber, however, will emit sulfur when exposed to light or heat causing the rubber to degrade and become brittle. Since the 19th century, small amounts of wax have been added to the rubber during vulcanization. The wax slowly migrates to the surface and provides a thin layer of protection from oxidation."@en ;
    dcterms:identifier "CC00306" ;
    owl:sameAs <http://vocab.getty.edu/aat/300012941> .

cc:CC00307 a owl:NamedIndividual ;
    rdfs:label "sequins"@en ;
    dcterms:description [ rdfs:label "Adornment consisting of a small piece of shiny material used to decorate clothing (Wordnet)"@en ;
            dcterms:creator "The J. Paul Getty Trust" ;
            dcterms:license <https://opendatacommons.org/licenses/by/1-0/> ;
            dcterms:rights <https://rightsstatements.org/vocab/InC/1.0/> ;
            dcterms:source <http://www.getty.edu/research/tools/vocabularies/aat/> ],
        "Adornment consisting of a small piece of shiny material used to decorate clothing (Wordnet)"@en ;
    dcterms:identifier "CC00307" ;
    owl:sameAs <http://vocab.getty.edu/aat/300183896> .

cc:CC00308 a owl:NamedIndividual ;
    rdfs:label "skin"@en ;
    dcterms:description [ rdfs:label "Integument of animals such as sheep, calves, or goats, separated from the body, with or without hair, whether green, dry, tanned, or dressed. For the integument of large animals use \"hide.\" For tanned skin, use \"leather.\" For dried and stretched skin, use \"parchment\" or \"vellum.\""@en ;
            dcterms:creator "The J. Paul Getty Trust" ;
            dcterms:license <https://opendatacommons.org/licenses/by/1-0/> ;
            dcterms:rights <https://rightsstatements.org/vocab/InC/1.0/> ;
            dcterms:source <http://www.getty.edu/research/tools/vocabularies/aat/> ],
        "Integument of animals such as sheep, calves, or goats, separated from the body, with or without hair, whether green, dry, tanned, or dressed. For the integument of large animals use \"hide.\" For tanned skin, use \"leather.\" For dried and stretched skin, use \"parchment\" or \"vellum.\""@en ;
    dcterms:identifier "CC00308" ;
    owl:sameAs <http://vocab.getty.edu/aat/300011840> .

cc:CC00311 a owl:NamedIndividual ;
    rdfs:label "straw"@en ;
    dcterms:description [ rdfs:label "Dried stalks of cereals or other grasses, used for many purposes, including weaving, plaiting, and braiding."@en ;
            dcterms:creator "The J. Paul Getty Trust" ;
            dcterms:license <https://opendatacommons.org/licenses/by/1-0/> ;
            dcterms:rights <https://rightsstatements.org/vocab/InC/1.0/> ;
            dcterms:source <http://www.getty.edu/research/tools/vocabularies/aat/> ],
        "Dried stalks of cereals or other grasses, used for many purposes, including weaving, plaiting, and braiding."@en ;
    dcterms:identifier "CC00311" ;
    owl:sameAs <http://vocab.getty.edu/aat/300011908> .

cc:CC00312 a owl:NamedIndividual ;
    rdfs:label "tassel"@en ;
    dcterms:description [ rdfs:label "Pendant trimming. Before the 20th century, usually a wooden mold covered with strands of silk or worsted; now often merely a bunch of threads, cords, or other strands gathered together at the top."@en ;
            dcterms:creator "The J. Paul Getty Trust" ;
            dcterms:license <https://opendatacommons.org/licenses/by/1-0/> ;
            dcterms:rights <https://rightsstatements.org/vocab/InC/1.0/> ;
            dcterms:source <http://www.getty.edu/research/tools/vocabularies/aat/> ],
        "Pendant trimming. Before the 20th century, usually a wooden mold covered with strands of silk or worsted; now often merely a bunch of threads, cords, or other strands gathered together at the top."@en ;
    dcterms:identifier "CC00312" ;
    owl:sameAs <http://vocab.getty.edu/aat/300232185> .

cc:CC00313 a owl:NamedIndividual ;
    rdfs:label "thread"@en ;
    dcterms:description [ rdfs:label "Single filaments of fiber, groups of such filaments twisted tightly together, or filamentous lengths formed by spinning and twisting short fibers into a continuous strand."@en ;
            dcterms:creator "The J. Paul Getty Trust" ;
            dcterms:license <https://opendatacommons.org/licenses/by/1-0/> ;
            dcterms:rights <https://rightsstatements.org/vocab/InC/1.0/> ;
            dcterms:source <http://www.getty.edu/research/tools/vocabularies/aat/> ],
        "Single filaments of fiber, groups of such filaments twisted tightly together, or filamentous lengths formed by spinning and twisting short fibers into a continuous strand."@en ;
    dcterms:identifier "CC00313" ;
    owl:sameAs <http://vocab.getty.edu/aat/300014250> .

cc:CC00315 a owl:NamedIndividual ;
    rdfs:label "tulle"@en ;
    dcterms:description [ rdfs:label "Meshed textile made of sheer silk, nylon, or rayon with a hexagonal mesh; used for hats, veils, ballet costumes, and women's dresses."@en ;
            dcterms:creator "The J. Paul Getty Trust" ;
            dcterms:license <https://opendatacommons.org/licenses/by/1-0/> ;
            dcterms:rights <https://rightsstatements.org/vocab/InC/1.0/> ;
            dcterms:source <http://www.getty.edu/research/tools/vocabularies/aat/> ],
        "Meshed textile made of sheer silk, nylon, or rayon with a hexagonal mesh; used for hats, veils, ballet costumes, and women's dresses."@en ;
    dcterms:identifier "CC00315" ;
    owl:sameAs <http://vocab.getty.edu/aat/300256611> .

cc:CC00316 a owl:NamedIndividual ;
    rdfs:label "twill"@en ;
    dcterms:description [ rdfs:label "Refers to a woven textile characterized by parallel diagonal ridges or ribs, produced by passing the weft threads over one and under two or more threads of the warp, instead of over and under in regular succession, as in plain weaving. Regular twill features a diagonal line that is repeated regularly, usually running from the left to right at a 45-degree angle and upward. The weave may be varied in several ways, including changing the angle or direction of the twill line, as exemplified in herringbone twill."@en ;
            dcterms:creator "The J. Paul Getty Trust" ;
            dcterms:license <https://opendatacommons.org/licenses/by/1-0/> ;
            dcterms:rights <https://rightsstatements.org/vocab/InC/1.0/> ;
            dcterms:source <http://www.getty.edu/research/tools/vocabularies/aat/> ],
        "Refers to a woven textile characterized by parallel diagonal ridges or ribs, produced by passing the weft threads over one and under two or more threads of the warp, instead of over and under in regular succession, as in plain weaving. Regular twill features a diagonal line that is repeated regularly, usually running from the left to right at a 45-degree angle and upward. The weave may be varied in several ways, including changing the angle or direction of the twill line, as exemplified in herringbone twill."@en ;
    dcterms:identifier "CC00316" ;
    owl:sameAs <http://vocab.getty.edu/aat/300227915> .

cc:CC00318 a owl:NamedIndividual ;
    rdfs:label "vinyl"@en ;
    dcterms:description [ rdfs:label "Generic term for materials derived from vinyl chloride, vinyl acetate, or vinylidene chloride. Commonly used with reference to all polymers and copolymers of which vinyl chloride is a constituent. Use more precise terminology for known materials such as \"polyvinyl chloride\" or \"polyvinyl acetate.\""@en ;
            dcterms:creator "The J. Paul Getty Trust" ;
            dcterms:license <https://opendatacommons.org/licenses/by/1-0/> ;
            dcterms:rights <https://rightsstatements.org/vocab/InC/1.0/> ;
            dcterms:source <http://www.getty.edu/research/tools/vocabularies/aat/> ],
        "Generic term for materials derived from vinyl chloride, vinyl acetate, or vinylidene chloride. Commonly used with reference to all polymers and copolymers of which vinyl chloride is a constituent. Use more precise terminology for known materials such as \"polyvinyl chloride\" or \"polyvinyl acetate.\""@en ;
    dcterms:identifier "CC00318" ;
    owl:sameAs <http://vocab.getty.edu/aat/300014502> .

cc:CC00319 a owl:NamedIndividual ;
    rdfs:label "voile"@en ;
    dcterms:description [ rdfs:label "Lightweight, sheer, plain-weave fabric made of various fibers."@en ;
            dcterms:creator "Wikidata contributors" ;
            dcterms:license <https://creativecommons.org/publicdomain/mark/1.0/> ;
            dcterms:rights <https://creativecommons.org/publicdomain/mark/1.0/> ;
            dcterms:source <https://www.wikidata.org/wiki/Wikidata:Data_access/en> ],
        "Lightweight, sheer, plain-weave fabric made of various fibers."@en ;
    dcterms:identifier "CC00319" ;
    owl:sameAs <http://www.wikidata.org/entity/Q2143346> .

cc:CC00321 a owl:NamedIndividual ;
    rdfs:label "webbing"@en ;
    dcterms:description [ rdfs:label "Strong bands of tightly woven cloth, designed for bearing weight; commonly used as the first layer of support for seating furniture."@en ;
            dcterms:creator "The J. Paul Getty Trust" ;
            dcterms:license <https://opendatacommons.org/licenses/by/1-0/> ;
            dcterms:rights <https://rightsstatements.org/vocab/InC/1.0/> ;
            dcterms:source <http://www.getty.edu/research/tools/vocabularies/aat/> ],
        "Strong bands of tightly woven cloth, designed for bearing weight; commonly used as the first layer of support for seating furniture."@en ;
    dcterms:identifier "CC00321" ;
    owl:sameAs <http://vocab.getty.edu/aat/300204912> .

cc:CC00322 a owl:NamedIndividual ;
    rdfs:label "wire"@en ;
    dcterms:description [ rdfs:label "Filament or slender rod of drawn metal."@en ;
            dcterms:creator "The J. Paul Getty Trust" ;
            dcterms:license <https://opendatacommons.org/licenses/by/1-0/> ;
            dcterms:rights <https://rightsstatements.org/vocab/InC/1.0/> ;
            dcterms:source <http://www.getty.edu/research/tools/vocabularies/aat/> ],
        "Filament or slender rod of drawn metal."@en ;
    dcterms:identifier "CC00322" ;
    owl:sameAs <http://vocab.getty.edu/aat/300011063> .

cc:CC00323 a owl:NamedIndividual ;
    rdfs:label "coatdress"@en ;
    dcterms:description [ rdfs:label "Tailored dresses styled like a coat and generally worn without an outer garment."@en ;
            dcterms:creator "The J. Paul Getty Trust" ;
            dcterms:license <https://opendatacommons.org/licenses/by/1-0/> ;
            dcterms:rights <https://rightsstatements.org/vocab/InC/1.0/> ;
            dcterms:source <http://www.getty.edu/research/tools/vocabularies/aat/> ],
        "Tailored dresses styled like a coat and generally worn without an outer garment."@en ;
    dcterms:identifier "CC00323" ;
    owl:sameAs <http://vocab.getty.edu/aat/300209826>,
        <http://www.wikidata.org/entity/Q16949531> .

cc:CC00327 a owl:NamedIndividual ;
    rdfs:label "engageante"@en ;
    dcterms:description [ rdfs:label "tiered sleeve ruffles of lace or other cloth that serve as cuffs, or detachable undersleeves edged with lace or embroidery"@en ;
            dcterms:creator "The J. Paul Getty Trust" ;
            dcterms:license <https://opendatacommons.org/licenses/by/1-0/> ;
            dcterms:rights <https://rightsstatements.org/vocab/InC/1.0/> ;
            dcterms:source <http://www.getty.edu/research/tools/vocabularies/aat/> ],
        "tiered sleeve ruffles of lace or other cloth that serve as cuffs, or detachable undersleeves edged with lace or embroidery"@en ;
    dcterms:identifier "CC00327" ;
    owl:sameAs <http://vocab.getty.edu/aat/300253720>,
        <http://www.wikidata.org/entity/Q1341710> .

cc:CC00356 a owl:NamedIndividual ;
    rdfs:label "oversleeve"@en ;
    dcterms:description [ rdfs:label "sleeve worn over another sleeve, often of fur, sometimes with a matching collar or partlet"@en ;
            dcterms:creator "The J. Paul Getty Trust" ;
            dcterms:license <https://opendatacommons.org/licenses/by/1-0/> ;
            dcterms:rights <https://rightsstatements.org/vocab/InC/1.0/> ;
            dcterms:source <http://www.getty.edu/research/tools/vocabularies/aat/> ],
        "sleeve worn over another sleeve, often of fur, sometimes with a matching collar or partlet"@en ;
    dcterms:identifier "CC00356" ;
    owl:sameAs <http://vocab.getty.edu/aat/300210015>,
        <http://www.wikidata.org/entity/Q29129961> .

cc:CC00357 a owl:NamedIndividual ;
    rdfs:label "pagoda sleeve"@en ;
    dcterms:description [ rdfs:label "wide flared sleeve"@en ;
            dcterms:creator "The J. Paul Getty Trust" ;
            dcterms:license <https://opendatacommons.org/licenses/by/1-0/> ;
            dcterms:rights <https://rightsstatements.org/vocab/InC/1.0/> ;
            dcterms:source <http://www.getty.edu/research/tools/vocabularies/aat/> ],
        "wide flared sleeve"@en ;
    dcterms:identifier "CC00357" ;
    owl:sameAs <http://vocab.getty.edu/aat/300253741>,
        <http://www.wikidata.org/entity/Q21972880> .

cc:CC00367 a owl:NamedIndividual ;
    rdfs:label "undersleeve"@en ;
    dcterms:description [ rdfs:label "separate lightweight sleeve worn under another sleeve and showing through or extending beyond it"@en ;
            dcterms:creator "The J. Paul Getty Trust" ;
            dcterms:license <https://opendatacommons.org/licenses/by/1-0/> ;
            dcterms:rights <https://rightsstatements.org/vocab/InC/1.0/> ;
            dcterms:source <http://www.getty.edu/research/tools/vocabularies/aat/> ],
        "separate lightweight sleeve worn under another sleeve and showing through or extending beyond it"@en ;
    dcterms:identifier "CC00367" ;
    owl:sameAs <http://vocab.getty.edu/aat/300210535>,
        <http://www.wikidata.org/entity/Q29130192> .

cc:CC00371 a owl:NamedIndividual ;
    rdfs:label "academic costume"@en ;
    dcterms:description [ rdfs:label "Refers to the various costumes worn by university and collegiate faculty, administrators, and graduating students at graduation ceremonies and other special occasions. The most common element of academic costume is the gown, a tradition dating to the Middle Ages. Decorative hoods and various caps, including the mortarboard, are other common elements of academic costume. Trimmings of various colors may be used to refer to different disciplines of study."@en ;
            dcterms:creator "The J. Paul Getty Trust" ;
            dcterms:license <https://opendatacommons.org/licenses/by/1-0/> ;
            dcterms:rights <https://rightsstatements.org/vocab/InC/1.0/> ;
            dcterms:source <http://www.getty.edu/research/tools/vocabularies/aat/> ],
        "Refers to the various costumes worn by university and collegiate faculty, administrators, and graduating students at graduation ceremonies and other special occasions. The most common element of academic costume is the gown, a tradition dating to the Middle Ages. Decorative hoods and various caps, including the mortarboard, are other common elements of academic costume. Trimmings of various colors may be used to refer to different disciplines of study."@en ;
    dcterms:identifier "CC00371" ;
    owl:sameAs <http://vocab.getty.edu/aat/300265060>,
        <http://www.wikidata.org/entity/Q1349227> .

cc:CC00428 a owl:NamedIndividual ;
    rdfs:label "overalls"@en ;
    dcterms:description [ rdfs:label "Close-fitting trousers that fit over footwear and strap under the sole, worn especially as part of a military uniform or for horseback riding. Use also for loose-fitting trousers worn over breeches or other bifurcated garments as protective wear by military personnel and others, especially during the 18th and 19th centuries."@en ;
            dcterms:creator "The J. Paul Getty Trust" ;
            dcterms:license <https://opendatacommons.org/licenses/by/1-0/> ;
            dcterms:rights <https://rightsstatements.org/vocab/InC/1.0/> ;
            dcterms:source <http://www.getty.edu/research/tools/vocabularies/aat/> ],
        "Close-fitting trousers that fit over footwear and strap under the sole, worn especially as part of a military uniform or for horseback riding. Use also for loose-fitting trousers worn over breeches or other bifurcated garments as protective wear by military personnel and others, especially during the 18th and 19th centuries."@en ;
    dcterms:identifier "CC00428" ;
    owl:sameAs <http://vocab.getty.edu/aat/300260366>,
        <http://www.wikidata.org/entity/Q13383825> .

cc:CC00458 a owl:NamedIndividual ;
    rdfs:label "outerwear"@en ;
    dcterms:description [ rdfs:label "Garments worn over other garments as the outer layer, especially those worn for protection from the natural elements. For garments worn for protection from dirt or danger, use descriptors listed under \"<protective wear>.\""@en ;
            dcterms:creator "The J. Paul Getty Trust" ;
            dcterms:license <https://opendatacommons.org/licenses/by/1-0/> ;
            dcterms:rights <https://rightsstatements.org/vocab/InC/1.0/> ;
            dcterms:source <http://www.getty.edu/research/tools/vocabularies/aat/> ],
        "Garments worn over other garments as the outer layer, especially those worn for protection from the natural elements. For garments worn for protection from dirt or danger, use descriptors listed under \"<protective wear>.\""@en ;
    dcterms:identifier "CC00458" ;
    owl:sameAs <http://vocab.getty.edu/aat/300209265> .

cc:CC00493 a owl:NamedIndividual ;
    rdfs:label "stomacher"@en ;
    dcterms:description [ rdfs:label "Stiff panels, usually triangular in shape and often heavily decorated, inserted in an open bodice to cover the corset."@en ;
            dcterms:creator "The J. Paul Getty Trust" ;
            dcterms:license <https://opendatacommons.org/licenses/by/1-0/> ;
            dcterms:rights <https://rightsstatements.org/vocab/InC/1.0/> ;
            dcterms:source <http://www.getty.edu/research/tools/vocabularies/aat/> ],
        "Stiff panels, usually triangular in shape and often heavily decorated, inserted in an open bodice to cover the corset."@en ;
    dcterms:identifier "CC00493" ;
    owl:sameAs <http://vocab.getty.edu/aat/300215860>,
        <http://www.wikidata.org/entity/Q1615371> .

cc:CC00514 a owl:NamedIndividual ;
    rdfs:label "slashing"@en ;
    dcterms:description [ rdfs:label "decorative slit cut in any part of a garment, especially sleeves and legs, to reveal an inner garment or lining"@en ;
            dcterms:creator "The J. Paul Getty Trust" ;
            dcterms:license <https://opendatacommons.org/licenses/by/1-0/> ;
            dcterms:rights <https://rightsstatements.org/vocab/InC/1.0/> ;
            dcterms:source <http://www.getty.edu/research/tools/vocabularies/aat/> ],
        "decorative slit cut in any part of a garment, especially sleeves and legs, to reveal an inner garment or lining"@en ;
    dcterms:identifier "CC00514" ;
    owl:sameAs <http://vocab.getty.edu/aat/300254833>,
        <http://www.wikidata.org/entity/Q10461476> .

cc:CC00525 a owl:NamedIndividual ;
    rdfs:label "shorts"@en ;
    dcterms:description [ rdfs:label "Exposed bifurcated garments extending from the waist or hip to any portion of the leg above the knee."@en ;
            dcterms:creator "The J. Paul Getty Trust" ;
            dcterms:license <https://opendatacommons.org/licenses/by/1-0/> ;
            dcterms:rights <https://rightsstatements.org/vocab/InC/1.0/> ;
            dcterms:source <http://www.getty.edu/research/tools/vocabularies/aat/> ],
        "Exposed bifurcated garments extending from the waist or hip to any portion of the leg above the knee."@en ;
    dcterms:identifier "CC00525" ;
    owl:sameAs <http://vocab.getty.edu/aat/300209930>,
        <http://www.wikidata.org/entity/Q223269> .

cc:CC00580 a owl:NamedIndividual ;
    rdfs:label "gusset"@en ;
    dcterms:description [ rdfs:label "Variously shaped inserts, as of cloth or leather, placed in a seam, as in a sleeve or glove, to strenghten or enlarge some part; also, pieces of chain mail or plate at the openings of the joints in a suit of armor."@en ;
            dcterms:creator "The J. Paul Getty Trust" ;
            dcterms:license <https://opendatacommons.org/licenses/by/1-0/> ;
            dcterms:rights <https://rightsstatements.org/vocab/InC/1.0/> ;
            dcterms:source <http://www.getty.edu/research/tools/vocabularies/aat/> ],
        "Variously shaped inserts, as of cloth or leather, placed in a seam, as in a sleeve or glove, to strenghten or enlarge some part; also, pieces of chain mail or plate at the openings of the joints in a suit of armor."@en ;
    dcterms:identifier "CC00580" ;
    owl:sameAs <http://vocab.getty.edu/aat/300239408>,
        <http://www.wikidata.org/entity/Q244554> .

cc:CC00581 a owl:NamedIndividual ;
    rdfs:label "ruffle"@en ;
    dcterms:description [ rdfs:label "Strip of lace, cloth, leather, or another material that is gathered on one edge or cut on the bias, so that when attached to the hem, button placard, neckline, or wrist of a garment it produces an ornamental frill or flounce."@en ;
            dcterms:creator "The J. Paul Getty Trust" ;
            dcterms:license <https://opendatacommons.org/licenses/by/1-0/> ;
            dcterms:rights <https://rightsstatements.org/vocab/InC/1.0/> ;
            dcterms:source <http://www.getty.edu/research/tools/vocabularies/aat/> ],
        "Strip of lace, cloth, leather, or another material that is gathered on one edge or cut on the bias, so that when attached to the hem, button placard, neckline, or wrist of a garment it produces an ornamental frill or flounce."@en ;
    dcterms:identifier "CC00581" ;
    owl:sameAs <http://vocab.getty.edu/aat/300253712>,
        <http://www.wikidata.org/entity/Q2204140> .

cc:CC00594 a owl:NamedIndividual ;
    rdfs:label "tweed"@en ;
    dcterms:description [ rdfs:label "Wool textile with a rough, homespun surface effect."@en ;
            dcterms:creator "The J. Paul Getty Trust" ;
            dcterms:license <https://opendatacommons.org/licenses/by/1-0/> ;
            dcterms:rights <https://rightsstatements.org/vocab/InC/1.0/> ;
            dcterms:source <http://www.getty.edu/research/tools/vocabularies/aat/> ],
        "Wool textile with a rough, homespun surface effect."@en ;
    dcterms:identifier "CC00594" ;
    owl:sameAs <http://www.wikidata.org/entity/Q40601> .

cc:CC00600 a owl:NamedIndividual ;
    rdfs:label "accessory"@en ;
    dcterms:description [ rdfs:label "Objects or devices that are not essential in themselves but add to the beauty, convenience, or effectiveness of other things, as, for example, to costume or automobiles."@en ;
            dcterms:creator "The J. Paul Getty Trust" ;
            dcterms:license <https://opendatacommons.org/licenses/by/1-0/> ;
            dcterms:rights <https://rightsstatements.org/vocab/InC/1.0/> ;
            dcterms:source <http://www.getty.edu/research/tools/vocabularies/aat/> ],
        "Objects or devices that are not essential in themselves but add to the beauty, convenience, or effectiveness of other things, as, for example, to costume or automobiles."@en ;
    dcterms:identifier "CC00600" ;
    owl:sameAs <http://vocab.getty.edu/aat/300251645>,
        <http://www.wikidata.org/entity/Q362200> .

cc:CC00602 a owl:NamedIndividual ;
    rdfs:label "cape"@en ;
    dcterms:description [ rdfs:label "Sleeveless outer garments of varying lengths, fastening at the neck and falling loosely from the shoulders that function as either separate garments or attach to longer coats or cloaks."@en ;
            dcterms:creator "The J. Paul Getty Trust" ;
            dcterms:license <https://opendatacommons.org/licenses/by/1-0/> ;
            dcterms:rights <https://rightsstatements.org/vocab/InC/1.0/> ;
            dcterms:source <http://www.getty.edu/research/tools/vocabularies/aat/> ],
        "Sleeveless outer garments of varying lengths, fastening at the neck and falling loosely from the shoulders that function as either separate garments or attach to longer coats or cloaks."@en ;
    dcterms:identifier "CC00602" ;
    owl:sameAs <http://vocab.getty.edu/aat/300046140>,
        <http://www.wikidata.org/entity/Q1034198> .

cc:CC00603 a owl:NamedIndividual ;
    rdfs:label "footwear"@en ;
    dcterms:description [ rdfs:label "Coverings for the feet that sometimes extend above the ankle; generally made of durable materials. Distinguished from \"hosiery,\" which is primarily leg coverings."@en ;
            dcterms:creator "The J. Paul Getty Trust" ;
            dcterms:license <https://opendatacommons.org/licenses/by/1-0/> ;
            dcterms:rights <https://rightsstatements.org/vocab/InC/1.0/> ;
            dcterms:source <http://www.getty.edu/research/tools/vocabularies/aat/> ],
        "Coverings for the feet that sometimes extend above the ankle; generally made of durable materials. Distinguished from \"hosiery,\" which is primarily leg coverings."@en ;
    dcterms:identifier "CC00603" ;
    owl:sameAs <http://vocab.getty.edu/aat/300209280>,
        <http://www.wikidata.org/entity/Q161928> .

cc:CC00604 a owl:NamedIndividual ;
    rdfs:label "robe"@en ;
    dcterms:description [ rdfs:label "Long, loose garments that tend to be of one piece and to open down the front. Examples include ordinary wear for men and women, dating from the Middle Ages forward in the West and common yet today in Asian and African countries; and similar garments often of elegant style worn for ceremonial or official occasions or as a symbol of office or profession. For womens dresses, use \"gowns.\" For loose-fitting garments, often wraparound and worn to the bath or informally around the house use \"bathrobes.\""@en ;
            dcterms:creator "The J. Paul Getty Trust" ;
            dcterms:license <https://opendatacommons.org/licenses/by/1-0/> ;
            dcterms:rights <https://rightsstatements.org/vocab/InC/1.0/> ;
            dcterms:source <http://www.getty.edu/research/tools/vocabularies/aat/> ],
        "Long, loose garments that tend to be of one piece and to open down the front. Examples include ordinary wear for men and women, dating from the Middle Ages forward in the West and common yet today in Asian and African countries; and similar garments often of elegant style worn for ceremonial or official occasions or as a symbol of office or profession. For womens dresses, use \"gowns.\" For loose-fitting garments, often wraparound and worn to the bath or informally around the house use \"bathrobes.\""@en ;
    dcterms:identifier "CC00604" ;
    owl:sameAs <http://vocab.getty.edu/aat/300209852>,
        <http://www.wikidata.org/entity/Q345127> .

cc:CC00605 a owl:NamedIndividual ;
    rdfs:label "legwear"@en ;
    dcterms:description [ rdfs:label "Leg coverings, sometimes woven in one with panties, that extend to the ankle and usually cover the foot; generally knitted or woven, sheer or opaque, and of lightweight or heavy fabric. Distinguish from \"footwear\", which is primarily worn as coverings for the feet."@en ;
            dcterms:creator "The J. Paul Getty Trust" ;
            dcterms:license <https://opendatacommons.org/licenses/by/1-0/> ;
            dcterms:rights <https://rightsstatements.org/vocab/InC/1.0/> ;
            dcterms:source <http://www.getty.edu/research/tools/vocabularies/aat/> ],
        "Leg coverings, sometimes woven in one with panties, that extend to the ankle and usually cover the foot; generally knitted or woven, sheer or opaque, and of lightweight or heavy fabric. Distinguish from \"footwear\", which is primarily worn as coverings for the feet."@en ;
    dcterms:identifier "CC00605" ;
    owl:sameAs <http://vocab.getty.edu/aat/300209984>,
        <http://www.wikidata.org/entity/Q2524539> .

cc:CC00606 a owl:NamedIndividual ;
    rdfs:label "gloves"@en ;
    dcterms:description [ rdfs:label "Coverings for the hand enclosing each finger separately, sometimes extending over the wrist and arm."@en ;
            dcterms:creator "The J. Paul Getty Trust" ;
            dcterms:license <https://opendatacommons.org/licenses/by/1-0/> ;
            dcterms:rights <https://rightsstatements.org/vocab/InC/1.0/> ;
            dcterms:source <http://www.getty.edu/research/tools/vocabularies/aat/> ],
        "Coverings for the hand enclosing each finger separately, sometimes extending over the wrist and arm."@en ;
    dcterms:identifier "CC00606" ;
    owl:sameAs <http://vocab.getty.edu/aat/300148821>,
        <http://www.wikidata.org/entity/Q169031> .

cc:CC00607 a owl:NamedIndividual ;
    rdfs:label "top"@en ;
    dcterms:description [ rdfs:label "General term for clothing worn on the upper part of the body, above the waist, excluding outerwear and underwear. Typically not used in reference to men's clothing."@en ;
            dcterms:creator "The J. Paul Getty Trust" ;
            dcterms:license <https://opendatacommons.org/licenses/by/1-0/> ;
            dcterms:rights <https://rightsstatements.org/vocab/InC/1.0/> ;
            dcterms:source <http://www.getty.edu/research/tools/vocabularies/aat/> ],
        "General term for clothing worn on the upper part of the body, above the waist, excluding outerwear and underwear. Typically not used in reference to men's clothing."@en ;
    dcterms:identifier "CC00607" ;
    owl:sameAs <http://vocab.getty.edu/aat/300411736>,
        <http://www.wikidata.org/entity/Q1435365> .

cc:CC00608 a owl:NamedIndividual ;
    rdfs:label "headwear"@en ;
    dcterms:description [ rdfs:label "Any covering for the head."@en ;
            dcterms:creator "The J. Paul Getty Trust" ;
            dcterms:license <https://opendatacommons.org/licenses/by/1-0/> ;
            dcterms:rights <https://rightsstatements.org/vocab/InC/1.0/> ;
            dcterms:source <http://www.getty.edu/research/tools/vocabularies/aat/> ],
        "Any covering for the head."@en ;
    dcterms:identifier "CC00608" ;
    owl:sameAs <http://vocab.getty.edu/aat/300209285>,
        <http://www.wikidata.org/entity/Q14952> .

cc:CC00610 a owl:NamedIndividual ;
    rdfs:label "jewelry"@en ;
    dcterms:description [ rdfs:label "Ornaments such as bracelets, necklaces, and rings, of precious or semiprecious materials worn or carried on the person for adornment; also includes similar articles worn or carried for devotional or mourning purposes."@en ;
            dcterms:creator "The J. Paul Getty Trust" ;
            dcterms:license <https://opendatacommons.org/licenses/by/1-0/> ;
            dcterms:rights <https://rightsstatements.org/vocab/InC/1.0/> ;
            dcterms:source <http://www.getty.edu/research/tools/vocabularies/aat/> ],
        "Ornaments such as bracelets, necklaces, and rings, of precious or semiprecious materials worn or carried on the person for adornment; also includes similar articles worn or carried for devotional or mourning purposes."@en ;
    dcterms:identifier "CC00610" ;
    owl:sameAs <http://vocab.getty.edu/aat/300209286>,
        <http://www.wikidata.org/entity/Q161439> .

cc:CC00611 a owl:NamedIndividual ;
    rdfs:label "ensemble"@en ;
    dcterms:description [ rdfs:label "Complete costume, including garments and accessories, worn for a harmonious effect. Also, two or more garments or accessories designed to complement one another."@en ;
            dcterms:creator "The J. Paul Getty Trust" ;
            dcterms:license <https://opendatacommons.org/licenses/by/1-0/> ;
            dcterms:rights <https://rightsstatements.org/vocab/InC/1.0/> ;
            dcterms:source <http://www.getty.edu/research/tools/vocabularies/aat/> ],
        "Complete costume, including garments and accessories, worn for a harmonious effect. Also, two or more garments or accessories designed to complement one another."@en ;
    dcterms:identifier "CC00611" ;
    owl:sameAs <http://vocab.getty.edu/aat/300209844>,
        <http://www.wikidata.org/entity/Q29353484> .

cc:CC00058 a owl:NamedIndividual ;
    rdfs:label "gray"@en ;
    dcterms:description [ rdfs:label "Hue name for any color intermediate between black and white, or composed of a mixture of black and white with little or no positive hue. (AAT)"@en ;
            dcterms:creator "The J. Paul Getty Trust" ;
            dcterms:license <https://opendatacommons.org/licenses/by/1-0/> ;
            dcterms:rights <https://rightsstatements.org/vocab/InC/1.0/> ;
            dcterms:source <http://www.getty.edu/research/tools/vocabularies/aat/> ],
        "Hue name for any color intermediate between black and white, or composed of a mixture of black and white with little or no positive hue. (AAT)"@en ;
    dcterms:identifier "CC00058" ;
    owl:sameAs <http://vocab.getty.edu/aat/300130811>,
        <http://www.wikidata.org/entity/Q42519> .

cc:CC00199 a owl:NamedIndividual ;
    rdfs:label "boning"@en ;
    dcterms:description [ rdfs:label "strip of rigid material used to stiffen corsets, bodices, collars, or other types of costume"@en ;
            dcterms:creator "Wikidata contributors" ;
            dcterms:license <https://creativecommons.org/publicdomain/mark/1.0/> ;
            dcterms:rights <https://creativecommons.org/publicdomain/mark/1.0/> ;
            dcterms:source <https://www.wikidata.org/wiki/Wikidata:Data_access/en> ],
        "strip of rigid material used to stiffen corsets, bodices, collars, or other types of costume"@en ;
    dcterms:identifier "CC00199" ;
    owl:sameAs <http://vocab.getty.edu/aat/300253790>,
        <http://www.wikidata.org/entity/Q881659> .

cc:CC00244 a owl:NamedIndividual ;
    rdfs:label "synthetic fiber"@en ;
    dcterms:description [ rdfs:label "Fiber made from chemical substances, used for textile production."@en ;
            dcterms:creator "The J. Paul Getty Trust" ;
            dcterms:license <https://opendatacommons.org/licenses/by/1-0/> ;
            dcterms:rights <https://rightsstatements.org/vocab/InC/1.0/> ;
            dcterms:source <http://www.getty.edu/research/tools/vocabularies/aat/> ],
        "Fiber made from chemical substances, used for textile production."@en ;
    dcterms:identifier "CC00244" ;
    owl:sameAs <http://vocab.getty.edu/aat/300014058>,
        <http://www.wikidata.org/entity/Q5856> .

cc:CC00345 a owl:NamedIndividual ;
    rdfs:label "underwear"@en ;
    dcterms:description [ rdfs:label "Garments worn beneath main garments, usually next to the skin."@en ;
            dcterms:creator "The J. Paul Getty Trust" ;
            dcterms:license <https://opendatacommons.org/licenses/by/1-0/> ;
            dcterms:rights <https://rightsstatements.org/vocab/InC/1.0/> ;
            dcterms:source <http://www.getty.edu/research/tools/vocabularies/aat/> ],
        "Garments worn beneath main garments, usually next to the skin."@en ;
    dcterms:identifier "CC00345" ;
    owl:sameAs <http://vocab.getty.edu/aat/300209267> .

cc:CC00628 a owl:NamedIndividual ;
    rdfs:label "fringe"@en ;
    dcterms:description [ rdfs:label "Trimming consisting of long or short lengths of straight or twisted thread, cord, or tassel; often grouped or knotted in various designs."@en ;
            dcterms:creator "The J. Paul Getty Trust" ;
            dcterms:license <https://opendatacommons.org/licenses/by/1-0/> ;
            dcterms:rights <https://rightsstatements.org/vocab/InC/1.0/> ;
            dcterms:source <http://www.getty.edu/research/tools/vocabularies/aat/> ],
        "Trimming consisting of long or short lengths of straight or twisted thread, cord, or tassel; often grouped or knotted in various designs."@en ;
    dcterms:identifier "CC00628" ;
    owl:sameAs <http://vocab.getty.edu/aat/300227830>,
        <http://www.wikidata.org/entity/Q1353860> .

cc:CC00630 a owl:NamedIndividual ;
    rdfs:label "flax"@en ;
    dcterms:description [ rdfs:label "Fiber derived from the bast or skin of the stem of the species Linum usitatissimum. Soft, flexible fibers are produced by retting the stem of the flax plant, then washing and cleaning the fibers. Flax fibers of thinner and longer than cotton, but the fiber tube has thicker walls resulting in a stronger thread. Additionally, flax fibers are used for linen fabric, thread for making shoes and bookbinding, fish line, and twine. Waste flax fibers are used in banknotes, cigarette covers, and writing and drawing paper."@en ;
            dcterms:creator "The J. Paul Getty Trust" ;
            dcterms:license <https://opendatacommons.org/licenses/by/1-0/> ;
            dcterms:rights <https://rightsstatements.org/vocab/InC/1.0/> ;
            dcterms:source <http://www.getty.edu/research/tools/vocabularies/aat/> ],
        "Fiber derived from the bast or skin of the stem of the species Linum usitatissimum. Soft, flexible fibers are produced by retting the stem of the flax plant, then washing and cleaning the fibers. Flax fibers of thinner and longer than cotton, but the fiber tube has thicker walls resulting in a stronger thread. Additionally, flax fibers are used for linen fabric, thread for making shoes and bookbinding, fish line, and twine. Waste flax fibers are used in banknotes, cigarette covers, and writing and drawing paper."@en ;
    dcterms:identifier "CC00630" ;
    owl:sameAs <http://vocab.getty.edu/aat/300014041>,
        <http://www.wikidata.org/entity/Q47089651> .

